@prefix dcterms: <http://purl.org/dc/terms/> .
@prefix ns1: <https://spdx.org/rdf/3.0.1/terms/Core/> .
@prefix ns2: <https://spdx.org/rdf/3.0.1/terms/Software/> .
@prefix ns3: <https://spdx.org/rdf/3.0.1/terms/Security/> .
@prefix ns4: <https://spdx.org/rdf/3.0.1/terms/AI/> .
@prefix ns5: <https://spdx.org/rdf/3.0.1/terms/Dataset/> .
@prefix ns6: <https://spdx.org/rdf/3.0.1/terms/ExpandedLicensing/> .
@prefix omg-ann: <https://www.omg.org/spec/Commons/AnnotationVocabulary/> .
@prefix owl: <http://www.w3.org/2002/07/owl#> .
@prefix rdf: <http://www.w3.org/1999/02/22-rdf-syntax-ns#> .
@prefix rdfs: <http://www.w3.org/2000/01/rdf-schema#> .
@prefix sh: <http://www.w3.org/ns/shacl#> .
@prefix spdx: <https://spdx.org/rdf/3.0.1/terms/> .
@prefix xsd: <http://www.w3.org/2001/XMLSchema#> .

_:N568e6ba102414daeb0cc9a88c6cc3b4e {
    ns4:AIPackage a owl:Class,
            sh:NodeShape ;
        rdfs:comment "Specifies an AI package and its associated information."@en ;
        rdfs:subClassOf ns2:Package ;
        sh:nodeKind sh:IRI ;
        sh:property _:N0fe19c10b0404ecca1b3c2651b040358,
            _:N180f2ecfb0d74d59bfdeefaeabb39288,
            _:N1fa42a3d9da34087baaa8c7892211524,
            _:N25a0cb36988640c4b945c1ac0f2310a5,
            _:N4ffa4b0fbd9545269f7365d293f45afd,
            _:N53ce511f21824a0bad0607a29d13b55e,
            _:N802270e023784500a8ae0fac28a696c3,
            _:N990927fcdbab47dd9aa94d5b66bcec04,
            _:Nb3f306a76df5403290b7c52fb7c130f9,
            _:Nbc465417c25c47d59406fb8be56750ab,
            _:Nc4fceb9c34e84e4fafc753adffe79156,
            _:Nf68d5ece5e9048618433f794c917391d,
            _:Nf7723676f78c465082f370aa66673665,
            _:Nf841a206f30a429a9e1cbeed0e2e102f,
            _:Nfe30d0e9941a4ea8a330bf63192fe968 .

    <https://spdx.org/rdf/3.0.1/terms/Build/Build> a owl:Class,
            sh:NodeShape ;
        rdfs:comment "Class that describes a build instance of software/artifacts."@en ;
        rdfs:subClassOf ns1:Element ;
        sh:nodeKind sh:IRI ;
        sh:property _:N0b485de1e2a74db28b6f6b7f5c8c114d,
            _:N3343e15c4f72473ebbfc546fb9ac3c23,
            _:N3c5062897ef2459ab30d9ecffc9b8324,
            _:N5cb42ed80e484315b98ff5a6006e1649,
            _:N6d06a87ba9564b1686aca2e55466693f,
            _:N787361abd52c45ff88c62ab4069645cb,
            _:N8d30523f8928470fb33e9c71f058a726,
            _:N982ba8180ed94a77899dff62913fe63e,
            _:Ndf979723179648f495f1ba2ce971220b .

    ns1:Annotation a owl:Class,
            sh:NodeShape ;
        rdfs:comment "An assertion made in relation to one or more elements."@en ;
        rdfs:subClassOf ns1:Element ;
        sh:nodeKind sh:IRI ;
        sh:property _:N0d84cf0c0792460ea6248149d0eee551,
            _:N2014a2d4464246758ac5ad1b90e7355c,
            _:Nb5ff4f1d41e643ff944fa4ca63680131,
            _:Nb9a41ca33e8b4bb8979db11ee7f9ee26 .

    ns1:LifecycleScopedRelationship a owl:Class,
            sh:NodeShape ;
        rdfs:comment "Provide context for a relationship that occurs in the lifecycle."@en ;
        rdfs:subClassOf ns1:Relationship ;
        sh:nodeKind sh:IRI ;
        sh:property _:Nb6ad836edee444b7af4e39055772c19d .

    ns1:NoAssertionElement a owl:NamedIndividual,
            ns1:IndividualElement ;
        rdfs:comment """An Individual Value for Element representing a set of Elements of unknown
identify or cardinality (number)."""@en ;
        ns1:creationInfo <https://spdx.org/rdf/3.0.1/creationInfo_NoAssertionElement> .

    ns1:NoneElement a owl:NamedIndividual,
            ns1:IndividualElement ;
        rdfs:comment """An Individual Value for Element representing a set of Elements with
cardinality (number/count) of zero."""@en ;
        ns1:creationInfo <https://spdx.org/rdf/3.0.1/creationInfo_NoneElement> .

    ns1:PackageVerificationCode a owl:Class,
            sh:NodeShape ;
        rdfs:comment "An SPDX version 2.X compatible verification method for software packages."@en ;
        rdfs:subClassOf ns1:IntegrityMethod ;
        sh:nodeKind sh:BlankNodeOrIRI ;
        sh:property _:N12267f2523f648ee866e621b0d8f1813,
            _:N7f1ad87c28114ee7bc0725fb58b20ca9,
            _:Na7fe9a9442ae4ab48e050da75cf7fd9b .

    ns1:Person a owl:Class ;
        rdfs:comment "An individual human being."@en ;
        rdfs:subClassOf ns1:Agent ;
        sh:nodeKind sh:IRI .

    ns1:SoftwareAgent a owl:Class ;
        rdfs:comment "A software agent."@en ;
        rdfs:subClassOf ns1:Agent ;
        sh:nodeKind sh:IRI .

    ns1:SpdxDocument a owl:Class,
            sh:NodeShape ;
        rdfs:comment "A collection of SPDX Elements that could potentially be serialized."@en ;
        rdfs:subClassOf ns1:ElementCollection ;
        sh:nodeKind sh:IRI ;
        sh:property _:N942452bba40a472880cf56ce7944c65b,
            _:Na1b3987084df4a0893f69ad4ee6679b6,
            _:Nf87704a94ca4450f8dd886c348a8a30f .

    ns5:DatasetPackage a owl:Class,
            sh:NodeShape ;
        rdfs:comment "Specifies a data package and its associated information."@en ;
        rdfs:subClassOf ns2:Package ;
        sh:nodeKind sh:IRI ;
        sh:property _:N00b58432199d4232a8b3fbf92ce42646,
            _:N11f4f26ee5534d1ca4e24eef77922411,
            _:N303b56ee3bd24539a79e6e86ea2b00b2,
            _:N6b0753cb9cf74582bbf870095e9a692f,
            _:N73da8aa44e7149a8af8639082044141a,
            _:N7bbd717f73924fdd82520407da9bf371,
            _:Nb7e49e28e70b485b94a91d9e9ca7f4ce,
            _:Nb8343569c43d4d259d82b46fc7aca5c5,
            _:Nc1353b07fba04cb49000857276d12cfa,
            _:Nd09e69a597cd43079761fc0d8051bce5,
            _:Nd4845c86c2ed49d88fcef6b52e75d8cd,
            _:Ne5201624bfcf4f99ab0db3b6d2e24290,
            _:Nfab4dd42d8a74ea2b147d597f33b984f .

    ns6:ConjunctiveLicenseSet a owl:Class,
            sh:NodeShape ;
        rdfs:comment """Portion of an AnyLicenseInfo representing a set of licensing information
where all elements apply."""@en ;
        rdfs:subClassOf <https://spdx.org/rdf/3.0.1/terms/SimpleLicensing/AnyLicenseInfo> ;
        sh:nodeKind sh:IRI ;
        sh:property _:N6d9713b048484df2a5edddea8f2e9e7c .

    ns6:CustomLicense a owl:Class ;
        rdfs:comment "A license that is not listed on the SPDX License List."@en ;
        rdfs:subClassOf ns6:License ;
        sh:nodeKind sh:IRI .

    ns6:CustomLicenseAddition a owl:Class ;
        rdfs:comment "A license addition that is not listed on the SPDX Exceptions List."@en ;
        rdfs:subClassOf ns6:LicenseAddition ;
        sh:nodeKind sh:IRI .

    ns6:DisjunctiveLicenseSet a owl:Class,
            sh:NodeShape ;
        rdfs:comment """Portion of an AnyLicenseInfo representing a set of licensing information where
only one of the elements applies."""@en ;
        rdfs:subClassOf <https://spdx.org/rdf/3.0.1/terms/SimpleLicensing/AnyLicenseInfo> ;
        sh:nodeKind sh:IRI ;
        sh:property _:Nfc2362f61f554fa28c87aefb63bb7aaa .

    ns6:ListedLicense a owl:Class,
            sh:NodeShape ;
        rdfs:comment "A license that is listed on the SPDX License List."@en ;
        rdfs:subClassOf ns6:License ;
        sh:nodeKind sh:IRI ;
        sh:property _:N85d91bf18a8e4340901a74314a2a4a56,
            _:N9ab8f5212b9e4a0c84030a7fde89d4a5 .

    ns6:ListedLicenseException a owl:Class,
            sh:NodeShape ;
        rdfs:comment "A license exception that is listed on the SPDX Exceptions list."@en ;
        rdfs:subClassOf ns6:LicenseAddition ;
        sh:nodeKind sh:IRI ;
        sh:property _:N10cc734ac08e44819863beb021240480,
            _:N5efb7706d0b3407baf344bdb97f9c1a0 .

    ns6:NoAssertionLicense a owl:NamedIndividual,
            ns6:IndividualLicensingInfo ;
        rdfs:comment """An Individual Value for License when no assertion can be made about its actual
value."""@en ;
        owl:sameAs <https://spdx.org/rdf/3.0.1/terms/Licensing/NoAssertion> ;
        ns1:creationInfo <https://spdx.org/rdf/3.0.1/creationInfo_NoAssertionLicense> .

    ns6:NoneLicense a owl:NamedIndividual,
            ns6:IndividualLicensingInfo ;
        rdfs:comment """An Individual Value for License where the SPDX data creator determines that no
license is present."""@en ;
        owl:sameAs <https://spdx.org/rdf/3.0.1/terms/Licensing/None> ;
        ns1:creationInfo <https://spdx.org/rdf/3.0.1/creationInfo_NoneLicense> .

    ns6:OrLaterOperator a owl:Class,
            sh:NodeShape ;
        rdfs:comment """Portion of an AnyLicenseInfo representing this version, or any later version,
of the indicated License."""@en ;
        rdfs:subClassOf ns6:ExtendableLicense ;
        sh:nodeKind sh:IRI ;
        sh:property _:N8d51fc8fc521483d85792bd30b47cade .

    ns6:WithAdditionOperator a owl:Class,
            sh:NodeShape ;
        rdfs:comment """Portion of an AnyLicenseInfo representing a License which has additional
text applied to it."""@en ;
        rdfs:subClassOf <https://spdx.org/rdf/3.0.1/terms/SimpleLicensing/AnyLicenseInfo> ;
        sh:nodeKind sh:IRI ;
        sh:property _:N0c6b033e1de9470b841f93eb50058a0f,
            _:N45f93548cb7d4b5f8882568324cdbbc3 .

    <https://spdx.org/rdf/3.0.1/terms/Extension/CdxPropertiesExtension> a owl:Class,
            sh:NodeShape ;
        rdfs:comment "A type of extension consisting of a list of name value pairs."@en ;
        rdfs:subClassOf <https://spdx.org/rdf/3.0.1/terms/Extension/Extension> ;
        sh:nodeKind sh:BlankNodeOrIRI ;
        sh:property _:Nf6d27b818a8849d5928e3b8f3d90a57a .

    ns3:CvssV2VulnAssessmentRelationship a owl:Class,
            sh:NodeShape ;
        rdfs:comment "Provides a CVSS version 2.0 assessment for a vulnerability."@en ;
        rdfs:subClassOf ns3:VulnAssessmentRelationship ;
        sh:nodeKind sh:IRI ;
        sh:property _:N62d7707875a0400ebdf8b04ae8add96c,
            _:N8461c39477864d659431548b72f253a4 .

    ns3:CvssV3VulnAssessmentRelationship a owl:Class,
            sh:NodeShape ;
        rdfs:comment "Provides a CVSS version 3 assessment for a vulnerability."@en ;
        rdfs:subClassOf ns3:VulnAssessmentRelationship ;
        sh:nodeKind sh:IRI ;
        sh:property _:N2313768eecea43dfbce33ea9abb10b56,
            _:N27eec11210c94b568bd4cadc90bdc1b3,
            _:Nb9f068a614cb433690e515991de940e2 .

    ns3:CvssV4VulnAssessmentRelationship a owl:Class,
            sh:NodeShape ;
        rdfs:comment "Provides a CVSS version 4 assessment for a vulnerability."@en ;
        rdfs:subClassOf ns3:VulnAssessmentRelationship ;
        sh:nodeKind sh:IRI ;
        sh:property _:N0d896e6ea1824fb3a4ecd9a1e7fe690b,
            _:N53b67006a5804ef6aaadd5d4387b7e71,
            _:N5fcdd8adc1c543c8b4d7594bf3657d43 .

    ns3:EpssVulnAssessmentRelationship a owl:Class,
            sh:NodeShape ;
        rdfs:comment "Provides an EPSS assessment for a vulnerability."@en ;
        rdfs:subClassOf ns3:VulnAssessmentRelationship ;
        sh:nodeKind sh:IRI ;
        sh:property _:N6ca973580af24785ad2f13872c5321a7,
            _:N921fdfd13fd7435bb8e9a2a862a02269 .

    ns3:ExploitCatalogVulnAssessmentRelationship a owl:Class,
            sh:NodeShape ;
        rdfs:comment "Provides an exploit assessment of a vulnerability."@en ;
        rdfs:subClassOf ns3:VulnAssessmentRelationship ;
        sh:nodeKind sh:IRI ;
        sh:property _:Na7c582248f8a4da08f39b510f5695b65,
            _:Nc81ae3ec31284874b9c71d4b0c84588d,
            _:Nf18b2b0b18d24739be254a0caccb68c2 .

    ns3:SsvcVulnAssessmentRelationship a owl:Class,
            sh:NodeShape ;
        rdfs:comment "Provides an SSVC assessment for a vulnerability."@en ;
        rdfs:subClassOf ns3:VulnAssessmentRelationship ;
        sh:nodeKind sh:IRI ;
        sh:property _:Nca26c79ce5d04845979e1252bcde1edc .

    ns3:VexAffectedVulnAssessmentRelationship a owl:Class,
            sh:NodeShape ;
        rdfs:comment """Connects a vulnerability and an element designating the element as a product
affected by the vulnerability."""@en ;
        rdfs:subClassOf ns3:VexVulnAssessmentRelationship ;
        sh:nodeKind sh:IRI ;
        sh:property _:N9bb7d51fbdb64ad48dbbf71ee81f69db,
            _:Nf24a922499724d41b0bbedfdb59993a8 .

    ns3:VexFixedVulnAssessmentRelationship a owl:Class ;
        rdfs:comment """Links a vulnerability and elements representing products (in the VEX sense) where
a fix has been applied and are no longer affected."""@en ;
        rdfs:subClassOf ns3:VexVulnAssessmentRelationship ;
        sh:nodeKind sh:IRI .

    ns3:VexNotAffectedVulnAssessmentRelationship a owl:Class,
            sh:NodeShape ;
        rdfs:comment """Links a vulnerability and one or more elements designating the latter as products
not affected by the vulnerability."""@en ;
        rdfs:subClassOf ns3:VexVulnAssessmentRelationship ;
        sh:nodeKind sh:IRI ;
        sh:property _:N14e47cb6a3474796844dd20924129ab6,
            _:N9fdcb40f9bc24613ae75374946dc3163,
            _:Nbc38aabeeaa542fbb91658ff6336efe7 .

    ns3:VexUnderInvestigationVulnAssessmentRelationship a owl:Class ;
        rdfs:comment """Designates elements as products where the impact of a vulnerability is being
investigated."""@en ;
        rdfs:subClassOf ns3:VexVulnAssessmentRelationship ;
        sh:nodeKind sh:IRI .

    ns3:Vulnerability a owl:Class,
            sh:NodeShape ;
        rdfs:comment "Specifies a vulnerability and its associated information."@en ;
        rdfs:subClassOf ns1:Artifact ;
        sh:nodeKind sh:IRI ;
        sh:property _:N05a05a340bc1470fa1fe3d4528b8bcb0,
            _:N61bbc8ebf97841c3b566bb7d1795e8df,
            _:N951f8090463a4c9a99b9396ff1f62c60 .

    <https://spdx.org/rdf/3.0.1/terms/SimpleLicensing/LicenseExpression> a owl:Class,
            sh:NodeShape ;
        rdfs:comment "An SPDX Element containing an SPDX license expression string."@en ;
        rdfs:subClassOf <https://spdx.org/rdf/3.0.1/terms/SimpleLicensing/AnyLicenseInfo> ;
        sh:nodeKind sh:IRI ;
        sh:property _:N6aee3408cdaa46a6bb0ccb864eb33899,
            _:N9c9620b9738a48ffa797d861125a90b6,
            _:Nd0e089337a33424fabe3fdff5e9353f2 .

    <https://spdx.org/rdf/3.0.1/terms/SimpleLicensing/SimpleLicensingText> a owl:Class,
            sh:NodeShape ;
        rdfs:comment "A license or addition that is not listed on the SPDX License List."@en ;
        rdfs:subClassOf ns1:Element ;
        sh:nodeKind sh:IRI ;
        sh:property _:N189799efa65545fab51f17d5bb4eb46c .

    ns2:Sbom a owl:Class,
            sh:NodeShape ;
        rdfs:comment "A collection of SPDX Elements describing a single package."@en ;
        rdfs:subClassOf ns1:Bom ;
        sh:nodeKind sh:IRI ;
        sh:property _:Nd7ce9307a16247cb86d95f5c40e0baed .

    ns2:Snippet a owl:Class,
            sh:NodeShape ;
        rdfs:comment "Describes a certain part of a file."@en ;
        rdfs:subClassOf ns2:SoftwareArtifact ;
        sh:nodeKind sh:IRI ;
        sh:property _:N735b7ed5ff0c4e14898aa20824d3f3d1,
            _:N89c1049758874ee193ceacd3663eff21,
            _:Nfd5dcb568f8744a58f8df95723e02649 .

    <https://spdx.org/rdf/3.0.1/creationInfo_NoAssertionElement> a ns1:CreationInfo ;
        rdfs:comment "This individual element was defined by the spec."@en ;
        ns1:created "2024-11-22T03:00:01Z"^^xsd:dateTimeStamp ;
        ns1:createdBy ns1:SpdxOrganization ;
        ns1:specVersion "3.0.1" .

    <https://spdx.org/rdf/3.0.1/creationInfo_NoAssertionLicense> a ns1:CreationInfo ;
        rdfs:comment "This individual element was defined by the spec."@en ;
        ns1:created "2024-11-22T03:00:01Z"^^xsd:dateTimeStamp ;
        ns1:createdBy ns1:SpdxOrganization ;
        ns1:specVersion "3.0.1" .

    <https://spdx.org/rdf/3.0.1/creationInfo_NoneElement> a ns1:CreationInfo ;
        rdfs:comment "This individual element was defined by the spec."@en ;
        ns1:created "2024-11-22T03:00:01Z"^^xsd:dateTimeStamp ;
        ns1:createdBy ns1:SpdxOrganization ;
        ns1:specVersion "3.0.1" .

    <https://spdx.org/rdf/3.0.1/creationInfo_NoneLicense> a ns1:CreationInfo ;
        rdfs:comment "This individual element was defined by the spec."@en ;
        ns1:created "2024-11-22T03:00:01Z"^^xsd:dateTimeStamp ;
        ns1:createdBy ns1:SpdxOrganization ;
        ns1:specVersion "3.0.1" .

    <https://spdx.org/rdf/3.0.1/creationInfo_SpdxOrganization> a ns1:CreationInfo ;
        rdfs:comment "This individual element was defined by the spec."@en ;
        ns1:created "2024-11-22T03:00:01Z"^^xsd:dateTimeStamp ;
        ns1:createdBy ns1:SpdxOrganization ;
        ns1:specVersion "3.0.1" .

    spdx: a owl:Ontology ;
        rdfs:label "System Package Data Exchange (SPDX) Ontology"@en ;
        dcterms:abstract "This ontology defines the terms and relationships used in the SPDX specification to describe system packages"@en ;
        dcterms:created "2024-04-05"^^xsd:date ;
        dcterms:creator "SPDX Project"@en ;
        dcterms:license <https://spdx.org/licenses/Community-Spec-1.0.html> ;
        dcterms:references <https://spdx.dev/specifications/> ;
        dcterms:title "System Package Data Exchange (SPDX) Ontology"@en ;
        owl:versionIRI spdx: ;
        omg-ann:copyright "Copyright (C) 2024 SPDX Project"@en .

    <https://spdx.org/rdf/3.0.1/terms/AI/EnergyUnitType/kilowattHour> a owl:NamedIndividual,
            ns4:EnergyUnitType ;
        rdfs:label "kilowattHour" ;
        rdfs:comment "Kilowatt-hour."@en .

    <https://spdx.org/rdf/3.0.1/terms/AI/EnergyUnitType/megajoule> a owl:NamedIndividual,
            ns4:EnergyUnitType ;
        rdfs:label "megajoule" ;
        rdfs:comment "Megajoule."@en .

    <https://spdx.org/rdf/3.0.1/terms/AI/EnergyUnitType/other> a owl:NamedIndividual,
            ns4:EnergyUnitType ;
        rdfs:label "other" ;
        rdfs:comment "Any other units of energy measurement."@en .

    <https://spdx.org/rdf/3.0.1/terms/AI/SafetyRiskAssessmentType/high> a owl:NamedIndividual,
            ns4:SafetyRiskAssessmentType ;
        rdfs:label "high" ;
        rdfs:comment "The second-highest level of risk posed by an AI system."@en .

    <https://spdx.org/rdf/3.0.1/terms/AI/SafetyRiskAssessmentType/low> a owl:NamedIndividual,
            ns4:SafetyRiskAssessmentType ;
        rdfs:label "low" ;
        rdfs:comment "Low/no risk is posed by an AI system."@en .

    <https://spdx.org/rdf/3.0.1/terms/AI/SafetyRiskAssessmentType/medium> a owl:NamedIndividual,
            ns4:SafetyRiskAssessmentType ;
        rdfs:label "medium" ;
        rdfs:comment "The third-highest level of risk posed by an AI system."@en .

    <https://spdx.org/rdf/3.0.1/terms/AI/SafetyRiskAssessmentType/serious> a owl:NamedIndividual,
            ns4:SafetyRiskAssessmentType ;
        rdfs:label "serious" ;
        rdfs:comment "The highest level of risk posed by an AI system."@en .

    ns4:autonomyType a owl:ObjectProperty ;
        rdfs:comment """Indicates whether the system can perform a decision or action without human
involvement or guidance."""@en ;
        rdfs:range ns1:PresenceType .

    ns4:domain a owl:DatatypeProperty ;
        rdfs:comment "Captures the domain in which the AI package can be used."@en ;
        rdfs:range xsd:string .

    ns4:energyConsumption a owl:ObjectProperty ;
        rdfs:comment "Indicates the amount of energy consumption incurred by an AI model."@en ;
        rdfs:range ns4:EnergyConsumption .

    ns4:energyQuantity a owl:DatatypeProperty ;
        rdfs:comment "Represents the energy quantity."@en ;
        rdfs:range xsd:decimal .

    ns4:energyUnit a owl:ObjectProperty ;
        rdfs:comment "Specifies the unit in which energy is measured."@en ;
        rdfs:range ns4:EnergyUnitType .

    ns4:finetuningEnergyConsumption a owl:ObjectProperty ;
        rdfs:comment """Specifies the amount of energy consumed when finetuning the AI model that is
being used in the AI system."""@en ;
        rdfs:range ns4:EnergyConsumptionDescription .

    ns4:hyperparameter a owl:ObjectProperty ;
        rdfs:comment """Records a hyperparameter used to build the AI model contained in the AI
package."""@en ;
        rdfs:range ns1:DictionaryEntry .

    ns4:inferenceEnergyConsumption a owl:ObjectProperty ;
        rdfs:comment """Specifies the amount of energy consumed during inference time by an AI model
that is being used in the AI system."""@en ;
        rdfs:range ns4:EnergyConsumptionDescription .

    ns4:informationAboutApplication a owl:DatatypeProperty ;
        rdfs:comment """Provides relevant information about the AI software, not including the model
description."""@en ;
        rdfs:range xsd:string .

    ns4:informationAboutTraining a owl:DatatypeProperty ;
        rdfs:comment "Describes relevant information about different steps of the training process."@en ;
        rdfs:range xsd:string .

    ns4:limitation a owl:DatatypeProperty ;
        rdfs:comment "Captures a limitation of the AI software."@en ;
        rdfs:range xsd:string .

    ns4:metric a owl:ObjectProperty ;
        rdfs:comment "Records the measurement of prediction quality of the AI model."@en ;
        rdfs:range ns1:DictionaryEntry .

    ns4:metricDecisionThreshold a owl:ObjectProperty ;
        rdfs:comment """Captures the threshold that was used for computation of a metric described in
the metric field."""@en ;
        rdfs:range ns1:DictionaryEntry .

    ns4:modelDataPreprocessing a owl:DatatypeProperty ;
        rdfs:comment """Describes all the preprocessing steps applied to the training data before the
model training."""@en ;
        rdfs:range xsd:string .

    ns4:modelExplainability a owl:DatatypeProperty ;
        rdfs:comment "Describes methods that can be used to explain the results from the AI model."@en ;
        rdfs:range xsd:string .

    ns4:safetyRiskAssessment a owl:ObjectProperty ;
        rdfs:comment "Records the results of general safety risk assessment of the AI system."@en ;
        rdfs:range ns4:SafetyRiskAssessmentType .

    ns4:standardCompliance a owl:DatatypeProperty ;
        rdfs:comment "Captures a standard that is being complied with."@en ;
        rdfs:range xsd:string .

    ns4:trainingEnergyConsumption a owl:ObjectProperty ;
        rdfs:comment """Specifies the amount of energy consumed when training the AI model that is
being used in the AI system."""@en ;
        rdfs:range ns4:EnergyConsumptionDescription .

    ns4:typeOfModel a owl:DatatypeProperty ;
        rdfs:comment "Records the type of the model used in the AI software."@en ;
        rdfs:range xsd:string .

    ns4:useSensitivePersonalInformation a owl:ObjectProperty ;
        rdfs:comment """Records if sensitive personal information is used during model training or
could be used during the inference."""@en ;
        rdfs:range ns1:PresenceType .

    <https://spdx.org/rdf/3.0.1/terms/Build/buildEndTime> a owl:DatatypeProperty ;
        rdfs:comment "Property that describes the time at which a build stops."@en ;
        rdfs:range xsd:dateTimeStamp .

    <https://spdx.org/rdf/3.0.1/terms/Build/buildId> a owl:DatatypeProperty ;
        rdfs:comment """A buildId is a locally unique identifier used by a builder to identify a unique
instance of a build produced by it."""@en ;
        rdfs:range xsd:string .

    <https://spdx.org/rdf/3.0.1/terms/Build/buildStartTime> a owl:DatatypeProperty ;
        rdfs:comment "Property describing the start time of a build."@en ;
        rdfs:range xsd:dateTimeStamp .

    <https://spdx.org/rdf/3.0.1/terms/Build/buildType> a owl:DatatypeProperty ;
        rdfs:comment """A buildType is a hint that is used to indicate the toolchain, platform, or
infrastructure that the build was invoked on."""@en ;
        rdfs:range xsd:anyURI .

    <https://spdx.org/rdf/3.0.1/terms/Build/configSourceDigest> a owl:ObjectProperty ;
        rdfs:comment """Property that describes the digest of the build configuration file used to
invoke a build."""@en ;
        rdfs:range ns1:Hash .

    <https://spdx.org/rdf/3.0.1/terms/Build/configSourceEntrypoint> a owl:DatatypeProperty ;
        rdfs:comment "Property describes the invocation entrypoint of a build."@en ;
        rdfs:range xsd:string .

    <https://spdx.org/rdf/3.0.1/terms/Build/configSourceUri> a owl:DatatypeProperty ;
        rdfs:comment "Property that describes the URI of the build configuration source file."@en ;
        rdfs:range xsd:anyURI .

    <https://spdx.org/rdf/3.0.1/terms/Build/environment> a owl:ObjectProperty ;
        rdfs:comment "Property describing the session in which a build is invoked."@en ;
        rdfs:range ns1:DictionaryEntry .

    <https://spdx.org/rdf/3.0.1/terms/Build/parameter> a owl:ObjectProperty ;
        rdfs:comment "Property describing a parameter used in an instance of a build."@en ;
        rdfs:range ns1:DictionaryEntry .

    <https://spdx.org/rdf/3.0.1/terms/Core/AnnotationType/other> a owl:NamedIndividual,
            ns1:AnnotationType ;
        rdfs:label "other" ;
        rdfs:comment "Used to store extra information about an Element which is not part of a review (e.g. extra information provided during the creation of the Element)."@en .

    <https://spdx.org/rdf/3.0.1/terms/Core/AnnotationType/review> a owl:NamedIndividual,
            ns1:AnnotationType ;
        rdfs:label "review" ;
        rdfs:comment "Used when someone reviews the Element."@en .

    ns1:Bom a owl:Class ;
        rdfs:comment """A container for a grouping of SPDX-3.0 content characterizing details
(provenence, composition, licensing, etc.) about a product."""@en ;
        rdfs:subClassOf ns1:Bundle ;
        sh:nodeKind sh:IRI .

    ns1:Bundle a owl:Class,
            sh:NodeShape ;
        rdfs:comment "A collection of Elements that have a shared context."@en ;
        rdfs:subClassOf ns1:ElementCollection ;
        sh:nodeKind sh:IRI ;
        sh:property _:N35836a4c17134e0a83641bd266843b1f .

    <https://spdx.org/rdf/3.0.1/terms/Core/ExternalIdentifierType/cpe22> a owl:NamedIndividual,
            ns1:ExternalIdentifierType ;
        rdfs:label "cpe22" ;
        rdfs:comment "[Common Platform Enumeration Specification 2.2](https://cpe.mitre.org/files/cpe-specification_2.2.pdf)"@en .

    <https://spdx.org/rdf/3.0.1/terms/Core/ExternalIdentifierType/cpe23> a owl:NamedIndividual,
            ns1:ExternalIdentifierType ;
        rdfs:label "cpe23" ;
        rdfs:comment "[Common Platform Enumeration: Naming Specification Version 2.3](https://csrc.nist.gov/publications/detail/nistir/7695/final)"@en .

    <https://spdx.org/rdf/3.0.1/terms/Core/ExternalIdentifierType/cve> a owl:NamedIndividual,
            ns1:ExternalIdentifierType ;
        rdfs:label "cve" ;
        rdfs:comment "Common Vulnerabilities and Exposures identifiers, an identifier for a specific software flaw defined within the official CVE Dictionary and that conforms to the [CVE specification](https://csrc.nist.gov/glossary/term/cve_id)."@en .

    <https://spdx.org/rdf/3.0.1/terms/Core/ExternalIdentifierType/email> a owl:NamedIndividual,
            ns1:ExternalIdentifierType ;
        rdfs:label "email" ;
        rdfs:comment "Email address, as defined in [RFC 3696](https://datatracker.ietf.org/doc/rfc3986/) Section 3."@en .

    <https://spdx.org/rdf/3.0.1/terms/Core/ExternalIdentifierType/gitoid> a owl:NamedIndividual,
            ns1:ExternalIdentifierType ;
        rdfs:label "gitoid" ;
        rdfs:comment "[Gitoid](https://www.iana.org/assignments/uri-schemes/prov/gitoid), stands for [Git Object ID](https://git-scm.com/book/en/v2/Git-Internals-Git-Objects). A gitoid of type blob is a unique hash of a binary artifact. A gitoid may represent either an [Artifact Identifier](https://github.com/omnibor/spec/blob/eb1ee5c961c16215eb8709b2975d193a2007a35d/spec/SPEC.md#artifact-identifier-types) for the software artifact or an [Input Manifest Identifier](https://github.com/omnibor/spec/blob/eb1ee5c961c16215eb8709b2975d193a2007a35d/spec/SPEC.md#input-manifest-identifier) for the software artifact's associated [Artifact Input Manifest](https://github.com/omnibor/spec/blob/eb1ee5c961c16215eb8709b2975d193a2007a35d/spec/SPEC.md#artifact-input-manifest); this ambiguity exists because the Artifact Input Manifest is itself an artifact, and the gitoid of that artifact is its valid identifier. Gitoids calculated on software artifacts (Snippet, File, or Package Elements) should be recorded in the SPDX 3.0 SoftwareArtifact's contentIdentifier property. Gitoids calculated on the Artifact Input Manifest (Input Manifest Identifier) should be recorded in the SPDX 3.0 Element's externalIdentifier property. See [OmniBOR Specification](https://github.com/omnibor/spec/), a minimalistic specification for describing software [Artifact Dependency Graphs](https://github.com/omnibor/spec/blob/eb1ee5c961c16215eb8709b2975d193a2007a35d/spec/SPEC.md#artifact-dependency-graph-adg)."@en .

    <https://spdx.org/rdf/3.0.1/terms/Core/ExternalIdentifierType/other> a owl:NamedIndividual,
            ns1:ExternalIdentifierType ;
        rdfs:label "other" ;
        rdfs:comment "Used when the type does not match any of the other options."@en .

    <https://spdx.org/rdf/3.0.1/terms/Core/ExternalIdentifierType/packageUrl> a owl:NamedIndividual,
            ns1:ExternalIdentifierType ;
        rdfs:label "packageUrl" ;
        rdfs:comment "Package URL, as defined in the corresponding [Annex](../../../annexes/pkg-url-specification.md) of this specification."@en .

    <https://spdx.org/rdf/3.0.1/terms/Core/ExternalIdentifierType/securityOther> a owl:NamedIndividual,
            ns1:ExternalIdentifierType ;
        rdfs:label "securityOther" ;
        rdfs:comment "Used when there is a security related identifier of unspecified type."@en .

    <https://spdx.org/rdf/3.0.1/terms/Core/ExternalIdentifierType/swhid> a owl:NamedIndividual,
            ns1:ExternalIdentifierType ;
        rdfs:label "swhid" ;
        rdfs:comment "SoftWare Hash IDentifier, a persistent intrinsic identifier for digital artifacts, such as files, trees (also known as directories or folders), commits, and other objects typically found in version control systems. The format of the identifiers is defined in the [SWHID specification](https://www.swhid.org/specification/v1.1/4.Syntax) (ISO/IEC DIS 18670). They typically look like `swh:1:cnt:94a9ed024d3859793618152ea559a168bbcbb5e2`."@en .

    <https://spdx.org/rdf/3.0.1/terms/Core/ExternalIdentifierType/swid> a owl:NamedIndividual,
            ns1:ExternalIdentifierType ;
        rdfs:label "swid" ;
        rdfs:comment "Concise Software Identification (CoSWID) tag, as defined in [RFC 9393](https://datatracker.ietf.org/doc/rfc9393/) Section 2.3."@en .

    <https://spdx.org/rdf/3.0.1/terms/Core/ExternalIdentifierType/urlScheme> a owl:NamedIndividual,
            ns1:ExternalIdentifierType ;
        rdfs:label "urlScheme" ;
        rdfs:comment "[Uniform Resource Identifier (URI) Schemes](https://www.iana.org/assignments/uri-schemes/uri-schemes.xhtml). The scheme used in order to locate a resource."@en .

    <https://spdx.org/rdf/3.0.1/terms/Core/ExternalRefType/altDownloadLocation> a owl:NamedIndividual,
            ns1:ExternalRefType ;
        rdfs:label "altDownloadLocation" ;
        rdfs:comment "A reference to an alternative download location."@en .

    <https://spdx.org/rdf/3.0.1/terms/Core/ExternalRefType/altWebPage> a owl:NamedIndividual,
            ns1:ExternalRefType ;
        rdfs:label "altWebPage" ;
        rdfs:comment "A reference to an alternative web page."@en .

    <https://spdx.org/rdf/3.0.1/terms/Core/ExternalRefType/binaryArtifact> a owl:NamedIndividual,
            ns1:ExternalRefType ;
        rdfs:label "binaryArtifact" ;
        rdfs:comment "A reference to binary artifacts related to a package."@en .

    <https://spdx.org/rdf/3.0.1/terms/Core/ExternalRefType/bower> a owl:NamedIndividual,
            ns1:ExternalRefType ;
        rdfs:label "bower" ;
        rdfs:comment "A reference to a Bower package. The package locator format, looks like `package#version`, is defined in the \"install\" section of [Bower API documentation](https://bower.io/docs/api/#install)."@en .

    <https://spdx.org/rdf/3.0.1/terms/Core/ExternalRefType/buildMeta> a owl:NamedIndividual,
            ns1:ExternalRefType ;
        rdfs:label "buildMeta" ;
        rdfs:comment "A reference build metadata related to a published package."@en .

    <https://spdx.org/rdf/3.0.1/terms/Core/ExternalRefType/buildSystem> a owl:NamedIndividual,
            ns1:ExternalRefType ;
        rdfs:label "buildSystem" ;
        rdfs:comment "A reference build system used to create or publish the package."@en .

    <https://spdx.org/rdf/3.0.1/terms/Core/ExternalRefType/certificationReport> a owl:NamedIndividual,
            ns1:ExternalRefType ;
        rdfs:label "certificationReport" ;
        rdfs:comment "A reference to a certification report for a package from an accredited/independent body."@en .

    <https://spdx.org/rdf/3.0.1/terms/Core/ExternalRefType/chat> a owl:NamedIndividual,
            ns1:ExternalRefType ;
        rdfs:label "chat" ;
        rdfs:comment "A reference to the instant messaging system used by the maintainer for a package."@en .

    <https://spdx.org/rdf/3.0.1/terms/Core/ExternalRefType/componentAnalysisReport> a owl:NamedIndividual,
            ns1:ExternalRefType ;
        rdfs:label "componentAnalysisReport" ;
        rdfs:comment "A reference to a Software Composition Analysis (SCA) report."@en .

    <https://spdx.org/rdf/3.0.1/terms/Core/ExternalRefType/cwe> a owl:NamedIndividual,
            ns1:ExternalRefType ;
        rdfs:label "cwe" ;
        rdfs:comment "[Common Weakness Enumeration](https://csrc.nist.gov/glossary/term/common_weakness_enumeration). A reference to a source of software flaw defined within the official [CWE List](https://cwe.mitre.org/data/) that conforms to the [CWE specification](https://cwe.mitre.org/)."@en .

    <https://spdx.org/rdf/3.0.1/terms/Core/ExternalRefType/documentation> a owl:NamedIndividual,
            ns1:ExternalRefType ;
        rdfs:label "documentation" ;
        rdfs:comment "A reference to the documentation for a package."@en .

    <https://spdx.org/rdf/3.0.1/terms/Core/ExternalRefType/dynamicAnalysisReport> a owl:NamedIndividual,
            ns1:ExternalRefType ;
        rdfs:label "dynamicAnalysisReport" ;
        rdfs:comment "A reference to a dynamic analysis report for a package."@en .

    <https://spdx.org/rdf/3.0.1/terms/Core/ExternalRefType/eolNotice> a owl:NamedIndividual,
            ns1:ExternalRefType ;
        rdfs:label "eolNotice" ;
        rdfs:comment "A reference to the End Of Sale (EOS) and/or End Of Life (EOL) information related to a package."@en .

    <https://spdx.org/rdf/3.0.1/terms/Core/ExternalRefType/exportControlAssessment> a owl:NamedIndividual,
            ns1:ExternalRefType ;
        rdfs:label "exportControlAssessment" ;
        rdfs:comment "A reference to a export control assessment for a package."@en .

    <https://spdx.org/rdf/3.0.1/terms/Core/ExternalRefType/funding> a owl:NamedIndividual,
            ns1:ExternalRefType ;
        rdfs:label "funding" ;
        rdfs:comment "A reference to funding information related to a package."@en .

    <https://spdx.org/rdf/3.0.1/terms/Core/ExternalRefType/issueTracker> a owl:NamedIndividual,
            ns1:ExternalRefType ;
        rdfs:label "issueTracker" ;
        rdfs:comment "A reference to the issue tracker for a package."@en .

    <https://spdx.org/rdf/3.0.1/terms/Core/ExternalRefType/license> a owl:NamedIndividual,
            ns1:ExternalRefType ;
        rdfs:label "license" ;
        rdfs:comment "A reference to additional license information related to an artifact."@en .

    <https://spdx.org/rdf/3.0.1/terms/Core/ExternalRefType/mailingList> a owl:NamedIndividual,
            ns1:ExternalRefType ;
        rdfs:label "mailingList" ;
        rdfs:comment "A reference to the mailing list used by the maintainer for a package."@en .

    <https://spdx.org/rdf/3.0.1/terms/Core/ExternalRefType/mavenCentral> a owl:NamedIndividual,
            ns1:ExternalRefType ;
        rdfs:label "mavenCentral" ;
        rdfs:comment "A reference to a Maven repository artifact. The artifact locator format is defined in the [Maven documentation](https://maven.apache.org/guides/mini/guide-naming-conventions.html) and looks like `groupId:artifactId[:version]`."@en .

    <https://spdx.org/rdf/3.0.1/terms/Core/ExternalRefType/metrics> a owl:NamedIndividual,
            ns1:ExternalRefType ;
        rdfs:label "metrics" ;
        rdfs:comment "A reference to metrics related to package such as OpenSSF scorecards."@en .

    <https://spdx.org/rdf/3.0.1/terms/Core/ExternalRefType/npm> a owl:NamedIndividual,
            ns1:ExternalRefType ;
        rdfs:label "npm" ;
        rdfs:comment "A reference to an npm package. The package locator format is defined in the [npm documentation](https://docs.npmjs.com/cli/v10/configuring-npm/package-json) and looks like `package@version`."@en .

    <https://spdx.org/rdf/3.0.1/terms/Core/ExternalRefType/nuget> a owl:NamedIndividual,
            ns1:ExternalRefType ;
        rdfs:label "nuget" ;
        rdfs:comment "A reference to a NuGet package. The package locator format is defined in the [NuGet documentation](https://docs.nuget.org) and looks like `package/version`."@en .

    <https://spdx.org/rdf/3.0.1/terms/Core/ExternalRefType/other> a owl:NamedIndividual,
            ns1:ExternalRefType ;
        rdfs:label "other" ;
        rdfs:comment "Used when the type does not match any of the other options."@en .

    <https://spdx.org/rdf/3.0.1/terms/Core/ExternalRefType/privacyAssessment> a owl:NamedIndividual,
            ns1:ExternalRefType ;
        rdfs:label "privacyAssessment" ;
        rdfs:comment "A reference to a privacy assessment for a package."@en .

    <https://spdx.org/rdf/3.0.1/terms/Core/ExternalRefType/productMetadata> a owl:NamedIndividual,
            ns1:ExternalRefType ;
        rdfs:label "productMetadata" ;
        rdfs:comment "A reference to additional product metadata such as reference within organization's product catalog."@en .

    <https://spdx.org/rdf/3.0.1/terms/Core/ExternalRefType/purchaseOrder> a owl:NamedIndividual,
            ns1:ExternalRefType ;
        rdfs:label "purchaseOrder" ;
        rdfs:comment "A reference to a purchase order for a package."@en .

    <https://spdx.org/rdf/3.0.1/terms/Core/ExternalRefType/qualityAssessmentReport> a owl:NamedIndividual,
            ns1:ExternalRefType ;
        rdfs:label "qualityAssessmentReport" ;
        rdfs:comment "A reference to a quality assessment for a package."@en .

    <https://spdx.org/rdf/3.0.1/terms/Core/ExternalRefType/releaseHistory> a owl:NamedIndividual,
            ns1:ExternalRefType ;
        rdfs:label "releaseHistory" ;
        rdfs:comment "A reference to a published list of releases for a package."@en .

    <https://spdx.org/rdf/3.0.1/terms/Core/ExternalRefType/releaseNotes> a owl:NamedIndividual,
            ns1:ExternalRefType ;
        rdfs:label "releaseNotes" ;
        rdfs:comment "A reference to the release notes for a package."@en .

    <https://spdx.org/rdf/3.0.1/terms/Core/ExternalRefType/riskAssessment> a owl:NamedIndividual,
            ns1:ExternalRefType ;
        rdfs:label "riskAssessment" ;
        rdfs:comment "A reference to a risk assessment for a package."@en .

    <https://spdx.org/rdf/3.0.1/terms/Core/ExternalRefType/runtimeAnalysisReport> a owl:NamedIndividual,
            ns1:ExternalRefType ;
        rdfs:label "runtimeAnalysisReport" ;
        rdfs:comment "A reference to a runtime analysis report for a package."@en .

    <https://spdx.org/rdf/3.0.1/terms/Core/ExternalRefType/secureSoftwareAttestation> a owl:NamedIndividual,
            ns1:ExternalRefType ;
        rdfs:label "secureSoftwareAttestation" ;
        rdfs:comment "A reference to information assuring that the software is developed using security practices as defined by [NIST SP 800-218 Secure Software Development Framework (SSDF) Version 1.1](https://csrc.nist.gov/pubs/sp/800/218/final) or [CISA Secure Software Development Attestation Form](https://www.cisa.gov/resources-tools/resources/secure-software-development-attestation-form)."@en .

    <https://spdx.org/rdf/3.0.1/terms/Core/ExternalRefType/securityAdversaryModel> a owl:NamedIndividual,
            ns1:ExternalRefType ;
        rdfs:label "securityAdversaryModel" ;
        rdfs:comment "A reference to the security adversary model for a package."@en .

    <https://spdx.org/rdf/3.0.1/terms/Core/ExternalRefType/securityAdvisory> a owl:NamedIndividual,
            ns1:ExternalRefType ;
        rdfs:label "securityAdvisory" ;
        rdfs:comment "A reference to a published security advisory (where advisory as defined per [ISO 29147:2018](https://www.iso.org/standard/72311.html)) that may affect one or more elements, e.g., vendor advisories or specific NVD entries."@en .

    <https://spdx.org/rdf/3.0.1/terms/Core/ExternalRefType/securityFix> a owl:NamedIndividual,
            ns1:ExternalRefType ;
        rdfs:label "securityFix" ;
        rdfs:comment "A reference to the patch or source code that fixes a vulnerability."@en .

    <https://spdx.org/rdf/3.0.1/terms/Core/ExternalRefType/securityOther> a owl:NamedIndividual,
            ns1:ExternalRefType ;
        rdfs:label "securityOther" ;
        rdfs:comment "A reference to related security information of unspecified type."@en .

    <https://spdx.org/rdf/3.0.1/terms/Core/ExternalRefType/securityPenTestReport> a owl:NamedIndividual,
            ns1:ExternalRefType ;
        rdfs:label "securityPenTestReport" ;
        rdfs:comment "A reference to a [penetration test](https://en.wikipedia.org/wiki/Penetration_test) report for a package."@en .

    <https://spdx.org/rdf/3.0.1/terms/Core/ExternalRefType/securityPolicy> a owl:NamedIndividual,
            ns1:ExternalRefType ;
        rdfs:label "securityPolicy" ;
        rdfs:comment "A reference to instructions for reporting newly discovered security vulnerabilities for a package."@en .

    <https://spdx.org/rdf/3.0.1/terms/Core/ExternalRefType/securityThreatModel> a owl:NamedIndividual,
            ns1:ExternalRefType ;
        rdfs:label "securityThreatModel" ;
        rdfs:comment "A reference the [security threat model](https://en.wikipedia.org/wiki/Threat_model) for a package."@en .

    <https://spdx.org/rdf/3.0.1/terms/Core/ExternalRefType/socialMedia> a owl:NamedIndividual,
            ns1:ExternalRefType ;
        rdfs:label "socialMedia" ;
        rdfs:comment "A reference to a social media channel for a package."@en .

    <https://spdx.org/rdf/3.0.1/terms/Core/ExternalRefType/sourceArtifact> a owl:NamedIndividual,
            ns1:ExternalRefType ;
        rdfs:label "sourceArtifact" ;
        rdfs:comment "A reference to an artifact containing the sources for a package."@en .

    <https://spdx.org/rdf/3.0.1/terms/Core/ExternalRefType/staticAnalysisReport> a owl:NamedIndividual,
            ns1:ExternalRefType ;
        rdfs:label "staticAnalysisReport" ;
        rdfs:comment "A reference to a static analysis report for a package."@en .

    <https://spdx.org/rdf/3.0.1/terms/Core/ExternalRefType/support> a owl:NamedIndividual,
            ns1:ExternalRefType ;
        rdfs:label "support" ;
        rdfs:comment "A reference to the software support channel or other support information for a package."@en .

    <https://spdx.org/rdf/3.0.1/terms/Core/ExternalRefType/vcs> a owl:NamedIndividual,
            ns1:ExternalRefType ;
        rdfs:label "vcs" ;
        rdfs:comment "A reference to a version control system related to a software artifact."@en .

    <https://spdx.org/rdf/3.0.1/terms/Core/ExternalRefType/vulnerabilityDisclosureReport> a owl:NamedIndividual,
            ns1:ExternalRefType ;
        rdfs:label "vulnerabilityDisclosureReport" ;
        rdfs:comment "A reference to a Vulnerability Disclosure Report (VDR) which provides the software supplier's analysis and findings describing the impact (or lack of impact) that reported vulnerabilities have on packages or products in the supplier's SBOM as defined in [NIST SP 800-161 Cybersecurity Supply Chain Risk Management Practices for Systems and Organizations](https://csrc.nist.gov/pubs/sp/800/161/r1/final)."@en .

    <https://spdx.org/rdf/3.0.1/terms/Core/ExternalRefType/vulnerabilityExploitabilityAssessment> a owl:NamedIndividual,
            ns1:ExternalRefType ;
        rdfs:label "vulnerabilityExploitabilityAssessment" ;
        rdfs:comment "A reference to a Vulnerability Exploitability eXchange (VEX) statement which provides information on whether a product is impacted by a specific vulnerability in an included package and, if affected, whether there are actions recommended to remediate. See also [NTIA VEX one-page summary](https://ntia.gov/files/ntia/publications/vex_one-page_summary.pdf)."@en .

    <https://spdx.org/rdf/3.0.1/terms/Core/LifecycleScopeType/build> a owl:NamedIndividual,
            ns1:LifecycleScopeType ;
        rdfs:label "build" ;
        rdfs:comment "A relationship has specific context implications during an element's build phase, during development."@en .

    <https://spdx.org/rdf/3.0.1/terms/Core/LifecycleScopeType/design> a owl:NamedIndividual,
            ns1:LifecycleScopeType ;
        rdfs:label "design" ;
        rdfs:comment "A relationship has specific context implications during an element's design."@en .

    <https://spdx.org/rdf/3.0.1/terms/Core/LifecycleScopeType/development> a owl:NamedIndividual,
            ns1:LifecycleScopeType ;
        rdfs:label "development" ;
        rdfs:comment "A relationship has specific context implications during development phase of an element."@en .

    <https://spdx.org/rdf/3.0.1/terms/Core/LifecycleScopeType/other> a owl:NamedIndividual,
            ns1:LifecycleScopeType ;
        rdfs:label "other" ;
        rdfs:comment "A relationship has other specific context information necessary to capture that the above set of enumerations does not handle."@en .

    <https://spdx.org/rdf/3.0.1/terms/Core/LifecycleScopeType/runtime> a owl:NamedIndividual,
            ns1:LifecycleScopeType ;
        rdfs:label "runtime" ;
        rdfs:comment "A relationship has specific context implications during the execution phase of an element."@en .

    <https://spdx.org/rdf/3.0.1/terms/Core/LifecycleScopeType/test> a owl:NamedIndividual,
            ns1:LifecycleScopeType ;
        rdfs:label "test" ;
        rdfs:comment "A relationship has specific context implications during an element's testing phase, during development."@en .

    ns1:Organization a owl:Class ;
        rdfs:comment "A group of people who work together in an organized way for a shared purpose."@en ;
        rdfs:subClassOf ns1:Agent ;
        sh:nodeKind sh:IRI .

    <https://spdx.org/rdf/3.0.1/terms/Core/ProfileIdentifierType/ai> a owl:NamedIndividual,
            ns1:ProfileIdentifierType ;
        rdfs:label "ai" ;
        rdfs:comment "the element follows the AI profile specification"@en .

    <https://spdx.org/rdf/3.0.1/terms/Core/ProfileIdentifierType/build> a owl:NamedIndividual,
            ns1:ProfileIdentifierType ;
        rdfs:label "build" ;
        rdfs:comment "the element follows the Build profile specification"@en .

    <https://spdx.org/rdf/3.0.1/terms/Core/ProfileIdentifierType/core> a owl:NamedIndividual,
            ns1:ProfileIdentifierType ;
        rdfs:label "core" ;
        rdfs:comment "the element follows the Core profile specification"@en .

    <https://spdx.org/rdf/3.0.1/terms/Core/ProfileIdentifierType/dataset> a owl:NamedIndividual,
            ns1:ProfileIdentifierType ;
        rdfs:label "dataset" ;
        rdfs:comment "the element follows the Dataset profile specification"@en .

    <https://spdx.org/rdf/3.0.1/terms/Core/ProfileIdentifierType/expandedLicensing> a owl:NamedIndividual,
            ns1:ProfileIdentifierType ;
        rdfs:label "expandedLicensing" ;
        rdfs:comment "the element follows the ExpandedLicensing profile specification"@en .

    <https://spdx.org/rdf/3.0.1/terms/Core/ProfileIdentifierType/extension> a owl:NamedIndividual,
            ns1:ProfileIdentifierType ;
        rdfs:label "extension" ;
        rdfs:comment "the element follows the Extension profile specification"@en .

    <https://spdx.org/rdf/3.0.1/terms/Core/ProfileIdentifierType/lite> a owl:NamedIndividual,
            ns1:ProfileIdentifierType ;
        rdfs:label "lite" ;
        rdfs:comment "the element follows the Lite profile specification"@en .

    <https://spdx.org/rdf/3.0.1/terms/Core/ProfileIdentifierType/security> a owl:NamedIndividual,
            ns1:ProfileIdentifierType ;
        rdfs:label "security" ;
        rdfs:comment "the element follows the Security profile specification"@en .

    <https://spdx.org/rdf/3.0.1/terms/Core/ProfileIdentifierType/simpleLicensing> a owl:NamedIndividual,
            ns1:ProfileIdentifierType ;
        rdfs:label "simpleLicensing" ;
        rdfs:comment "the element follows the SimpleLicensing profile specification"@en .

    <https://spdx.org/rdf/3.0.1/terms/Core/ProfileIdentifierType/software> a owl:NamedIndividual,
            ns1:ProfileIdentifierType ;
        rdfs:label "software" ;
        rdfs:comment "the element follows the Software profile specification"@en .

    <https://spdx.org/rdf/3.0.1/terms/Core/RelationshipCompleteness/complete> a owl:NamedIndividual,
            ns1:RelationshipCompleteness ;
        rdfs:label "complete" ;
        rdfs:comment "The relationship is known to be exhaustive."@en .

    <https://spdx.org/rdf/3.0.1/terms/Core/RelationshipCompleteness/incomplete> a owl:NamedIndividual,
            ns1:RelationshipCompleteness ;
        rdfs:label "incomplete" ;
        rdfs:comment "The relationship is known not to be exhaustive."@en .

    <https://spdx.org/rdf/3.0.1/terms/Core/RelationshipCompleteness/noAssertion> a owl:NamedIndividual,
            ns1:RelationshipCompleteness ;
        rdfs:label "noAssertion" ;
        rdfs:comment "No assertion can be made about the completeness of the relationship."@en .

    <https://spdx.org/rdf/3.0.1/terms/Core/RelationshipType/affects> a owl:NamedIndividual,
            ns1:RelationshipType ;
        rdfs:label "affects" ;
        rdfs:comment "The `from` Vulnerability affects each `to` Element. The use of the `affects` type is constrained to `VexAffectedVulnAssessmentRelationship` classed relationships."@en .

    <https://spdx.org/rdf/3.0.1/terms/Core/RelationshipType/amendedBy> a owl:NamedIndividual,
            ns1:RelationshipType ;
        rdfs:label "amendedBy" ;
        rdfs:comment "The `from` Element is amended by each `to` Element."@en .

    <https://spdx.org/rdf/3.0.1/terms/Core/RelationshipType/ancestorOf> a owl:NamedIndividual,
            ns1:RelationshipType ;
        rdfs:label "ancestorOf" ;
        rdfs:comment "The `from` Element is an ancestor of each `to` Element."@en .

    <https://spdx.org/rdf/3.0.1/terms/Core/RelationshipType/availableFrom> a owl:NamedIndividual,
            ns1:RelationshipType ;
        rdfs:label "availableFrom" ;
        rdfs:comment "The `from` Element is available from the additional supplier described by each `to` Element."@en .

    <https://spdx.org/rdf/3.0.1/terms/Core/RelationshipType/configures> a owl:NamedIndividual,
            ns1:RelationshipType ;
        rdfs:label "configures" ;
        rdfs:comment "The `from` Element is a configuration applied to each `to` Element, during a LifecycleScopeType period."@en .

    <https://spdx.org/rdf/3.0.1/terms/Core/RelationshipType/contains> a owl:NamedIndividual,
            ns1:RelationshipType ;
        rdfs:label "contains" ;
        rdfs:comment "The `from` Element contains each `to` Element."@en .

    <https://spdx.org/rdf/3.0.1/terms/Core/RelationshipType/coordinatedBy> a owl:NamedIndividual,
            ns1:RelationshipType ;
        rdfs:label "coordinatedBy" ;
        rdfs:comment "The `from` Vulnerability is coordinatedBy the `to` Agent(s) (vendor, researcher, or consumer agent)."@en .

    <https://spdx.org/rdf/3.0.1/terms/Core/RelationshipType/copiedTo> a owl:NamedIndividual,
            ns1:RelationshipType ;
        rdfs:label "copiedTo" ;
        rdfs:comment "The `from` Element has been copied to each `to` Element."@en .

    <https://spdx.org/rdf/3.0.1/terms/Core/RelationshipType/delegatedTo> a owl:NamedIndividual,
            ns1:RelationshipType ;
        rdfs:label "delegatedTo" ;
        rdfs:comment "The `from` Agent is delegating an action to the Agent of the `to` Relationship (which must be of type invokedBy), during a LifecycleScopeType (e.g. the `to` invokedBy Relationship is being done on behalf of `from`)."@en .

    <https://spdx.org/rdf/3.0.1/terms/Core/RelationshipType/dependsOn> a owl:NamedIndividual,
            ns1:RelationshipType ;
        rdfs:label "dependsOn" ;
        rdfs:comment "The `from` Element depends on each `to` Element, during a LifecycleScopeType period."@en .

    <https://spdx.org/rdf/3.0.1/terms/Core/RelationshipType/descendantOf> a owl:NamedIndividual,
            ns1:RelationshipType ;
        rdfs:label "descendantOf" ;
        rdfs:comment "The `from` Element is a descendant of each `to` Element."@en .

    <https://spdx.org/rdf/3.0.1/terms/Core/RelationshipType/describes> a owl:NamedIndividual,
            ns1:RelationshipType ;
        rdfs:label "describes" ;
        rdfs:comment "The `from` Element describes each `to` Element. To denote the root(s) of a tree of elements in a collection, the rootElement property should be used."@en .

    <https://spdx.org/rdf/3.0.1/terms/Core/RelationshipType/doesNotAffect> a owl:NamedIndividual,
            ns1:RelationshipType ;
        rdfs:label "doesNotAffect" ;
        rdfs:comment "The `from` Vulnerability has no impact on each `to` Element. The use of the `doesNotAffect` is constrained to `VexNotAffectedVulnAssessmentRelationship` classed relationships."@en .

    <https://spdx.org/rdf/3.0.1/terms/Core/RelationshipType/expandsTo> a owl:NamedIndividual,
            ns1:RelationshipType ;
        rdfs:label "expandsTo" ;
        rdfs:comment "The `from` archive expands out as an artifact described by each `to` Element."@en .

    <https://spdx.org/rdf/3.0.1/terms/Core/RelationshipType/exploitCreatedBy> a owl:NamedIndividual,
            ns1:RelationshipType ;
        rdfs:label "exploitCreatedBy" ;
        rdfs:comment "The `from` Vulnerability has had an exploit created against it by each `to` Agent."@en .

    <https://spdx.org/rdf/3.0.1/terms/Core/RelationshipType/fixedBy> a owl:NamedIndividual,
            ns1:RelationshipType ;
        rdfs:label "fixedBy" ;
        rdfs:comment "Designates a `from` Vulnerability has been fixed by the `to` Agent(s)."@en .

    <https://spdx.org/rdf/3.0.1/terms/Core/RelationshipType/fixedIn> a owl:NamedIndividual,
            ns1:RelationshipType ;
        rdfs:label "fixedIn" ;
        rdfs:comment "A `from` Vulnerability has been fixed in each `to` Element. The use of the `fixedIn` type is constrained to `VexFixedVulnAssessmentRelationship` classed relationships."@en .

    <https://spdx.org/rdf/3.0.1/terms/Core/RelationshipType/foundBy> a owl:NamedIndividual,
            ns1:RelationshipType ;
        rdfs:label "foundBy" ;
        rdfs:comment "Designates a `from` Vulnerability was originally discovered by the `to` Agent(s)."@en .

    <https://spdx.org/rdf/3.0.1/terms/Core/RelationshipType/generates> a owl:NamedIndividual,
            ns1:RelationshipType ;
        rdfs:label "generates" ;
        rdfs:comment "The `from` Element generates each `to` Element."@en .

    <https://spdx.org/rdf/3.0.1/terms/Core/RelationshipType/hasAddedFile> a owl:NamedIndividual,
            ns1:RelationshipType ;
        rdfs:label "hasAddedFile" ;
        rdfs:comment "Every `to` Element is a file added to the `from` Element (`from` hasAddedFile `to`)."@en .

    <https://spdx.org/rdf/3.0.1/terms/Core/RelationshipType/hasAssessmentFor> a owl:NamedIndividual,
            ns1:RelationshipType ;
        rdfs:label "hasAssessmentFor" ;
        rdfs:comment "Relates a `from` Vulnerability and each `to` Element with a security assessment. To be used with `VulnAssessmentRelationship` types."@en .

    <https://spdx.org/rdf/3.0.1/terms/Core/RelationshipType/hasAssociatedVulnerability> a owl:NamedIndividual,
            ns1:RelationshipType ;
        rdfs:label "hasAssociatedVulnerability" ;
        rdfs:comment "Used to associate a `from` Artifact with each `to` Vulnerability."@en .

    <https://spdx.org/rdf/3.0.1/terms/Core/RelationshipType/hasConcludedLicense> a owl:NamedIndividual,
            ns1:RelationshipType ;
        rdfs:label "hasConcludedLicense" ;
        rdfs:comment "The `from` SoftwareArtifact is concluded by the SPDX data creator to be governed by each `to` license."@en .

    <https://spdx.org/rdf/3.0.1/terms/Core/RelationshipType/hasDataFile> a owl:NamedIndividual,
            ns1:RelationshipType ;
        rdfs:label "hasDataFile" ;
        rdfs:comment "The `from` Element treats each `to` Element as a data file. A data file is an artifact that stores data required or optional for the `from` Element's functionality. A data file can be a database file, an index file, a log file, an AI model file, a calibration data file, a temporary file, a backup file, and more. For AI training dataset, test dataset, test artifact, configuration data, build input data, and build output data, please consider using the more specific relationship types: `trainedOn`, `testedOn`, `hasTest`, `configures`, `hasInput`, and `hasOutput`, respectively. This relationship does not imply dependency."@en .

    <https://spdx.org/rdf/3.0.1/terms/Core/RelationshipType/hasDeclaredLicense> a owl:NamedIndividual,
            ns1:RelationshipType ;
        rdfs:label "hasDeclaredLicense" ;
        rdfs:comment "The `from` SoftwareArtifact was discovered to actually contain each `to` license, for example as detected by use of automated tooling."@en .

    <https://spdx.org/rdf/3.0.1/terms/Core/RelationshipType/hasDeletedFile> a owl:NamedIndividual,
            ns1:RelationshipType ;
        rdfs:label "hasDeletedFile" ;
        rdfs:comment "Every `to` Element is a file deleted from the `from` Element (`from` hasDeletedFile `to`)."@en .

    <https://spdx.org/rdf/3.0.1/terms/Core/RelationshipType/hasDependencyManifest> a owl:NamedIndividual,
            ns1:RelationshipType ;
        rdfs:label "hasDependencyManifest" ;
        rdfs:comment "The `from` Element has manifest files that contain dependency information in each `to` Element."@en .

    <https://spdx.org/rdf/3.0.1/terms/Core/RelationshipType/hasDistributionArtifact> a owl:NamedIndividual,
            ns1:RelationshipType ;
        rdfs:label "hasDistributionArtifact" ;
        rdfs:comment "The `from` Element is distributed as an artifact in each `to` Element (e.g. an RPM or archive file)."@en .

    <https://spdx.org/rdf/3.0.1/terms/Core/RelationshipType/hasDocumentation> a owl:NamedIndividual,
            ns1:RelationshipType ;
        rdfs:label "hasDocumentation" ;
        rdfs:comment "The `from` Element is documented by each `to` Element."@en .

    <https://spdx.org/rdf/3.0.1/terms/Core/RelationshipType/hasDynamicLink> a owl:NamedIndividual,
            ns1:RelationshipType ;
        rdfs:label "hasDynamicLink" ;
        rdfs:comment "The `from` Element dynamically links in each `to` Element, during a LifecycleScopeType period."@en .

    <https://spdx.org/rdf/3.0.1/terms/Core/RelationshipType/hasEvidence> a owl:NamedIndividual,
            ns1:RelationshipType ;
        rdfs:label "hasEvidence" ;
        rdfs:comment "Every `to` Element is considered as evidence for the `from` Element (`from` hasEvidence `to`)."@en .

    <https://spdx.org/rdf/3.0.1/terms/Core/RelationshipType/hasExample> a owl:NamedIndividual,
            ns1:RelationshipType ;
        rdfs:label "hasExample" ;
        rdfs:comment "Every `to` Element is an example for the `from` Element (`from` hasExample `to`)."@en .

    <https://spdx.org/rdf/3.0.1/terms/Core/RelationshipType/hasHost> a owl:NamedIndividual,
            ns1:RelationshipType ;
        rdfs:label "hasHost" ;
        rdfs:comment "The `from` Build was run on the `to` Element during a LifecycleScopeType period (e.g. the host that the build runs on)."@en .

    <https://spdx.org/rdf/3.0.1/terms/Core/RelationshipType/hasInput> a owl:NamedIndividual,
            ns1:RelationshipType ;
        rdfs:label "hasInput" ;
        rdfs:comment "The `from` Build has each `to` Element as an input, during a LifecycleScopeType period."@en .

    <https://spdx.org/rdf/3.0.1/terms/Core/RelationshipType/hasMetadata> a owl:NamedIndividual,
            ns1:RelationshipType ;
        rdfs:label "hasMetadata" ;
        rdfs:comment "Every `to` Element is metadata about the `from` Element (`from` hasMetadata `to`)."@en .

    <https://spdx.org/rdf/3.0.1/terms/Core/RelationshipType/hasOptionalComponent> a owl:NamedIndividual,
            ns1:RelationshipType ;
        rdfs:label "hasOptionalComponent" ;
        rdfs:comment "Every `to` Element is an optional component of the `from` Element (`from` hasOptionalComponent `to`)."@en .

    <https://spdx.org/rdf/3.0.1/terms/Core/RelationshipType/hasOptionalDependency> a owl:NamedIndividual,
            ns1:RelationshipType ;
        rdfs:label "hasOptionalDependency" ;
        rdfs:comment "The `from` Element optionally depends on each `to` Element, during a LifecycleScopeType period."@en .

    <https://spdx.org/rdf/3.0.1/terms/Core/RelationshipType/hasOutput> a owl:NamedIndividual,
            ns1:RelationshipType ;
        rdfs:label "hasOutput" ;
        rdfs:comment "The `from` Build element generates each `to` Element as an output, during a LifecycleScopeType period."@en .

    <https://spdx.org/rdf/3.0.1/terms/Core/RelationshipType/hasPrerequisite> a owl:NamedIndividual,
            ns1:RelationshipType ;
        rdfs:label "hasPrerequisite" ;
        rdfs:comment "The `from` Element has a prerequisite on each `to` Element, during a LifecycleScopeType period."@en .

    <https://spdx.org/rdf/3.0.1/terms/Core/RelationshipType/hasProvidedDependency> a owl:NamedIndividual,
            ns1:RelationshipType ;
        rdfs:label "hasProvidedDependency" ;
        rdfs:comment "The `from` Element has a dependency on each `to` Element, dependency is not in the distributed artifact, but assumed to be provided, during a LifecycleScopeType period."@en .

    <https://spdx.org/rdf/3.0.1/terms/Core/RelationshipType/hasRequirement> a owl:NamedIndividual,
            ns1:RelationshipType ;
        rdfs:label "hasRequirement" ;
        rdfs:comment "The `from` Element has a requirement on each `to` Element, during a LifecycleScopeType period."@en .

    <https://spdx.org/rdf/3.0.1/terms/Core/RelationshipType/hasSpecification> a owl:NamedIndividual,
            ns1:RelationshipType ;
        rdfs:label "hasSpecification" ;
        rdfs:comment "Every `to` Element is a specification for the `from` Element (`from` hasSpecification `to`), during a LifecycleScopeType period."@en .

    <https://spdx.org/rdf/3.0.1/terms/Core/RelationshipType/hasStaticLink> a owl:NamedIndividual,
            ns1:RelationshipType ;
        rdfs:label "hasStaticLink" ;
        rdfs:comment "The `from` Element statically links in each `to` Element, during a LifecycleScopeType period."@en .

    <https://spdx.org/rdf/3.0.1/terms/Core/RelationshipType/hasTest> a owl:NamedIndividual,
            ns1:RelationshipType ;
        rdfs:label "hasTest" ;
        rdfs:comment "Every `to` Element is a test artifact for the `from` Element (`from` hasTest `to`), during a LifecycleScopeType period."@en .

    <https://spdx.org/rdf/3.0.1/terms/Core/RelationshipType/hasTestCase> a owl:NamedIndividual,
            ns1:RelationshipType ;
        rdfs:label "hasTestCase" ;
        rdfs:comment "Every `to` Element is a test case for the `from` Element (`from` hasTestCase `to`)."@en .

    <https://spdx.org/rdf/3.0.1/terms/Core/RelationshipType/hasVariant> a owl:NamedIndividual,
            ns1:RelationshipType ;
        rdfs:label "hasVariant" ;
        rdfs:comment "Every `to` Element is a variant the `from` Element (`from` hasVariant `to`)."@en .

    <https://spdx.org/rdf/3.0.1/terms/Core/RelationshipType/invokedBy> a owl:NamedIndividual,
            ns1:RelationshipType ;
        rdfs:label "invokedBy" ;
        rdfs:comment "The `from` Element was invoked by the `to` Agent, during a LifecycleScopeType period (for example, a Build element that describes a build step)."@en .

    <https://spdx.org/rdf/3.0.1/terms/Core/RelationshipType/modifiedBy> a owl:NamedIndividual,
            ns1:RelationshipType ;
        rdfs:label "modifiedBy" ;
        rdfs:comment "The `from` Element is modified by each `to` Element."@en .

    <https://spdx.org/rdf/3.0.1/terms/Core/RelationshipType/other> a owl:NamedIndividual,
            ns1:RelationshipType ;
        rdfs:label "other" ;
        rdfs:comment "Every `to` Element is related to the `from` Element where the relationship type is not described by any of the SPDX relationship types (this relationship is directionless)."@en .

    <https://spdx.org/rdf/3.0.1/terms/Core/RelationshipType/packagedBy> a owl:NamedIndividual,
            ns1:RelationshipType ;
        rdfs:label "packagedBy" ;
        rdfs:comment "Every `to` Element is a packaged instance of the `from` Element (`from` packagedBy `to`)."@en .

    <https://spdx.org/rdf/3.0.1/terms/Core/RelationshipType/patchedBy> a owl:NamedIndividual,
            ns1:RelationshipType ;
        rdfs:label "patchedBy" ;
        rdfs:comment "Every `to` Element is a patch for the `from` Element (`from` patchedBy `to`)."@en .

    <https://spdx.org/rdf/3.0.1/terms/Core/RelationshipType/publishedBy> a owl:NamedIndividual,
            ns1:RelationshipType ;
        rdfs:label "publishedBy" ;
        rdfs:comment "Designates a `from` Vulnerability was made available for public use or reference by each `to` Agent."@en .

    <https://spdx.org/rdf/3.0.1/terms/Core/RelationshipType/reportedBy> a owl:NamedIndividual,
            ns1:RelationshipType ;
        rdfs:label "reportedBy" ;
        rdfs:comment "Designates a `from` Vulnerability was first reported to a project, vendor, or tracking database for formal identification by each `to` Agent."@en .

    <https://spdx.org/rdf/3.0.1/terms/Core/RelationshipType/republishedBy> a owl:NamedIndividual,
            ns1:RelationshipType ;
        rdfs:label "republishedBy" ;
        rdfs:comment "Designates a `from` Vulnerability's details were tracked, aggregated, and/or enriched to improve context (i.e. NVD) by each `to` Agent."@en .

    <https://spdx.org/rdf/3.0.1/terms/Core/RelationshipType/serializedInArtifact> a owl:NamedIndividual,
            ns1:RelationshipType ;
        rdfs:label "serializedInArtifact" ;
        rdfs:comment "The `from` SpdxDocument can be found in a serialized form in each `to` Artifact."@en .

    <https://spdx.org/rdf/3.0.1/terms/Core/RelationshipType/testedOn> a owl:NamedIndividual,
            ns1:RelationshipType ;
        rdfs:label "testedOn" ;
        rdfs:comment "The `from` Element has been tested on the `to` Element(s)."@en .

    <https://spdx.org/rdf/3.0.1/terms/Core/RelationshipType/trainedOn> a owl:NamedIndividual,
            ns1:RelationshipType ;
        rdfs:label "trainedOn" ;
        rdfs:comment "The `from` Element has been trained on the `to` Element(s)."@en .

    <https://spdx.org/rdf/3.0.1/terms/Core/RelationshipType/underInvestigationFor> a owl:NamedIndividual,
            ns1:RelationshipType ;
        rdfs:label "underInvestigationFor" ;
        rdfs:comment "The `from` Vulnerability impact is being investigated for each `to` Element. The use of the `underInvestigationFor` type is constrained to `VexUnderInvestigationVulnAssessmentRelationship` classed relationships."@en .

    <https://spdx.org/rdf/3.0.1/terms/Core/RelationshipType/usesTool> a owl:NamedIndividual,
            ns1:RelationshipType ;
        rdfs:label "usesTool" ;
        rdfs:comment "The `from` Element uses each `to` Element as a tool, during a LifecycleScopeType period."@en .

    <https://spdx.org/rdf/3.0.1/terms/Core/SupportType/deployed> a owl:NamedIndividual,
            ns1:SupportType ;
        rdfs:label "deployed" ;
        rdfs:comment "in addition to being supported by the supplier, the software is known to have been deployed and is in use.  For a software as a service provider, this implies the software is now available as a service."@en .

    <https://spdx.org/rdf/3.0.1/terms/Core/SupportType/development> a owl:NamedIndividual,
            ns1:SupportType ;
        rdfs:label "development" ;
        rdfs:comment "the artifact is in active development and is not considered ready for formal support from the supplier."@en .

    <https://spdx.org/rdf/3.0.1/terms/Core/SupportType/endOfSupport> a owl:NamedIndividual,
            ns1:SupportType ;
        rdfs:label "endOfSupport" ;
        rdfs:comment "there is a defined end of support for the artifact from the supplier.  This may also be referred to as end of life. There is a validUntilDate that can be used to signal when support ends for the artifact."@en .

    <https://spdx.org/rdf/3.0.1/terms/Core/SupportType/limitedSupport> a owl:NamedIndividual,
            ns1:SupportType ;
        rdfs:label "limitedSupport" ;
        rdfs:comment "the artifact has been released, and there is limited support available from the supplier. There is a validUntilDate that can provide additional information about the duration of support."@en .

    <https://spdx.org/rdf/3.0.1/terms/Core/SupportType/noAssertion> a owl:NamedIndividual,
            ns1:SupportType ;
        rdfs:label "noAssertion" ;
        rdfs:comment "no assertion about the type of support is made.   This is considered the default if no other support type is used."@en .

    <https://spdx.org/rdf/3.0.1/terms/Core/SupportType/noSupport> a owl:NamedIndividual,
            ns1:SupportType ;
        rdfs:label "noSupport" ;
        rdfs:comment "there is no support for the artifact from the supplier, consumer assumes any support obligations."@en .

    <https://spdx.org/rdf/3.0.1/terms/Core/SupportType/support> a owl:NamedIndividual,
            ns1:SupportType ;
        rdfs:label "support" ;
        rdfs:comment "the artifact has been released, and is supported from the supplier.   There is a validUntilDate that can provide additional information about the duration of support."@en .

    ns1:annotationType a owl:ObjectProperty ;
        rdfs:comment "Describes the type of annotation."@en ;
        rdfs:range ns1:AnnotationType .

    ns1:beginIntegerRange a owl:DatatypeProperty ;
        rdfs:comment "Defines the beginning of a range."@en ;
        rdfs:range xsd:positiveInteger .

    ns1:builtTime a owl:DatatypeProperty ;
        rdfs:comment "Specifies the time an artifact was built."@en ;
        rdfs:range xsd:dateTimeStamp .

    ns1:completeness a owl:ObjectProperty ;
        rdfs:comment "Provides information about the completeness of relationships."@en ;
        rdfs:range ns1:RelationshipCompleteness .

    ns1:context a owl:DatatypeProperty ;
        rdfs:comment """Gives information about the circumstances or unifying properties
that Elements of the bundle have been assembled under."""@en ;
        rdfs:range xsd:string .

    ns1:created a owl:DatatypeProperty ;
        rdfs:comment "Identifies when the Element was originally created."@en ;
        rdfs:range xsd:dateTimeStamp .

    ns1:createdBy a owl:ObjectProperty ;
        rdfs:comment "Identifies who or what created the Element."@en ;
        rdfs:range ns1:Agent .

    ns1:createdUsing a owl:ObjectProperty ;
        rdfs:comment "Identifies the tooling that was used during the creation of the Element."@en ;
        rdfs:range ns1:Tool .

    ns1:creationInfo a owl:ObjectProperty ;
        rdfs:comment "Provides information about the creation of the Element."@en ;
        rdfs:range ns1:CreationInfo .

    ns1:dataLicense a owl:ObjectProperty ;
        rdfs:comment """Provides the license under which the SPDX documentation of the Element can be
used."""@en ;
        rdfs:range <https://spdx.org/rdf/3.0.1/terms/SimpleLicensing/AnyLicenseInfo> .

    ns1:definingArtifact a owl:ObjectProperty ;
        rdfs:comment """Artifact representing a serialization instance of SPDX data containing the
definition of a particular Element."""@en ;
        rdfs:range ns1:Artifact .

    ns1:description a owl:DatatypeProperty ;
        rdfs:comment "Provides a detailed description of the Element."@en ;
        rdfs:range xsd:string .

    ns1:element a owl:ObjectProperty ;
        rdfs:comment "Refers to one or more Elements that are part of an ElementCollection."@en ;
        rdfs:range ns1:Element .

    ns1:endIntegerRange a owl:DatatypeProperty ;
        rdfs:comment "Defines the end of a range."@en ;
        rdfs:range xsd:positiveInteger .

    ns1:endTime a owl:DatatypeProperty ;
        rdfs:comment "Specifies the time from which an element is no longer applicable / valid."@en ;
        rdfs:range xsd:dateTimeStamp .

    ns1:extension a owl:ObjectProperty ;
        rdfs:comment "Specifies an Extension characterization of some aspect of an Element."@en ;
        rdfs:range <https://spdx.org/rdf/3.0.1/terms/Extension/Extension> .

    ns1:externalIdentifier a owl:ObjectProperty ;
        rdfs:comment """Provides a reference to a resource outside the scope of SPDX-3.0 content
that uniquely identifies an Element."""@en ;
        rdfs:range ns1:ExternalIdentifier .

    ns1:externalIdentifierType a owl:ObjectProperty ;
        rdfs:comment "Specifies the type of the external identifier."@en ;
        rdfs:range ns1:ExternalIdentifierType .

    ns1:externalRef a owl:ObjectProperty ;
        rdfs:comment """Points to a resource outside the scope of the SPDX-3.0 content
that provides additional characteristics of an Element."""@en ;
        rdfs:range ns1:ExternalRef .

    ns1:externalRefType a owl:ObjectProperty ;
        rdfs:comment "Specifies the type of the external reference."@en ;
        rdfs:range ns1:ExternalRefType .

    ns1:externalSpdxId a owl:DatatypeProperty ;
        rdfs:comment """Identifies an external Element used within an SpdxDocument but defined
external to that SpdxDocument."""@en ;
        rdfs:range xsd:anyURI .

    ns1:from a owl:ObjectProperty ;
        rdfs:comment "References the Element on the left-hand side of a relationship."@en ;
        rdfs:range ns1:Element .

    ns1:identifier a owl:DatatypeProperty ;
        rdfs:comment "Uniquely identifies an external element."@en ;
        rdfs:range xsd:string .

    ns1:identifierLocator a owl:DatatypeProperty ;
        rdfs:comment "Provides the location for more information regarding an external identifier."@en ;
        rdfs:range xsd:anyURI .

    ns1:import a owl:ObjectProperty ;
        rdfs:comment "Provides an ExternalMap of Element identifiers."@en ;
        rdfs:range ns1:ExternalMap .

    ns1:issuingAuthority a owl:DatatypeProperty ;
        rdfs:comment "An entity that is authorized to issue identification credentials."@en ;
        rdfs:range xsd:string .

    ns1:key a owl:DatatypeProperty ;
        rdfs:comment "A key used in a generic key-value pair."@en ;
        rdfs:range xsd:string .

    ns1:locationHint a owl:DatatypeProperty ;
        rdfs:comment "Provides an indication of where to retrieve an external Element."@en ;
        rdfs:range xsd:anyURI .

    ns1:locator a owl:DatatypeProperty ;
        rdfs:comment "Provides the location of an external reference."@en ;
        rdfs:range xsd:string .

    ns1:name a owl:DatatypeProperty ;
        rdfs:comment "Identifies the name of an Element as designated by the creator."@en ;
        rdfs:range xsd:string .

    ns1:namespace a owl:DatatypeProperty ;
        rdfs:comment """Provides an unambiguous mechanism for conveying a URI fragment portion of an
Element ID."""@en ;
        rdfs:range xsd:anyURI .

    ns1:namespaceMap a owl:ObjectProperty ;
        rdfs:comment "Provides a NamespaceMap of prefixes and associated namespace partial URIs applicable to an SpdxDocument and independent of any specific serialization format or instance."@en ;
        rdfs:range ns1:NamespaceMap .

    ns1:originatedBy a owl:ObjectProperty ;
        rdfs:comment "Identifies from where or whom the Element originally came."@en ;
        rdfs:range ns1:Agent .

    ns1:packageVerificationCodeExcludedFile a owl:DatatypeProperty ;
        rdfs:comment """The relative file name of a file to be excluded from the
`PackageVerificationCode`."""@en ;
        rdfs:range xsd:string .

    ns1:prefix a owl:DatatypeProperty ;
        rdfs:comment "A substitute for a URI."@en ;
        rdfs:range xsd:string .

    ns1:profileConformance a owl:ObjectProperty ;
        rdfs:comment """Describes one a profile which the creator of this ElementCollection intends to
conform to."""@en ;
        rdfs:range ns1:ProfileIdentifierType .

    ns1:relationshipType a owl:ObjectProperty ;
        rdfs:comment "Information about the relationship between two Elements."@en ;
        rdfs:range ns1:RelationshipType .

    ns1:releaseTime a owl:DatatypeProperty ;
        rdfs:comment "Specifies the time an artifact was released."@en ;
        rdfs:range xsd:dateTimeStamp .

    ns1:rootElement a owl:ObjectProperty ;
        rdfs:comment "This property is used to denote the root Element(s) of a tree of elements contained in a BOM."@en ;
        rdfs:range ns1:Element .

    ns1:scope a owl:ObjectProperty ;
        rdfs:comment "Capture the scope of information about a specific relationship between elements."@en ;
        rdfs:range ns1:LifecycleScopeType .

    ns1:specVersion a owl:DatatypeProperty ;
        rdfs:comment """Provides a reference number that can be used to understand how to parse and
interpret an Element."""@en ;
        rdfs:range xsd:string .

    ns1:standardName a owl:DatatypeProperty ;
        rdfs:comment "The name of a relevant standard that may apply to an artifact."@en ;
        rdfs:range xsd:string .

    ns1:startTime a owl:DatatypeProperty ;
        rdfs:comment "Specifies the time from which an element is applicable / valid."@en ;
        rdfs:range xsd:dateTimeStamp .

    ns1:statement a owl:DatatypeProperty ;
        rdfs:comment "Commentary on an assertion that an annotator has made."@en ;
        rdfs:range xsd:string .

    ns1:subject a owl:ObjectProperty ;
        rdfs:comment "An Element an annotator has made an assertion about."@en ;
        rdfs:range ns1:Element .

    ns1:summary a owl:DatatypeProperty ;
        rdfs:comment "A short description of an Element."@en ;
        rdfs:range xsd:string .

    ns1:supportLevel a owl:ObjectProperty ;
        rdfs:comment "Specifies the level of support associated with an artifact."@en ;
        rdfs:range ns1:SupportType .

    ns1:to a owl:ObjectProperty ;
        rdfs:comment "References an Element on the right-hand side of a relationship."@en ;
        rdfs:range ns1:Element .

    ns1:validUntilTime a owl:DatatypeProperty ;
        rdfs:comment """Specifies until when the artifact can be used before its usage needs to be
reassessed."""@en ;
        rdfs:range xsd:dateTimeStamp .

    ns1:value a owl:DatatypeProperty ;
        rdfs:comment "A value used in a generic key-value pair."@en ;
        rdfs:range xsd:string .

    <https://spdx.org/rdf/3.0.1/terms/Dataset/ConfidentialityLevelType/amber> a owl:NamedIndividual,
            ns5:ConfidentialityLevelType ;
        rdfs:label "amber" ;
        rdfs:comment "Data points in the dataset can be shared only with specific organizations and their clients on a need to know basis."@en .

    <https://spdx.org/rdf/3.0.1/terms/Dataset/ConfidentialityLevelType/clear> a owl:NamedIndividual,
            ns5:ConfidentialityLevelType ;
        rdfs:label "clear" ;
        rdfs:comment "Dataset may be distributed freely, without restriction."@en .

    <https://spdx.org/rdf/3.0.1/terms/Dataset/ConfidentialityLevelType/green> a owl:NamedIndividual,
            ns5:ConfidentialityLevelType ;
        rdfs:label "green" ;
        rdfs:comment "Dataset can be shared within a community of peers and partners."@en .

    <https://spdx.org/rdf/3.0.1/terms/Dataset/ConfidentialityLevelType/red> a owl:NamedIndividual,
            ns5:ConfidentialityLevelType ;
        rdfs:label "red" ;
        rdfs:comment "Data points in the dataset are highly confidential and can only be shared with named recipients."@en .

    <https://spdx.org/rdf/3.0.1/terms/Dataset/DatasetAvailabilityType/clickthrough> a owl:NamedIndividual,
            ns5:DatasetAvailabilityType ;
        rdfs:label "clickthrough" ;
        rdfs:comment "the dataset is not publicly available and can only be accessed after affirmatively accepting terms on a clickthrough webpage."@en .

    <https://spdx.org/rdf/3.0.1/terms/Dataset/DatasetAvailabilityType/directDownload> a owl:NamedIndividual,
            ns5:DatasetAvailabilityType ;
        rdfs:label "directDownload" ;
        rdfs:comment "the dataset is publicly available and can be downloaded directly."@en .

    <https://spdx.org/rdf/3.0.1/terms/Dataset/DatasetAvailabilityType/query> a owl:NamedIndividual,
            ns5:DatasetAvailabilityType ;
        rdfs:label "query" ;
        rdfs:comment "the dataset is publicly available, but not all at once, and can only be accessed through queries which return parts of the dataset."@en .

    <https://spdx.org/rdf/3.0.1/terms/Dataset/DatasetAvailabilityType/registration> a owl:NamedIndividual,
            ns5:DatasetAvailabilityType ;
        rdfs:label "registration" ;
        rdfs:comment "the dataset is not publicly available and an email registration is required before accessing the dataset, although without an affirmative acceptance of terms."@en .

    <https://spdx.org/rdf/3.0.1/terms/Dataset/DatasetAvailabilityType/scrapingScript> a owl:NamedIndividual,
            ns5:DatasetAvailabilityType ;
        rdfs:label "scrapingScript" ;
        rdfs:comment "the dataset provider is not making available the underlying data and the dataset must be reassembled, typically using the provided script for scraping the data."@en .

    <https://spdx.org/rdf/3.0.1/terms/Dataset/DatasetType/audio> a owl:NamedIndividual,
            ns5:DatasetType ;
        rdfs:label "audio" ;
        rdfs:comment "data is audio based, such as a collection of music from the 80s."@en .

    <https://spdx.org/rdf/3.0.1/terms/Dataset/DatasetType/categorical> a owl:NamedIndividual,
            ns5:DatasetType ;
        rdfs:label "categorical" ;
        rdfs:comment "data that is classified into a discrete number of categories, such as the eye color of a population of people."@en .

    <https://spdx.org/rdf/3.0.1/terms/Dataset/DatasetType/graph> a owl:NamedIndividual,
            ns5:DatasetType ;
        rdfs:label "graph" ;
        rdfs:comment "data is in the form of a graph where entries are somehow related to each other through edges, such a social network of friends."@en .

    <https://spdx.org/rdf/3.0.1/terms/Dataset/DatasetType/image> a owl:NamedIndividual,
            ns5:DatasetType ;
        rdfs:label "image" ;
        rdfs:comment "data is a collection of images such as pictures of animals."@en .

    <https://spdx.org/rdf/3.0.1/terms/Dataset/DatasetType/noAssertion> a owl:NamedIndividual,
            ns5:DatasetType ;
        rdfs:label "noAssertion" ;
        rdfs:comment "data type is not known."@en .

    <https://spdx.org/rdf/3.0.1/terms/Dataset/DatasetType/numeric> a owl:NamedIndividual,
            ns5:DatasetType ;
        rdfs:label "numeric" ;
        rdfs:comment "data consists only of numeric entries."@en .

    <https://spdx.org/rdf/3.0.1/terms/Dataset/DatasetType/other> a owl:NamedIndividual,
            ns5:DatasetType ;
        rdfs:label "other" ;
        rdfs:comment "data is of a type not included in this list."@en .

    <https://spdx.org/rdf/3.0.1/terms/Dataset/DatasetType/sensor> a owl:NamedIndividual,
            ns5:DatasetType ;
        rdfs:label "sensor" ;
        rdfs:comment "data is recorded from a physical sensor, such as a thermometer reading or biometric device."@en .

    <https://spdx.org/rdf/3.0.1/terms/Dataset/DatasetType/structured> a owl:NamedIndividual,
            ns5:DatasetType ;
        rdfs:label "structured" ;
        rdfs:comment "data is stored in tabular format or retrieved from a relational database."@en .

    <https://spdx.org/rdf/3.0.1/terms/Dataset/DatasetType/syntactic> a owl:NamedIndividual,
            ns5:DatasetType ;
        rdfs:label "syntactic" ;
        rdfs:comment "data describes the syntax or semantics of a language or text, such as a parse tree used for natural language processing."@en .

    <https://spdx.org/rdf/3.0.1/terms/Dataset/DatasetType/text> a owl:NamedIndividual,
            ns5:DatasetType ;
        rdfs:label "text" ;
        rdfs:comment "data consists of unstructured text, such as a book, Wikipedia article (without images), or transcript."@en .

    <https://spdx.org/rdf/3.0.1/terms/Dataset/DatasetType/timeseries> a owl:NamedIndividual,
            ns5:DatasetType ;
        rdfs:label "timeseries" ;
        rdfs:comment "data is recorded in an ordered sequence of timestamped entries, such as the price of a stock over the course of a day."@en .

    <https://spdx.org/rdf/3.0.1/terms/Dataset/DatasetType/timestamp> a owl:NamedIndividual,
            ns5:DatasetType ;
        rdfs:label "timestamp" ;
        rdfs:comment "data is recorded with a timestamp for each entry, but not necessarily ordered or at specific intervals, such as when a taxi ride starts and ends."@en .

    <https://spdx.org/rdf/3.0.1/terms/Dataset/DatasetType/video> a owl:NamedIndividual,
            ns5:DatasetType ;
        rdfs:label "video" ;
        rdfs:comment "data is video based, such as a collection of movie clips featuring Tom Hanks."@en .

    ns5:anonymizationMethodUsed a owl:DatatypeProperty ;
        rdfs:comment "Describes the anonymization methods used."@en ;
        rdfs:range xsd:string .

    ns5:confidentialityLevel a owl:ObjectProperty ;
        rdfs:comment "Describes the confidentiality level of the data points contained in the dataset."@en ;
        rdfs:range ns5:ConfidentialityLevelType .

    ns5:dataCollectionProcess a owl:DatatypeProperty ;
        rdfs:comment "Describes how the dataset was collected."@en ;
        rdfs:range xsd:string .

    ns5:dataPreprocessing a owl:DatatypeProperty ;
        rdfs:comment "Describes the preprocessing steps that were applied to the raw data to create the given dataset."@en ;
        rdfs:range xsd:string .

    ns5:datasetAvailability a owl:ObjectProperty ;
        rdfs:comment "The field describes the availability of a dataset."@en ;
        rdfs:range ns5:DatasetAvailabilityType .

    ns5:datasetNoise a owl:DatatypeProperty ;
        rdfs:comment "Describes potentially noisy elements of the dataset."@en ;
        rdfs:range xsd:string .

    ns5:datasetSize a owl:DatatypeProperty ;
        rdfs:comment "Captures the size of the dataset."@en ;
        rdfs:range xsd:nonNegativeInteger .

    ns5:datasetType a owl:ObjectProperty ;
        rdfs:comment "Describes the type of the given dataset."@en ;
        rdfs:range ns5:DatasetType .

    ns5:datasetUpdateMechanism a owl:DatatypeProperty ;
        rdfs:comment "Describes a mechanism to update the dataset."@en ;
        rdfs:range xsd:string .

    ns5:hasSensitivePersonalInformation a owl:ObjectProperty ;
        rdfs:comment "Describes if any sensitive personal information is present in the dataset."@en ;
        rdfs:range ns1:PresenceType .

    ns5:intendedUse a owl:DatatypeProperty ;
        rdfs:comment "Describes what the given dataset should be used for."@en ;
        rdfs:range xsd:string .

    ns5:knownBias a owl:DatatypeProperty ;
        rdfs:comment "Records the biases that the dataset is known to encompass."@en ;
        rdfs:range xsd:string .

    ns5:sensor a owl:ObjectProperty ;
        rdfs:comment "Describes a sensor used for collecting the data."@en ;
        rdfs:range ns1:DictionaryEntry .

    ns6:additionText a owl:DatatypeProperty ;
        rdfs:comment "Identifies the full text of a LicenseAddition."@en ;
        rdfs:range xsd:string .

    ns6:isDeprecatedAdditionId a owl:DatatypeProperty ;
        rdfs:comment "Specifies whether an additional text identifier has been marked as deprecated."@en ;
        rdfs:range xsd:boolean .

    ns6:isDeprecatedLicenseId a owl:DatatypeProperty ;
        rdfs:comment """Specifies whether a license or additional text identifier has been marked as
deprecated."""@en ;
        rdfs:range xsd:boolean .

    ns6:isFsfLibre a owl:DatatypeProperty ;
        rdfs:comment """Specifies whether the License is listed as free by the
Free Software Foundation (FSF)."""@en ;
        rdfs:range xsd:boolean .

    ns6:isOsiApproved a owl:DatatypeProperty ;
        rdfs:comment """Specifies whether the License is listed as approved by the
Open Source Initiative (OSI)."""@en ;
        rdfs:range xsd:boolean .

    ns6:standardAdditionTemplate a owl:DatatypeProperty ;
        rdfs:comment "Identifies the full text of a LicenseAddition, in SPDX templating format."@en ;
        rdfs:range xsd:string .

    ns6:standardLicenseHeader a owl:DatatypeProperty ;
        rdfs:comment """Provides a License author's preferred text to indicate that a file is covered
by the License."""@en ;
        rdfs:range xsd:string .

    ns6:standardLicenseTemplate a owl:DatatypeProperty ;
        rdfs:comment "Identifies the full text of a License, in SPDX templating format."@en ;
        rdfs:range xsd:string .

    ns6:subjectAddition a owl:ObjectProperty ;
        rdfs:comment "A LicenseAddition participating in a 'with addition' model."@en ;
        rdfs:range ns6:LicenseAddition .

    ns6:subjectExtendableLicense a owl:ObjectProperty ;
        rdfs:comment "A License participating in a 'with addition' model."@en ;
        rdfs:range ns6:ExtendableLicense .

    ns6:subjectLicense a owl:ObjectProperty ;
        rdfs:comment "A License participating in an 'or later' model."@en ;
        rdfs:range ns6:License .

    <https://spdx.org/rdf/3.0.1/terms/Extension/cdxPropName> a owl:DatatypeProperty ;
        rdfs:comment "A name used in a CdxPropertyEntry name-value pair."@en ;
        rdfs:range xsd:string .

    <https://spdx.org/rdf/3.0.1/terms/Extension/cdxPropValue> a owl:DatatypeProperty ;
        rdfs:comment "A value used in a CdxPropertyEntry name-value pair."@en ;
        rdfs:range xsd:string .

    <https://spdx.org/rdf/3.0.1/terms/Extension/cdxProperty> a owl:ObjectProperty ;
        rdfs:comment "Provides a map of a property names to a values."@en ;
        rdfs:range <https://spdx.org/rdf/3.0.1/terms/Extension/CdxPropertyEntry> .

    <https://spdx.org/rdf/3.0.1/terms/Security/ExploitCatalogType/kev> a owl:NamedIndividual,
            ns3:ExploitCatalogType ;
        rdfs:label "kev" ;
        rdfs:comment "CISA's Known Exploited Vulnerability (KEV) Catalog"@en .

    <https://spdx.org/rdf/3.0.1/terms/Security/ExploitCatalogType/other> a owl:NamedIndividual,
            ns3:ExploitCatalogType ;
        rdfs:label "other" ;
        rdfs:comment "Other exploit catalogs"@en .

    <https://spdx.org/rdf/3.0.1/terms/Security/SsvcDecisionType/act> a owl:NamedIndividual,
            ns3:SsvcDecisionType ;
        rdfs:label "act" ;
        rdfs:comment "The vulnerability requires attention from the organization's internal, supervisory-level and leadership-level individuals. Necessary actions include requesting assistance or information about the vulnerability, as well as publishing a notification either internally and/or externally. Typically, internal groups would meet to determine the overall response and then execute agreed upon actions. CISA recommends remediating Act vulnerabilities as soon as possible."@en .

    <https://spdx.org/rdf/3.0.1/terms/Security/SsvcDecisionType/attend> a owl:NamedIndividual,
            ns3:SsvcDecisionType ;
        rdfs:label "attend" ;
        rdfs:comment "The vulnerability requires attention from the organization's internal, supervisory-level individuals. Necessary actions include requesting assistance or information about the vulnerability, and may involve publishing a notification either internally and/or externally. CISA recommends remediating Attend vulnerabilities sooner than standard update timelines."@en .

    <https://spdx.org/rdf/3.0.1/terms/Security/SsvcDecisionType/track> a owl:NamedIndividual,
            ns3:SsvcDecisionType ;
        rdfs:label "track" ;
        rdfs:comment "The vulnerability does not require action at this time. The organization would continue to track the vulnerability and reassess it if new information becomes available. CISA recommends remediating Track vulnerabilities within standard update timelines."@en .

    <https://spdx.org/rdf/3.0.1/terms/Security/SsvcDecisionType/trackStar> a owl:NamedIndividual,
            ns3:SsvcDecisionType ;
        rdfs:label "trackStar" ;
        rdfs:comment "(\"Track\\*\" in the SSVC spec) The vulnerability contains specific characteristics that may require closer monitoring for changes. CISA recommends remediating Track\\* vulnerabilities within standard update timelines."@en .

    <https://spdx.org/rdf/3.0.1/terms/Security/VexJustificationType/componentNotPresent> a owl:NamedIndividual,
            ns3:VexJustificationType ;
        rdfs:label "componentNotPresent" ;
        rdfs:comment "The software is not affected because the vulnerable component is not in the product."@en .

    <https://spdx.org/rdf/3.0.1/terms/Security/VexJustificationType/inlineMitigationsAlreadyExist> a owl:NamedIndividual,
            ns3:VexJustificationType ;
        rdfs:label "inlineMitigationsAlreadyExist" ;
        rdfs:comment "Built-in inline controls or mitigations prevent an adversary from leveraging the vulnerability."@en .

    <https://spdx.org/rdf/3.0.1/terms/Security/VexJustificationType/vulnerableCodeCannotBeControlledByAdversary> a owl:NamedIndividual,
            ns3:VexJustificationType ;
        rdfs:label "vulnerableCodeCannotBeControlledByAdversary" ;
        rdfs:comment "The vulnerable component is present, and the component contains the vulnerable code. However, vulnerable code is used in such a way that an attacker cannot mount any anticipated attack."@en .

    <https://spdx.org/rdf/3.0.1/terms/Security/VexJustificationType/vulnerableCodeNotInExecutePath> a owl:NamedIndividual,
            ns3:VexJustificationType ;
        rdfs:label "vulnerableCodeNotInExecutePath" ;
        rdfs:comment "The affected code is not reachable through the execution of the code, including non-anticipated states of the product."@en .

    <https://spdx.org/rdf/3.0.1/terms/Security/VexJustificationType/vulnerableCodeNotPresent> a owl:NamedIndividual,
            ns3:VexJustificationType ;
        rdfs:label "vulnerableCodeNotPresent" ;
        rdfs:comment "The product is not affected because the code underlying the vulnerability is not present in the product."@en .

    ns3:actionStatement a owl:DatatypeProperty ;
        rdfs:comment """Provides advise on how to mitigate or remediate a vulnerability when a VEX product
is affected by it."""@en ;
        rdfs:range xsd:string .

    ns3:actionStatementTime a owl:DatatypeProperty ;
        rdfs:comment """Records the time when a recommended action was communicated in a VEX statement
to mitigate a vulnerability."""@en ;
        rdfs:range xsd:dateTimeStamp .

    ns3:assessedElement a owl:ObjectProperty ;
        rdfs:comment """Specifies an Element contained in a piece of software where a vulnerability was
found."""@en ;
        rdfs:range ns2:SoftwareArtifact .

    ns3:catalogType a owl:ObjectProperty ;
        rdfs:comment "Specifies the exploit catalog type."@en ;
        rdfs:range ns3:ExploitCatalogType .

    ns3:decisionType a owl:ObjectProperty ;
        rdfs:comment """Provide the enumeration of possible decisions in the
[Stakeholder-Specific Vulnerability Categorization (SSVC) decision tree](https://www.cisa.gov/stakeholder-specific-vulnerability-categorization-ssvc)."""@en ;
        rdfs:range ns3:SsvcDecisionType .

    ns3:exploited a owl:DatatypeProperty ;
        rdfs:comment "Describe that a CVE is known to have an exploit because it's been listed in an exploit catalog."@en ;
        rdfs:range xsd:boolean .

    ns3:impactStatement a owl:DatatypeProperty ;
        rdfs:comment """Explains why a VEX product is not affected by a vulnerability. It is an
alternative in VexNotAffectedVulnAssessmentRelationship to the machine-readable
justification label."""@en ;
        rdfs:range xsd:string .

    ns3:impactStatementTime a owl:DatatypeProperty ;
        rdfs:comment "Timestamp of impact statement."@en ;
        rdfs:range xsd:dateTimeStamp .

    ns3:justificationType a owl:ObjectProperty ;
        rdfs:comment """Impact justification label to be used when linking a vulnerability to an element
representing a VEX product with a VexNotAffectedVulnAssessmentRelationship
relationship."""@en ;
        rdfs:range ns3:VexJustificationType .

    ns3:locator a owl:DatatypeProperty ;
        rdfs:comment "Provides the location of an exploit catalog."@en ;
        rdfs:range xsd:anyURI .

    ns3:percentile a owl:DatatypeProperty ;
        rdfs:comment "The percentile of the current probability score."@en ;
        rdfs:range xsd:decimal .

    ns3:probability a owl:DatatypeProperty ;
        rdfs:comment "A probability score between 0 and 1 of a vulnerability being exploited."@en ;
        rdfs:range xsd:decimal .

    ns3:statusNotes a owl:DatatypeProperty ;
        rdfs:comment "Conveys information about how VEX status was determined."@en ;
        rdfs:range xsd:string .

    ns3:vexVersion a owl:DatatypeProperty ;
        rdfs:comment "Specifies the version of a VEX statement."@en ;
        rdfs:range xsd:string .

    <https://spdx.org/rdf/3.0.1/terms/SimpleLicensing/customIdToUri> a owl:ObjectProperty ;
        rdfs:comment """Maps a LicenseRef or AdditionRef string for a Custom License or a Custom
License Addition to its URI ID."""@en ;
        rdfs:range ns1:DictionaryEntry .

    <https://spdx.org/rdf/3.0.1/terms/SimpleLicensing/licenseExpression> a owl:DatatypeProperty ;
        rdfs:comment "A string in the license expression format."@en ;
        rdfs:range xsd:string .

    <https://spdx.org/rdf/3.0.1/terms/SimpleLicensing/licenseListVersion> a owl:DatatypeProperty ;
        rdfs:comment "The version of the SPDX License List used in the license expression."@en ;
        rdfs:range xsd:string .

    <https://spdx.org/rdf/3.0.1/terms/Software/ContentIdentifierType/gitoid> a owl:NamedIndividual,
            ns2:ContentIdentifierType ;
        rdfs:label "gitoid" ;
        rdfs:comment "[Gitoid](https://www.iana.org/assignments/uri-schemes/prov/gitoid), stands for [Git Object ID](https://git-scm.com/book/en/v2/Git-Internals-Git-Objects). A gitoid of type blob is a unique hash of a binary artifact. A gitoid may represent either an [Artifact Identifier](https://github.com/omnibor/spec/blob/eb1ee5c961c16215eb8709b2975d193a2007a35d/spec/SPEC.md#artifact-identifier-types) for the software artifact or an [Input Manifest Identifier](https://github.com/omnibor/spec/blob/eb1ee5c961c16215eb8709b2975d193a2007a35d/spec/SPEC.md#input-manifest-identifier) for the software artifact's associated [Artifact Input Manifest](https://github.com/omnibor/spec/blob/eb1ee5c961c16215eb8709b2975d193a2007a35d/spec/SPEC.md#artifact-input-manifest); this ambiguity exists because the Artifact Input Manifest is itself an artifact, and the gitoid of that artifact is its valid identifier. Gitoids calculated on software artifacts (Snippet, File, or Package Elements) should be recorded in the SPDX 3.0 SoftwareArtifact's contentIdentifier property. Gitoids calculated on the Artifact Input Manifest (Input Manifest Identifier) should be recorded in the SPDX 3.0 Element's externalIdentifier property. See [OmniBOR Specification](https://github.com/omnibor/spec/), a minimalistic specification for describing software [Artifact Dependency Graphs](https://github.com/omnibor/spec/blob/eb1ee5c961c16215eb8709b2975d193a2007a35d/spec/SPEC.md#artifact-dependency-graph-adg)."@en .

    <https://spdx.org/rdf/3.0.1/terms/Software/ContentIdentifierType/swhid> a owl:NamedIndividual,
            ns2:ContentIdentifierType ;
        rdfs:label "swhid" ;
        rdfs:comment "SoftWare Hash IDentifier, a persistent intrinsic identifier for digital artifacts, such as files, trees (also known as directories or folders), commits, and other objects typically found in version control systems. The format of the identifiers is defined in the [SWHID specification](https://www.swhid.org/specification/v1.1/4.Syntax) (ISO/IEC DIS 18670). They typically look like `swh:1:cnt:94a9ed024d3859793618152ea559a168bbcbb5e2`."@en .

    <https://spdx.org/rdf/3.0.1/terms/Software/FileKindType/directory> a owl:NamedIndividual,
            ns2:FileKindType ;
        rdfs:label "directory" ;
        rdfs:comment "The file represents a directory and all content stored in that directory."@en .

    <https://spdx.org/rdf/3.0.1/terms/Software/FileKindType/file> a owl:NamedIndividual,
            ns2:FileKindType ;
        rdfs:label "file" ;
        rdfs:comment "The file represents a single file (default)."@en .

    <https://spdx.org/rdf/3.0.1/terms/Software/SbomType/analyzed> a owl:NamedIndividual,
            ns2:SbomType ;
        rdfs:label "analyzed" ;
        rdfs:comment "SBOM generated through analysis of artifacts (e.g., executables, packages, containers, and virtual machine images) after its build. Such analysis generally requires a variety of heuristics. In some contexts, this may also be referred to as a \"3rd party\" SBOM."@en .

    <https://spdx.org/rdf/3.0.1/terms/Software/SbomType/build> a owl:NamedIndividual,
            ns2:SbomType ;
        rdfs:label "build" ;
        rdfs:comment "SBOM generated as part of the process of building the software to create a releasable artifact (e.g., executable or package) from data such as source files, dependencies, built components, build process ephemeral data, and other SBOMs."@en .

    <https://spdx.org/rdf/3.0.1/terms/Software/SbomType/deployed> a owl:NamedIndividual,
            ns2:SbomType ;
        rdfs:label "deployed" ;
        rdfs:comment "SBOM provides an inventory of software that is present on a system. This may be an assembly of other SBOMs that combines analysis of configuration options, and examination of execution behavior in a (potentially simulated) deployment environment."@en .

    <https://spdx.org/rdf/3.0.1/terms/Software/SbomType/design> a owl:NamedIndividual,
            ns2:SbomType ;
        rdfs:label "design" ;
        rdfs:comment "SBOM of intended, planned software project or product with included components (some of which may not yet exist) for a new software artifact."@en .

    <https://spdx.org/rdf/3.0.1/terms/Software/SbomType/runtime> a owl:NamedIndividual,
            ns2:SbomType ;
        rdfs:label "runtime" ;
        rdfs:comment "SBOM generated through instrumenting the system running the software, to capture only components present in the system, as well as external call-outs or dynamically loaded components. In some contexts, this may also be referred to as an \"Instrumented\" or \"Dynamic\" SBOM."@en .

    <https://spdx.org/rdf/3.0.1/terms/Software/SbomType/source> a owl:NamedIndividual,
            ns2:SbomType ;
        rdfs:label "source" ;
        rdfs:comment "SBOM created directly from the development environment, source files, and included dependencies used to build an product artifact."@en .

    ns2:additionalPurpose a owl:ObjectProperty ;
        rdfs:comment "Provides additional purpose information of the software artifact."@en ;
        rdfs:range ns2:SoftwarePurpose .

    ns2:attributionText a owl:DatatypeProperty ;
        rdfs:comment """Provides a place for the SPDX data creator to record acknowledgement text for
a software Package, File or Snippet."""@en ;
        rdfs:range xsd:string .

    ns2:byteRange a owl:DatatypeProperty ;
        rdfs:comment """Defines the byte range in the original host file that the snippet information
applies to."""@en ;
        rdfs:range ns1:PositiveIntegerRange .

    ns2:contentIdentifier a owl:DatatypeProperty ;
        rdfs:comment """A canonical, unique, immutable identifier of the artifact content, that may be
used for verifying its identity and/or integrity."""@en ;
        rdfs:range ns2:ContentIdentifier .

    ns2:contentIdentifierType a owl:ObjectProperty ;
        rdfs:comment "Specifies the type of the content identifier."@en ;
        rdfs:range ns2:ContentIdentifierType .

    ns2:contentIdentifierValue a owl:DatatypeProperty ;
        rdfs:comment "Specifies the value of the content identifier."@en ;
        rdfs:range xsd:anyURI .

    ns2:copyrightText a owl:DatatypeProperty ;
        rdfs:comment """Identifies the text of one or more copyright notices for a software Package,
File or Snippet, if any."""@en ;
        rdfs:range xsd:string .

    ns2:downloadLocation a owl:DatatypeProperty ;
        rdfs:comment """Identifies the download Uniform Resource Identifier for the package at the time
that the document was created."""@en ;
        rdfs:range xsd:anyURI .

    ns2:fileKind a owl:ObjectProperty ;
        rdfs:comment "Describes if a given file is a directory or non-directory kind of file."@en ;
        rdfs:range ns2:FileKindType .

    ns2:homePage a owl:DatatypeProperty ;
        rdfs:comment """A place for the SPDX document creator to record a website that serves as the
package's home page."""@en ;
        rdfs:range xsd:anyURI .

    ns2:lineRange a owl:DatatypeProperty ;
        rdfs:comment """Defines the line range in the original host file that the snippet information
applies to."""@en ;
        rdfs:range ns1:PositiveIntegerRange .

    ns2:packageUrl a owl:DatatypeProperty ;
        rdfs:comment """Provides a place for the SPDX data creator to record the package URL string
(in accordance with the Package URL specification) for a software Package."""@en ;
        rdfs:range xsd:anyURI .

    ns2:packageVersion a owl:DatatypeProperty ;
        rdfs:comment "Identify the version of a package."@en ;
        rdfs:range xsd:string .

    ns2:primaryPurpose a owl:ObjectProperty ;
        rdfs:comment "Provides information about the primary purpose of the software artifact."@en ;
        rdfs:range ns2:SoftwarePurpose .

    ns2:sbomType a owl:ObjectProperty ;
        rdfs:comment "Provides information about the type of an SBOM."@en ;
        rdfs:range ns2:SbomType .

    ns2:snippetFromFile a owl:ObjectProperty ;
        rdfs:comment "Defines the original host file that the snippet information applies to."@en ;
        rdfs:range ns2:File .

    ns2:sourceInfo a owl:DatatypeProperty ;
        rdfs:comment """Records any relevant background information or additional comments
about the origin of the package."""@en ;
        rdfs:range xsd:string .

    ns4:EnergyConsumption a owl:Class,
            sh:NodeShape ;
        rdfs:comment """A class for describing the energy consumption incurred by an AI model in
different stages of its lifecycle."""@en ;
        sh:nodeKind sh:BlankNodeOrIRI ;
        sh:property _:N9111c10d9fb94856a73b98e13b7a47bd,
            _:Nc7f0e867cdc148a6a3b6a15ffebab59f,
            _:Ndd9c27ec175a4f028fe9688b608d7b81 .

    ns1:ExternalIdentifier a owl:Class,
            sh:NodeShape ;
        rdfs:comment "A reference to a resource identifier defined outside the scope of SPDX-3.0 content that uniquely identifies an Element."@en ;
        sh:nodeKind sh:BlankNodeOrIRI ;
        sh:property _:N10a0a33d835147168e667e794740d037,
            _:N397df444dbe1469ebb7eec950c2015b5,
            _:N5e9bcf2d0c714e6a9e1b996f845a0a9f,
            _:Nbab338ccec5f425db60782a45394e3b5,
            _:Nbc05456f325c4505bf75f26e68fbb31c .

    ns1:ExternalMap a owl:Class,
            sh:NodeShape ;
        rdfs:comment """A map of Element identifiers that are used within an SpdxDocument but defined
external to that SpdxDocument."""@en ;
        sh:nodeKind sh:BlankNodeOrIRI ;
        sh:property _:N7005d82c23df4154835c9c275887b1e4,
            _:N7450e5f23ee34ddf90d69f61d5f62c87,
            _:Nacd46caa1cf74e399511d6e46de2c8c7,
            _:Nd2b4b8ceb1424471a1f401c56908b8d7 .

    ns1:ExternalRef a owl:Class,
            sh:NodeShape ;
        rdfs:comment "A reference to a resource outside the scope of SPDX-3.0 content related to an Element."@en ;
        sh:nodeKind sh:BlankNodeOrIRI ;
        sh:property _:N12f123f6f5f0432695eadd7ebcb196b0,
            _:N4148ad351ad4456284b5e6de7a31ae4e,
            _:N9e2593cb36b740d3be8bddd390b67fe7,
            _:Nd2de0ed500c448f792eb6382b9c9daab .

    ns1:Hash a owl:Class,
            sh:NodeShape ;
        rdfs:comment "A mathematically calculated representation of a grouping of data."@en ;
        rdfs:subClassOf ns1:IntegrityMethod ;
        sh:nodeKind sh:BlankNodeOrIRI ;
        sh:property _:N6b83da998edf4da3a5c86600ef22ed5f,
            _:Na67d6b4681614d69afdd1a2d31e21023 .

    <https://spdx.org/rdf/3.0.1/terms/Core/HashAlgorithm/adler32> a owl:NamedIndividual,
            ns1:HashAlgorithm ;
        rdfs:label "adler32" ;
        rdfs:comment "Adler-32 checksum is part of the widely used zlib compression library as defined in [RFC 1950](https://datatracker.ietf.org/doc/rfc1950/) Section 2.3."@en .

    <https://spdx.org/rdf/3.0.1/terms/Core/HashAlgorithm/blake2b256> a owl:NamedIndividual,
            ns1:HashAlgorithm ;
        rdfs:label "blake2b256" ;
        rdfs:comment "BLAKE2b algorithm with a digest size of 256, as defined in [RFC 7693](https://datatracker.ietf.org/doc/rfc7693/) Section 4."@en .

    <https://spdx.org/rdf/3.0.1/terms/Core/HashAlgorithm/blake2b384> a owl:NamedIndividual,
            ns1:HashAlgorithm ;
        rdfs:label "blake2b384" ;
        rdfs:comment "BLAKE2b algorithm with a digest size of 384, as defined in [RFC 7693](https://datatracker.ietf.org/doc/rfc7693/) Section 4."@en .

    <https://spdx.org/rdf/3.0.1/terms/Core/HashAlgorithm/blake2b512> a owl:NamedIndividual,
            ns1:HashAlgorithm ;
        rdfs:label "blake2b512" ;
        rdfs:comment "BLAKE2b algorithm with a digest size of 512, as defined in [RFC 7693](https://datatracker.ietf.org/doc/rfc7693/) Section 4."@en .

    <https://spdx.org/rdf/3.0.1/terms/Core/HashAlgorithm/blake3> a owl:NamedIndividual,
            ns1:HashAlgorithm ;
        rdfs:label "blake3" ;
        rdfs:comment "[BLAKE3](https://github.com/BLAKE3-team/BLAKE3-specs/blob/master/blake3.pdf)"@en .

    <https://spdx.org/rdf/3.0.1/terms/Core/HashAlgorithm/crystalsDilithium> a owl:NamedIndividual,
            ns1:HashAlgorithm ;
        rdfs:label "crystalsDilithium" ;
        rdfs:comment "[Dilithium](https://pq-crystals.org/dilithium/)"@en .

    <https://spdx.org/rdf/3.0.1/terms/Core/HashAlgorithm/crystalsKyber> a owl:NamedIndividual,
            ns1:HashAlgorithm ;
        rdfs:label "crystalsKyber" ;
        rdfs:comment "[Kyber](https://pq-crystals.org/kyber/)"@en .

    <https://spdx.org/rdf/3.0.1/terms/Core/HashAlgorithm/falcon> a owl:NamedIndividual,
            ns1:HashAlgorithm ;
        rdfs:label "falcon" ;
        rdfs:comment "[FALCON](https://falcon-sign.info/falcon.pdf)"@en .

    <https://spdx.org/rdf/3.0.1/terms/Core/HashAlgorithm/md2> a owl:NamedIndividual,
            ns1:HashAlgorithm ;
        rdfs:label "md2" ;
        rdfs:comment "MD2 message-digest algorithm, as defined in [RFC 1319](https://datatracker.ietf.org/doc/rfc1319/)."@en .

    <https://spdx.org/rdf/3.0.1/terms/Core/HashAlgorithm/md4> a owl:NamedIndividual,
            ns1:HashAlgorithm ;
        rdfs:label "md4" ;
        rdfs:comment "MD4 message-digest algorithm, as defined in [RFC 1186](https://datatracker.ietf.org/doc/rfc1186/)."@en .

    <https://spdx.org/rdf/3.0.1/terms/Core/HashAlgorithm/md5> a owl:NamedIndividual,
            ns1:HashAlgorithm ;
        rdfs:label "md5" ;
        rdfs:comment "MD5 message-digest algorithm, as defined in [RFC 1321](https://datatracker.ietf.org/doc/rfc1321/)."@en .

    <https://spdx.org/rdf/3.0.1/terms/Core/HashAlgorithm/md6> a owl:NamedIndividual,
            ns1:HashAlgorithm ;
        rdfs:label "md6" ;
        rdfs:comment "[MD6 hash function](https://people.csail.mit.edu/rivest/pubs/RABCx08.pdf)"@en .

    <https://spdx.org/rdf/3.0.1/terms/Core/HashAlgorithm/other> a owl:NamedIndividual,
            ns1:HashAlgorithm ;
        rdfs:label "other" ;
        rdfs:comment "any hashing algorithm that does not exist in this list of entries"@en .

    <https://spdx.org/rdf/3.0.1/terms/Core/HashAlgorithm/sha1> a owl:NamedIndividual,
            ns1:HashAlgorithm ;
        rdfs:label "sha1" ;
        rdfs:comment "SHA-1, a secure hashing algorithm, as defined in [RFC 3174](https://datatracker.ietf.org/doc/rfc3174/)."@en .

    <https://spdx.org/rdf/3.0.1/terms/Core/HashAlgorithm/sha224> a owl:NamedIndividual,
            ns1:HashAlgorithm ;
        rdfs:label "sha224" ;
        rdfs:comment "SHA-2 with a digest length of 224, as defined in [RFC 3874](https://datatracker.ietf.org/doc/rfc3874/)."@en .

    <https://spdx.org/rdf/3.0.1/terms/Core/HashAlgorithm/sha256> a owl:NamedIndividual,
            ns1:HashAlgorithm ;
        rdfs:label "sha256" ;
        rdfs:comment "SHA-2 with a digest length of 256, as defined in [RFC 6234](https://datatracker.ietf.org/doc/rfc6234/)."@en .

    <https://spdx.org/rdf/3.0.1/terms/Core/HashAlgorithm/sha384> a owl:NamedIndividual,
            ns1:HashAlgorithm ;
        rdfs:label "sha384" ;
        rdfs:comment "SHA-2 with a digest length of 384, as defined in [RFC 6234](https://datatracker.ietf.org/doc/rfc6234/)."@en .

    <https://spdx.org/rdf/3.0.1/terms/Core/HashAlgorithm/sha3_224> a owl:NamedIndividual,
            ns1:HashAlgorithm ;
        rdfs:label "sha3_224" ;
        rdfs:comment "SHA-3 with a digest length of 224, as defined in [FIPS 202](https://csrc.nist.gov/pubs/fips/202/final)."@en .

    <https://spdx.org/rdf/3.0.1/terms/Core/HashAlgorithm/sha3_256> a owl:NamedIndividual,
            ns1:HashAlgorithm ;
        rdfs:label "sha3_256" ;
        rdfs:comment "SHA-3 with a digest length of 256, as defined in [FIPS 202](https://csrc.nist.gov/pubs/fips/202/final)."@en .

    <https://spdx.org/rdf/3.0.1/terms/Core/HashAlgorithm/sha3_384> a owl:NamedIndividual,
            ns1:HashAlgorithm ;
        rdfs:label "sha3_384" ;
        rdfs:comment "SHA-3 with a digest length of 384, as defined in [FIPS 202](https://csrc.nist.gov/pubs/fips/202/final)."@en .

    <https://spdx.org/rdf/3.0.1/terms/Core/HashAlgorithm/sha3_512> a owl:NamedIndividual,
            ns1:HashAlgorithm ;
        rdfs:label "sha3_512" ;
        rdfs:comment "SHA-3 with a digest length of 512, as defined in [FIPS 202](https://csrc.nist.gov/pubs/fips/202/final)."@en .

    <https://spdx.org/rdf/3.0.1/terms/Core/HashAlgorithm/sha512> a owl:NamedIndividual,
            ns1:HashAlgorithm ;
        rdfs:label "sha512" ;
        rdfs:comment "SHA-2 with a digest length of 512, as defined in [RFC 6234](https://datatracker.ietf.org/doc/rfc6234/)."@en .

    ns1:IndividualElement a owl:Class ;
        rdfs:comment """A concrete subclass of Element used by Individuals in the
Core profile."""@en ;
        rdfs:subClassOf ns1:Element ;
        sh:nodeKind sh:IRI .

    ns1:NamespaceMap a owl:Class,
            sh:NodeShape ;
        rdfs:comment "A mapping between prefixes and namespace partial URIs."@en ;
        sh:nodeKind sh:BlankNodeOrIRI ;
        sh:property _:N5d132aff09b440f59ba2720d679260b0,
            _:N7495455ebc1a485091680d44af0fed6e .

    ns1:Relationship a owl:Class,
            sh:NodeShape ;
        rdfs:comment "Describes a relationship between one or more elements."@en ;
        rdfs:subClassOf ns1:Element ;
        sh:nodeKind sh:IRI ;
        sh:property _:N01102945df74418fb5e5d1d74b8bf17f,
            _:N7a01e1ee4d5040288bd6d52941764a70,
            _:Nb03705dfc9524babbc8adb93ad2b4062,
            _:Nbeba224eb8864897a66ad9eb4c13fd52,
            _:Nda66589397164e3e8b13693c43d08638,
            _:Ne51c4c707e4f41a1b4da38412adebb44 .

    ns1:Tool a owl:Class ;
        rdfs:comment "An element of hardware and/or software utilized to carry out a particular function."@en ;
        rdfs:subClassOf ns1:Element ;
        sh:nodeKind sh:IRI .

    ns1:algorithm a owl:ObjectProperty ;
        rdfs:comment "Specifies the algorithm used for calculating the hash value."@en ;
        rdfs:range ns1:HashAlgorithm .

    ns1:hashValue a owl:DatatypeProperty ;
        rdfs:comment "The result of applying a hash algorithm to an Element."@en ;
        rdfs:range xsd:string .

    ns1:suppliedBy a owl:ObjectProperty ;
        rdfs:comment """Identifies who or what supplied the artifact or VulnAssessmentRelationship
referenced by the Element."""@en ;
        rdfs:range ns1:Agent .

    ns1:verifiedUsing a owl:ObjectProperty ;
        rdfs:comment """Provides an IntegrityMethod with which the integrity of an Element can be
asserted."""@en ;
        rdfs:range ns1:IntegrityMethod .

    ns6:IndividualLicensingInfo a owl:Class ;
        rdfs:comment """A concrete subclass of AnyLicenseInfo used by Individuals in the
ExpandedLicensing profile."""@en ;
        rdfs:subClassOf <https://spdx.org/rdf/3.0.1/terms/SimpleLicensing/AnyLicenseInfo> ;
        sh:nodeKind sh:IRI .

    ns6:deprecatedVersion a owl:DatatypeProperty ;
        rdfs:comment """Specifies the SPDX License List version in which this license or exception
identifier was deprecated."""@en ;
        rdfs:range xsd:string .

    ns6:licenseXml a owl:DatatypeProperty ;
        rdfs:comment """Identifies all the text and metadata associated with a license in the license
XML format."""@en ;
        rdfs:range xsd:string .

    ns6:listVersionAdded a owl:DatatypeProperty ;
        rdfs:comment """Specifies the SPDX License List version in which this ListedLicense or
ListedLicenseException identifier was first added."""@en ;
        rdfs:range xsd:string .

    ns6:member a owl:ObjectProperty ;
        rdfs:comment "A license expression participating in a license set."@en ;
        rdfs:range <https://spdx.org/rdf/3.0.1/terms/SimpleLicensing/AnyLicenseInfo> .

    ns6:obsoletedBy a owl:DatatypeProperty ;
        rdfs:comment """Specifies the licenseId that is preferred to be used in place of a deprecated
License or LicenseAddition."""@en ;
        rdfs:range xsd:string .

    ns6:seeAlso a owl:DatatypeProperty ;
        rdfs:comment "Contains a URL where the License or LicenseAddition can be found in use."@en ;
        rdfs:range xsd:anyURI .

    <https://spdx.org/rdf/3.0.1/terms/Extension/CdxPropertyEntry> a owl:Class,
            sh:NodeShape ;
        rdfs:comment "A property name with an associated value."@en ;
        sh:nodeKind sh:BlankNodeOrIRI ;
        sh:property _:N913effc8986249ddbf450a571d06d45e,
            _:N9f736b62e774479ca799c05a49ab2af6 .

    <https://spdx.org/rdf/3.0.1/terms/Security/CvssSeverityType/critical> a owl:NamedIndividual,
            ns3:CvssSeverityType ;
        rdfs:label "critical" ;
        rdfs:comment "When a CVSS score is between 9.0 - 10.0"@en .

    <https://spdx.org/rdf/3.0.1/terms/Security/CvssSeverityType/high> a owl:NamedIndividual,
            ns3:CvssSeverityType ;
        rdfs:label "high" ;
        rdfs:comment "When a CVSS score is between 7.0 - 8.9"@en .

    <https://spdx.org/rdf/3.0.1/terms/Security/CvssSeverityType/low> a owl:NamedIndividual,
            ns3:CvssSeverityType ;
        rdfs:label "low" ;
        rdfs:comment "When a CVSS score is between 0.1 - 3.9"@en .

    <https://spdx.org/rdf/3.0.1/terms/Security/CvssSeverityType/medium> a owl:NamedIndividual,
            ns3:CvssSeverityType ;
        rdfs:label "medium" ;
        rdfs:comment "When a CVSS score is between 4.0 - 6.9"@en .

    <https://spdx.org/rdf/3.0.1/terms/Security/CvssSeverityType/none> a owl:NamedIndividual,
            ns3:CvssSeverityType ;
        rdfs:label "none" ;
        rdfs:comment "When a CVSS score is 0.0"@en .

    ns3:modifiedTime a owl:DatatypeProperty ;
        rdfs:comment "Specifies a time when a vulnerability assessment was modified"@en ;
        rdfs:range xsd:dateTimeStamp .

    ns3:publishedTime a owl:DatatypeProperty ;
        rdfs:comment "Specifies the time when a vulnerability was published."@en ;
        rdfs:range xsd:dateTimeStamp .

    ns3:severity a owl:ObjectProperty ;
        rdfs:comment "Specifies the CVSS qualitative severity rating of a vulnerability in relation to a piece of software."@en ;
        rdfs:range ns3:CvssSeverityType .

    ns3:withdrawnTime a owl:DatatypeProperty ;
        rdfs:comment "Specified the time and date when a vulnerability was withdrawn."@en ;
        rdfs:range xsd:dateTimeStamp .

    <https://spdx.org/rdf/3.0.1/terms/SimpleLicensing/licenseText> a owl:DatatypeProperty ;
        rdfs:comment "Identifies the full text of a License or Addition."@en ;
        rdfs:range xsd:string .

    ns2:ContentIdentifier a owl:Class,
            sh:NodeShape ;
        rdfs:comment "A canonical, unique, immutable identifier"@en ;
        rdfs:subClassOf ns1:IntegrityMethod ;
        sh:nodeKind sh:BlankNodeOrIRI ;
        sh:property _:N97a6578de8ef458ba572f30b64456e83,
            _:Nbe63329c930b4ada8dafd59ab2a6d17f .

    ns2:File a owl:Class,
            sh:NodeShape ;
        rdfs:comment "Refers to any object that stores content on a computer."@en ;
        rdfs:subClassOf ns2:SoftwareArtifact ;
        sh:nodeKind sh:IRI ;
        sh:property _:Ne89807f76836447eb0705178b28eb703,
            _:Ne8e3a0b318ce4f5aa1caff37d2fcb20a .

    ns2:Package a owl:Class,
            sh:NodeShape ;
        rdfs:comment """Refers to any unit of content that can be associated with a distribution of
software."""@en ;
        rdfs:subClassOf ns2:SoftwareArtifact ;
        sh:nodeKind sh:IRI ;
        sh:property _:N17a7e638822c4c1080384386cc9a1f1e,
            _:N366fd9b9b76b4bc08ca7165010e37d97,
            _:N4abe73c07c824471919274e19e60d372,
            _:Nd4ed37fcf1fd4068bb0deee0221ce837,
            _:Nfd7fff7459584d6a8b9be92d44234a7f .

    <https://spdx.org/rdf/3.0.1/terms/Software/SoftwarePurpose/application> a owl:NamedIndividual,
            ns2:SoftwarePurpose ;
        rdfs:label "application" ;
        rdfs:comment "The Element is a software application."@en .

    <https://spdx.org/rdf/3.0.1/terms/Software/SoftwarePurpose/archive> a owl:NamedIndividual,
            ns2:SoftwarePurpose ;
        rdfs:label "archive" ;
        rdfs:comment "The Element is an archived collection of one or more files (.tar, .zip, etc.)."@en .

    <https://spdx.org/rdf/3.0.1/terms/Software/SoftwarePurpose/bom> a owl:NamedIndividual,
            ns2:SoftwarePurpose ;
        rdfs:label "bom" ;
        rdfs:comment "The Element is a bill of materials."@en .

    <https://spdx.org/rdf/3.0.1/terms/Software/SoftwarePurpose/configuration> a owl:NamedIndividual,
            ns2:SoftwarePurpose ;
        rdfs:label "configuration" ;
        rdfs:comment "The Element is configuration data."@en .

    <https://spdx.org/rdf/3.0.1/terms/Software/SoftwarePurpose/container> a owl:NamedIndividual,
            ns2:SoftwarePurpose ;
        rdfs:label "container" ;
        rdfs:comment "The Element is a container image which can be used by a container runtime application."@en .

    <https://spdx.org/rdf/3.0.1/terms/Software/SoftwarePurpose/data> a owl:NamedIndividual,
            ns2:SoftwarePurpose ;
        rdfs:label "data" ;
        rdfs:comment "The Element is data."@en .

    <https://spdx.org/rdf/3.0.1/terms/Software/SoftwarePurpose/device> a owl:NamedIndividual,
            ns2:SoftwarePurpose ;
        rdfs:label "device" ;
        rdfs:comment "The Element refers to a chipset, processor, or electronic board."@en .

    <https://spdx.org/rdf/3.0.1/terms/Software/SoftwarePurpose/deviceDriver> a owl:NamedIndividual,
            ns2:SoftwarePurpose ;
        rdfs:label "deviceDriver" ;
        rdfs:comment "The Element represents software that controls hardware devices."@en .

    <https://spdx.org/rdf/3.0.1/terms/Software/SoftwarePurpose/diskImage> a owl:NamedIndividual,
            ns2:SoftwarePurpose ;
        rdfs:label "diskImage" ;
        rdfs:comment "The Element refers to a disk image that can be written to a disk, booted in a VM, etc. A disk image typically contains most or all of the components necessary to boot, such as bootloaders, kernels, firmware, userspace, etc."@en .

    <https://spdx.org/rdf/3.0.1/terms/Software/SoftwarePurpose/documentation> a owl:NamedIndividual,
            ns2:SoftwarePurpose ;
        rdfs:label "documentation" ;
        rdfs:comment "The Element is documentation."@en .

    <https://spdx.org/rdf/3.0.1/terms/Software/SoftwarePurpose/evidence> a owl:NamedIndividual,
            ns2:SoftwarePurpose ;
        rdfs:label "evidence" ;
        rdfs:comment "The Element is the evidence that a specification or requirement has been fulfilled."@en .

    <https://spdx.org/rdf/3.0.1/terms/Software/SoftwarePurpose/executable> a owl:NamedIndividual,
            ns2:SoftwarePurpose ;
        rdfs:label "executable" ;
        rdfs:comment "The Element is an Artifact that can be run on a computer."@en .

    <https://spdx.org/rdf/3.0.1/terms/Software/SoftwarePurpose/file> a owl:NamedIndividual,
            ns2:SoftwarePurpose ;
        rdfs:label "file" ;
        rdfs:comment "The Element is a single file which can be independently distributed (configuration file, statically linked binary, Kubernetes deployment, etc.)."@en .

    <https://spdx.org/rdf/3.0.1/terms/Software/SoftwarePurpose/filesystemImage> a owl:NamedIndividual,
            ns2:SoftwarePurpose ;
        rdfs:label "filesystemImage" ;
        rdfs:comment "The Element is a file system image that can be written to a disk (or virtual) partition."@en .

    <https://spdx.org/rdf/3.0.1/terms/Software/SoftwarePurpose/firmware> a owl:NamedIndividual,
            ns2:SoftwarePurpose ;
        rdfs:label "firmware" ;
        rdfs:comment "The Element provides low level control over a device's hardware."@en .

    <https://spdx.org/rdf/3.0.1/terms/Software/SoftwarePurpose/framework> a owl:NamedIndividual,
            ns2:SoftwarePurpose ;
        rdfs:label "framework" ;
        rdfs:comment "The Element is a software framework."@en .

    <https://spdx.org/rdf/3.0.1/terms/Software/SoftwarePurpose/install> a owl:NamedIndividual,
            ns2:SoftwarePurpose ;
        rdfs:label "install" ;
        rdfs:comment "The Element is used to install software on disk."@en .

    <https://spdx.org/rdf/3.0.1/terms/Software/SoftwarePurpose/library> a owl:NamedIndividual,
            ns2:SoftwarePurpose ;
        rdfs:label "library" ;
        rdfs:comment "The Element is a software library."@en .

    <https://spdx.org/rdf/3.0.1/terms/Software/SoftwarePurpose/manifest> a owl:NamedIndividual,
            ns2:SoftwarePurpose ;
        rdfs:label "manifest" ;
        rdfs:comment "The Element is a software manifest."@en .

    <https://spdx.org/rdf/3.0.1/terms/Software/SoftwarePurpose/model> a owl:NamedIndividual,
            ns2:SoftwarePurpose ;
        rdfs:label "model" ;
        rdfs:comment "The Element is a machine learning or artificial intelligence model."@en .

    <https://spdx.org/rdf/3.0.1/terms/Software/SoftwarePurpose/module> a owl:NamedIndividual,
            ns2:SoftwarePurpose ;
        rdfs:label "module" ;
        rdfs:comment "The Element is a module of a piece of software."@en .

    <https://spdx.org/rdf/3.0.1/terms/Software/SoftwarePurpose/operatingSystem> a owl:NamedIndividual,
            ns2:SoftwarePurpose ;
        rdfs:label "operatingSystem" ;
        rdfs:comment "The Element is an operating system."@en .

    <https://spdx.org/rdf/3.0.1/terms/Software/SoftwarePurpose/other> a owl:NamedIndividual,
            ns2:SoftwarePurpose ;
        rdfs:label "other" ;
        rdfs:comment "The Element doesn't fit into any of the other categories."@en .

    <https://spdx.org/rdf/3.0.1/terms/Software/SoftwarePurpose/patch> a owl:NamedIndividual,
            ns2:SoftwarePurpose ;
        rdfs:label "patch" ;
        rdfs:comment "The Element contains a set of changes to update, fix, or improve another Element."@en .

    <https://spdx.org/rdf/3.0.1/terms/Software/SoftwarePurpose/platform> a owl:NamedIndividual,
            ns2:SoftwarePurpose ;
        rdfs:label "platform" ;
        rdfs:comment "The Element represents a runtime environment."@en .

    <https://spdx.org/rdf/3.0.1/terms/Software/SoftwarePurpose/requirement> a owl:NamedIndividual,
            ns2:SoftwarePurpose ;
        rdfs:label "requirement" ;
        rdfs:comment "The Element provides a requirement needed as input for another Element."@en .

    <https://spdx.org/rdf/3.0.1/terms/Software/SoftwarePurpose/source> a owl:NamedIndividual,
            ns2:SoftwarePurpose ;
        rdfs:label "source" ;
        rdfs:comment "The Element is a single or a collection of source files."@en .

    <https://spdx.org/rdf/3.0.1/terms/Software/SoftwarePurpose/specification> a owl:NamedIndividual,
            ns2:SoftwarePurpose ;
        rdfs:label "specification" ;
        rdfs:comment "The Element is a plan, guideline or strategy how to create, perform or analyze an application."@en .

    <https://spdx.org/rdf/3.0.1/terms/Software/SoftwarePurpose/test> a owl:NamedIndividual,
            ns2:SoftwarePurpose ;
        rdfs:label "test" ;
        rdfs:comment "The Element is a test used to verify functionality on an software element."@en .

    ns1:ElementCollection a owl:Class,
            sh:NodeShape ;
        rdfs:comment "A collection of Elements, not necessarily with unifying context."@en ;
        rdfs:subClassOf ns1:Element ;
        sh:nodeKind sh:IRI ;
        sh:property _:N0d8ab67fef5a462782a0f0148ebbfd14,
            _:N2bb25b7428344e1fba7d66839c2f61b1,
            _:N45414da51a244066a02218d1ebe6fb31,
            _:N8277ba52ec1d49079b2448e68d672999 .

    <https://spdx.org/rdf/3.0.1/terms/Core/PresenceType/no> a owl:NamedIndividual,
            ns1:PresenceType ;
        rdfs:label "no" ;
        rdfs:comment "Indicates absence of the field."@en .

    <https://spdx.org/rdf/3.0.1/terms/Core/PresenceType/noAssertion> a owl:NamedIndividual,
            ns1:PresenceType ;
        rdfs:label "noAssertion" ;
        rdfs:comment "Makes no assertion about the field."@en .

    <https://spdx.org/rdf/3.0.1/terms/Core/PresenceType/yes> a owl:NamedIndividual,
            ns1:PresenceType ;
        rdfs:label "yes" ;
        rdfs:comment "Indicates presence of the field."@en .

    ns1:contentType a owl:DatatypeProperty ;
        rdfs:comment "Provides information about the content type of an Element or a Property."@en ;
        rdfs:range xsd:string .

    ns3:score a owl:DatatypeProperty ;
        rdfs:comment "Provides a numerical (0-10) representation of the severity of a vulnerability."@en ;
        rdfs:range xsd:decimal .

    ns3:vectorString a owl:DatatypeProperty ;
        rdfs:comment "Specifies the CVSS vector string for a vulnerability."@en ;
        rdfs:range xsd:string .

    ns1:AnnotationType a owl:Class ;
        rdfs:comment "Specifies the type of an annotation."@en .

    ns1:PositiveIntegerRange a owl:Class,
            sh:NodeShape ;
        rdfs:comment "A tuple of two positive integers that define a range."@en ;
        sh:nodeKind sh:BlankNodeOrIRI ;
        sh:property _:N2f9be71ecf104b7e813465456ba1e423,
            _:Nd7b0801994b24e409fe5c6d54edb8618 .

    <https://spdx.org/rdf/3.0.1/terms/Extension/Extension> a owl:Class ;
        rdfs:comment "A characterization of some aspect of an Element that is associated with the Element in a generalized fashion."@en ;
        sh:nodeKind sh:BlankNodeOrIRI ;
        sh:property _:Nc7e2cbf4e3484223ac825b08c7c397c1 .

    ns3:ExploitCatalogType a owl:Class ;
        rdfs:comment "Specifies the exploit catalog type."@en .

    ns2:ContentIdentifierType a owl:Class ;
        rdfs:comment "Specifies the type of a content identifier."@en .

    ns2:FileKindType a owl:Class ;
        rdfs:comment "Enumeration of the different kinds of SPDX file."@en .

    ns4:EnergyUnitType a owl:Class ;
        rdfs:comment "Specifies the unit of energy consumption."@en .

    ns1:Artifact a owl:Class,
            sh:NodeShape ;
        rdfs:comment "A distinct article or unit within the digital domain."@en ;
        rdfs:subClassOf ns1:Element ;
        sh:nodeKind sh:IRI ;
        sh:property _:N3bacd14e00cd43ec8e1a380d19b80f1c,
            _:N51fe6b029f2a4c248a031cce1ef80bbf,
            _:N5eaa4fa988944c7a9423ee9461519d03,
            _:N6ac9d864a4e742c68b114de0bb33e8c3,
            _:N730b491010ab4f9bafd08494e408c982,
            _:Necfaa34feca646d2bbdae7cf330b0d21,
            _:Nf411b42be5ac4dcc8a50125556eabe37,
            _:Nfdbfecf7fd1f4fbe972985748c2fb51f .

    ns1:RelationshipCompleteness a owl:Class ;
        rdfs:comment "Indicates whether a relationship is known to be complete, incomplete, or if no assertion is made with respect to relationship completeness."@en .

    ns1:SpdxOrganization a owl:NamedIndividual,
            ns1:Organization ;
        rdfs:comment "An Organization representing the SPDX Project."@en ;
        owl:sameAs <https://spdx.org/> ;
        ns1:creationInfo <https://spdx.org/rdf/3.0.1/creationInfo_SpdxOrganization> .

    ns1:comment a owl:DatatypeProperty ;
        rdfs:comment """Provide consumers with comments by the creator of the Element about the
Element."""@en ;
        rdfs:range xsd:string .

    ns6:ExtendableLicense a owl:Class ;
        rdfs:comment "Abstract class representing a License or an OrLaterOperator."@en ;
        rdfs:subClassOf <https://spdx.org/rdf/3.0.1/terms/SimpleLicensing/AnyLicenseInfo> ;
        sh:nodeKind sh:IRI ;
        sh:property _:N310b971e33114ae2ba90bb1031704dcb .

    ns6:License a owl:Class,
            sh:NodeShape ;
        rdfs:comment "Abstract class for the portion of an AnyLicenseInfo representing a license."@en ;
        rdfs:subClassOf ns6:ExtendableLicense ;
        sh:nodeKind sh:IRI ;
        sh:property _:N317b60f774da4d7b8498a148dc2596b8,
            _:N3482d1d4103c44329fb2b6d0fd07d1d8,
            _:Na67ca3acaea24305b83b762bb3b5ece7,
            _:Naaabaeb0746945a2b67c9fbd19352387,
            _:Nb6694670c0bd4d9bbe1584c6f432d254,
            _:Nb9ebb94743d44ed8a77201960c92de33,
            _:Nc2c772a4e30946299238d1ddc3e1703f,
            _:Ne288e79e880942c88b00de65120682a6,
            _:Ne3c3e73bf0024056b48f227a5a1a82b4,
            _:Ne43e2e4ed2284b8faf28cc074be90105 .

    ns6:LicenseAddition a owl:Class,
            sh:NodeShape ;
        rdfs:comment """Abstract class for additional text intended to be added to a License, but
which is not itself a standalone License."""@en ;
        rdfs:subClassOf ns1:Element ;
        sh:nodeKind sh:IRI ;
        sh:property _:N14b04433b77f41cd8ab23bf7d9581144,
            _:N2ecf638c2cd34c9488be93286bfeaf81,
            _:N3152dc6f33cc4847a973c6e7c1cece5e,
            _:N58eec31acc944eefac091c246f27a7f1,
            _:N7e0a9e9a6b7b402bbf68b76243025f34,
            _:Na025116d022643e2beeb87ce5077615a,
            _:Nf9bbec9b6b924452ac692c71f561aa1d .

    ns3:VexVulnAssessmentRelationship a owl:Class,
            sh:NodeShape ;
        rdfs:comment "Abstract ancestor class for all VEX relationships"@en ;
        rdfs:subClassOf ns3:VulnAssessmentRelationship ;
        sh:nodeKind sh:IRI ;
        sh:property _:N995bc073d1bb493782caa95bd840ac7d,
            _:Ne7e5a05ecc9543c1886186899803709a,
            _:Nfedcce2ec4334b5dbcd72a892757bcfb .

    ns4:EnergyConsumptionDescription a owl:Class,
            sh:NodeShape ;
        rdfs:comment """The class that helps note down the quantity of energy consumption and the unit
used for measurement."""@en ;
        sh:nodeKind sh:BlankNodeOrIRI ;
        sh:property _:Ne77d3a4557c448f4ac0a95430be9327a,
            _:Nf539274bb41f4f0aad37bb02b1e1ad05 .

    ns4:SafetyRiskAssessmentType a owl:Class ;
        rdfs:comment "Specifies the safety risk level."@en .

    ns5:ConfidentialityLevelType a owl:Class ;
        rdfs:comment "Categories of confidentiality level."@en .

    ns3:SsvcDecisionType a owl:Class ;
        rdfs:comment "Specifies the SSVC decision type."@en .

    ns2:SoftwareArtifact a owl:Class,
            sh:NodeShape ;
        rdfs:comment "A distinct article or unit related to Software."@en ;
        rdfs:subClassOf ns1:Artifact ;
        sh:nodeKind sh:IRI ;
        sh:property _:N57e7f375488f4e6e8c8862f77c82dcec,
            _:N5800e826741c40a4b0356163725fb8ff,
            _:N5a157fd1df584770bbabc6970f51ccf2,
            _:N5ad0acebc6e649fbbe183acddf8af24c,
            _:N87484f238313462d86eb931a8e656419,
            _:Nf0383326d60f4bc6bc14664a2e85ec74 .

    ns1:CreationInfo a owl:Class,
            sh:NodeShape ;
        rdfs:comment "Provides information about the creation of the Element."@en ;
        sh:nodeKind sh:BlankNodeOrIRI ;
        sh:property _:N27f0016e8ca74bccbbbe464b2548f1b5,
            _:N690e144eccf540c0bdf8b5006d4d10b0,
            _:N6ea4943e498c4dd1b48743b06fa1f4ac,
            _:N8fba128d40804e9da2b1794c012fb0d0,
            _:Nd4bee614558747679a512d0df577540b .

    ns1:IntegrityMethod a owl:Class,
            sh:NodeShape ;
        rdfs:comment "Provides an independently reproducible mechanism that permits verification of a specific Element."@en ;
        sh:nodeKind sh:BlankNodeOrIRI ;
        sh:property _:N27fc956376b64f42a9eba01aa0464e5d,
            _:N79d84a9512cc4810940269e53d06703f .

    ns5:DatasetAvailabilityType a owl:Class ;
        rdfs:comment "Availability of dataset."@en .

    ns3:VexJustificationType a owl:Class ;
        rdfs:comment "Specifies the VEX justification type."@en .

    ns1:LifecycleScopeType a owl:Class ;
        rdfs:comment "Provide an enumerated set of lifecycle phases that can provide context to relationships."@en .

    ns3:CvssSeverityType a owl:Class ;
        rdfs:comment "Specifies the CVSS base, temporal, threat, or environmental severity type."@en .

    ns3:VulnAssessmentRelationship a owl:Class,
            sh:NodeShape ;
        rdfs:comment "Abstract ancestor class for all vulnerability assessments"@en ;
        rdfs:subClassOf ns1:Relationship ;
        sh:nodeKind sh:IRI ;
        sh:property _:N44383a20cc57437d807fa42adc1120a1,
            _:N5af2023939dd4cdaa456efa9c2789ef9,
            _:N5c7c7a7867f94c258c1deed98c95cfae,
            _:N86dd9cfc30c44518bd414964b7fbae8b,
            _:Na02e1b7ab4ab4241a581e9c0bf13fb7d,
            _:Naadc48528c324fbfaeb8eb293f4febe4 .

    ns2:SbomType a owl:Class ;
        rdfs:comment """Provides a set of values to be used to describe the common types of SBOMs that
tools may create."""@en .

    ns1:PresenceType a owl:Class ;
        rdfs:comment "Categories of presence or absence."@en .

    ns1:SupportType a owl:Class ;
        rdfs:comment "Indicates the type of support that is associated with an artifact."@en .

    ns1:Agent a owl:Class ;
        rdfs:comment "Agent represents anything with the potential to act on a system."@en ;
        rdfs:subClassOf ns1:Element ;
        sh:nodeKind sh:IRI .

    ns1:ProfileIdentifierType a owl:Class ;
        rdfs:comment "Enumeration of the valid profiles."@en .

    <https://spdx.org/rdf/3.0.1/terms/SimpleLicensing/AnyLicenseInfo> a owl:Class ;
        rdfs:comment "Abstract class representing a license combination consisting of one or more licenses."@en ;
        rdfs:subClassOf ns1:Element ;
        sh:nodeKind sh:IRI ;
        sh:property _:N5e1a4e1ad13f4508bae4883983e83867 .

    ns1:ExternalIdentifierType a owl:Class ;
        rdfs:comment "Specifies the type of an external identifier."@en .

    ns1:DictionaryEntry a owl:Class,
            sh:NodeShape ;
        rdfs:comment "A key with an associated value."@en ;
        sh:nodeKind sh:BlankNodeOrIRI ;
        sh:property _:Nbfe64e0eb7844cb39384263cf19da3b5,
            _:Nd91d7910edf44e0683080e7e6530cf13 .

    ns5:DatasetType a owl:Class ;
        rdfs:comment "Enumeration of dataset types."@en .

    ns1:Element a owl:Class,
            sh:NodeShape ;
        rdfs:comment "Base domain class from which all other SPDX-3.0 domain classes derive."@en ;
        sh:nodeKind sh:IRI ;
        sh:property _:N1b3f16fc6edf445691f46007166ee54a,
            _:N4dde5c3db9e44e0db1c1051e698b0aed,
            _:N693a0ac59cbf4f04a09a47000f92bf97,
            _:N7419f22add2b4107ab0c5b25f53b788b,
            _:N7d70a3f168464a16aaa2ce14fe3f54a2,
            _:N906b4e4cb5ba41b1bf9345ba1c8b1f5a,
            _:Nc484f7d89c4d48dba9c5086fad8a3f71,
            _:Ncc33c607adee40068ee304956b2dc382,
            _:Ndd38650fb33a437387707abd8ca9f4a0,
            _:Ne6c4aa6804e944f8bd7a0ef6b63f41b3 .

    ns1:HashAlgorithm a owl:Class ;
        rdfs:comment "A mathematical algorithm that maps data of arbitrary size to a bit string."@en .

    ns2:SoftwarePurpose a owl:Class ;
        rdfs:comment "Provides information about the primary purpose of an Element."@en .

    ns1:ExternalRefType a owl:Class ;
        rdfs:comment "Specifies the type of an external reference."@en .

    ns1:RelationshipType a owl:Class ;
        rdfs:comment "Information about the relationship between two Elements."@en .

    _:N008447ea57994f4ba18f202542dbb1fe rdf:first <https://spdx.org/rdf/3.0.1/terms/Core/ExternalRefType/securityPolicy> ;
        rdf:rest _:N1cf6c5cdbb7d499ea3088257df2391f6 .

    _:N00b58432199d4232a8b3fbf92ce42646 sh:datatype xsd:string ;
        sh:maxCount 1 ;
        sh:nodeKind sh:Literal ;
        sh:path ns5:datasetNoise .

    _:N00e704d327644d128a02819a171bb18d rdf:first <https://spdx.org/rdf/3.0.1/terms/Software/SoftwarePurpose/model> ;
        rdf:rest _:N2aadb3148a98468da6a856cede38e266 .

    _:N01102945df74418fb5e5d1d74b8bf17f sh:class ns1:RelationshipCompleteness ;
        sh:in _:Nd338fc87819546f6b745436b92c129a8 ;
        sh:maxCount 1 ;
        sh:nodeKind sh:IRI ;
        sh:path ns1:completeness .

    _:N01334926969a4a02ba648f9ae9cc0f83 rdf:first <https://spdx.org/rdf/3.0.1/terms/Dataset/DatasetType/image> ;
        rdf:rest _:Ne5a3b834457f4513b0d88d69c7a6165e .

    _:N0178bde213704f7e8468fbebd80cadcc rdf:first <https://spdx.org/rdf/3.0.1/terms/Security/ExploitCatalogType/other> ;
        rdf:rest () .

    _:N031bef5cc13746728e9d4a2bff4d5a99 rdf:first <https://spdx.org/rdf/3.0.1/terms/Software/SoftwarePurpose/manifest> ;
        rdf:rest _:N5929480f8a8844d3bad4d00a8c1536fd .

    _:N04c2c5076d534149865b12f9107c8c74 rdf:first <https://spdx.org/rdf/3.0.1/terms/Software/SbomType/deployed> ;
        rdf:rest _:N9d9ec4b5217e40f884dec6a2317cb4cd .

    _:N050ac1461eee41578dc14b28c0764ec0 rdf:first <https://spdx.org/rdf/3.0.1/terms/Software/SoftwarePurpose/library> ;
        rdf:rest _:Nc4b1e255f762490aaddc557a77379dfd .

    _:N054c6a610eb1434cbd912c9c3616c8db rdf:first <https://spdx.org/rdf/3.0.1/terms/Core/HashAlgorithm/md6> ;
        rdf:rest _:N2bfa9956fbb143dd924ac62a919c9c1f .

    _:N05a05a340bc1470fa1fe3d4528b8bcb0 sh:datatype xsd:dateTimeStamp ;
        sh:maxCount 1 ;
        sh:nodeKind sh:Literal ;
        sh:path ns3:withdrawnTime ;
        sh:pattern "^\\d\\d\\d\\d-\\d\\d-\\d\\dT\\d\\d:\\d\\d:\\d\\dZ$" .

    _:N05b14287499e40d4a351b15252bc652e rdf:first <https://spdx.org/rdf/3.0.1/terms/Core/HashAlgorithm/sha3_512> ;
        rdf:rest () .

    _:N05d54708c5954ef0b3ec6bc915712cc6 rdf:first <https://spdx.org/rdf/3.0.1/terms/Core/RelationshipType/hasHost> ;
        rdf:rest _:N349239d89edf4bea9f937007b0ef0381 .

    _:N06a47b60376c47aaac92b0a69159a1c0 rdf:first <https://spdx.org/rdf/3.0.1/terms/Core/HashAlgorithm/sha512> ;
        rdf:rest _:Nca907d776f8d4f5fa2254d492fb5d42a .

    _:N071319e2191b40ac86da6f2ec69be2fb rdf:first <https://spdx.org/rdf/3.0.1/terms/Core/ExternalRefType/staticAnalysisReport> ;
        rdf:rest _:N868e3594ba004020921e8238c75bc3b6 .

    _:N07457d45373c466ca415734a33afa350 rdf:first <https://spdx.org/rdf/3.0.1/terms/Core/ExternalRefType/bower> ;
        rdf:rest _:Naf8b909011f84634ab93339ae3001573 .

    _:N078b0758ac424dedab46bf98c3086c58 rdf:first <https://spdx.org/rdf/3.0.1/terms/Core/HashAlgorithm/blake2b256> ;
        rdf:rest _:N5fbd994d60b045a485f4161c29979d15 .

    _:N080d1530fe424885b2b334e1d3e9a22d rdf:first <https://spdx.org/rdf/3.0.1/terms/Core/RelationshipType/hasDocumentation> ;
        rdf:rest _:Nde571d96a80f4e85a264a336caf64f29 .

    _:N0890ae69e65244faaedb4c3978a6a3cf sh:hasValue <https://spdx.org/rdf/3.0.1/terms/SimpleLicensing/AnyLicenseInfo> .

    _:N0999c63e144249578cbe239e5cf95dd1 rdf:first <https://spdx.org/rdf/3.0.1/terms/Software/SoftwarePurpose/evidence> ;
        rdf:rest _:N79ea886ccc984e4ebac49b2a2ba05b8f .

    _:N0a0a67d1a9dc4ec7ab3b94209b868dff rdf:first <https://spdx.org/rdf/3.0.1/terms/Core/ExternalRefType/issueTracker> ;
        rdf:rest _:Ndcd4af75b0f549f59e8e7fb96c6b8e6d .

    _:N0afc30bb743f4d009a5d45f696c981ee rdf:first <https://spdx.org/rdf/3.0.1/terms/Software/SbomType/source> ;
        rdf:rest _:N3b75ee5664f246fba72f68de7ebbb459 .

    _:N0b485de1e2a74db28b6f6b7f5c8c114d sh:datatype xsd:string ;
        sh:maxCount 1 ;
        sh:nodeKind sh:Literal ;
        sh:path <https://spdx.org/rdf/3.0.1/terms/Build/buildId> .

    _:N0c46b9d033a048349acd598c3b002b65 rdf:first <https://spdx.org/rdf/3.0.1/terms/Core/RelationshipType/dependsOn> ;
        rdf:rest _:N2648b80a8ae84d97ad3d5cb789ee25e3 .

    _:N0c6b033e1de9470b841f93eb50058a0f sh:class ns6:ExtendableLicense ;
        sh:maxCount 1 ;
        sh:minCount 1 ;
        sh:nodeKind sh:IRI ;
        sh:path ns6:subjectExtendableLicense .

    _:N0d84cf0c0792460ea6248149d0eee551 sh:class ns1:AnnotationType ;
        sh:in _:N223565b5ce8043208abb5cc0a9bb2286 ;
        sh:maxCount 1 ;
        sh:minCount 1 ;
        sh:nodeKind sh:IRI ;
        sh:path ns1:annotationType .

    _:N0d896e6ea1824fb3a4ecd9a1e7fe690b sh:datatype xsd:decimal ;
        sh:maxCount 1 ;
        sh:minCount 1 ;
        sh:nodeKind sh:Literal ;
        sh:path ns3:score .

    _:N0d8ab67fef5a462782a0f0148ebbfd14 sh:message "https://spdx.org/rdf/3.0.1/terms/Core/ElementCollection is an abstract class and should not be instantiated directly. Instantiate a subclass instead."@en ;
        sh:not _:N42594dbee6274964a3d1d8726756dfae ;
        sh:path rdf:type .

    _:N0e18ea55685146fa9078163a7c3ff3d5 rdf:first <https://spdx.org/rdf/3.0.1/terms/Core/RelationshipType/exploitCreatedBy> ;
        rdf:rest _:Nff2e796ec34649ed9122145035384de4 .

    _:N0ee599289d3445dd98544cb7d542ad0f rdf:first <https://spdx.org/rdf/3.0.1/terms/Software/SoftwarePurpose/test> ;
        rdf:rest () .

    _:N0fe19c10b0404ecca1b3c2651b040358 sh:datatype xsd:string ;
        sh:maxCount 1 ;
        sh:nodeKind sh:Literal ;
        sh:path ns4:informationAboutTraining .

    _:N104ad32768b2480d979d26e4f5c885a6 rdf:first <https://spdx.org/rdf/3.0.1/terms/Core/ExternalRefType/chat> ;
        rdf:rest _:N93eaecf4ad5e433a924257276c8fd50c .

    _:N10a0a33d835147168e667e794740d037 sh:datatype xsd:anyURI ;
        sh:nodeKind sh:Literal ;
        sh:path ns1:identifierLocator .

    _:N10cc734ac08e44819863beb021240480 sh:datatype xsd:string ;
        sh:maxCount 1 ;
        sh:nodeKind sh:Literal ;
        sh:path ns6:deprecatedVersion .

    _:N10ebcc0edef24f468825cf6c178ee1c4 rdf:first <https://spdx.org/rdf/3.0.1/terms/Software/SoftwarePurpose/requirement> ;
        rdf:rest _:Nafe95e6667734b698498cff03063a128 .

    _:N1126ca33ef024311af0f994505ba646e rdf:first <https://spdx.org/rdf/3.0.1/terms/Core/HashAlgorithm/blake3> ;
        rdf:rest _:N71e76630f7fb413988a49c5df05f7010 .

    _:N11f4f26ee5534d1ca4e24eef77922411 sh:datatype xsd:string ;
        sh:nodeKind sh:Literal ;
        sh:path ns5:dataPreprocessing .

    _:N12267f2523f648ee866e621b0d8f1813 sh:class ns1:HashAlgorithm ;
        sh:in _:Nc7b576a90fb2450f98d1bc492f4fbe06 ;
        sh:maxCount 1 ;
        sh:minCount 1 ;
        sh:nodeKind sh:IRI ;
        sh:path ns1:algorithm .

    _:N12f123f6f5f0432695eadd7ebcb196b0 sh:datatype xsd:string ;
        sh:maxCount 1 ;
        sh:nodeKind sh:Literal ;
        sh:path ns1:contentType ;
        sh:pattern "^[^\\/]+\\/[^\\/]+$" .

    _:N13cc50f2fe3a4e479d1d76a35f55d81b rdf:first <https://spdx.org/rdf/3.0.1/terms/Software/SoftwarePurpose/specification> ;
        rdf:rest _:N4ed0fca567474133b4e3f3d20d02eeb5 .

    _:N149b28ab06e84c0f9c7a748fe270d619 rdf:first <https://spdx.org/rdf/3.0.1/terms/Dataset/DatasetType/other> ;
        rdf:rest _:N17fc35513d244f289a7301b6b0cdbf6c .

    _:N14b04433b77f41cd8ab23bf7d9581144 sh:datatype xsd:anyURI ;
        sh:nodeKind sh:Literal ;
        sh:path ns6:seeAlso .

    _:N14e47cb6a3474796844dd20924129ab6 sh:datatype xsd:dateTimeStamp ;
        sh:maxCount 1 ;
        sh:nodeKind sh:Literal ;
        sh:path ns3:impactStatementTime ;
        sh:pattern "^\\d\\d\\d\\d-\\d\\d-\\d\\dT\\d\\d:\\d\\d:\\d\\dZ$" .

    _:N15cc6817db284c3ca6607af958e89374 rdf:first <https://spdx.org/rdf/3.0.1/terms/Core/ExternalRefType/documentation> ;
        rdf:rest _:Nccd8642028564e56a31dc2ca5e9bde7d .

    _:N160083f6100f4e10a59b9acb061ad7a7 rdf:first <https://spdx.org/rdf/3.0.1/terms/Core/ExternalRefType/sourceArtifact> ;
        rdf:rest _:N071319e2191b40ac86da6f2ec69be2fb .

    _:N165e76779b954f6c829861fe80b13f8b sh:hasValue ns1:IntegrityMethod .

    _:N1677f5bfd8fa4911b5a3653d2c1a3263 rdf:first <https://spdx.org/rdf/3.0.1/terms/Security/CvssSeverityType/high> ;
        rdf:rest _:Na0bd1e47bbbf4e559d1a6f8399113223 .

    _:N169badfc343741d8b91b256cd37c91ef rdf:first <https://spdx.org/rdf/3.0.1/terms/Software/SoftwarePurpose/deviceDriver> ;
        rdf:rest _:Na8b27545614648d89e4b539a936b6592 .

    _:N179cf083985f41f09e2541d2ac40a243 rdf:first <https://spdx.org/rdf/3.0.1/terms/Core/RelationshipType/hasEvidence> ;
        rdf:rest _:Na9b18112b463447ebbfc551b36a6a936 .

    _:N17a7e638822c4c1080384386cc9a1f1e sh:datatype xsd:string ;
        sh:maxCount 1 ;
        sh:nodeKind sh:Literal ;
        sh:path ns2:sourceInfo .

    _:N17fc35513d244f289a7301b6b0cdbf6c rdf:first <https://spdx.org/rdf/3.0.1/terms/Dataset/DatasetType/sensor> ;
        rdf:rest _:Nf194d1d57fa14930b63cf53846dd5d0f .

    _:N180f2ecfb0d74d59bfdeefaeabb39288 sh:class ns1:DictionaryEntry ;
        sh:nodeKind sh:BlankNodeOrIRI ;
        sh:path ns4:metricDecisionThreshold .

    _:N189799efa65545fab51f17d5bb4eb46c sh:datatype xsd:string ;
        sh:maxCount 1 ;
        sh:minCount 1 ;
        sh:nodeKind sh:Literal ;
        sh:path <https://spdx.org/rdf/3.0.1/terms/SimpleLicensing/licenseText> .

    _:N1a47f2006ba941ce9bf72f120f3e0bd0 rdf:first <https://spdx.org/rdf/3.0.1/terms/Core/RelationshipType/hasDeletedFile> ;
        rdf:rest _:N7886db0616614a89abf7cbeff8975003 .

    _:N1acc6ac0c09846f9ba914ec4d6009865 rdf:first <https://spdx.org/rdf/3.0.1/terms/Software/SoftwarePurpose/configuration> ;
        rdf:rest _:N6c00277a300e432bb161c276667652ee .

    _:N1adb71f64c494276bd8ce6ba1835bb14 rdf:first <https://spdx.org/rdf/3.0.1/terms/Software/SoftwarePurpose/framework> ;
        rdf:rest _:N42dececf6d66453da82386bb8b6fcea9 .

    _:N1b3f16fc6edf445691f46007166ee54a sh:datatype xsd:string ;
        sh:maxCount 1 ;
        sh:nodeKind sh:Literal ;
        sh:path ns1:description .

    _:N1bd34863d96b4d6b8a6a7312d11b368a rdf:first <https://spdx.org/rdf/3.0.1/terms/Core/HashAlgorithm/crystalsKyber> ;
        rdf:rest _:N455be9fd7fe3499d944d70756225532d .

    _:N1c7200275aa241b5ae9a577d9c06b2d9 rdf:first <https://spdx.org/rdf/3.0.1/terms/Core/ProfileIdentifierType/lite> ;
        rdf:rest () .

    _:N1cf6c5cdbb7d499ea3088257df2391f6 rdf:first <https://spdx.org/rdf/3.0.1/terms/Core/ExternalRefType/securityThreatModel> ;
        rdf:rest _:Ndc33c03c6f3b4f76b2a9c5f0755b4682 .

    _:N1d299962dcc94d1dbe7ee3cf2bb5cf2e rdf:first <https://spdx.org/rdf/3.0.1/terms/Software/FileKindType/directory> ;
        rdf:rest () .

    _:N1de5d4dc34e04f919447cf643142160b rdf:first <https://spdx.org/rdf/3.0.1/terms/Software/SoftwarePurpose/platform> ;
        rdf:rest _:N10ebcc0edef24f468825cf6c178ee1c4 .

    _:N1fa42a3d9da34087baaa8c7892211524 sh:datatype xsd:string ;
        sh:maxCount 1 ;
        sh:nodeKind sh:Literal ;
        sh:path ns4:informationAboutApplication .

    _:N2014a2d4464246758ac5ad1b90e7355c sh:datatype xsd:string ;
        sh:maxCount 1 ;
        sh:nodeKind sh:Literal ;
        sh:path ns1:statement .

    _:N223565b5ce8043208abb5cc0a9bb2286 rdf:first <https://spdx.org/rdf/3.0.1/terms/Core/AnnotationType/other> ;
        rdf:rest _:N847e87312f6946cd8b8fec377fd7adb3 .

    _:N22f5d668ae27446e95d634e5bf09c6b4 rdf:first <https://spdx.org/rdf/3.0.1/terms/Core/PresenceType/no> ;
        rdf:rest _:N32ebad2ed20a45dabcae2791b60933f4 .

    _:N2313768eecea43dfbce33ea9abb10b56 sh:datatype xsd:string ;
        sh:maxCount 1 ;
        sh:minCount 1 ;
        sh:nodeKind sh:Literal ;
        sh:path ns3:vectorString .

    _:N2471049aadfe49bfbb3571150159e22b rdf:first <https://spdx.org/rdf/3.0.1/terms/Core/HashAlgorithm/sha224> ;
        rdf:rest _:Na5178b61d5c74a49b2cc0e95bd0413e3 .

    _:N249e05ef4c8e4ed4b3a9224a648e8214 rdf:first <https://spdx.org/rdf/3.0.1/terms/Dataset/DatasetAvailabilityType/clickthrough> ;
        rdf:rest _:Naabc7b3d9517403492a673579cb72ee4 .

    _:N2503b0811da5495eb93b56e326fe7b4c rdf:first <https://spdx.org/rdf/3.0.1/terms/Software/SoftwarePurpose/library> ;
        rdf:rest _:N031bef5cc13746728e9d4a2bff4d5a99 .

    _:N251d3a9324334560aa67860046a96fc1 rdf:first <https://spdx.org/rdf/3.0.1/terms/Security/VexJustificationType/vulnerableCodeCannotBeControlledByAdversary> ;
        rdf:rest _:Nb83e9b80aedb47339c27bc5911218377 .

    _:N255ae5aa8e194c4ebfebf8eaac503824 rdf:first <https://spdx.org/rdf/3.0.1/terms/Core/HashAlgorithm/blake2b512> ;
        rdf:rest _:N88f78664702e4bdea779a7798748be2b .

    _:N25a0cb36988640c4b945c1ac0f2310a5 sh:class ns1:PresenceType ;
        sh:in _:N900d8bbce1cb4f42aab5d1056bf72096 ;
        sh:maxCount 1 ;
        sh:nodeKind sh:IRI ;
        sh:path ns4:autonomyType .

    _:N261bda6457754a918bbf3d1ce47d7dc3 rdf:first <https://spdx.org/rdf/3.0.1/terms/Core/RelationshipType/describes> ;
        rdf:rest _:N73bb282ea8ee49f083cb4e6dcb4c48c9 .

    _:N2648b80a8ae84d97ad3d5cb789ee25e3 rdf:first <https://spdx.org/rdf/3.0.1/terms/Core/RelationshipType/descendantOf> ;
        rdf:rest _:N261bda6457754a918bbf3d1ce47d7dc3 .

    _:N267727c5fe684dc2ac36ab3119a5ed43 rdf:first <https://spdx.org/rdf/3.0.1/terms/Software/SoftwarePurpose/data> ;
        rdf:rest _:N8ba3fbb7ca24445899ad850b46665417 .

    _:N274fe2dfc06d45aba61fab2d4ea8b9c8 rdf:first <https://spdx.org/rdf/3.0.1/terms/Core/RelationshipType/modifiedBy> ;
        rdf:rest _:N32e7b310b886416a973c30b3890adae9 .

    _:N27738122637d491d85271152fecfd26f rdf:first <https://spdx.org/rdf/3.0.1/terms/Core/HashAlgorithm/sha3_256> ;
        rdf:rest _:N77e0eea96e97406d9a7905066b10496e .

    _:N27eec11210c94b568bd4cadc90bdc1b3 sh:class ns3:CvssSeverityType ;
        sh:in _:Na915e9a792b64c9786cfd8c87264640a ;
        sh:maxCount 1 ;
        sh:minCount 1 ;
        sh:nodeKind sh:IRI ;
        sh:path ns3:severity .

    _:N27f0016e8ca74bccbbbe464b2548f1b5 sh:class ns1:Tool ;
        sh:nodeKind sh:IRI ;
        sh:path ns1:createdUsing .

    _:N27fbe2fdc43f45f9b27acdb0cf013194 rdf:first <https://spdx.org/rdf/3.0.1/terms/Core/ExternalRefType/buildSystem> ;
        rdf:rest _:N104ad32768b2480d979d26e4f5c885a6 .

    _:N27fc956376b64f42a9eba01aa0464e5d sh:datatype xsd:string ;
        sh:maxCount 1 ;
        sh:nodeKind sh:Literal ;
        sh:path ns1:comment .

    _:N2835f5412cad42c19d531af2aacf35f8 rdf:first <https://spdx.org/rdf/3.0.1/terms/Security/CvssSeverityType/none> ;
        rdf:rest () .

    _:N28390bd265c84d20853195d19dd59cfd rdf:first <https://spdx.org/rdf/3.0.1/terms/Core/SupportType/noSupport> ;
        rdf:rest _:N3a2c99fb5ba145249e9a7d5cd4d1bdd9 .

    _:N289a16ee6acb48cda61c98a6c93a09f2 rdf:first <https://spdx.org/rdf/3.0.1/terms/Core/ExternalRefType/privacyAssessment> ;
        rdf:rest _:N64cfc55053e54172938d1a78640c50e5 .

    _:N28c5e025b6cd4f749e17d49a06be2088 rdf:first <https://spdx.org/rdf/3.0.1/terms/Software/SoftwarePurpose/framework> ;
        rdf:rest _:N4f12c0fe4f514024b31d0acfcfc7991f .

    _:N28fcc95b72af488aa4b1b2b9afe749f7 rdf:first <https://spdx.org/rdf/3.0.1/terms/Core/HashAlgorithm/md4> ;
        rdf:rest _:Nf4f02465310d47dfabbaa4e6912fe113 .

    _:N2a905386491c4c9cac82127b65420769 rdf:first <https://spdx.org/rdf/3.0.1/terms/Core/LifecycleScopeType/test> ;
        rdf:rest _:N6654e5e148e446fa86c0ce1e7aef1694 .

    _:N2aa8e89837d0409098ba6b5cdfcb9b94 rdf:first <https://spdx.org/rdf/3.0.1/terms/Core/ExternalRefType/vulnerabilityDisclosureReport> ;
        rdf:rest _:Naadfa67b12564b80b304aa24f2c9a003 .

    _:N2aadb3148a98468da6a856cede38e266 rdf:first <https://spdx.org/rdf/3.0.1/terms/Software/SoftwarePurpose/module> ;
        rdf:rest _:Ne015ec7355ad49feb860c0240976b3f6 .

    _:N2aee651aefbf4b5a9be9968800101d65 rdf:first <https://spdx.org/rdf/3.0.1/terms/Core/HashAlgorithm/blake2b512> ;
        rdf:rest _:N1126ca33ef024311af0f994505ba646e .

    _:N2b61f7a60cf0496da8338cf9cadd27ae rdf:first <https://spdx.org/rdf/3.0.1/terms/Software/SoftwarePurpose/operatingSystem> ;
        rdf:rest _:Nec315ded94b34cc7be920c90f7154835 .

    _:N2bb25b7428344e1fba7d66839c2f61b1 sh:class ns1:Element ;
        sh:nodeKind sh:IRI ;
        sh:path ns1:element .

    _:N2bfa9956fbb143dd924ac62a919c9c1f rdf:first <https://spdx.org/rdf/3.0.1/terms/Core/HashAlgorithm/other> ;
        rdf:rest _:N2df6fcad98b64375a6bb45b65c603b08 .

    _:N2d443860b51642498f3ba9b7de6dabb1 rdf:first <https://spdx.org/rdf/3.0.1/terms/Software/ContentIdentifierType/swhid> ;
        rdf:rest () .

    _:N2d6780949a1649e48604481718e229d2 rdf:first <https://spdx.org/rdf/3.0.1/terms/Core/RelationshipType/expandsTo> ;
        rdf:rest _:N0e18ea55685146fa9078163a7c3ff3d5 .

    _:N2d79c11911a54a1a8f337057c62255d0 rdf:first <https://spdx.org/rdf/3.0.1/terms/Core/RelationshipType/contains> ;
        rdf:rest _:N5d4473181a0f4a15800b655ce93bde62 .

    _:N2d7cf567343b45b3916d2f1bd14fa304 rdf:first <https://spdx.org/rdf/3.0.1/terms/Core/ExternalRefType/altWebPage> ;
        rdf:rest _:N2d849097ecac4461845a449426dd124e .

    _:N2d849097ecac4461845a449426dd124e rdf:first <https://spdx.org/rdf/3.0.1/terms/Core/ExternalRefType/binaryArtifact> ;
        rdf:rest _:N07457d45373c466ca415734a33afa350 .

    _:N2dedccafb91b4bcf83ecd2ea9f7bc3b4 rdf:first <https://spdx.org/rdf/3.0.1/terms/Core/HashAlgorithm/sha224> ;
        rdf:rest _:Nd54342913bcd4a3ea6a26935ed2dd422 .

    _:N2df6fcad98b64375a6bb45b65c603b08 rdf:first <https://spdx.org/rdf/3.0.1/terms/Core/HashAlgorithm/sha1> ;
        rdf:rest _:N2dedccafb91b4bcf83ecd2ea9f7bc3b4 .

    _:N2ecf638c2cd34c9488be93286bfeaf81 sh:message "https://spdx.org/rdf/3.0.1/terms/ExpandedLicensing/LicenseAddition is an abstract class and should not be instantiated directly. Instantiate a subclass instead."@en ;
        sh:not _:Nfd257672c0f8447bb2fe370e2da6108a ;
        sh:path rdf:type .

    _:N2ee2b766c01242548892800498fd2655 rdf:first <https://spdx.org/rdf/3.0.1/terms/Software/SoftwarePurpose/source> ;
        rdf:rest _:N89aedeba95014f5c9a45a4ffc4edc76b .

    _:N2f9be71ecf104b7e813465456ba1e423 sh:datatype xsd:positiveInteger ;
        sh:maxCount 1 ;
        sh:minCount 1 ;
        sh:nodeKind sh:Literal ;
        sh:path ns1:beginIntegerRange .

    _:N303b56ee3bd24539a79e6e86ea2b00b2 sh:class ns1:PresenceType ;
        sh:in _:Ndc68023588dd4e39a254912e522cbcb9 ;
        sh:maxCount 1 ;
        sh:nodeKind sh:IRI ;
        sh:path ns5:hasSensitivePersonalInformation .

    _:N310b971e33114ae2ba90bb1031704dcb sh:message "https://spdx.org/rdf/3.0.1/terms/ExpandedLicensing/ExtendableLicense is an abstract class and should not be instantiated directly. Instantiate a subclass instead."@en ;
        sh:not _:N3c8b3aa1d4f54b12aae13fd3768c69d6 ;
        sh:path rdf:type .

    _:N3152dc6f33cc4847a973c6e7c1cece5e sh:datatype xsd:string ;
        sh:maxCount 1 ;
        sh:minCount 1 ;
        sh:nodeKind sh:Literal ;
        sh:path ns6:additionText .

    _:N315f00e673e1400783fbaeb9b737f0e0 rdf:first <https://spdx.org/rdf/3.0.1/terms/Software/SoftwarePurpose/filesystemImage> ;
        rdf:rest _:N8f31918bfde04d2daa84b0754dec86bd .

    _:N317b60f774da4d7b8498a148dc2596b8 sh:datatype xsd:string ;
        sh:maxCount 1 ;
        sh:minCount 1 ;
        sh:nodeKind sh:Literal ;
        sh:path <https://spdx.org/rdf/3.0.1/terms/SimpleLicensing/licenseText> .

    _:N32759a712cfd43a2b573a645bc799937 rdf:first <https://spdx.org/rdf/3.0.1/terms/Dataset/ConfidentialityLevelType/green> ;
        rdf:rest _:N973b46c1a42343d49069b435c7273e72 .

    _:N32e7b310b886416a973c30b3890adae9 rdf:first <https://spdx.org/rdf/3.0.1/terms/Core/RelationshipType/other> ;
        rdf:rest _:Na574fa7d97c949139314ca99cc438dd5 .

    _:N32ebad2ed20a45dabcae2791b60933f4 rdf:first <https://spdx.org/rdf/3.0.1/terms/Core/PresenceType/noAssertion> ;
        rdf:rest () .

    _:N32f6eb21ae6b4c7fa4eeba186c255b53 rdf:first <https://spdx.org/rdf/3.0.1/terms/Core/ExternalIdentifierType/swid> ;
        rdf:rest _:Na89c4c2fd7ae49d6979e60b818c198d6 .

    _:N3310bd5aa0b84e6eb5c78f43313cbb4a rdf:first <https://spdx.org/rdf/3.0.1/terms/Software/SoftwarePurpose/evidence> ;
        rdf:rest _:N43ce71294f984133a4ff31d6640f38b5 .

    _:N3343e15c4f72473ebbfc546fb9ac3c23 sh:class ns1:DictionaryEntry ;
        sh:nodeKind sh:BlankNodeOrIRI ;
        sh:path <https://spdx.org/rdf/3.0.1/terms/Build/environment> .

    _:N3482d1d4103c44329fb2b6d0fd07d1d8 sh:message "https://spdx.org/rdf/3.0.1/terms/ExpandedLicensing/License is an abstract class and should not be instantiated directly. Instantiate a subclass instead."@en ;
        sh:not _:Nad61e60ebd944e07babf6645c9ef6ff5 ;
        sh:path rdf:type .

    _:N349239d89edf4bea9f937007b0ef0381 rdf:first <https://spdx.org/rdf/3.0.1/terms/Core/RelationshipType/hasInput> ;
        rdf:rest _:Nac2cb46be083464eb05e21fa57fef9ff .

    _:N35836a4c17134e0a83641bd266843b1f sh:datatype xsd:string ;
        sh:maxCount 1 ;
        sh:nodeKind sh:Literal ;
        sh:path ns1:context .

    _:N366fd9b9b76b4bc08ca7165010e37d97 sh:datatype xsd:string ;
        sh:maxCount 1 ;
        sh:nodeKind sh:Literal ;
        sh:path ns2:packageVersion .

    _:N37929166b5fe44e3aa34cddea5e3eef3 rdf:first <https://spdx.org/rdf/3.0.1/terms/Core/RelationshipType/foundBy> ;
        rdf:rest _:N5430fff14b2544a69d44644c066b4a3a .

    _:N3833dfea16ca487f88ee56d974e3135e rdf:first <https://spdx.org/rdf/3.0.1/terms/Core/ExternalRefType/other> ;
        rdf:rest _:N289a16ee6acb48cda61c98a6c93a09f2 .

    _:N39440260803745439d41569527a518f2 rdf:first <https://spdx.org/rdf/3.0.1/terms/Core/ExternalRefType/riskAssessment> ;
        rdf:rest _:Na7c36d0c91d440b8a279a19310da3dd7 .

    _:N395079a4589e43409d7dc314988c66b3 rdf:first <https://spdx.org/rdf/3.0.1/terms/Security/ExploitCatalogType/kev> ;
        rdf:rest _:N0178bde213704f7e8468fbebd80cadcc .

    _:N397df444dbe1469ebb7eec950c2015b5 sh:datatype xsd:string ;
        sh:maxCount 1 ;
        sh:minCount 1 ;
        sh:nodeKind sh:Literal ;
        sh:path ns1:identifier .

    _:N39b63541ed5948339549643d13449931 rdf:first <https://spdx.org/rdf/3.0.1/terms/Software/SbomType/analyzed> ;
        rdf:rest () .

    _:N3a1978042e6d4432b9f7a5e7661bc6d1 rdf:first <https://spdx.org/rdf/3.0.1/terms/Core/RelationshipType/usesTool> ;
        rdf:rest () .

    _:N3a2c99fb5ba145249e9a7d5cd4d1bdd9 rdf:first <https://spdx.org/rdf/3.0.1/terms/Core/SupportType/noAssertion> ;
        rdf:rest () .

    _:N3aeceae3663a4fb19126c7152560e7f3 rdf:first <https://spdx.org/rdf/3.0.1/terms/Core/RelationshipType/hasPrerequisite> ;
        rdf:rest _:Nddaef0505c8846cb8078511e66534d20 .

    _:N3b75ee5664f246fba72f68de7ebbb459 rdf:first <https://spdx.org/rdf/3.0.1/terms/Software/SbomType/build> ;
        rdf:rest _:N04c2c5076d534149865b12f9107c8c74 .

    _:N3bacd14e00cd43ec8e1a380d19b80f1c sh:message "https://spdx.org/rdf/3.0.1/terms/Core/Artifact is an abstract class and should not be instantiated directly. Instantiate a subclass instead."@en ;
        sh:not _:Nc4f2f317f5b74ffda8a534d8115021a0 ;
        sh:path rdf:type .

    _:N3c5062897ef2459ab30d9ecffc9b8324 sh:class ns1:Hash ;
        sh:nodeKind sh:BlankNodeOrIRI ;
        sh:path <https://spdx.org/rdf/3.0.1/terms/Build/configSourceDigest> .

    _:N3c8b3aa1d4f54b12aae13fd3768c69d6 sh:hasValue ns6:ExtendableLicense .

    _:N40d424d8b96741f0b3bd6b6e8df6248f rdf:first <https://spdx.org/rdf/3.0.1/terms/Core/ExternalIdentifierType/packageUrl> ;
        rdf:rest _:N48b75f64faaa48bcb7c8752907a45d1a .

    _:N4148ad351ad4456284b5e6de7a31ae4e sh:datatype xsd:string ;
        sh:maxCount 1 ;
        sh:nodeKind sh:Literal ;
        sh:path ns1:comment .

    _:N414a8299276840138167c2cfe582fe15 rdf:first <https://spdx.org/rdf/3.0.1/terms/Core/ProfileIdentifierType/expandedLicensing> ;
        rdf:rest _:N910672903cc24694891f023314b96554 .

    _:N42594dbee6274964a3d1d8726756dfae sh:hasValue ns1:ElementCollection .

    _:N42cff411a4ec44199c63b36da8d918ae rdf:first <https://spdx.org/rdf/3.0.1/terms/Core/RelationshipType/hasRequirement> ;
        rdf:rest _:N90818984f4cc4816916165173baa98a0 .

    _:N42d57ac597b748f9bf3e76623e662c29 rdf:first <https://spdx.org/rdf/3.0.1/terms/Core/HashAlgorithm/crystalsDilithium> ;
        rdf:rest _:Nd94ddbb247794b3f828de114beb815b4 .

    _:N42dececf6d66453da82386bb8b6fcea9 rdf:first <https://spdx.org/rdf/3.0.1/terms/Software/SoftwarePurpose/install> ;
        rdf:rest _:N050ac1461eee41578dc14b28c0764ec0 .

    _:N432205fe203e478e89d71b535134025e rdf:first <https://spdx.org/rdf/3.0.1/terms/Software/SoftwarePurpose/patch> ;
        rdf:rest _:N9ce0ce53bd3040da99eaea79d390ce47 .

    _:N43ce71294f984133a4ff31d6640f38b5 rdf:first <https://spdx.org/rdf/3.0.1/terms/Software/SoftwarePurpose/executable> ;
        rdf:rest _:Ne63b7372f8f848e1b95290b02cdb5b4b .

    _:N44383a20cc57437d807fa42adc1120a1 sh:datatype xsd:dateTimeStamp ;
        sh:maxCount 1 ;
        sh:nodeKind sh:Literal ;
        sh:path ns3:withdrawnTime ;
        sh:pattern "^\\d\\d\\d\\d-\\d\\d-\\d\\dT\\d\\d:\\d\\d:\\d\\dZ$" .

    _:N450e41ff31f14b2f8f02b111590ec074 rdf:first <https://spdx.org/rdf/3.0.1/terms/Core/RelationshipCompleteness/noAssertion> ;
        rdf:rest () .

    _:N453de8637a7c4769a1c6c7d22ab7d4b1 rdf:first <https://spdx.org/rdf/3.0.1/terms/Security/CvssSeverityType/high> ;
        rdf:rest _:Na01e2547c4044c50986ac025861990d9 .

    _:N45414da51a244066a02218d1ebe6fb31 sh:class ns1:Element ;
        sh:nodeKind sh:IRI ;
        sh:path ns1:rootElement .

    _:N455be9fd7fe3499d944d70756225532d rdf:first <https://spdx.org/rdf/3.0.1/terms/Core/HashAlgorithm/falcon> ;
        rdf:rest _:Nf8063a7692e44de79e8dd3cb56859bc7 .

    _:N45f93548cb7d4b5f8882568324cdbbc3 sh:class ns6:LicenseAddition ;
        sh:maxCount 1 ;
        sh:minCount 1 ;
        sh:nodeKind sh:IRI ;
        sh:path ns6:subjectAddition .

    _:N47b2b3528bff44a3852979c23cc33f55 rdf:first <https://spdx.org/rdf/3.0.1/terms/Software/SoftwarePurpose/device> ;
        rdf:rest _:Nea50294f6176494390eeae5709b2e306 .

    _:N489ecb902cae4ed68f7fefe6c4e8150c rdf:first <https://spdx.org/rdf/3.0.1/terms/Core/PresenceType/yes> ;
        rdf:rest _:N985d879bc68145da9e401772ba3b1bca .

    _:N48a7f32ef65a4710a46f9178452a5697 rdf:first <https://spdx.org/rdf/3.0.1/terms/Dataset/DatasetType/text> ;
        rdf:rest _:Nd563623ee8ae44a2aae208601aae8853 .

    _:N48b75f64faaa48bcb7c8752907a45d1a rdf:first <https://spdx.org/rdf/3.0.1/terms/Core/ExternalIdentifierType/securityOther> ;
        rdf:rest _:Nc5a7bca8248d45d383bedb3d1270d413 .

    _:N48dfd1f7541b4504b9518acfed910329 rdf:first <https://spdx.org/rdf/3.0.1/terms/Core/HashAlgorithm/adler32> ;
        rdf:rest _:Nfc510bb7e1284c82ab76da5c2a2a951c .

    _:N4a24ca08595e477b8337fe2a9a045c82 rdf:first <https://spdx.org/rdf/3.0.1/terms/Software/SoftwarePurpose/module> ;
        rdf:rest _:N2b61f7a60cf0496da8338cf9cadd27ae .

    _:N4abe73c07c824471919274e19e60d372 sh:datatype xsd:anyURI ;
        sh:maxCount 1 ;
        sh:nodeKind sh:Literal ;
        sh:path ns2:homePage .

    _:N4dde5c3db9e44e0db1c1051e698b0aed sh:message "https://spdx.org/rdf/3.0.1/terms/Core/Element is an abstract class and should not be instantiated directly. Instantiate a subclass instead."@en ;
        sh:not _:Nc2a7c95096f74ab3bdea52afc29ba71b ;
        sh:path rdf:type .

    _:N4ed0fca567474133b4e3f3d20d02eeb5 rdf:first <https://spdx.org/rdf/3.0.1/terms/Software/SoftwarePurpose/test> ;
        rdf:rest () .

    _:N4f12c0fe4f514024b31d0acfcfc7991f rdf:first <https://spdx.org/rdf/3.0.1/terms/Software/SoftwarePurpose/install> ;
        rdf:rest _:N2503b0811da5495eb93b56e326fe7b4c .

    _:N4f3f7581cb4c42cea580c5ad70c12c8f rdf:first <https://spdx.org/rdf/3.0.1/terms/Core/HashAlgorithm/sha3_224> ;
        rdf:rest _:N65dee02338ae48ff9488abeb9bed8206 .

    _:N4f55a950108140f0bef10a03e8e84ca7 rdf:first <https://spdx.org/rdf/3.0.1/terms/Core/PresenceType/noAssertion> ;
        rdf:rest () .

    _:N4ffa4b0fbd9545269f7365d293f45afd sh:datatype xsd:string ;
        sh:maxCount 1 ;
        sh:nodeKind sh:Literal ;
        sh:path ns4:limitation .

    _:N51c1ec6b89f5411b9fdacfc44fefd593 rdf:first <https://spdx.org/rdf/3.0.1/terms/Core/RelationshipType/delegatedTo> ;
        rdf:rest _:N0c46b9d033a048349acd598c3b002b65 .

    _:N51fe6b029f2a4c248a031cce1ef80bbf sh:class ns1:Agent ;
        sh:nodeKind sh:IRI ;
        sh:path ns1:originatedBy .

    _:N53b67006a5804ef6aaadd5d4387b7e71 sh:class ns3:CvssSeverityType ;
        sh:in _:N8d734c75192b45509ed89ccba678f6cb ;
        sh:maxCount 1 ;
        sh:minCount 1 ;
        sh:nodeKind sh:IRI ;
        sh:path ns3:severity .

    _:N53ce511f21824a0bad0607a29d13b55e sh:datatype xsd:string ;
        sh:nodeKind sh:Literal ;
        sh:path ns4:domain .

    _:N5430fff14b2544a69d44644c066b4a3a rdf:first <https://spdx.org/rdf/3.0.1/terms/Core/RelationshipType/generates> ;
        rdf:rest _:N9b9bd6005e634532aded8af6d21ebe8f .

    _:N57e7f375488f4e6e8c8862f77c82dcec sh:message "https://spdx.org/rdf/3.0.1/terms/Software/SoftwareArtifact is an abstract class and should not be instantiated directly. Instantiate a subclass instead."@en ;
        sh:not _:Na68bb014edc846bc9275f2377486515c ;
        sh:path rdf:type .

    _:N5800e826741c40a4b0356163725fb8ff sh:class ns2:SoftwarePurpose ;
        sh:in _:N6ee8868854df44d2ab8e09e2d7ff91b4 ;
        sh:nodeKind sh:IRI ;
        sh:path ns2:additionalPurpose .

    _:N58eec31acc944eefac091c246f27a7f1 sh:datatype xsd:string ;
        sh:maxCount 1 ;
        sh:nodeKind sh:Literal ;
        sh:path ns6:licenseXml .

    _:N5929480f8a8844d3bad4d00a8c1536fd rdf:first <https://spdx.org/rdf/3.0.1/terms/Software/SoftwarePurpose/model> ;
        rdf:rest _:N4a24ca08595e477b8337fe2a9a045c82 .

    _:N5a157fd1df584770bbabc6970f51ccf2 sh:datatype xsd:string ;
        sh:nodeKind sh:Literal ;
        sh:path ns2:attributionText .

    _:N5ad0acebc6e649fbbe183acddf8af24c sh:datatype xsd:string ;
        sh:maxCount 1 ;
        sh:nodeKind sh:Literal ;
        sh:path ns2:copyrightText .

    _:N5af2023939dd4cdaa456efa9c2789ef9 sh:message "https://spdx.org/rdf/3.0.1/terms/Security/VulnAssessmentRelationship is an abstract class and should not be instantiated directly. Instantiate a subclass instead."@en ;
        sh:not _:Ndad87f1ff2f2485e8c88dd126918131f ;
        sh:path rdf:type .

    _:N5b1e35fcbbd646748a005941f6a10486 rdf:first <https://spdx.org/rdf/3.0.1/terms/Core/RelationshipType/hasTestCase> ;
        rdf:rest _:N5d14ca6aa9204d32a39e8e9b3a3dd253 .

    _:N5c7c7a7867f94c258c1deed98c95cfae sh:class ns1:Agent ;
        sh:maxCount 1 ;
        sh:nodeKind sh:IRI ;
        sh:path ns1:suppliedBy .

    _:N5cb42ed80e484315b98ff5a6006e1649 sh:datatype xsd:anyURI ;
        sh:nodeKind sh:Literal ;
        sh:path <https://spdx.org/rdf/3.0.1/terms/Build/configSourceUri> .

    _:N5d132aff09b440f59ba2720d679260b0 sh:datatype xsd:string ;
        sh:maxCount 1 ;
        sh:minCount 1 ;
        sh:nodeKind sh:Literal ;
        sh:path ns1:prefix .

    _:N5d14ca6aa9204d32a39e8e9b3a3dd253 rdf:first <https://spdx.org/rdf/3.0.1/terms/Core/RelationshipType/hasVariant> ;
        rdf:rest _:N972bda73677b4c2aae06750fc5d23821 .

    _:N5d4473181a0f4a15800b655ce93bde62 rdf:first <https://spdx.org/rdf/3.0.1/terms/Core/RelationshipType/coordinatedBy> ;
        rdf:rest _:N7abd9e41a06740a49daf24088a7b6fd0 .

    _:N5e1a4e1ad13f4508bae4883983e83867 sh:message "https://spdx.org/rdf/3.0.1/terms/SimpleLicensing/AnyLicenseInfo is an abstract class and should not be instantiated directly. Instantiate a subclass instead."@en ;
        sh:not _:N0890ae69e65244faaedb4c3978a6a3cf ;
        sh:path rdf:type .

    _:N5e9bcf2d0c714e6a9e1b996f845a0a9f sh:datatype xsd:string ;
        sh:maxCount 1 ;
        sh:nodeKind sh:Literal ;
        sh:path ns1:issuingAuthority .

    _:N5eaa4fa988944c7a9423ee9461519d03 sh:datatype xsd:dateTimeStamp ;
        sh:maxCount 1 ;
        sh:nodeKind sh:Literal ;
        sh:path ns1:releaseTime ;
        sh:pattern "^\\d\\d\\d\\d-\\d\\d-\\d\\dT\\d\\d:\\d\\d:\\d\\dZ$" .

    _:N5efb7706d0b3407baf344bdb97f9c1a0 sh:datatype xsd:string ;
        sh:maxCount 1 ;
        sh:nodeKind sh:Literal ;
        sh:path ns6:listVersionAdded .

    _:N5f343653cdff44f9bb62e8379ac7884e rdf:first <https://spdx.org/rdf/3.0.1/terms/Core/RelationshipType/fixedIn> ;
        rdf:rest _:N37929166b5fe44e3aa34cddea5e3eef3 .

    _:N5fbd994d60b045a485f4161c29979d15 rdf:first <https://spdx.org/rdf/3.0.1/terms/Core/HashAlgorithm/blake2b384> ;
        rdf:rest _:N2aee651aefbf4b5a9be9968800101d65 .

    _:N5fcdd8adc1c543c8b4d7594bf3657d43 sh:datatype xsd:string ;
        sh:maxCount 1 ;
        sh:minCount 1 ;
        sh:nodeKind sh:Literal ;
        sh:path ns3:vectorString .

    _:N608336c4745d41e18e5f1c85ec83ddd7 rdf:first <https://spdx.org/rdf/3.0.1/terms/Core/HashAlgorithm/falcon> ;
        rdf:rest _:N982ee08ce55046e59027722eed572461 .

    _:N61bbc8ebf97841c3b566bb7d1795e8df sh:datatype xsd:dateTimeStamp ;
        sh:maxCount 1 ;
        sh:nodeKind sh:Literal ;
        sh:path ns3:modifiedTime ;
        sh:pattern "^\\d\\d\\d\\d-\\d\\d-\\d\\dT\\d\\d:\\d\\d:\\d\\dZ$" .

    _:N62c6de3503e24e62a556e92b063c0984 rdf:first <https://spdx.org/rdf/3.0.1/terms/Software/FileKindType/file> ;
        rdf:rest _:N1d299962dcc94d1dbe7ee3cf2bb5cf2e .

    _:N62d7707875a0400ebdf8b04ae8add96c sh:datatype xsd:string ;
        sh:maxCount 1 ;
        sh:minCount 1 ;
        sh:nodeKind sh:Literal ;
        sh:path ns3:vectorString .

    _:N636fed82d0e04a61a026d62b6958b716 rdf:first <https://spdx.org/rdf/3.0.1/terms/Software/SoftwarePurpose/archive> ;
        rdf:rest _:Nb2ba45a1abdd451d947ce76f4364bde8 .

    _:N64cfc55053e54172938d1a78640c50e5 rdf:first <https://spdx.org/rdf/3.0.1/terms/Core/ExternalRefType/productMetadata> ;
        rdf:rest _:Nd61a0d6f4c5b44a4a882de3953b8c716 .

    _:N65dee02338ae48ff9488abeb9bed8206 rdf:first <https://spdx.org/rdf/3.0.1/terms/Core/HashAlgorithm/sha3_256> ;
        rdf:rest _:Nb0662a3200b74d599b05e932ea138875 .

    _:N6654e5e148e446fa86c0ce1e7aef1694 rdf:first <https://spdx.org/rdf/3.0.1/terms/Core/LifecycleScopeType/runtime> ;
        rdf:rest _:N66bde88b66d64db99dca40b0007ad2c7 .

    _:N66bde88b66d64db99dca40b0007ad2c7 rdf:first <https://spdx.org/rdf/3.0.1/terms/Core/LifecycleScopeType/other> ;
        rdf:rest () .

    _:N68c2e83624d94d7da2e33e4a0e84a364 rdf:first <https://spdx.org/rdf/3.0.1/terms/Core/LifecycleScopeType/development> ;
        rdf:rest _:N89908d1a65034bf7a951a69cd0a92504 .

    _:N690e144eccf540c0bdf8b5006d4d10b0 sh:datatype xsd:string ;
        sh:maxCount 1 ;
        sh:minCount 1 ;
        sh:nodeKind sh:Literal ;
        sh:path ns1:specVersion ;
        sh:pattern "^(0|[1-9]\\d*)\\.(0|[1-9]\\d*)\\.(0|[1-9]\\d*)(?:-((?:0|[1-9]\\d*|\\d*[a-zA-Z-][0-9a-zA-Z-]*)(?:\\.(?:0|[1-9]\\d*|\\d*[a-zA-Z-][0-9a-zA-Z-]*))*))?(?:\\+([0-9a-zA-Z-]+(?:\\.[0-9a-zA-Z-]+)*))?$" .

    _:N693a0ac59cbf4f04a09a47000f92bf97 sh:class <https://spdx.org/rdf/3.0.1/terms/Extension/Extension> ;
        sh:nodeKind sh:BlankNodeOrIRI ;
        sh:path ns1:extension .

    _:N697dba6853a14fb29a838330aa6c7d28 rdf:first <https://spdx.org/rdf/3.0.1/terms/Core/ExternalRefType/nuget> ;
        rdf:rest _:Nd4e2d851f19e4c6f9629e565d0805f02 .

    _:N6ac9d864a4e742c68b114de0bb33e8c3 sh:class ns1:Agent ;
        sh:maxCount 1 ;
        sh:nodeKind sh:IRI ;
        sh:path ns1:suppliedBy .

    _:N6aee3408cdaa46a6bb0ccb864eb33899 sh:class ns1:DictionaryEntry ;
        sh:nodeKind sh:BlankNodeOrIRI ;
        sh:path <https://spdx.org/rdf/3.0.1/terms/SimpleLicensing/customIdToUri> .

    _:N6b0753cb9cf74582bbf870095e9a692f sh:class ns5:ConfidentialityLevelType ;
        sh:in _:Nca65717c3354405c874c1aff7975811e ;
        sh:maxCount 1 ;
        sh:nodeKind sh:IRI ;
        sh:path ns5:confidentialityLevel .

    _:N6b83da998edf4da3a5c86600ef22ed5f sh:datatype xsd:string ;
        sh:maxCount 1 ;
        sh:minCount 1 ;
        sh:nodeKind sh:Literal ;
        sh:path ns1:hashValue .

    _:N6b92f665373a4dd1959f3c765e7e3306 rdf:first <https://spdx.org/rdf/3.0.1/terms/Core/RelationshipType/serializedInArtifact> ;
        rdf:rest _:Ndcf79036b2984f98b7df79c8b9adab46 .

    _:N6c00277a300e432bb161c276667652ee rdf:first <https://spdx.org/rdf/3.0.1/terms/Software/SoftwarePurpose/container> ;
        rdf:rest _:N76e159545ba941b4a8aaf4a539719898 .

    _:N6ca973580af24785ad2f13872c5321a7 sh:datatype xsd:decimal ;
        sh:maxCount 1 ;
        sh:minCount 1 ;
        sh:nodeKind sh:Literal ;
        sh:path ns3:percentile .

    _:N6d06a87ba9564b1686aca2e55466693f sh:datatype xsd:dateTimeStamp ;
        sh:maxCount 1 ;
        sh:nodeKind sh:Literal ;
        sh:path <https://spdx.org/rdf/3.0.1/terms/Build/buildStartTime> ;
        sh:pattern "^\\d\\d\\d\\d-\\d\\d-\\d\\dT\\d\\d:\\d\\d:\\d\\dZ$" .

    _:N6d187fa41aab49559fc1e40fe096601d rdf:first <https://spdx.org/rdf/3.0.1/terms/AI/SafetyRiskAssessmentType/serious> ;
        rdf:rest _:Nf8731ab568e344619e5d2a29ff0c9e3c .

    _:N6d9713b048484df2a5edddea8f2e9e7c sh:class <https://spdx.org/rdf/3.0.1/terms/SimpleLicensing/AnyLicenseInfo> ;
        sh:minCount 2 ;
        sh:nodeKind sh:IRI ;
        sh:path ns6:member .

    _:N6db8b82bbd76401192e164fd3d83bc7d rdf:first <https://spdx.org/rdf/3.0.1/terms/Software/SoftwarePurpose/deviceDriver> ;
        rdf:rest _:Nb495361d74244ac4b60416b96f40b3c0 .

    _:N6ea4943e498c4dd1b48743b06fa1f4ac sh:datatype xsd:string ;
        sh:maxCount 1 ;
        sh:nodeKind sh:Literal ;
        sh:path ns1:comment .

    _:N6ee8868854df44d2ab8e09e2d7ff91b4 rdf:first <https://spdx.org/rdf/3.0.1/terms/Software/SoftwarePurpose/application> ;
        rdf:rest _:N636fed82d0e04a61a026d62b6958b716 .

    _:N6f376d6f51b6455ea533fab3a8daaa84 rdf:first <https://spdx.org/rdf/3.0.1/terms/Core/ExternalRefType/securityAdversaryModel> ;
        rdf:rest _:Nf2f414b51e3a4686a5cb9e3a84c327c8 .

    _:N7005d82c23df4154835c9c275887b1e4 sh:datatype xsd:anyURI ;
        sh:maxCount 1 ;
        sh:minCount 1 ;
        sh:nodeKind sh:Literal ;
        sh:path ns1:externalSpdxId .

    _:N71e76630f7fb413988a49c5df05f7010 rdf:first <https://spdx.org/rdf/3.0.1/terms/Core/HashAlgorithm/crystalsDilithium> ;
        rdf:rest _:N1bd34863d96b4d6b8a6a7312d11b368a .

    _:N72aea843a56b45d1b12778e8f3f24d8d rdf:first <https://spdx.org/rdf/3.0.1/terms/Core/ExternalRefType/vcs> ;
        rdf:rest _:N2aa8e89837d0409098ba6b5cdfcb9b94 .

    _:N730b491010ab4f9bafd08494e408c982 sh:class ns1:SupportType ;
        sh:in _:Nf740deac06444efb948d8e08b489ea6e ;
        sh:nodeKind sh:IRI ;
        sh:path ns1:supportLevel .

    _:N735b7ed5ff0c4e14898aa20824d3f3d1 sh:class ns2:File ;
        sh:maxCount 1 ;
        sh:minCount 1 ;
        sh:nodeKind sh:IRI ;
        sh:path ns2:snippetFromFile .

    _:N738a8d5957cb40f2a2fcf70c01d1d55c rdf:first <https://spdx.org/rdf/3.0.1/terms/Core/HashAlgorithm/sha512> ;
        rdf:rest _:N4f3f7581cb4c42cea580c5ad70c12c8f .

    _:N73bb282ea8ee49f083cb4e6dcb4c48c9 rdf:first <https://spdx.org/rdf/3.0.1/terms/Core/RelationshipType/doesNotAffect> ;
        rdf:rest _:N2d6780949a1649e48604481718e229d2 .

    _:N73da8aa44e7149a8af8639082044141a sh:class ns1:DictionaryEntry ;
        sh:nodeKind sh:BlankNodeOrIRI ;
        sh:path ns5:sensor .

    _:N7419f22add2b4107ab0c5b25f53b788b sh:class ns1:ExternalRef ;
        sh:nodeKind sh:BlankNodeOrIRI ;
        sh:path ns1:externalRef .

    _:N7450e5f23ee34ddf90d69f61d5f62c87 sh:class ns1:Artifact ;
        sh:maxCount 1 ;
        sh:nodeKind sh:IRI ;
        sh:path ns1:definingArtifact .

    _:N7495455ebc1a485091680d44af0fed6e sh:datatype xsd:anyURI ;
        sh:maxCount 1 ;
        sh:minCount 1 ;
        sh:nodeKind sh:Literal ;
        sh:path ns1:namespace .

    _:N74c9b0d0b2a44318a1794544b42e5081 rdf:first <https://spdx.org/rdf/3.0.1/terms/Dataset/DatasetType/video> ;
        rdf:rest () .

    _:N75c08d7cf8e1440cb4a9d99ed2a02f78 rdf:first <https://spdx.org/rdf/3.0.1/terms/Core/ProfileIdentifierType/ai> ;
        rdf:rest _:Nc14d6ee8bfc64b29959f55fdf61f8e37 .

    _:N76e159545ba941b4a8aaf4a539719898 rdf:first <https://spdx.org/rdf/3.0.1/terms/Software/SoftwarePurpose/data> ;
        rdf:rest _:N47b2b3528bff44a3852979c23cc33f55 .

    _:N771b730ffdb64c92b9866f170f5a077d rdf:first <https://spdx.org/rdf/3.0.1/terms/Core/RelationshipType/republishedBy> ;
        rdf:rest _:N6b92f665373a4dd1959f3c765e7e3306 .

    _:N7788f32c2dd54dbfba9ee468ee43207e rdf:first <https://spdx.org/rdf/3.0.1/terms/Security/VexJustificationType/vulnerableCodeNotPresent> ;
        rdf:rest _:N251d3a9324334560aa67860046a96fc1 .

    _:N77e0eea96e97406d9a7905066b10496e rdf:first <https://spdx.org/rdf/3.0.1/terms/Core/HashAlgorithm/sha3_384> ;
        rdf:rest _:Ndae5459fc26c4e94ba0292367c100cf2 .

    _:N7850efd1860843a6b5cbde6525a0b0d9 rdf:first <https://spdx.org/rdf/3.0.1/terms/Dataset/DatasetAvailabilityType/scrapingScript> ;
        rdf:rest () .

    _:N787361abd52c45ff88c62ab4069645cb sh:datatype xsd:anyURI ;
        sh:maxCount 1 ;
        sh:minCount 1 ;
        sh:nodeKind sh:Literal ;
        sh:path <https://spdx.org/rdf/3.0.1/terms/Build/buildType> .

    _:N7886db0616614a89abf7cbeff8975003 rdf:first <https://spdx.org/rdf/3.0.1/terms/Core/RelationshipType/hasDependencyManifest> ;
        rdf:rest _:Nbca6999757c44634acc82bca29955365 .

    _:N79092dd798854b9781723512b16e2df6 rdf:first <https://spdx.org/rdf/3.0.1/terms/Core/RelationshipType/configures> ;
        rdf:rest _:N2d79c11911a54a1a8f337057c62255d0 .

    _:N79201074c81a412eaee8c9b251c5ac80 rdf:first <https://spdx.org/rdf/3.0.1/terms/Core/HashAlgorithm/sha384> ;
        rdf:rest _:N06a47b60376c47aaac92b0a69159a1c0 .

    _:N79d84a9512cc4810940269e53d06703f sh:message "https://spdx.org/rdf/3.0.1/terms/Core/IntegrityMethod is an abstract class and should not be instantiated directly. Instantiate a subclass instead."@en ;
        sh:not _:N165e76779b954f6c829861fe80b13f8b ;
        sh:path rdf:type .

    _:N79ea886ccc984e4ebac49b2a2ba05b8f rdf:first <https://spdx.org/rdf/3.0.1/terms/Software/SoftwarePurpose/executable> ;
        rdf:rest _:Ne707f0a1c2b640dd8605aa3d18c23fe0 .

    _:N7a01e1ee4d5040288bd6d52941764a70 sh:class ns1:Element ;
        sh:minCount 1 ;
        sh:nodeKind sh:IRI ;
        sh:path ns1:to .

    _:N7a1f905837b84b0faa7bd8a062f960f1 rdf:first <https://spdx.org/rdf/3.0.1/terms/Core/ProfileIdentifierType/software> ;
        rdf:rest _:Nce8d42474a1842ffa06cef1e9067de1b .

    _:N7abd9e41a06740a49daf24088a7b6fd0 rdf:first <https://spdx.org/rdf/3.0.1/terms/Core/RelationshipType/copiedTo> ;
        rdf:rest _:N51c1ec6b89f5411b9fdacfc44fefd593 .

    _:N7bbd717f73924fdd82520407da9bf371 sh:datatype xsd:string ;
        sh:maxCount 1 ;
        sh:nodeKind sh:Literal ;
        sh:path ns5:dataCollectionProcess .

    _:N7d6920e1fda8401d8fee4b5dd11b7196 rdf:first <https://spdx.org/rdf/3.0.1/terms/Core/HashAlgorithm/other> ;
        rdf:rest _:N877cb90ddecf44f18e8d16d77f3cf783 .

    _:N7d70a3f168464a16aaa2ce14fe3f54a2 sh:class ns1:IntegrityMethod ;
        sh:nodeKind sh:BlankNodeOrIRI ;
        sh:path ns1:verifiedUsing .

    _:N7e0a9e9a6b7b402bbf68b76243025f34 sh:datatype xsd:string ;
        sh:maxCount 1 ;
        sh:nodeKind sh:Literal ;
        sh:path ns6:obsoletedBy .

    _:N7f1ad87c28114ee7bc0725fb58b20ca9 sh:datatype xsd:string ;
        sh:maxCount 1 ;
        sh:minCount 1 ;
        sh:nodeKind sh:Literal ;
        sh:path ns1:hashValue .

    _:N8013bcfb52cb4e51bbb49dc7a6710704 rdf:first <https://spdx.org/rdf/3.0.1/terms/Core/HashAlgorithm/md4> ;
        rdf:rest _:Nc647bd18250b49c690d79de4484b2c55 .

    _:N802270e023784500a8ae0fac28a696c3 sh:datatype xsd:string ;
        sh:nodeKind sh:Literal ;
        sh:path ns4:modelExplainability .

    _:N8277ba52ec1d49079b2448e68d672999 sh:class ns1:ProfileIdentifierType ;
        sh:in _:Naede8dcd34b546bd8ffb872d58865422 ;
        sh:nodeKind sh:IRI ;
        sh:path ns1:profileConformance .

    _:N843e3d8f3df146bf8c261dc7c18eed6a rdf:first <https://spdx.org/rdf/3.0.1/terms/Core/RelationshipType/availableFrom> ;
        rdf:rest _:N79092dd798854b9781723512b16e2df6 .

    _:N8461c39477864d659431548b72f253a4 sh:datatype xsd:decimal ;
        sh:maxCount 1 ;
        sh:minCount 1 ;
        sh:nodeKind sh:Literal ;
        sh:path ns3:score .

    _:N847e87312f6946cd8b8fec377fd7adb3 rdf:first <https://spdx.org/rdf/3.0.1/terms/Core/AnnotationType/review> ;
        rdf:rest () .

    _:N85d91bf18a8e4340901a74314a2a4a56 sh:datatype xsd:string ;
        sh:maxCount 1 ;
        sh:nodeKind sh:Literal ;
        sh:path ns6:deprecatedVersion .

    _:N8618f8df62f8426586277f411a3ea2a9 rdf:first <https://spdx.org/rdf/3.0.1/terms/Core/ExternalRefType/qualityAssessmentReport> ;
        rdf:rest _:Nb745a8df94a44b1c94d5a41371e693cc .

    _:N868e3594ba004020921e8238c75bc3b6 rdf:first <https://spdx.org/rdf/3.0.1/terms/Core/ExternalRefType/support> ;
        rdf:rest _:N72aea843a56b45d1b12778e8f3f24d8d .

    _:N86dd9cfc30c44518bd414964b7fbae8b sh:class ns2:SoftwareArtifact ;
        sh:maxCount 1 ;
        sh:nodeKind sh:IRI ;
        sh:path ns3:assessedElement .

    _:N87484f238313462d86eb931a8e656419 sh:class ns2:SoftwarePurpose ;
        sh:in _:N905f17d21fea497195ba2f0655442fae ;
        sh:maxCount 1 ;
        sh:nodeKind sh:IRI ;
        sh:path ns2:primaryPurpose .

    _:N877cb90ddecf44f18e8d16d77f3cf783 rdf:first <https://spdx.org/rdf/3.0.1/terms/Core/HashAlgorithm/sha1> ;
        rdf:rest _:N2471049aadfe49bfbb3571150159e22b .

    _:N8784ce86e26a44f8917c2cb04540f2fa rdf:first <https://spdx.org/rdf/3.0.1/terms/Software/SoftwarePurpose/patch> ;
        rdf:rest _:N1de5d4dc34e04f919447cf643142160b .

    _:N8795c3ed3b6645bcbfeae19e77e2655d rdf:first <https://spdx.org/rdf/3.0.1/terms/Core/RelationshipType/hasOptionalComponent> ;
        rdf:rest _:Ncfdc44469dd94616b893a53c66f417ea .

    _:N882f0a61a1954011a313d91950a91717 rdf:first <https://spdx.org/rdf/3.0.1/terms/Core/RelationshipType/hasAssessmentFor> ;
        rdf:rest _:Ne30c85bbf11b4c2b849b8440be508bee .

    _:N88f312000b15404f85118ab1f52c0d93 sh:hasValue ns3:VexVulnAssessmentRelationship .

    _:N88f78664702e4bdea779a7798748be2b rdf:first <https://spdx.org/rdf/3.0.1/terms/Core/HashAlgorithm/blake3> ;
        rdf:rest _:N42d57ac597b748f9bf3e76623e662c29 .

    _:N89908d1a65034bf7a951a69cd0a92504 rdf:first <https://spdx.org/rdf/3.0.1/terms/Core/LifecycleScopeType/build> ;
        rdf:rest _:N2a905386491c4c9cac82127b65420769 .

    _:N89aedeba95014f5c9a45a4ffc4edc76b rdf:first <https://spdx.org/rdf/3.0.1/terms/Software/SoftwarePurpose/specification> ;
        rdf:rest _:N0ee599289d3445dd98544cb7d542ad0f .

    _:N89c1049758874ee193ceacd3663eff21 sh:class ns1:PositiveIntegerRange ;
        sh:maxCount 1 ;
        sh:nodeKind sh:BlankNodeOrIRI ;
        sh:path ns2:byteRange .

    _:N8a3eb069ab8a42d9ba1b350b7c463fbb rdf:first <https://spdx.org/rdf/3.0.1/terms/Core/RelationshipType/hasTest> ;
        rdf:rest _:N5b1e35fcbbd646748a005941f6a10486 .

    _:N8b3541e2042542e19c148a7b6065af51 rdf:first <https://spdx.org/rdf/3.0.1/terms/Core/ExternalRefType/mavenCentral> ;
        rdf:rest _:Ncbdd7b9aaf92411289bbf1bed5771c04 .

    _:N8ba3fbb7ca24445899ad850b46665417 rdf:first <https://spdx.org/rdf/3.0.1/terms/Software/SoftwarePurpose/device> ;
        rdf:rest _:Ne327d40f301646b19534d8557a045729 .

    _:N8d30523f8928470fb33e9c71f058a726 sh:datatype xsd:string ;
        sh:nodeKind sh:Literal ;
        sh:path <https://spdx.org/rdf/3.0.1/terms/Build/configSourceEntrypoint> .

    _:N8d51fc8fc521483d85792bd30b47cade sh:class ns6:License ;
        sh:maxCount 1 ;
        sh:minCount 1 ;
        sh:nodeKind sh:IRI ;
        sh:path ns6:subjectLicense .

    _:N8d734c75192b45509ed89ccba678f6cb rdf:first <https://spdx.org/rdf/3.0.1/terms/Security/CvssSeverityType/critical> ;
        rdf:rest _:N1677f5bfd8fa4911b5a3653d2c1a3263 .

    _:N8f31918bfde04d2daa84b0754dec86bd rdf:first <https://spdx.org/rdf/3.0.1/terms/Software/SoftwarePurpose/firmware> ;
        rdf:rest _:N28c5e025b6cd4f749e17d49a06be2088 .

    _:N8fba128d40804e9da2b1794c012fb0d0 sh:datatype xsd:dateTimeStamp ;
        sh:maxCount 1 ;
        sh:minCount 1 ;
        sh:nodeKind sh:Literal ;
        sh:path ns1:created ;
        sh:pattern "^\\d\\d\\d\\d-\\d\\d-\\d\\dT\\d\\d:\\d\\d:\\d\\dZ$" .

    _:N900d8bbce1cb4f42aab5d1056bf72096 rdf:first <https://spdx.org/rdf/3.0.1/terms/Core/PresenceType/yes> ;
        rdf:rest _:Ned659fae654449459e07497f6e373a2f .

    _:N905f17d21fea497195ba2f0655442fae rdf:first <https://spdx.org/rdf/3.0.1/terms/Software/SoftwarePurpose/application> ;
        rdf:rest _:Ncd71557870a24229a05d5a04577849b9 .

    _:N906b4e4cb5ba41b1bf9345ba1c8b1f5a sh:datatype xsd:string ;
        sh:maxCount 1 ;
        sh:nodeKind sh:Literal ;
        sh:path ns1:comment .

    _:N90818984f4cc4816916165173baa98a0 rdf:first <https://spdx.org/rdf/3.0.1/terms/Core/RelationshipType/hasSpecification> ;
        rdf:rest _:Nff29bfb461de4653a0c106ee09905e74 .

    _:N910672903cc24694891f023314b96554 rdf:first <https://spdx.org/rdf/3.0.1/terms/Core/ProfileIdentifierType/security> ;
        rdf:rest _:Nd74a690a40a64a01b9cab2e0062d1fc7 .

    _:N9111c10d9fb94856a73b98e13b7a47bd sh:class ns4:EnergyConsumptionDescription ;
        sh:nodeKind sh:BlankNodeOrIRI ;
        sh:path ns4:finetuningEnergyConsumption .

    _:N913effc8986249ddbf450a571d06d45e sh:datatype xsd:string ;
        sh:maxCount 1 ;
        sh:nodeKind sh:Literal ;
        sh:path <https://spdx.org/rdf/3.0.1/terms/Extension/cdxPropValue> .

    _:N917ed0d86b38442e9b3e7e205aa94764 rdf:first <https://spdx.org/rdf/3.0.1/terms/Dataset/DatasetAvailabilityType/query> ;
        rdf:rest _:Nad7823d2540e4e83a052731ffecd7f89 .

    _:N921fdfd13fd7435bb8e9a2a862a02269 sh:datatype xsd:decimal ;
        sh:maxCount 1 ;
        sh:minCount 1 ;
        sh:nodeKind sh:Literal ;
        sh:path ns3:probability .

    _:N93eaecf4ad5e433a924257276c8fd50c rdf:first <https://spdx.org/rdf/3.0.1/terms/Core/ExternalRefType/certificationReport> ;
        rdf:rest _:Na3b3439ae8ab40f7b8aceafe342c168f .

    _:N942452bba40a472880cf56ce7944c65b sh:class ns1:ExternalMap ;
        sh:nodeKind sh:BlankNodeOrIRI ;
        sh:path ns1:import .

    _:N951f8090463a4c9a99b9396ff1f62c60 sh:datatype xsd:dateTimeStamp ;
        sh:maxCount 1 ;
        sh:nodeKind sh:Literal ;
        sh:path ns3:publishedTime ;
        sh:pattern "^\\d\\d\\d\\d-\\d\\d-\\d\\dT\\d\\d:\\d\\d:\\d\\dZ$" .

    _:N97062f00bfbe4738bee3ead0b37f9559 rdf:first <https://spdx.org/rdf/3.0.1/terms/Core/RelationshipType/hasConcludedLicense> ;
        rdf:rest _:Nc14ff109396a44f896779d4cdc6d3f9e .

    _:N972bda73677b4c2aae06750fc5d23821 rdf:first <https://spdx.org/rdf/3.0.1/terms/Core/RelationshipType/invokedBy> ;
        rdf:rest _:N274fe2dfc06d45aba61fab2d4ea8b9c8 .

    _:N973b46c1a42343d49069b435c7273e72 rdf:first <https://spdx.org/rdf/3.0.1/terms/Dataset/ConfidentialityLevelType/clear> ;
        rdf:rest () .

    _:N97a6578de8ef458ba572f30b64456e83 sh:datatype xsd:anyURI ;
        sh:maxCount 1 ;
        sh:minCount 1 ;
        sh:nodeKind sh:Literal ;
        sh:path ns2:contentIdentifierValue .

    _:N982ba8180ed94a77899dff62913fe63e sh:class ns1:DictionaryEntry ;
        sh:nodeKind sh:BlankNodeOrIRI ;
        sh:path <https://spdx.org/rdf/3.0.1/terms/Build/parameter> .

    _:N982ee08ce55046e59027722eed572461 rdf:first <https://spdx.org/rdf/3.0.1/terms/Core/HashAlgorithm/md2> ;
        rdf:rest _:N28fcc95b72af488aa4b1b2b9afe749f7 .

    _:N985d879bc68145da9e401772ba3b1bca rdf:first <https://spdx.org/rdf/3.0.1/terms/Core/PresenceType/no> ;
        rdf:rest _:N4f55a950108140f0bef10a03e8e84ca7 .

    _:N990927fcdbab47dd9aa94d5b66bcec04 sh:class ns1:PresenceType ;
        sh:in _:N489ecb902cae4ed68f7fefe6c4e8150c ;
        sh:maxCount 1 ;
        sh:nodeKind sh:IRI ;
        sh:path ns4:useSensitivePersonalInformation .

    _:N9931aa59b6d1496abf379e7856751daf rdf:first <https://spdx.org/rdf/3.0.1/terms/Core/RelationshipType/affects> ;
        rdf:rest _:Nc4bac3b7de8145d3907fb8042c381d25 .

    _:N995bc073d1bb493782caa95bd840ac7d sh:message "https://spdx.org/rdf/3.0.1/terms/Security/VexVulnAssessmentRelationship is an abstract class and should not be instantiated directly. Instantiate a subclass instead."@en ;
        sh:not _:N88f312000b15404f85118ab1f52c0d93 ;
        sh:path rdf:type .

    _:N9a6194fa9fd840fd9bc36e7a2f49e8fe rdf:first <https://spdx.org/rdf/3.0.1/terms/Security/SsvcDecisionType/attend> ;
        rdf:rest _:Nb5a9bb07f0ed4b6e95a2012807417d8b .

    _:N9ab8f5212b9e4a0c84030a7fde89d4a5 sh:datatype xsd:string ;
        sh:maxCount 1 ;
        sh:nodeKind sh:Literal ;
        sh:path ns6:listVersionAdded .

    _:N9b100afdb515432cab5b744e6ab3aad3 rdf:first <https://spdx.org/rdf/3.0.1/terms/Core/RelationshipType/trainedOn> ;
        rdf:rest _:Na0c09f09240840f7873b5a5fca33b91f .

    _:N9b235bcc4a91486eb87fc626fc1ab570 sh:hasValue <https://spdx.org/rdf/3.0.1/terms/Extension/Extension> .

    _:N9b9bd6005e634532aded8af6d21ebe8f rdf:first <https://spdx.org/rdf/3.0.1/terms/Core/RelationshipType/hasAddedFile> ;
        rdf:rest _:N882f0a61a1954011a313d91950a91717 .

    _:N9bb7d51fbdb64ad48dbbf71ee81f69db sh:datatype xsd:dateTimeStamp ;
        sh:maxCount 1 ;
        sh:nodeKind sh:Literal ;
        sh:path ns3:actionStatementTime ;
        sh:pattern "^\\d\\d\\d\\d-\\d\\d-\\d\\dT\\d\\d:\\d\\d:\\d\\dZ$" .

    _:N9bf956e203414b89929bf7146b83f11a rdf:first <https://spdx.org/rdf/3.0.1/terms/Core/ExternalIdentifierType/email> ;
        rdf:rest _:Ne14b7f7dceac423b869e219e73c16475 .

    _:N9c9620b9738a48ffa797d861125a90b6 sh:datatype xsd:string ;
        sh:maxCount 1 ;
        sh:nodeKind sh:Literal ;
        sh:path <https://spdx.org/rdf/3.0.1/terms/SimpleLicensing/licenseListVersion> ;
        sh:pattern "^(0|[1-9]\\d*)\\.(0|[1-9]\\d*)\\.(0|[1-9]\\d*)(?:-((?:0|[1-9]\\d*|\\d*[a-zA-Z-][0-9a-zA-Z-]*)(?:\\.(?:0|[1-9]\\d*|\\d*[a-zA-Z-][0-9a-zA-Z-]*))*))?(?:\\+([0-9a-zA-Z-]+(?:\\.[0-9a-zA-Z-]+)*))?$" .

    _:N9ce0ce53bd3040da99eaea79d390ce47 rdf:first <https://spdx.org/rdf/3.0.1/terms/Software/SoftwarePurpose/platform> ;
        rdf:rest _:Nc053d18d5def491f9582457af1776545 .

    _:N9d9ec4b5217e40f884dec6a2317cb4cd rdf:first <https://spdx.org/rdf/3.0.1/terms/Software/SbomType/runtime> ;
        rdf:rest _:N39b63541ed5948339549643d13449931 .

    _:N9e2593cb36b740d3be8bddd390b67fe7 sh:datatype xsd:string ;
        sh:nodeKind sh:Literal ;
        sh:path ns1:locator .

    _:N9f736b62e774479ca799c05a49ab2af6 sh:datatype xsd:string ;
        sh:maxCount 1 ;
        sh:minCount 1 ;
        sh:nodeKind sh:Literal ;
        sh:path <https://spdx.org/rdf/3.0.1/terms/Extension/cdxPropName> .

    _:N9fdcb40f9bc24613ae75374946dc3163 sh:datatype xsd:string ;
        sh:maxCount 1 ;
        sh:nodeKind sh:Literal ;
        sh:path ns3:impactStatement .

    _:Na01e2547c4044c50986ac025861990d9 rdf:first <https://spdx.org/rdf/3.0.1/terms/Security/CvssSeverityType/medium> ;
        rdf:rest _:Nf2006a25a5df4b449c058903cb4ddeba .

    _:Na025116d022643e2beeb87ce5077615a sh:datatype xsd:boolean ;
        sh:maxCount 1 ;
        sh:nodeKind sh:Literal ;
        sh:path ns6:isDeprecatedAdditionId .

    _:Na02e1b7ab4ab4241a581e9c0bf13fb7d sh:datatype xsd:dateTimeStamp ;
        sh:maxCount 1 ;
        sh:nodeKind sh:Literal ;
        sh:path ns3:publishedTime ;
        sh:pattern "^\\d\\d\\d\\d-\\d\\d-\\d\\dT\\d\\d:\\d\\d:\\d\\dZ$" .

    _:Na0bd1e47bbbf4e559d1a6f8399113223 rdf:first <https://spdx.org/rdf/3.0.1/terms/Security/CvssSeverityType/medium> ;
        rdf:rest _:Na91d8910dfaa4193aa3ed17360774321 .

    _:Na0c09f09240840f7873b5a5fca33b91f rdf:first <https://spdx.org/rdf/3.0.1/terms/Core/RelationshipType/underInvestigationFor> ;
        rdf:rest _:N3a1978042e6d4432b9f7a5e7661bc6d1 .

    _:Na13406b855df4150971e1c76ed24b827 rdf:first <https://spdx.org/rdf/3.0.1/terms/Core/SupportType/support> ;
        rdf:rest _:Nbbfc2c5bd25e451cabc0b232751ec9b3 .

    _:Na1afc73eaba1435383aaab5260aaef74 rdf:first <https://spdx.org/rdf/3.0.1/terms/Core/ExternalRefType/funding> ;
        rdf:rest _:N0a0a67d1a9dc4ec7ab3b94209b868dff .

    _:Na1b3987084df4a0893f69ad4ee6679b6 sh:class ns1:NamespaceMap ;
        sh:nodeKind sh:BlankNodeOrIRI ;
        sh:path ns1:namespaceMap .

    _:Na3b3439ae8ab40f7b8aceafe342c168f rdf:first <https://spdx.org/rdf/3.0.1/terms/Core/ExternalRefType/componentAnalysisReport> ;
        rdf:rest _:Na954d078246c4e94850d486646c66b84 .

    _:Na448701a1d1e497c8bdb122d21f1ab5c rdf:first <https://spdx.org/rdf/3.0.1/terms/Core/HashAlgorithm/blake2b384> ;
        rdf:rest _:N255ae5aa8e194c4ebfebf8eaac503824 .

    _:Na5178b61d5c74a49b2cc0e95bd0413e3 rdf:first <https://spdx.org/rdf/3.0.1/terms/Core/HashAlgorithm/sha256> ;
        rdf:rest _:N79201074c81a412eaee8c9b251c5ac80 .

    _:Na574fa7d97c949139314ca99cc438dd5 rdf:first <https://spdx.org/rdf/3.0.1/terms/Core/RelationshipType/packagedBy> ;
        rdf:rest _:Nfe09149c948a4591baf966eeef8021dd .

    _:Na67ca3acaea24305b83b762bb3b5ece7 sh:datatype xsd:boolean ;
        sh:maxCount 1 ;
        sh:nodeKind sh:Literal ;
        sh:path ns6:isFsfLibre .

    _:Na67d6b4681614d69afdd1a2d31e21023 sh:class ns1:HashAlgorithm ;
        sh:in _:N48dfd1f7541b4504b9518acfed910329 ;
        sh:maxCount 1 ;
        sh:minCount 1 ;
        sh:nodeKind sh:IRI ;
        sh:path ns1:algorithm .

    _:Na68bb014edc846bc9275f2377486515c sh:hasValue ns2:SoftwareArtifact .

    _:Na6acead2170947898371712adbc7f14a rdf:first <https://spdx.org/rdf/3.0.1/terms/Core/ExternalIdentifierType/other> ;
        rdf:rest _:N40d424d8b96741f0b3bd6b6e8df6248f .

    _:Na7c36d0c91d440b8a279a19310da3dd7 rdf:first <https://spdx.org/rdf/3.0.1/terms/Core/ExternalRefType/runtimeAnalysisReport> ;
        rdf:rest _:Ndef7db74c233459f9d05498eb61b3b05 .

    _:Na7c582248f8a4da08f39b510f5695b65 sh:datatype xsd:boolean ;
        sh:maxCount 1 ;
        sh:minCount 1 ;
        sh:nodeKind sh:Literal ;
        sh:path ns3:exploited .

    _:Na7fe9a9442ae4ab48e050da75cf7fd9b sh:datatype xsd:string ;
        sh:nodeKind sh:Literal ;
        sh:path ns1:packageVerificationCodeExcludedFile .

    _:Na832bfa638f84f83b70ca5cffea82294 rdf:first <https://spdx.org/rdf/3.0.1/terms/Core/ExternalRefType/securityAdvisory> ;
        rdf:rest _:N6f376d6f51b6455ea533fab3a8daaa84 .

    _:Na89c4c2fd7ae49d6979e60b818c198d6 rdf:first <https://spdx.org/rdf/3.0.1/terms/Core/ExternalIdentifierType/urlScheme> ;
        rdf:rest () .

    _:Na8b27545614648d89e4b539a936b6592 rdf:first <https://spdx.org/rdf/3.0.1/terms/Software/SoftwarePurpose/documentation> ;
        rdf:rest _:N0999c63e144249578cbe239e5cf95dd1 .

    _:Na900319e94314feaba887afe0e6feaf9 rdf:first <https://spdx.org/rdf/3.0.1/terms/Security/VexJustificationType/componentNotPresent> ;
        rdf:rest _:N7788f32c2dd54dbfba9ee468ee43207e .

    _:Na915e9a792b64c9786cfd8c87264640a rdf:first <https://spdx.org/rdf/3.0.1/terms/Security/CvssSeverityType/critical> ;
        rdf:rest _:N453de8637a7c4769a1c6c7d22ab7d4b1 .

    _:Na91d8910dfaa4193aa3ed17360774321 rdf:first <https://spdx.org/rdf/3.0.1/terms/Security/CvssSeverityType/low> ;
        rdf:rest _:Nbf80191aaa564593be8066e4cc1e9d0c .

    _:Na954d078246c4e94850d486646c66b84 rdf:first <https://spdx.org/rdf/3.0.1/terms/Core/ExternalRefType/cwe> ;
        rdf:rest _:N15cc6817db284c3ca6607af958e89374 .

    _:Na9b18112b463447ebbfc551b36a6a936 rdf:first <https://spdx.org/rdf/3.0.1/terms/Core/RelationshipType/hasExample> ;
        rdf:rest _:N05d54708c5954ef0b3ec6bc915712cc6 .

    _:Naa5226d3f3cb4f6b9ce15eb3a868e120 rdf:first <https://spdx.org/rdf/3.0.1/terms/Core/ExternalRefType/securityPenTestReport> ;
        rdf:rest _:N008447ea57994f4ba18f202542dbb1fe .

    _:Naaabaeb0746945a2b67c9fbd19352387 sh:datatype xsd:string ;
        sh:maxCount 1 ;
        sh:nodeKind sh:Literal ;
        sh:path ns6:standardLicenseTemplate .

    _:Naabc7b3d9517403492a673579cb72ee4 rdf:first <https://spdx.org/rdf/3.0.1/terms/Dataset/DatasetAvailabilityType/directDownload> ;
        rdf:rest _:N917ed0d86b38442e9b3e7e205aa94764 .

    _:Naadc48528c324fbfaeb8eb293f4febe4 sh:datatype xsd:dateTimeStamp ;
        sh:maxCount 1 ;
        sh:nodeKind sh:Literal ;
        sh:path ns3:modifiedTime ;
        sh:pattern "^\\d\\d\\d\\d-\\d\\d-\\d\\dT\\d\\d:\\d\\d:\\d\\dZ$" .

    _:Naadfa67b12564b80b304aa24f2c9a003 rdf:first <https://spdx.org/rdf/3.0.1/terms/Core/ExternalRefType/vulnerabilityExploitabilityAssessment> ;
        rdf:rest () .

    _:Nab13a4619bca44a1b737008bac25cba7 rdf:first <https://spdx.org/rdf/3.0.1/terms/Core/RelationshipType/hasDeclaredLicense> ;
        rdf:rest _:N1a47f2006ba941ce9bf72f120f3e0bd0 .

    _:Nac2cb46be083464eb05e21fa57fef9ff rdf:first <https://spdx.org/rdf/3.0.1/terms/Core/RelationshipType/hasMetadata> ;
        rdf:rest _:N8795c3ed3b6645bcbfeae19e77e2655d .

    _:Nac8ff406770f4d079ab81774c4430c62 rdf:first <https://spdx.org/rdf/3.0.1/terms/Core/ExternalIdentifierType/cpe22> ;
        rdf:rest _:Nd83bab2444c34c90b286de434eb07480 .

    _:Nacd46caa1cf74e399511d6e46de2c8c7 sh:datatype xsd:anyURI ;
        sh:maxCount 1 ;
        sh:nodeKind sh:Literal ;
        sh:path ns1:locationHint .

    _:Nad61e60ebd944e07babf6645c9ef6ff5 sh:hasValue ns6:License .

    _:Nad7823d2540e4e83a052731ffecd7f89 rdf:first <https://spdx.org/rdf/3.0.1/terms/Dataset/DatasetAvailabilityType/registration> ;
        rdf:rest _:N7850efd1860843a6b5cbde6525a0b0d9 .

    _:Nae8f1ff9b13b4fa49368f36cc43b7d3f rdf:first <https://spdx.org/rdf/3.0.1/terms/AI/EnergyUnitType/other> ;
        rdf:rest () .

    _:Naede8dcd34b546bd8ffb872d58865422 rdf:first <https://spdx.org/rdf/3.0.1/terms/Core/ProfileIdentifierType/core> ;
        rdf:rest _:N7a1f905837b84b0faa7bd8a062f960f1 .

    _:Naf131f389db841388f17aef46e96dde2 rdf:first <https://spdx.org/rdf/3.0.1/terms/Software/SoftwarePurpose/configuration> ;
        rdf:rest _:Ndf7aefc3bd774faea62fc45591e991b1 .

    _:Naf8b909011f84634ab93339ae3001573 rdf:first <https://spdx.org/rdf/3.0.1/terms/Core/ExternalRefType/buildMeta> ;
        rdf:rest _:N27fbe2fdc43f45f9b27acdb0cf013194 .

    _:Nafe95e6667734b698498cff03063a128 rdf:first <https://spdx.org/rdf/3.0.1/terms/Software/SoftwarePurpose/source> ;
        rdf:rest _:N13cc50f2fe3a4e479d1d76a35f55d81b .

    _:Nb03705dfc9524babbc8adb93ad2b4062 sh:class ns1:Element ;
        sh:maxCount 1 ;
        sh:minCount 1 ;
        sh:nodeKind sh:IRI ;
        sh:path ns1:from .

    _:Nb0662a3200b74d599b05e932ea138875 rdf:first <https://spdx.org/rdf/3.0.1/terms/Core/HashAlgorithm/sha3_384> ;
        rdf:rest _:N05b14287499e40d4a351b15252bc652e .

    _:Nb16e285c314944e99ea9be0a351754fe rdf:first <https://spdx.org/rdf/3.0.1/terms/Core/LifecycleScopeType/design> ;
        rdf:rest _:N68c2e83624d94d7da2e33e4a0e84a364 .

    _:Nb2ba45a1abdd451d947ce76f4364bde8 rdf:first <https://spdx.org/rdf/3.0.1/terms/Software/SoftwarePurpose/bom> ;
        rdf:rest _:Naf131f389db841388f17aef46e96dde2 .

    _:Nb305b6f6ad12405c86addc7b9fdd4a9a rdf:first <https://spdx.org/rdf/3.0.1/terms/Dataset/DatasetType/audio> ;
        rdf:rest _:Ncebd0643a8ea4c339ee6c83d91a2ac5b .

    _:Nb3a54a8aaab24e43b1d7430ba8709926 rdf:first <https://spdx.org/rdf/3.0.1/terms/Core/ExternalRefType/altDownloadLocation> ;
        rdf:rest _:N2d7cf567343b45b3916d2f1bd14fa304 .

    _:Nb3f306a76df5403290b7c52fb7c130f9 sh:class ns4:EnergyConsumption ;
        sh:maxCount 1 ;
        sh:nodeKind sh:BlankNodeOrIRI ;
        sh:path ns4:energyConsumption .

    _:Nb495361d74244ac4b60416b96f40b3c0 rdf:first <https://spdx.org/rdf/3.0.1/terms/Software/SoftwarePurpose/documentation> ;
        rdf:rest _:N3310bd5aa0b84e6eb5c78f43313cbb4a .

    _:Nb5a9bb07f0ed4b6e95a2012807417d8b rdf:first <https://spdx.org/rdf/3.0.1/terms/Security/SsvcDecisionType/track> ;
        rdf:rest _:Nc135cda445fa4efba0c9eab8ec6f4518 .

    _:Nb5ff4f1d41e643ff944fa4ca63680131 sh:class ns1:Element ;
        sh:maxCount 1 ;
        sh:minCount 1 ;
        sh:nodeKind sh:IRI ;
        sh:path ns1:subject .

    _:Nb6694670c0bd4d9bbe1584c6f432d254 sh:datatype xsd:string ;
        sh:maxCount 1 ;
        sh:nodeKind sh:Literal ;
        sh:path ns6:standardLicenseHeader .

    _:Nb6ad836edee444b7af4e39055772c19d sh:class ns1:LifecycleScopeType ;
        sh:in _:Nb16e285c314944e99ea9be0a351754fe ;
        sh:maxCount 1 ;
        sh:nodeKind sh:IRI ;
        sh:path ns1:scope .

    _:Nb722064cad6d4214ad52df8afc6d7396 rdf:first <https://spdx.org/rdf/3.0.1/terms/Core/PresenceType/noAssertion> ;
        rdf:rest () .

    _:Nb745a8df94a44b1c94d5a41371e693cc rdf:first <https://spdx.org/rdf/3.0.1/terms/Core/ExternalRefType/releaseNotes> ;
        rdf:rest _:Nf09f09f2d4c94e6893d629d040459750 .

    _:Nb7e49e28e70b485b94a91d9e9ca7f4ce sh:datatype xsd:string ;
        sh:nodeKind sh:Literal ;
        sh:path ns5:anonymizationMethodUsed .

    _:Nb8343569c43d4d259d82b46fc7aca5c5 sh:class ns5:DatasetAvailabilityType ;
        sh:in _:N249e05ef4c8e4ed4b3a9224a648e8214 ;
        sh:maxCount 1 ;
        sh:nodeKind sh:IRI ;
        sh:path ns5:datasetAvailability .

    _:Nb83795359b8b4c0193bc067356604bf8 rdf:first <https://spdx.org/rdf/3.0.1/terms/AI/SafetyRiskAssessmentType/low> ;
        rdf:rest () .

    _:Nb83e9b80aedb47339c27bc5911218377 rdf:first <https://spdx.org/rdf/3.0.1/terms/Security/VexJustificationType/vulnerableCodeNotInExecutePath> ;
        rdf:rest _:Ncf161cd13879424a9fcda8e80d86b6f5 .

    _:Nb88428df970a4c8a8ff23dc85f06298b rdf:first <https://spdx.org/rdf/3.0.1/terms/AI/EnergyUnitType/kilowattHour> ;
        rdf:rest _:Ncc5660adb1df4c5c8dba1f94eb65b95b .

    _:Nb9a41ca33e8b4bb8979db11ee7f9ee26 sh:datatype xsd:string ;
        sh:maxCount 1 ;
        sh:nodeKind sh:Literal ;
        sh:path ns1:contentType ;
        sh:pattern "^[^\\/]+\\/[^\\/]+$" .

    _:Nb9cc5f3908f74c15977e12e96ef1f311 rdf:first <https://spdx.org/rdf/3.0.1/terms/Core/RelationshipType/reportedBy> ;
        rdf:rest _:N771b730ffdb64c92b9866f170f5a077d .

    _:Nb9ebb94743d44ed8a77201960c92de33 sh:datatype xsd:anyURI ;
        sh:nodeKind sh:Literal ;
        sh:path ns6:seeAlso .

    _:Nb9f068a614cb433690e515991de940e2 sh:datatype xsd:decimal ;
        sh:maxCount 1 ;
        sh:minCount 1 ;
        sh:nodeKind sh:Literal ;
        sh:path ns3:score .

    _:Nbab338ccec5f425db60782a45394e3b5 sh:datatype xsd:string ;
        sh:maxCount 1 ;
        sh:nodeKind sh:Literal ;
        sh:path ns1:comment .

    _:Nbba38b40d19e4590be95ba3a41aaf46b rdf:first <https://spdx.org/rdf/3.0.1/terms/Dataset/ConfidentialityLevelType/amber> ;
        rdf:rest _:N32759a712cfd43a2b573a645bc799937 .

    _:Nbbfc2c5bd25e451cabc0b232751ec9b3 rdf:first <https://spdx.org/rdf/3.0.1/terms/Core/SupportType/deployed> ;
        rdf:rest _:Nee6738be59a44c5a9e38351f9687387b .

    _:Nbc05456f325c4505bf75f26e68fbb31c sh:class ns1:ExternalIdentifierType ;
        sh:in _:Nac8ff406770f4d079ab81774c4430c62 ;
        sh:maxCount 1 ;
        sh:minCount 1 ;
        sh:nodeKind sh:IRI ;
        sh:path ns1:externalIdentifierType .

    _:Nbc38aabeeaa542fbb91658ff6336efe7 sh:class ns3:VexJustificationType ;
        sh:in _:Na900319e94314feaba887afe0e6feaf9 ;
        sh:maxCount 1 ;
        sh:nodeKind sh:IRI ;
        sh:path ns3:justificationType .

    _:Nbc465417c25c47d59406fb8be56750ab sh:class ns1:DictionaryEntry ;
        sh:nodeKind sh:BlankNodeOrIRI ;
        sh:path ns4:metric .

    _:Nbca6999757c44634acc82bca29955365 rdf:first <https://spdx.org/rdf/3.0.1/terms/Core/RelationshipType/hasDistributionArtifact> ;
        rdf:rest _:N080d1530fe424885b2b334e1d3e9a22d .

    _:Nbe63329c930b4ada8dafd59ab2a6d17f sh:class ns2:ContentIdentifierType ;
        sh:in _:Ne0de946c97554e6592dc3026c3b255cb ;
        sh:maxCount 1 ;
        sh:minCount 1 ;
        sh:nodeKind sh:IRI ;
        sh:path ns2:contentIdentifierType .

    _:Nbeba224eb8864897a66ad9eb4c13fd52 sh:class ns1:RelationshipType ;
        sh:in _:N9931aa59b6d1496abf379e7856751daf ;
        sh:maxCount 1 ;
        sh:minCount 1 ;
        sh:nodeKind sh:IRI ;
        sh:path ns1:relationshipType .

    _:Nbf80191aaa564593be8066e4cc1e9d0c rdf:first <https://spdx.org/rdf/3.0.1/terms/Security/CvssSeverityType/none> ;
        rdf:rest () .

    _:Nbfe64e0eb7844cb39384263cf19da3b5 sh:datatype xsd:string ;
        sh:maxCount 1 ;
        sh:minCount 1 ;
        sh:nodeKind sh:Literal ;
        sh:path ns1:key .

    _:Nc0456d64dcd94263abc800bd8f468791 rdf:first <https://spdx.org/rdf/3.0.1/terms/Core/ExternalRefType/npm> ;
        rdf:rest _:N697dba6853a14fb29a838330aa6c7d28 .

    _:Nc053d18d5def491f9582457af1776545 rdf:first <https://spdx.org/rdf/3.0.1/terms/Software/SoftwarePurpose/requirement> ;
        rdf:rest _:N2ee2b766c01242548892800498fd2655 .

    _:Nc1353b07fba04cb49000857276d12cfa sh:datatype xsd:nonNegativeInteger ;
        sh:maxCount 1 ;
        sh:nodeKind sh:Literal ;
        sh:path ns5:datasetSize .

    _:Nc135cda445fa4efba0c9eab8ec6f4518 rdf:first <https://spdx.org/rdf/3.0.1/terms/Security/SsvcDecisionType/trackStar> ;
        rdf:rest () .

    _:Nc14d6ee8bfc64b29959f55fdf61f8e37 rdf:first <https://spdx.org/rdf/3.0.1/terms/Core/ProfileIdentifierType/dataset> ;
        rdf:rest _:Nd005d5a5407a4ac38c7e7791650920df .

    _:Nc14ff109396a44f896779d4cdc6d3f9e rdf:first <https://spdx.org/rdf/3.0.1/terms/Core/RelationshipType/hasDataFile> ;
        rdf:rest _:Nab13a4619bca44a1b737008bac25cba7 .

    _:Nc24185c7a52445009cdc997577d91935 rdf:first <https://spdx.org/rdf/3.0.1/terms/Core/RelationshipType/ancestorOf> ;
        rdf:rest _:N843e3d8f3df146bf8c261dc7c18eed6a .

    _:Nc2a7c95096f74ab3bdea52afc29ba71b sh:hasValue ns1:Element .

    _:Nc2c772a4e30946299238d1ddc3e1703f sh:datatype xsd:string ;
        sh:maxCount 1 ;
        sh:nodeKind sh:Literal ;
        sh:path ns6:licenseXml .

    _:Nc484f7d89c4d48dba9c5086fad8a3f71 sh:class ns1:CreationInfo ;
        sh:maxCount 1 ;
        sh:minCount 1 ;
        sh:nodeKind sh:BlankNodeOrIRI ;
        sh:path ns1:creationInfo .

    _:Nc4b1e255f762490aaddc557a77379dfd rdf:first <https://spdx.org/rdf/3.0.1/terms/Software/SoftwarePurpose/manifest> ;
        rdf:rest _:N00e704d327644d128a02819a171bb18d .

    _:Nc4bac3b7de8145d3907fb8042c381d25 rdf:first <https://spdx.org/rdf/3.0.1/terms/Core/RelationshipType/amendedBy> ;
        rdf:rest _:Nc24185c7a52445009cdc997577d91935 .

    _:Nc4f2f317f5b74ffda8a534d8115021a0 sh:hasValue ns1:Artifact .

    _:Nc4fceb9c34e84e4fafc753adffe79156 sh:class ns1:DictionaryEntry ;
        sh:nodeKind sh:BlankNodeOrIRI ;
        sh:path ns4:hyperparameter .

    _:Nc5a7bca8248d45d383bedb3d1270d413 rdf:first <https://spdx.org/rdf/3.0.1/terms/Core/ExternalIdentifierType/swhid> ;
        rdf:rest _:N32f6eb21ae6b4c7fa4eeba186c255b53 .

    _:Nc647bd18250b49c690d79de4484b2c55 rdf:first <https://spdx.org/rdf/3.0.1/terms/Core/HashAlgorithm/md5> ;
        rdf:rest _:N054c6a610eb1434cbd912c9c3616c8db .

    _:Nc7b576a90fb2450f98d1bc492f4fbe06 rdf:first <https://spdx.org/rdf/3.0.1/terms/Core/HashAlgorithm/adler32> ;
        rdf:rest _:N078b0758ac424dedab46bf98c3086c58 .

    _:Nc7e2cbf4e3484223ac825b08c7c397c1 sh:message "https://spdx.org/rdf/3.0.1/terms/Extension/Extension is an abstract class and should not be instantiated directly. Instantiate a subclass instead."@en ;
        sh:not _:N9b235bcc4a91486eb87fc626fc1ab570 ;
        sh:path rdf:type .

    _:Nc7f0e867cdc148a6a3b6a15ffebab59f sh:class ns4:EnergyConsumptionDescription ;
        sh:nodeKind sh:BlankNodeOrIRI ;
        sh:path ns4:inferenceEnergyConsumption .

    _:Nc81ae3ec31284874b9c71d4b0c84588d sh:datatype xsd:anyURI ;
        sh:maxCount 1 ;
        sh:minCount 1 ;
        sh:nodeKind sh:Literal ;
        sh:path ns3:locator .

    _:Nca26c79ce5d04845979e1252bcde1edc sh:class ns3:SsvcDecisionType ;
        sh:in _:Nea0d47f7c35642eea322e1f1c2414656 ;
        sh:maxCount 1 ;
        sh:minCount 1 ;
        sh:nodeKind sh:IRI ;
        sh:path ns3:decisionType .

    _:Nca3b23dabdfe4202b6f0730f38ac366b rdf:first <https://spdx.org/rdf/3.0.1/terms/Core/RelationshipType/hasOutput> ;
        rdf:rest _:N3aeceae3663a4fb19126c7152560e7f3 .

    _:Nca65717c3354405c874c1aff7975811e rdf:first <https://spdx.org/rdf/3.0.1/terms/Dataset/ConfidentialityLevelType/red> ;
        rdf:rest _:Nbba38b40d19e4590be95ba3a41aaf46b .

    _:Nca907d776f8d4f5fa2254d492fb5d42a rdf:first <https://spdx.org/rdf/3.0.1/terms/Core/HashAlgorithm/sha3_224> ;
        rdf:rest _:N27738122637d491d85271152fecfd26f .

    _:Ncbdd7b9aaf92411289bbf1bed5771c04 rdf:first <https://spdx.org/rdf/3.0.1/terms/Core/ExternalRefType/metrics> ;
        rdf:rest _:Nc0456d64dcd94263abc800bd8f468791 .

    _:Ncc33c607adee40068ee304956b2dc382 sh:datatype xsd:string ;
        sh:maxCount 1 ;
        sh:nodeKind sh:Literal ;
        sh:path ns1:name .

    _:Ncc5660adb1df4c5c8dba1f94eb65b95b rdf:first <https://spdx.org/rdf/3.0.1/terms/AI/EnergyUnitType/megajoule> ;
        rdf:rest _:Nae8f1ff9b13b4fa49368f36cc43b7d3f .

    _:Nccd8642028564e56a31dc2ca5e9bde7d rdf:first <https://spdx.org/rdf/3.0.1/terms/Core/ExternalRefType/dynamicAnalysisReport> ;
        rdf:rest _:Ne67faee0a41f4d349f60fc73df94f88c .

    _:Ncd71557870a24229a05d5a04577849b9 rdf:first <https://spdx.org/rdf/3.0.1/terms/Software/SoftwarePurpose/archive> ;
        rdf:rest _:Nf4e017dc7555464a813dca32da3f4ad6 .

    _:Ncd7cc4594b51490cb5085d42f92b0319 rdf:first <https://spdx.org/rdf/3.0.1/terms/Dataset/DatasetType/numeric> ;
        rdf:rest _:N149b28ab06e84c0f9c7a748fe270d619 .

    _:Nce8d42474a1842ffa06cef1e9067de1b rdf:first <https://spdx.org/rdf/3.0.1/terms/Core/ProfileIdentifierType/simpleLicensing> ;
        rdf:rest _:N414a8299276840138167c2cfe582fe15 .

    _:Nceb6751330ee48a1bad54900bc5edbca rdf:first <https://spdx.org/rdf/3.0.1/terms/Software/SoftwarePurpose/filesystemImage> ;
        rdf:rest _:Ne939dfb35d6145b790cf53a12c5a92ff .

    _:Ncebd0643a8ea4c339ee6c83d91a2ac5b rdf:first <https://spdx.org/rdf/3.0.1/terms/Dataset/DatasetType/categorical> ;
        rdf:rest _:Nfc55469d6b8e4923b4378b116ad09f22 .

    _:Ncf161cd13879424a9fcda8e80d86b6f5 rdf:first <https://spdx.org/rdf/3.0.1/terms/Security/VexJustificationType/inlineMitigationsAlreadyExist> ;
        rdf:rest () .

    _:Ncfdc44469dd94616b893a53c66f417ea rdf:first <https://spdx.org/rdf/3.0.1/terms/Core/RelationshipType/hasOptionalDependency> ;
        rdf:rest _:Nca3b23dabdfe4202b6f0730f38ac366b .

    _:Ncff928a0fc1a45b8bb4c13e9ebff923a rdf:first <https://spdx.org/rdf/3.0.1/terms/Core/ExternalRefType/exportControlAssessment> ;
        rdf:rest _:Na1afc73eaba1435383aaab5260aaef74 .

    _:Nd005d5a5407a4ac38c7e7791650920df rdf:first <https://spdx.org/rdf/3.0.1/terms/Core/ProfileIdentifierType/extension> ;
        rdf:rest _:N1c7200275aa241b5ae9a577d9c06b2d9 .

    _:Nd09e69a597cd43079761fc0d8051bce5 sh:datatype xsd:string ;
        sh:nodeKind sh:Literal ;
        sh:path ns5:knownBias .

    _:Nd0e089337a33424fabe3fdff5e9353f2 sh:datatype xsd:string ;
        sh:maxCount 1 ;
        sh:minCount 1 ;
        sh:nodeKind sh:Literal ;
        sh:path <https://spdx.org/rdf/3.0.1/terms/SimpleLicensing/licenseExpression> .

    _:Nd2b4b8ceb1424471a1f401c56908b8d7 sh:class ns1:IntegrityMethod ;
        sh:nodeKind sh:BlankNodeOrIRI ;
        sh:path ns1:verifiedUsing .

    _:Nd2de0ed500c448f792eb6382b9c9daab sh:class ns1:ExternalRefType ;
        sh:in _:Nb3a54a8aaab24e43b1d7430ba8709926 ;
        sh:maxCount 1 ;
        sh:nodeKind sh:IRI ;
        sh:path ns1:externalRefType .

    _:Nd338fc87819546f6b745436b92c129a8 rdf:first <https://spdx.org/rdf/3.0.1/terms/Core/RelationshipCompleteness/incomplete> ;
        rdf:rest _:Nec4db23197cf47f0ae849b9d7d207fb4 .

    _:Nd4845c86c2ed49d88fcef6b52e75d8cd sh:datatype xsd:string ;
        sh:maxCount 1 ;
        sh:nodeKind sh:Literal ;
        sh:path ns5:intendedUse .

    _:Nd4bee614558747679a512d0df577540b sh:class ns1:Agent ;
        sh:minCount 1 ;
        sh:nodeKind sh:IRI ;
        sh:path ns1:createdBy .

    _:Nd4e2d851f19e4c6f9629e565d0805f02 rdf:first <https://spdx.org/rdf/3.0.1/terms/Core/ExternalRefType/license> ;
        rdf:rest _:N3833dfea16ca487f88ee56d974e3135e .

    _:Nd4ed37fcf1fd4068bb0deee0221ce837 sh:datatype xsd:anyURI ;
        sh:maxCount 1 ;
        sh:nodeKind sh:Literal ;
        sh:path ns2:downloadLocation .

    _:Nd54342913bcd4a3ea6a26935ed2dd422 rdf:first <https://spdx.org/rdf/3.0.1/terms/Core/HashAlgorithm/sha256> ;
        rdf:rest _:Nd56e8e0c611647a68325bb512b471433 .

    _:Nd563623ee8ae44a2aae208601aae8853 rdf:first <https://spdx.org/rdf/3.0.1/terms/Dataset/DatasetType/timeseries> ;
        rdf:rest _:Nf03c6333536b4b6a97360b95b2264a6f .

    _:Nd56e8e0c611647a68325bb512b471433 rdf:first <https://spdx.org/rdf/3.0.1/terms/Core/HashAlgorithm/sha384> ;
        rdf:rest _:N738a8d5957cb40f2a2fcf70c01d1d55c .

    _:Nd61a0d6f4c5b44a4a882de3953b8c716 rdf:first <https://spdx.org/rdf/3.0.1/terms/Core/ExternalRefType/purchaseOrder> ;
        rdf:rest _:N8618f8df62f8426586277f411a3ea2a9 .

    _:Nd74a690a40a64a01b9cab2e0062d1fc7 rdf:first <https://spdx.org/rdf/3.0.1/terms/Core/ProfileIdentifierType/build> ;
        rdf:rest _:N75c08d7cf8e1440cb4a9d99ed2a02f78 .

    _:Nd7b0801994b24e409fe5c6d54edb8618 sh:datatype xsd:positiveInteger ;
        sh:maxCount 1 ;
        sh:minCount 1 ;
        sh:nodeKind sh:Literal ;
        sh:path ns1:endIntegerRange .

    _:Nd7ce9307a16247cb86d95f5c40e0baed sh:class ns2:SbomType ;
        sh:in _:Nee479af86fc1437f97737de274dff0ec ;
        sh:nodeKind sh:IRI ;
        sh:path ns2:sbomType .

    _:Nd83bab2444c34c90b286de434eb07480 rdf:first <https://spdx.org/rdf/3.0.1/terms/Core/ExternalIdentifierType/cpe23> ;
        rdf:rest _:Nfbf51eca9c974cd097d8b8fd5026d93e .

    _:Nd91d7910edf44e0683080e7e6530cf13 sh:datatype xsd:string ;
        sh:maxCount 1 ;
        sh:nodeKind sh:Literal ;
        sh:path ns1:value .

    _:Nd94ddbb247794b3f828de114beb815b4 rdf:first <https://spdx.org/rdf/3.0.1/terms/Core/HashAlgorithm/crystalsKyber> ;
        rdf:rest _:N608336c4745d41e18e5f1c85ec83ddd7 .

    _:Nda66589397164e3e8b13693c43d08638 sh:datatype xsd:dateTimeStamp ;
        sh:maxCount 1 ;
        sh:nodeKind sh:Literal ;
        sh:path ns1:startTime ;
        sh:pattern "^\\d\\d\\d\\d-\\d\\d-\\d\\dT\\d\\d:\\d\\d:\\d\\dZ$" .

    _:Ndad87f1ff2f2485e8c88dd126918131f sh:hasValue ns3:VulnAssessmentRelationship .

    _:Ndae5459fc26c4e94ba0292367c100cf2 rdf:first <https://spdx.org/rdf/3.0.1/terms/Core/HashAlgorithm/sha3_512> ;
        rdf:rest () .

    _:Ndc33c03c6f3b4f76b2a9c5f0755b4682 rdf:first <https://spdx.org/rdf/3.0.1/terms/Core/ExternalRefType/socialMedia> ;
        rdf:rest _:N160083f6100f4e10a59b9acb061ad7a7 .

    _:Ndc68023588dd4e39a254912e522cbcb9 rdf:first <https://spdx.org/rdf/3.0.1/terms/Core/PresenceType/yes> ;
        rdf:rest _:N22f5d668ae27446e95d634e5bf09c6b4 .

    _:Ndcd4af75b0f549f59e8e7fb96c6b8e6d rdf:first <https://spdx.org/rdf/3.0.1/terms/Core/ExternalRefType/mailingList> ;
        rdf:rest _:N8b3541e2042542e19c148a7b6065af51 .

    _:Ndcf79036b2984f98b7df79c8b9adab46 rdf:first <https://spdx.org/rdf/3.0.1/terms/Core/RelationshipType/testedOn> ;
        rdf:rest _:N9b100afdb515432cab5b744e6ab3aad3 .

    _:Ndd38650fb33a437387707abd8ca9f4a0 sh:datatype xsd:string ;
        sh:maxCount 1 ;
        sh:nodeKind sh:Literal ;
        sh:path ns1:summary .

    _:Ndd9c27ec175a4f028fe9688b608d7b81 sh:class ns4:EnergyConsumptionDescription ;
        sh:nodeKind sh:BlankNodeOrIRI ;
        sh:path ns4:trainingEnergyConsumption .

    _:Nddaef0505c8846cb8078511e66534d20 rdf:first <https://spdx.org/rdf/3.0.1/terms/Core/RelationshipType/hasProvidedDependency> ;
        rdf:rest _:N42cff411a4ec44199c63b36da8d918ae .

    _:Nddc401bd8e504a29b9751ba14b64084c rdf:first <https://spdx.org/rdf/3.0.1/terms/Core/ExternalRefType/securityOther> ;
        rdf:rest _:Naa5226d3f3cb4f6b9ce15eb3a868e120 .

    _:Nde571d96a80f4e85a264a336caf64f29 rdf:first <https://spdx.org/rdf/3.0.1/terms/Core/RelationshipType/hasDynamicLink> ;
        rdf:rest _:N179cf083985f41f09e2541d2ac40a243 .

    _:Ndef7db74c233459f9d05498eb61b3b05 rdf:first <https://spdx.org/rdf/3.0.1/terms/Core/ExternalRefType/secureSoftwareAttestation> ;
        rdf:rest _:Na832bfa638f84f83b70ca5cffea82294 .

    _:Ndf7aefc3bd774faea62fc45591e991b1 rdf:first <https://spdx.org/rdf/3.0.1/terms/Software/SoftwarePurpose/container> ;
        rdf:rest _:N267727c5fe684dc2ac36ab3119a5ed43 .

    _:Ndf979723179648f495f1ba2ce971220b sh:datatype xsd:dateTimeStamp ;
        sh:maxCount 1 ;
        sh:nodeKind sh:Literal ;
        sh:path <https://spdx.org/rdf/3.0.1/terms/Build/buildEndTime> ;
        sh:pattern "^\\d\\d\\d\\d-\\d\\d-\\d\\dT\\d\\d:\\d\\d:\\d\\dZ$" .

    _:Ne015ec7355ad49feb860c0240976b3f6 rdf:first <https://spdx.org/rdf/3.0.1/terms/Software/SoftwarePurpose/operatingSystem> ;
        rdf:rest _:Nfe3b06afa8144419b0c38b64e8c69e95 .

    _:Ne0de946c97554e6592dc3026c3b255cb rdf:first <https://spdx.org/rdf/3.0.1/terms/Software/ContentIdentifierType/gitoid> ;
        rdf:rest _:N2d443860b51642498f3ba9b7de6dabb1 .

    _:Ne14b7f7dceac423b869e219e73c16475 rdf:first <https://spdx.org/rdf/3.0.1/terms/Core/ExternalIdentifierType/gitoid> ;
        rdf:rest _:Na6acead2170947898371712adbc7f14a .

    _:Ne288e79e880942c88b00de65120682a6 sh:datatype xsd:boolean ;
        sh:maxCount 1 ;
        sh:nodeKind sh:Literal ;
        sh:path ns6:isOsiApproved .

    _:Ne30c85bbf11b4c2b849b8440be508bee rdf:first <https://spdx.org/rdf/3.0.1/terms/Core/RelationshipType/hasAssociatedVulnerability> ;
        rdf:rest _:N97062f00bfbe4738bee3ead0b37f9559 .

    _:Ne327d40f301646b19534d8557a045729 rdf:first <https://spdx.org/rdf/3.0.1/terms/Software/SoftwarePurpose/diskImage> ;
        rdf:rest _:N6db8b82bbd76401192e164fd3d83bc7d .

    _:Ne3c3e73bf0024056b48f227a5a1a82b4 sh:datatype xsd:boolean ;
        sh:maxCount 1 ;
        sh:nodeKind sh:Literal ;
        sh:path ns6:isDeprecatedLicenseId .

    _:Ne43e2e4ed2284b8faf28cc074be90105 sh:datatype xsd:string ;
        sh:maxCount 1 ;
        sh:nodeKind sh:Literal ;
        sh:path ns6:obsoletedBy .

    _:Ne51c4c707e4f41a1b4da38412adebb44 sh:datatype xsd:dateTimeStamp ;
        sh:maxCount 1 ;
        sh:nodeKind sh:Literal ;
        sh:path ns1:endTime ;
        sh:pattern "^\\d\\d\\d\\d-\\d\\d-\\d\\dT\\d\\d:\\d\\d:\\d\\dZ$" .

    _:Ne5201624bfcf4f99ab0db3b6d2e24290 sh:class ns5:DatasetType ;
        sh:in _:Nb305b6f6ad12405c86addc7b9fdd4a9a ;
        sh:minCount 1 ;
        sh:nodeKind sh:IRI ;
        sh:path ns5:datasetType .

    _:Ne52e90f5af784f2390f0418ed3d386af rdf:first <https://spdx.org/rdf/3.0.1/terms/AI/SafetyRiskAssessmentType/medium> ;
        rdf:rest _:Nb83795359b8b4c0193bc067356604bf8 .

    _:Ne5a3b834457f4513b0d88d69c7a6165e rdf:first <https://spdx.org/rdf/3.0.1/terms/Dataset/DatasetType/noAssertion> ;
        rdf:rest _:Ncd7cc4594b51490cb5085d42f92b0319 .

    _:Ne63b7372f8f848e1b95290b02cdb5b4b rdf:first <https://spdx.org/rdf/3.0.1/terms/Software/SoftwarePurpose/file> ;
        rdf:rest _:N315f00e673e1400783fbaeb9b737f0e0 .

    _:Ne67faee0a41f4d349f60fc73df94f88c rdf:first <https://spdx.org/rdf/3.0.1/terms/Core/ExternalRefType/eolNotice> ;
        rdf:rest _:Ncff928a0fc1a45b8bb4c13e9ebff923a .

    _:Ne6c4aa6804e944f8bd7a0ef6b63f41b3 sh:class ns1:ExternalIdentifier ;
        sh:nodeKind sh:BlankNodeOrIRI ;
        sh:path ns1:externalIdentifier .

    _:Ne707f0a1c2b640dd8605aa3d18c23fe0 rdf:first <https://spdx.org/rdf/3.0.1/terms/Software/SoftwarePurpose/file> ;
        rdf:rest _:Nceb6751330ee48a1bad54900bc5edbca .

    _:Ne77d3a4557c448f4ac0a95430be9327a sh:class ns4:EnergyUnitType ;
        sh:in _:Nb88428df970a4c8a8ff23dc85f06298b ;
        sh:maxCount 1 ;
        sh:minCount 1 ;
        sh:nodeKind sh:IRI ;
        sh:path ns4:energyUnit .

    _:Ne7e5a05ecc9543c1886186899803709a sh:datatype xsd:string ;
        sh:maxCount 1 ;
        sh:nodeKind sh:Literal ;
        sh:path ns3:statusNotes .

    _:Ne89807f76836447eb0705178b28eb703 sh:datatype xsd:string ;
        sh:maxCount 1 ;
        sh:nodeKind sh:Literal ;
        sh:path ns1:contentType ;
        sh:pattern "^[^\\/]+\\/[^\\/]+$" .

    _:Ne8e3a0b318ce4f5aa1caff37d2fcb20a sh:class ns2:FileKindType ;
        sh:in _:N62c6de3503e24e62a556e92b063c0984 ;
        sh:maxCount 1 ;
        sh:nodeKind sh:IRI ;
        sh:path ns2:fileKind .

    _:Ne939dfb35d6145b790cf53a12c5a92ff rdf:first <https://spdx.org/rdf/3.0.1/terms/Software/SoftwarePurpose/firmware> ;
        rdf:rest _:N1adb71f64c494276bd8ce6ba1835bb14 .

    _:Ne9d2cb66eb1941d7bea887a1b7626842 rdf:first <https://spdx.org/rdf/3.0.1/terms/Core/RelationshipType/publishedBy> ;
        rdf:rest _:Nb9cc5f3908f74c15977e12e96ef1f311 .

    _:Nea0d47f7c35642eea322e1f1c2414656 rdf:first <https://spdx.org/rdf/3.0.1/terms/Security/SsvcDecisionType/act> ;
        rdf:rest _:N9a6194fa9fd840fd9bc36e7a2f49e8fe .

    _:Nea50294f6176494390eeae5709b2e306 rdf:first <https://spdx.org/rdf/3.0.1/terms/Software/SoftwarePurpose/diskImage> ;
        rdf:rest _:N169badfc343741d8b91b256cd37c91ef .

    _:Nec315ded94b34cc7be920c90f7154835 rdf:first <https://spdx.org/rdf/3.0.1/terms/Software/SoftwarePurpose/other> ;
        rdf:rest _:N8784ce86e26a44f8917c2cb04540f2fa .

    _:Nec4db23197cf47f0ae849b9d7d207fb4 rdf:first <https://spdx.org/rdf/3.0.1/terms/Core/RelationshipCompleteness/complete> ;
        rdf:rest _:N450e41ff31f14b2f8f02b111590ec074 .

    _:Necfaa34feca646d2bbdae7cf330b0d21 sh:datatype xsd:dateTimeStamp ;
        sh:maxCount 1 ;
        sh:nodeKind sh:Literal ;
        sh:path ns1:builtTime ;
        sh:pattern "^\\d\\d\\d\\d-\\d\\d-\\d\\dT\\d\\d:\\d\\d:\\d\\dZ$" .

    _:Ned659fae654449459e07497f6e373a2f rdf:first <https://spdx.org/rdf/3.0.1/terms/Core/PresenceType/no> ;
        rdf:rest _:Nb722064cad6d4214ad52df8afc6d7396 .

    _:Nee479af86fc1437f97737de274dff0ec rdf:first <https://spdx.org/rdf/3.0.1/terms/Software/SbomType/design> ;
        rdf:rest _:N0afc30bb743f4d009a5d45f696c981ee .

    _:Nee6738be59a44c5a9e38351f9687387b rdf:first <https://spdx.org/rdf/3.0.1/terms/Core/SupportType/limitedSupport> ;
        rdf:rest _:Nf27db8760dff42a4b239c48ca214a971 .

    _:Nee7eba2d955d4cf287820533f6f0294c rdf:first <https://spdx.org/rdf/3.0.1/terms/Dataset/DatasetType/syntactic> ;
        rdf:rest _:N48a7f32ef65a4710a46f9178452a5697 .

    _:Nf0383326d60f4bc6bc14664a2e85ec74 sh:class ns2:ContentIdentifier ;
        sh:nodeKind sh:BlankNodeOrIRI ;
        sh:path ns2:contentIdentifier .

    _:Nf03c6333536b4b6a97360b95b2264a6f rdf:first <https://spdx.org/rdf/3.0.1/terms/Dataset/DatasetType/timestamp> ;
        rdf:rest _:N74c9b0d0b2a44318a1794544b42e5081 .

    _:Nf09f09f2d4c94e6893d629d040459750 rdf:first <https://spdx.org/rdf/3.0.1/terms/Core/ExternalRefType/releaseHistory> ;
        rdf:rest _:N39440260803745439d41569527a518f2 .

    _:Nf18b2b0b18d24739be254a0caccb68c2 sh:class ns3:ExploitCatalogType ;
        sh:in _:N395079a4589e43409d7dc314988c66b3 ;
        sh:maxCount 1 ;
        sh:minCount 1 ;
        sh:nodeKind sh:IRI ;
        sh:path ns3:catalogType .

    _:Nf194d1d57fa14930b63cf53846dd5d0f rdf:first <https://spdx.org/rdf/3.0.1/terms/Dataset/DatasetType/structured> ;
        rdf:rest _:Nee7eba2d955d4cf287820533f6f0294c .

    _:Nf2006a25a5df4b449c058903cb4ddeba rdf:first <https://spdx.org/rdf/3.0.1/terms/Security/CvssSeverityType/low> ;
        rdf:rest _:N2835f5412cad42c19d531af2aacf35f8 .

    _:Nf24a922499724d41b0bbedfdb59993a8 sh:datatype xsd:string ;
        sh:maxCount 1 ;
        sh:minCount 1 ;
        sh:nodeKind sh:Literal ;
        sh:path ns3:actionStatement .

    _:Nf27db8760dff42a4b239c48ca214a971 rdf:first <https://spdx.org/rdf/3.0.1/terms/Core/SupportType/endOfSupport> ;
        rdf:rest _:N28390bd265c84d20853195d19dd59cfd .

    _:Nf2f414b51e3a4686a5cb9e3a84c327c8 rdf:first <https://spdx.org/rdf/3.0.1/terms/Core/ExternalRefType/securityFix> ;
        rdf:rest _:Nddc401bd8e504a29b9751ba14b64084c .

    _:Nf411b42be5ac4dcc8a50125556eabe37 sh:datatype xsd:dateTimeStamp ;
        sh:maxCount 1 ;
        sh:nodeKind sh:Literal ;
        sh:path ns1:validUntilTime ;
        sh:pattern "^\\d\\d\\d\\d-\\d\\d-\\d\\dT\\d\\d:\\d\\d:\\d\\dZ$" .

    _:Nf4e017dc7555464a813dca32da3f4ad6 rdf:first <https://spdx.org/rdf/3.0.1/terms/Software/SoftwarePurpose/bom> ;
        rdf:rest _:N1acc6ac0c09846f9ba914ec4d6009865 .

    _:Nf4f02465310d47dfabbaa4e6912fe113 rdf:first <https://spdx.org/rdf/3.0.1/terms/Core/HashAlgorithm/md5> ;
        rdf:rest _:Nfe48a96b178f45be876339c916de5092 .

    _:Nf539274bb41f4f0aad37bb02b1e1ad05 sh:datatype xsd:decimal ;
        sh:maxCount 1 ;
        sh:minCount 1 ;
        sh:nodeKind sh:Literal ;
        sh:path ns4:energyQuantity .

    _:Nf68d5ece5e9048618433f794c917391d sh:datatype xsd:string ;
        sh:nodeKind sh:Literal ;
        sh:path ns4:standardCompliance .

    _:Nf6d27b818a8849d5928e3b8f3d90a57a sh:class <https://spdx.org/rdf/3.0.1/terms/Extension/CdxPropertyEntry> ;
        sh:minCount 1 ;
        sh:nodeKind sh:BlankNodeOrIRI ;
        sh:path <https://spdx.org/rdf/3.0.1/terms/Extension/cdxProperty> .

    _:Nf740deac06444efb948d8e08b489ea6e rdf:first <https://spdx.org/rdf/3.0.1/terms/Core/SupportType/development> ;
        rdf:rest _:Na13406b855df4150971e1c76ed24b827 .

    _:Nf7723676f78c465082f370aa66673665 sh:datatype xsd:string ;
        sh:nodeKind sh:Literal ;
        sh:path ns4:typeOfModel .

    _:Nf8063a7692e44de79e8dd3cb56859bc7 rdf:first <https://spdx.org/rdf/3.0.1/terms/Core/HashAlgorithm/md2> ;
        rdf:rest _:N8013bcfb52cb4e51bbb49dc7a6710704 .

    _:Nf841a206f30a429a9e1cbeed0e2e102f sh:class ns4:SafetyRiskAssessmentType ;
        sh:in _:N6d187fa41aab49559fc1e40fe096601d ;
        sh:maxCount 1 ;
        sh:nodeKind sh:IRI ;
        sh:path ns4:safetyRiskAssessment .

    _:Nf8731ab568e344619e5d2a29ff0c9e3c rdf:first <https://spdx.org/rdf/3.0.1/terms/AI/SafetyRiskAssessmentType/high> ;
        rdf:rest _:Ne52e90f5af784f2390f0418ed3d386af .

    _:Nf87704a94ca4450f8dd886c348a8a30f sh:class <https://spdx.org/rdf/3.0.1/terms/SimpleLicensing/AnyLicenseInfo> ;
        sh:maxCount 1 ;
        sh:nodeKind sh:IRI ;
        sh:path ns1:dataLicense .

    _:Nf9bbec9b6b924452ac692c71f561aa1d sh:datatype xsd:string ;
        sh:maxCount 1 ;
        sh:nodeKind sh:Literal ;
        sh:path ns6:standardAdditionTemplate .

    _:Nfab4dd42d8a74ea2b147d597f33b984f sh:datatype xsd:string ;
        sh:maxCount 1 ;
        sh:nodeKind sh:Literal ;
        sh:path ns5:datasetUpdateMechanism .

    _:Nfbf51eca9c974cd097d8b8fd5026d93e rdf:first <https://spdx.org/rdf/3.0.1/terms/Core/ExternalIdentifierType/cve> ;
        rdf:rest _:N9bf956e203414b89929bf7146b83f11a .

    _:Nfc2362f61f554fa28c87aefb63bb7aaa sh:class <https://spdx.org/rdf/3.0.1/terms/SimpleLicensing/AnyLicenseInfo> ;
        sh:minCount 2 ;
        sh:nodeKind sh:IRI ;
        sh:path ns6:member .

    _:Nfc510bb7e1284c82ab76da5c2a2a951c rdf:first <https://spdx.org/rdf/3.0.1/terms/Core/HashAlgorithm/blake2b256> ;
        rdf:rest _:Na448701a1d1e497c8bdb122d21f1ab5c .

    _:Nfc55469d6b8e4923b4378b116ad09f22 rdf:first <https://spdx.org/rdf/3.0.1/terms/Dataset/DatasetType/graph> ;
        rdf:rest _:N01334926969a4a02ba648f9ae9cc0f83 .

    _:Nfd257672c0f8447bb2fe370e2da6108a sh:hasValue ns6:LicenseAddition .

    _:Nfd5dcb568f8744a58f8df95723e02649 sh:class ns1:PositiveIntegerRange ;
        sh:maxCount 1 ;
        sh:nodeKind sh:BlankNodeOrIRI ;
        sh:path ns2:lineRange .

    _:Nfd7fff7459584d6a8b9be92d44234a7f sh:datatype xsd:anyURI ;
        sh:maxCount 1 ;
        sh:nodeKind sh:Literal ;
        sh:path ns2:packageUrl .

    _:Nfdbfecf7fd1f4fbe972985748c2fb51f sh:datatype xsd:string ;
        sh:nodeKind sh:Literal ;
        sh:path ns1:standardName .

    _:Nfe09149c948a4591baf966eeef8021dd rdf:first <https://spdx.org/rdf/3.0.1/terms/Core/RelationshipType/patchedBy> ;
        rdf:rest _:Ne9d2cb66eb1941d7bea887a1b7626842 .

    _:Nfe30d0e9941a4ea8a330bf63192fe968 sh:datatype xsd:string ;
        sh:nodeKind sh:Literal ;
        sh:path ns4:modelDataPreprocessing .

    _:Nfe3b06afa8144419b0c38b64e8c69e95 rdf:first <https://spdx.org/rdf/3.0.1/terms/Software/SoftwarePurpose/other> ;
        rdf:rest _:N432205fe203e478e89d71b535134025e .

    _:Nfe48a96b178f45be876339c916de5092 rdf:first <https://spdx.org/rdf/3.0.1/terms/Core/HashAlgorithm/md6> ;
        rdf:rest _:N7d6920e1fda8401d8fee4b5dd11b7196 .

    _:Nfedcce2ec4334b5dbcd72a892757bcfb sh:datatype xsd:string ;
        sh:maxCount 1 ;
        sh:nodeKind sh:Literal ;
        sh:path ns3:vexVersion .

    _:Nff29bfb461de4653a0c106ee09905e74 rdf:first <https://spdx.org/rdf/3.0.1/terms/Core/RelationshipType/hasStaticLink> ;
        rdf:rest _:N8a3eb069ab8a42d9ba1b350b7c463fbb .

    _:Nff2e796ec34649ed9122145035384de4 rdf:first <https://spdx.org/rdf/3.0.1/terms/Core/RelationshipType/fixedBy> ;
        rdf:rest _:N5f343653cdff44f9bb62e8379ac7884e .
}

