@prefix dcterms: <http://purl.org/dc/terms/> .
@prefix ns1: <https://spdx.org/rdf/3.0.1/terms/Core/> .
@prefix ns2: <https://spdx.org/rdf/3.0.1/terms/AI/> .
@prefix ns3: <https://spdx.org/rdf/3.0.1/terms/Software/> .
@prefix ns4: <https://spdx.org/rdf/3.0.1/terms/Security/> .
@prefix ns5: <https://spdx.org/rdf/3.0.1/terms/ExpandedLicensing/> .
@prefix ns6: <https://spdx.org/rdf/3.0.1/terms/Dataset/> .
@prefix omg-ann: <https://www.omg.org/spec/Commons/AnnotationVocabulary/> .
@prefix owl: <http://www.w3.org/2002/07/owl#> .
@prefix rdf: <http://www.w3.org/1999/02/22-rdf-syntax-ns#> .
@prefix rdfs: <http://www.w3.org/2000/01/rdf-schema#> .
@prefix sh: <http://www.w3.org/ns/shacl#> .
@prefix spdx: <https://spdx.org/rdf/3.0.1/terms/> .
@prefix xsd: <http://www.w3.org/2001/XMLSchema#> .

_:N1c770fdb6e14494b87eac716e909c48e {
    ns2:AIPackage a owl:Class,
            sh:NodeShape ;
        rdfs:comment "Specifies an AI package and its associated information."@en ;
        rdfs:subClassOf ns3:Package ;
        sh:nodeKind sh:IRI ;
        sh:property _:N19ca4558cdb341ee9c37bfe7dbd5725f,
            _:N1f22a6fa2025402ebb1d66bae0bbfd63,
            _:N29eb269c4389443f8ded26f8ac3ba6b6,
            _:N32ea05029eca4d0cb9b3191393efdb1c,
            _:N370ed73a1c1e4ff09d768ae422e135dd,
            _:N47fb54a94ed9447280f7321c48e2982b,
            _:N683ff685a95941dfbff264b5fb2feb94,
            _:N6f7c535ec5984714bdc5cd9e6f23c8a7,
            _:N7c2570f4196247ea90dd5b3d7ca0b22e,
            _:N7dc5b81f3a044db6ba8e80d052ea722f,
            _:N840f91254c8c467788b8d2ccb69e172c,
            _:Nb6114b281470409dba07ab5b55d23066,
            _:Ne1a811cecaeb4f3ea40377cb54d1a8ad,
            _:Nedc283c28c9b44ccad4b01a90a31f2ca,
            _:Nfb56dda28f4e4167ae11a43fab219b2f .

    <https://spdx.org/rdf/3.0.1/terms/Build/Build> a owl:Class,
            sh:NodeShape ;
        rdfs:comment "Class that describes a build instance of software/artifacts."@en ;
        rdfs:subClassOf ns1:Element ;
        sh:nodeKind sh:IRI ;
        sh:property _:N15521aa0152f4af5a3545aa71f2c4b78,
            _:N17b11e9782cb42ceba98928679b0f78b,
            _:N3cf836c0e1cc41a780ab94e0d629cfc8,
            _:N3d3db55210ce441eb305cdf967d96a2d,
            _:N81443e2b66644d6f8f751bad29789396,
            _:N9d3e8c20daa5400b957c25be113efe89,
            _:Na8466e22ae484f8ab197aa7b0d012695,
            _:Nd70830e62e09431f9f5ac0ca57ad91de,
            _:Nea626a2a6c9a4deab1b1cdd962d00ea7 .

    ns1:Annotation a owl:Class,
            sh:NodeShape ;
        rdfs:comment "An assertion made in relation to one or more elements."@en ;
        rdfs:subClassOf ns1:Element ;
        sh:nodeKind sh:IRI ;
        sh:property _:N1599c92508f549eeadacc4250040a171,
            _:N5448c070514c428eaa4d89cbdbc61908,
            _:N943f36b7c5ef4596ab447543bb558d7e,
            _:Nfa8ad30b19ec414288e9039e2e1f534e .

    ns1:LifecycleScopedRelationship a owl:Class,
            sh:NodeShape ;
        rdfs:comment "Provide context for a relationship that occurs in the lifecycle."@en ;
        rdfs:subClassOf ns1:Relationship ;
        sh:nodeKind sh:IRI ;
        sh:property _:Nef0aceefa2a54c08adc29b69c2987c08 .

    ns1:NoAssertionElement a owl:NamedIndividual,
            ns1:IndividualElement ;
        rdfs:comment """An Individual Value for Element representing a set of Elements of unknown
identify or cardinality (number)."""@en ;
        ns1:creationInfo <https://spdx.org/rdf/3.0.1/creationInfo_NoAssertionElement> .

    ns1:NoneElement a owl:NamedIndividual,
            ns1:IndividualElement ;
        rdfs:comment """An Individual Value for Element representing a set of Elements with
cardinality (number/count) of zero."""@en ;
        ns1:creationInfo <https://spdx.org/rdf/3.0.1/creationInfo_NoneElement> .

    ns1:PackageVerificationCode a owl:Class,
            sh:NodeShape ;
        rdfs:comment "An SPDX version 2.X compatible verification method for software packages."@en ;
        rdfs:subClassOf ns1:IntegrityMethod ;
        sh:nodeKind sh:BlankNodeOrIRI ;
        sh:property _:N4fc5b94e528a42f7afe6c41473174094,
            _:N9d2d3f5922e74c2ea3e0b15c523461bb,
            _:Nc8909d7de8dc47cb82651301dd403cf5 .

    ns1:Person a owl:Class ;
        rdfs:comment "An individual human being."@en ;
        rdfs:subClassOf ns1:Agent ;
        sh:nodeKind sh:IRI .

    ns1:SoftwareAgent a owl:Class ;
        rdfs:comment "A software agent."@en ;
        rdfs:subClassOf ns1:Agent ;
        sh:nodeKind sh:IRI .

    ns1:SpdxDocument a owl:Class,
            sh:NodeShape ;
        rdfs:comment "A collection of SPDX Elements that could potentially be serialized."@en ;
        rdfs:subClassOf ns1:ElementCollection ;
        sh:nodeKind sh:IRI ;
        sh:property _:Nae0ececb588e4377a9d54f80ce52155c,
            _:Nd0757799307e48a4b05ca61c03827be6,
            _:Nee0116ffe8b74e748a52829e474a1d0a .

    ns6:DatasetPackage a owl:Class,
            sh:NodeShape ;
        rdfs:comment "Specifies a data package and its associated information."@en ;
        rdfs:subClassOf ns3:Package ;
        sh:nodeKind sh:IRI ;
        sh:property _:N0e42e2b59c914ea49f056fa11e0247af,
            _:N308ac8913c6440c68ef5331eaaef0508,
            _:N4acbfeca863a47f48ea0ccfc2d69b6c6,
            _:N65d68fe531bd4a79bbf148d2cb0e410e,
            _:N6f332b14dad848a1a73af602a8bf6c70,
            _:N7e77bec6ff6048d28db32877de71ab9e,
            _:N89a86d261e23427e9d1f83e49522a1db,
            _:N9ef0c5442da84b0fae93ce92032c52f8,
            _:Nb341386f04fc4f4fbd57a5ececcf95ae,
            _:Nc135d7690cec4e9eacf2c4b3838d3ce0,
            _:Nd22fb99bf3914c40933f3c2889844f93,
            _:Nde0b031cd5a84bd9b7232a8ab9b869b1,
            _:Ne852771926b4432ab9b7910fdcae1056 .

    ns5:ConjunctiveLicenseSet a owl:Class,
            sh:NodeShape ;
        rdfs:comment """Portion of an AnyLicenseInfo representing a set of licensing information
where all elements apply."""@en ;
        rdfs:subClassOf <https://spdx.org/rdf/3.0.1/terms/SimpleLicensing/AnyLicenseInfo> ;
        sh:nodeKind sh:IRI ;
        sh:property _:Na7ae4c31f5884568a3bf48b6f9676216 .

    ns5:CustomLicense a owl:Class ;
        rdfs:comment "A license that is not listed on the SPDX License List."@en ;
        rdfs:subClassOf ns5:License ;
        sh:nodeKind sh:IRI .

    ns5:CustomLicenseAddition a owl:Class ;
        rdfs:comment "A license addition that is not listed on the SPDX Exceptions List."@en ;
        rdfs:subClassOf ns5:LicenseAddition ;
        sh:nodeKind sh:IRI .

    ns5:DisjunctiveLicenseSet a owl:Class,
            sh:NodeShape ;
        rdfs:comment """Portion of an AnyLicenseInfo representing a set of licensing information where
only one of the elements applies."""@en ;
        rdfs:subClassOf <https://spdx.org/rdf/3.0.1/terms/SimpleLicensing/AnyLicenseInfo> ;
        sh:nodeKind sh:IRI ;
        sh:property _:N23238f039f16407faa4dfddc2d622573 .

    ns5:ListedLicense a owl:Class,
            sh:NodeShape ;
        rdfs:comment "A license that is listed on the SPDX License List."@en ;
        rdfs:subClassOf ns5:License ;
        sh:nodeKind sh:IRI ;
        sh:property _:N354ff8b540a0427a97dc3c7fe3fcaba2,
            _:N424a5985e65648579f3f351d5ddcbe9a .

    ns5:ListedLicenseException a owl:Class,
            sh:NodeShape ;
        rdfs:comment "A license exception that is listed on the SPDX Exceptions list."@en ;
        rdfs:subClassOf ns5:LicenseAddition ;
        sh:nodeKind sh:IRI ;
        sh:property _:N2aca376e7fa643248d0ae1615af9bc14,
            _:Nb195befe2d4c41458b75e269d6d5d20d .

    ns5:NoAssertionLicense a owl:NamedIndividual,
            ns5:IndividualLicensingInfo ;
        rdfs:comment """An Individual Value for License when no assertion can be made about its actual
value."""@en ;
        owl:sameAs <https://spdx.org/rdf/3.0.1/terms/Licensing/NoAssertion> ;
        ns1:creationInfo <https://spdx.org/rdf/3.0.1/creationInfo_NoAssertionLicense> .

    ns5:NoneLicense a owl:NamedIndividual,
            ns5:IndividualLicensingInfo ;
        rdfs:comment """An Individual Value for License where the SPDX data creator determines that no
license is present."""@en ;
        owl:sameAs <https://spdx.org/rdf/3.0.1/terms/Licensing/None> ;
        ns1:creationInfo <https://spdx.org/rdf/3.0.1/creationInfo_NoneLicense> .

    ns5:OrLaterOperator a owl:Class,
            sh:NodeShape ;
        rdfs:comment """Portion of an AnyLicenseInfo representing this version, or any later version,
of the indicated License."""@en ;
        rdfs:subClassOf ns5:ExtendableLicense ;
        sh:nodeKind sh:IRI ;
        sh:property _:N9fba27fae73449d2b5c74d5d14893170 .

    ns5:WithAdditionOperator a owl:Class,
            sh:NodeShape ;
        rdfs:comment """Portion of an AnyLicenseInfo representing a License which has additional
text applied to it."""@en ;
        rdfs:subClassOf <https://spdx.org/rdf/3.0.1/terms/SimpleLicensing/AnyLicenseInfo> ;
        sh:nodeKind sh:IRI ;
        sh:property _:N277e37dd63f24c76a29e15a02660e003,
            _:N8801efb6feb44626a0acd767c310b7a5 .

    <https://spdx.org/rdf/3.0.1/terms/Extension/CdxPropertiesExtension> a owl:Class,
            sh:NodeShape ;
        rdfs:comment "A type of extension consisting of a list of name value pairs."@en ;
        rdfs:subClassOf <https://spdx.org/rdf/3.0.1/terms/Extension/Extension> ;
        sh:nodeKind sh:BlankNodeOrIRI ;
        sh:property _:N72245f846f4c4a56aaff12fd8a595f1b .

    ns4:CvssV2VulnAssessmentRelationship a owl:Class,
            sh:NodeShape ;
        rdfs:comment "Provides a CVSS version 2.0 assessment for a vulnerability."@en ;
        rdfs:subClassOf ns4:VulnAssessmentRelationship ;
        sh:nodeKind sh:IRI ;
        sh:property _:N81d1f1b7a8ee4fb8b9c8253b4eb9aac0,
            _:Nd15fc2a0dfc74dfebb9e5275ca4e5990 .

    ns4:CvssV3VulnAssessmentRelationship a owl:Class,
            sh:NodeShape ;
        rdfs:comment "Provides a CVSS version 3 assessment for a vulnerability."@en ;
        rdfs:subClassOf ns4:VulnAssessmentRelationship ;
        sh:nodeKind sh:IRI ;
        sh:property _:N392736ad660c4444b162925f2f85a971,
            _:N655a4f76a80043e59c274b12cb5b98cb,
            _:Nd97fd6bc795a4c92b7847c716752f010 .

    ns4:CvssV4VulnAssessmentRelationship a owl:Class,
            sh:NodeShape ;
        rdfs:comment "Provides a CVSS version 4 assessment for a vulnerability."@en ;
        rdfs:subClassOf ns4:VulnAssessmentRelationship ;
        sh:nodeKind sh:IRI ;
        sh:property _:N54ddca5880464f17bd5206be1ecb8932,
            _:N84436e39e61e449db908a48de410450c,
            _:N9dca46da15a4481796f46a2098859f31 .

    ns4:EpssVulnAssessmentRelationship a owl:Class,
            sh:NodeShape ;
        rdfs:comment "Provides an EPSS assessment for a vulnerability."@en ;
        rdfs:subClassOf ns4:VulnAssessmentRelationship ;
        sh:nodeKind sh:IRI ;
        sh:property _:Nb32bea549ae34bab9c5aef4829b9ee83,
            _:Ndf582cda94a94023a3f5a11a839021c1 .

    ns4:ExploitCatalogVulnAssessmentRelationship a owl:Class,
            sh:NodeShape ;
        rdfs:comment "Provides an exploit assessment of a vulnerability."@en ;
        rdfs:subClassOf ns4:VulnAssessmentRelationship ;
        sh:nodeKind sh:IRI ;
        sh:property _:N642e588df72d4639b95a7dcaf108f295,
            _:N7ada87a7db754bf287181abb5c49bac4,
            _:Na8e8b62a6c9243ecb48de2e3205d6272 .

    ns4:SsvcVulnAssessmentRelationship a owl:Class,
            sh:NodeShape ;
        rdfs:comment "Provides an SSVC assessment for a vulnerability."@en ;
        rdfs:subClassOf ns4:VulnAssessmentRelationship ;
        sh:nodeKind sh:IRI ;
        sh:property _:N4f0b7830361d4b38bff91506e120cb77 .

    ns4:VexAffectedVulnAssessmentRelationship a owl:Class,
            sh:NodeShape ;
        rdfs:comment """Connects a vulnerability and an element designating the element as a product
affected by the vulnerability."""@en ;
        rdfs:subClassOf ns4:VexVulnAssessmentRelationship ;
        sh:nodeKind sh:IRI ;
        sh:property _:N7f3e7e368ced487d87e98dc363b6b5cf,
            _:Nd1687fdd5f6e44d68f2b4f7da570cb9f .

    ns4:VexFixedVulnAssessmentRelationship a owl:Class ;
        rdfs:comment """Links a vulnerability and elements representing products (in the VEX sense) where
a fix has been applied and are no longer affected."""@en ;
        rdfs:subClassOf ns4:VexVulnAssessmentRelationship ;
        sh:nodeKind sh:IRI .

    ns4:VexNotAffectedVulnAssessmentRelationship a owl:Class,
            sh:NodeShape ;
        rdfs:comment """Links a vulnerability and one or more elements designating the latter as products
not affected by the vulnerability."""@en ;
        rdfs:subClassOf ns4:VexVulnAssessmentRelationship ;
        sh:nodeKind sh:IRI ;
        sh:property _:N0d825a0c45ee44bca0cb57c439a3a445,
            _:N45c6754475234fb3981040e1eb691220,
            _:Nc0c5231e0c44437eaef8bba4677a31f6 .

    ns4:VexUnderInvestigationVulnAssessmentRelationship a owl:Class ;
        rdfs:comment """Designates elements as products where the impact of a vulnerability is being
investigated."""@en ;
        rdfs:subClassOf ns4:VexVulnAssessmentRelationship ;
        sh:nodeKind sh:IRI .

    ns4:Vulnerability a owl:Class,
            sh:NodeShape ;
        rdfs:comment "Specifies a vulnerability and its associated information."@en ;
        rdfs:subClassOf ns1:Artifact ;
        sh:nodeKind sh:IRI ;
        sh:property _:N6acc1c288e61445bb0a50d0490a0c267,
            _:Na76c1d0d30514ffb8beb4d48a0b220ff,
            _:Nd66d5f38bdf145a99b1715d40993517c .

    <https://spdx.org/rdf/3.0.1/terms/SimpleLicensing/LicenseExpression> a owl:Class,
            sh:NodeShape ;
        rdfs:comment "An SPDX Element containing an SPDX license expression string."@en ;
        rdfs:subClassOf <https://spdx.org/rdf/3.0.1/terms/SimpleLicensing/AnyLicenseInfo> ;
        sh:nodeKind sh:IRI ;
        sh:property _:N5451d9c16af6442d9bcc23c043b3d0da,
            _:Na8df8b76bfd84e51baaca8c4cdbfaec2,
            _:Nc7843f2d449645178198127dcec9cd3e .

    <https://spdx.org/rdf/3.0.1/terms/SimpleLicensing/SimpleLicensingText> a owl:Class,
            sh:NodeShape ;
        rdfs:comment "A license or addition that is not listed on the SPDX License List."@en ;
        rdfs:subClassOf ns1:Element ;
        sh:nodeKind sh:IRI ;
        sh:property _:N8a001b06f8f846f58ca16289c8bb98e9 .

    ns3:Sbom a owl:Class,
            sh:NodeShape ;
        rdfs:comment "A collection of SPDX Elements describing a single package."@en ;
        rdfs:subClassOf ns1:Bom ;
        sh:nodeKind sh:IRI ;
        sh:property _:N7f4bec2d3c5e42af9f82b5964d720ac9 .

    ns3:Snippet a owl:Class,
            sh:NodeShape ;
        rdfs:comment "Describes a certain part of a file."@en ;
        rdfs:subClassOf ns3:SoftwareArtifact ;
        sh:nodeKind sh:IRI ;
        sh:property _:N49255f1d76a848aa802391a2afe0cbe1,
            _:N580b2e41639f459ca779e7f403e8a1a0,
            _:Nd7add987f24d4d6680bce9a2d944db6a .

    <https://spdx.org/rdf/3.0.1/creationInfo_NoAssertionElement> a ns1:CreationInfo ;
        rdfs:comment "This individual element was defined by the spec."@en ;
        ns1:created "2024-11-22T03:00:01Z"^^xsd:dateTimeStamp ;
        ns1:createdBy ns1:SpdxOrganization ;
        ns1:specVersion "3.0.1" .

    <https://spdx.org/rdf/3.0.1/creationInfo_NoAssertionLicense> a ns1:CreationInfo ;
        rdfs:comment "This individual element was defined by the spec."@en ;
        ns1:created "2024-11-22T03:00:01Z"^^xsd:dateTimeStamp ;
        ns1:createdBy ns1:SpdxOrganization ;
        ns1:specVersion "3.0.1" .

    <https://spdx.org/rdf/3.0.1/creationInfo_NoneElement> a ns1:CreationInfo ;
        rdfs:comment "This individual element was defined by the spec."@en ;
        ns1:created "2024-11-22T03:00:01Z"^^xsd:dateTimeStamp ;
        ns1:createdBy ns1:SpdxOrganization ;
        ns1:specVersion "3.0.1" .

    <https://spdx.org/rdf/3.0.1/creationInfo_NoneLicense> a ns1:CreationInfo ;
        rdfs:comment "This individual element was defined by the spec."@en ;
        ns1:created "2024-11-22T03:00:01Z"^^xsd:dateTimeStamp ;
        ns1:createdBy ns1:SpdxOrganization ;
        ns1:specVersion "3.0.1" .

    <https://spdx.org/rdf/3.0.1/creationInfo_SpdxOrganization> a ns1:CreationInfo ;
        rdfs:comment "This individual element was defined by the spec."@en ;
        ns1:created "2024-11-22T03:00:01Z"^^xsd:dateTimeStamp ;
        ns1:createdBy ns1:SpdxOrganization ;
        ns1:specVersion "3.0.1" .

    spdx: a owl:Ontology ;
        rdfs:label "System Package Data Exchange (SPDX) Ontology"@en ;
        dcterms:abstract "This ontology defines the terms and relationships used in the SPDX specification to describe system packages"@en ;
        dcterms:created "2024-04-05"^^xsd:date ;
        dcterms:creator "SPDX Project"@en ;
        dcterms:license <https://spdx.org/licenses/Community-Spec-1.0.html> ;
        dcterms:references <https://spdx.dev/specifications/> ;
        dcterms:title "System Package Data Exchange (SPDX) Ontology"@en ;
        owl:versionIRI spdx: ;
        omg-ann:copyright "Copyright (C) 2024 SPDX Project"@en .

    <https://spdx.org/rdf/3.0.1/terms/AI/EnergyUnitType/kilowattHour> a owl:NamedIndividual,
            ns2:EnergyUnitType ;
        rdfs:label "kilowattHour" ;
        rdfs:comment "Kilowatt-hour."@en .

    <https://spdx.org/rdf/3.0.1/terms/AI/EnergyUnitType/megajoule> a owl:NamedIndividual,
            ns2:EnergyUnitType ;
        rdfs:label "megajoule" ;
        rdfs:comment "Megajoule."@en .

    <https://spdx.org/rdf/3.0.1/terms/AI/EnergyUnitType/other> a owl:NamedIndividual,
            ns2:EnergyUnitType ;
        rdfs:label "other" ;
        rdfs:comment "Any other units of energy measurement."@en .

    <https://spdx.org/rdf/3.0.1/terms/AI/SafetyRiskAssessmentType/high> a owl:NamedIndividual,
            ns2:SafetyRiskAssessmentType ;
        rdfs:label "high" ;
        rdfs:comment "The second-highest level of risk posed by an AI system."@en .

    <https://spdx.org/rdf/3.0.1/terms/AI/SafetyRiskAssessmentType/low> a owl:NamedIndividual,
            ns2:SafetyRiskAssessmentType ;
        rdfs:label "low" ;
        rdfs:comment "Low/no risk is posed by an AI system."@en .

    <https://spdx.org/rdf/3.0.1/terms/AI/SafetyRiskAssessmentType/medium> a owl:NamedIndividual,
            ns2:SafetyRiskAssessmentType ;
        rdfs:label "medium" ;
        rdfs:comment "The third-highest level of risk posed by an AI system."@en .

    <https://spdx.org/rdf/3.0.1/terms/AI/SafetyRiskAssessmentType/serious> a owl:NamedIndividual,
            ns2:SafetyRiskAssessmentType ;
        rdfs:label "serious" ;
        rdfs:comment "The highest level of risk posed by an AI system."@en .

    ns2:autonomyType a owl:ObjectProperty ;
        rdfs:comment """Indicates whether the system can perform a decision or action without human
involvement or guidance."""@en ;
        rdfs:range ns1:PresenceType .

    ns2:domain a owl:DatatypeProperty ;
        rdfs:comment "Captures the domain in which the AI package can be used."@en ;
        rdfs:range xsd:string .

    ns2:energyConsumption a owl:ObjectProperty ;
        rdfs:comment "Indicates the amount of energy consumption incurred by an AI model."@en ;
        rdfs:range ns2:EnergyConsumption .

    ns2:energyQuantity a owl:DatatypeProperty ;
        rdfs:comment "Represents the energy quantity."@en ;
        rdfs:range xsd:decimal .

    ns2:energyUnit a owl:ObjectProperty ;
        rdfs:comment "Specifies the unit in which energy is measured."@en ;
        rdfs:range ns2:EnergyUnitType .

    ns2:finetuningEnergyConsumption a owl:ObjectProperty ;
        rdfs:comment """Specifies the amount of energy consumed when finetuning the AI model that is
being used in the AI system."""@en ;
        rdfs:range ns2:EnergyConsumptionDescription .

    ns2:hyperparameter a owl:ObjectProperty ;
        rdfs:comment """Records a hyperparameter used to build the AI model contained in the AI
package."""@en ;
        rdfs:range ns1:DictionaryEntry .

    ns2:inferenceEnergyConsumption a owl:ObjectProperty ;
        rdfs:comment """Specifies the amount of energy consumed during inference time by an AI model
that is being used in the AI system."""@en ;
        rdfs:range ns2:EnergyConsumptionDescription .

    ns2:informationAboutApplication a owl:DatatypeProperty ;
        rdfs:comment """Provides relevant information about the AI software, not including the model
description."""@en ;
        rdfs:range xsd:string .

    ns2:informationAboutTraining a owl:DatatypeProperty ;
        rdfs:comment "Describes relevant information about different steps of the training process."@en ;
        rdfs:range xsd:string .

    ns2:limitation a owl:DatatypeProperty ;
        rdfs:comment "Captures a limitation of the AI software."@en ;
        rdfs:range xsd:string .

    ns2:metric a owl:ObjectProperty ;
        rdfs:comment "Records the measurement of prediction quality of the AI model."@en ;
        rdfs:range ns1:DictionaryEntry .

    ns2:metricDecisionThreshold a owl:ObjectProperty ;
        rdfs:comment """Captures the threshold that was used for computation of a metric described in
the metric field."""@en ;
        rdfs:range ns1:DictionaryEntry .

    ns2:modelDataPreprocessing a owl:DatatypeProperty ;
        rdfs:comment """Describes all the preprocessing steps applied to the training data before the
model training."""@en ;
        rdfs:range xsd:string .

    ns2:modelExplainability a owl:DatatypeProperty ;
        rdfs:comment "Describes methods that can be used to explain the results from the AI model."@en ;
        rdfs:range xsd:string .

    ns2:safetyRiskAssessment a owl:ObjectProperty ;
        rdfs:comment "Records the results of general safety risk assessment of the AI system."@en ;
        rdfs:range ns2:SafetyRiskAssessmentType .

    ns2:standardCompliance a owl:DatatypeProperty ;
        rdfs:comment "Captures a standard that is being complied with."@en ;
        rdfs:range xsd:string .

    ns2:trainingEnergyConsumption a owl:ObjectProperty ;
        rdfs:comment """Specifies the amount of energy consumed when training the AI model that is
being used in the AI system."""@en ;
        rdfs:range ns2:EnergyConsumptionDescription .

    ns2:typeOfModel a owl:DatatypeProperty ;
        rdfs:comment "Records the type of the model used in the AI software."@en ;
        rdfs:range xsd:string .

    ns2:useSensitivePersonalInformation a owl:ObjectProperty ;
        rdfs:comment """Records if sensitive personal information is used during model training or
could be used during the inference."""@en ;
        rdfs:range ns1:PresenceType .

    <https://spdx.org/rdf/3.0.1/terms/Build/buildEndTime> a owl:DatatypeProperty ;
        rdfs:comment "Property that describes the time at which a build stops."@en ;
        rdfs:range xsd:dateTimeStamp .

    <https://spdx.org/rdf/3.0.1/terms/Build/buildId> a owl:DatatypeProperty ;
        rdfs:comment """A buildId is a locally unique identifier used by a builder to identify a unique
instance of a build produced by it."""@en ;
        rdfs:range xsd:string .

    <https://spdx.org/rdf/3.0.1/terms/Build/buildStartTime> a owl:DatatypeProperty ;
        rdfs:comment "Property describing the start time of a build."@en ;
        rdfs:range xsd:dateTimeStamp .

    <https://spdx.org/rdf/3.0.1/terms/Build/buildType> a owl:DatatypeProperty ;
        rdfs:comment """A buildType is a hint that is used to indicate the toolchain, platform, or
infrastructure that the build was invoked on."""@en ;
        rdfs:range xsd:anyURI .

    <https://spdx.org/rdf/3.0.1/terms/Build/configSourceDigest> a owl:ObjectProperty ;
        rdfs:comment """Property that describes the digest of the build configuration file used to
invoke a build."""@en ;
        rdfs:range ns1:Hash .

    <https://spdx.org/rdf/3.0.1/terms/Build/configSourceEntrypoint> a owl:DatatypeProperty ;
        rdfs:comment "Property describes the invocation entrypoint of a build."@en ;
        rdfs:range xsd:string .

    <https://spdx.org/rdf/3.0.1/terms/Build/configSourceUri> a owl:DatatypeProperty ;
        rdfs:comment "Property that describes the URI of the build configuration source file."@en ;
        rdfs:range xsd:anyURI .

    <https://spdx.org/rdf/3.0.1/terms/Build/environment> a owl:ObjectProperty ;
        rdfs:comment "Property describing the session in which a build is invoked."@en ;
        rdfs:range ns1:DictionaryEntry .

    <https://spdx.org/rdf/3.0.1/terms/Build/parameter> a owl:ObjectProperty ;
        rdfs:comment "Property describing a parameter used in an instance of a build."@en ;
        rdfs:range ns1:DictionaryEntry .

    <https://spdx.org/rdf/3.0.1/terms/Core/AnnotationType/other> a owl:NamedIndividual,
            ns1:AnnotationType ;
        rdfs:label "other" ;
        rdfs:comment "Used to store extra information about an Element which is not part of a review (e.g. extra information provided during the creation of the Element)."@en .

    <https://spdx.org/rdf/3.0.1/terms/Core/AnnotationType/review> a owl:NamedIndividual,
            ns1:AnnotationType ;
        rdfs:label "review" ;
        rdfs:comment "Used when someone reviews the Element."@en .

    ns1:Bom a owl:Class ;
        rdfs:comment """A container for a grouping of SPDX-3.0 content characterizing details
(provenence, composition, licensing, etc.) about a product."""@en ;
        rdfs:subClassOf ns1:Bundle ;
        sh:nodeKind sh:IRI .

    ns1:Bundle a owl:Class,
            sh:NodeShape ;
        rdfs:comment "A collection of Elements that have a shared context."@en ;
        rdfs:subClassOf ns1:ElementCollection ;
        sh:nodeKind sh:IRI ;
        sh:property _:N9fbdc56679684b249b8cc7d20288fa52 .

    <https://spdx.org/rdf/3.0.1/terms/Core/ExternalIdentifierType/cpe22> a owl:NamedIndividual,
            ns1:ExternalIdentifierType ;
        rdfs:label "cpe22" ;
        rdfs:comment "[Common Platform Enumeration Specification 2.2](https://cpe.mitre.org/files/cpe-specification_2.2.pdf)"@en .

    <https://spdx.org/rdf/3.0.1/terms/Core/ExternalIdentifierType/cpe23> a owl:NamedIndividual,
            ns1:ExternalIdentifierType ;
        rdfs:label "cpe23" ;
        rdfs:comment "[Common Platform Enumeration: Naming Specification Version 2.3](https://csrc.nist.gov/publications/detail/nistir/7695/final)"@en .

    <https://spdx.org/rdf/3.0.1/terms/Core/ExternalIdentifierType/cve> a owl:NamedIndividual,
            ns1:ExternalIdentifierType ;
        rdfs:label "cve" ;
        rdfs:comment "Common Vulnerabilities and Exposures identifiers, an identifier for a specific software flaw defined within the official CVE Dictionary and that conforms to the [CVE specification](https://csrc.nist.gov/glossary/term/cve_id)."@en .

    <https://spdx.org/rdf/3.0.1/terms/Core/ExternalIdentifierType/email> a owl:NamedIndividual,
            ns1:ExternalIdentifierType ;
        rdfs:label "email" ;
        rdfs:comment "Email address, as defined in [RFC 3696](https://datatracker.ietf.org/doc/rfc3986/) Section 3."@en .

    <https://spdx.org/rdf/3.0.1/terms/Core/ExternalIdentifierType/gitoid> a owl:NamedIndividual,
            ns1:ExternalIdentifierType ;
        rdfs:label "gitoid" ;
        rdfs:comment "[Gitoid](https://www.iana.org/assignments/uri-schemes/prov/gitoid), stands for [Git Object ID](https://git-scm.com/book/en/v2/Git-Internals-Git-Objects). A gitoid of type blob is a unique hash of a binary artifact. A gitoid may represent either an [Artifact Identifier](https://github.com/omnibor/spec/blob/eb1ee5c961c16215eb8709b2975d193a2007a35d/spec/SPEC.md#artifact-identifier-types) for the software artifact or an [Input Manifest Identifier](https://github.com/omnibor/spec/blob/eb1ee5c961c16215eb8709b2975d193a2007a35d/spec/SPEC.md#input-manifest-identifier) for the software artifact's associated [Artifact Input Manifest](https://github.com/omnibor/spec/blob/eb1ee5c961c16215eb8709b2975d193a2007a35d/spec/SPEC.md#artifact-input-manifest); this ambiguity exists because the Artifact Input Manifest is itself an artifact, and the gitoid of that artifact is its valid identifier. Gitoids calculated on software artifacts (Snippet, File, or Package Elements) should be recorded in the SPDX 3.0 SoftwareArtifact's contentIdentifier property. Gitoids calculated on the Artifact Input Manifest (Input Manifest Identifier) should be recorded in the SPDX 3.0 Element's externalIdentifier property. See [OmniBOR Specification](https://github.com/omnibor/spec/), a minimalistic specification for describing software [Artifact Dependency Graphs](https://github.com/omnibor/spec/blob/eb1ee5c961c16215eb8709b2975d193a2007a35d/spec/SPEC.md#artifact-dependency-graph-adg)."@en .

    <https://spdx.org/rdf/3.0.1/terms/Core/ExternalIdentifierType/other> a owl:NamedIndividual,
            ns1:ExternalIdentifierType ;
        rdfs:label "other" ;
        rdfs:comment "Used when the type does not match any of the other options."@en .

    <https://spdx.org/rdf/3.0.1/terms/Core/ExternalIdentifierType/packageUrl> a owl:NamedIndividual,
            ns1:ExternalIdentifierType ;
        rdfs:label "packageUrl" ;
        rdfs:comment "Package URL, as defined in the corresponding [Annex](../../../annexes/pkg-url-specification.md) of this specification."@en .

    <https://spdx.org/rdf/3.0.1/terms/Core/ExternalIdentifierType/securityOther> a owl:NamedIndividual,
            ns1:ExternalIdentifierType ;
        rdfs:label "securityOther" ;
        rdfs:comment "Used when there is a security related identifier of unspecified type."@en .

    <https://spdx.org/rdf/3.0.1/terms/Core/ExternalIdentifierType/swhid> a owl:NamedIndividual,
            ns1:ExternalIdentifierType ;
        rdfs:label "swhid" ;
        rdfs:comment "SoftWare Hash IDentifier, a persistent intrinsic identifier for digital artifacts, such as files, trees (also known as directories or folders), commits, and other objects typically found in version control systems. The format of the identifiers is defined in the [SWHID specification](https://www.swhid.org/specification/v1.1/4.Syntax) (ISO/IEC DIS 18670). They typically look like `swh:1:cnt:94a9ed024d3859793618152ea559a168bbcbb5e2`."@en .

    <https://spdx.org/rdf/3.0.1/terms/Core/ExternalIdentifierType/swid> a owl:NamedIndividual,
            ns1:ExternalIdentifierType ;
        rdfs:label "swid" ;
        rdfs:comment "Concise Software Identification (CoSWID) tag, as defined in [RFC 9393](https://datatracker.ietf.org/doc/rfc9393/) Section 2.3."@en .

    <https://spdx.org/rdf/3.0.1/terms/Core/ExternalIdentifierType/urlScheme> a owl:NamedIndividual,
            ns1:ExternalIdentifierType ;
        rdfs:label "urlScheme" ;
        rdfs:comment "[Uniform Resource Identifier (URI) Schemes](https://www.iana.org/assignments/uri-schemes/uri-schemes.xhtml). The scheme used in order to locate a resource."@en .

    <https://spdx.org/rdf/3.0.1/terms/Core/ExternalRefType/altDownloadLocation> a owl:NamedIndividual,
            ns1:ExternalRefType ;
        rdfs:label "altDownloadLocation" ;
        rdfs:comment "A reference to an alternative download location."@en .

    <https://spdx.org/rdf/3.0.1/terms/Core/ExternalRefType/altWebPage> a owl:NamedIndividual,
            ns1:ExternalRefType ;
        rdfs:label "altWebPage" ;
        rdfs:comment "A reference to an alternative web page."@en .

    <https://spdx.org/rdf/3.0.1/terms/Core/ExternalRefType/binaryArtifact> a owl:NamedIndividual,
            ns1:ExternalRefType ;
        rdfs:label "binaryArtifact" ;
        rdfs:comment "A reference to binary artifacts related to a package."@en .

    <https://spdx.org/rdf/3.0.1/terms/Core/ExternalRefType/bower> a owl:NamedIndividual,
            ns1:ExternalRefType ;
        rdfs:label "bower" ;
        rdfs:comment "A reference to a Bower package. The package locator format, looks like `package#version`, is defined in the \"install\" section of [Bower API documentation](https://bower.io/docs/api/#install)."@en .

    <https://spdx.org/rdf/3.0.1/terms/Core/ExternalRefType/buildMeta> a owl:NamedIndividual,
            ns1:ExternalRefType ;
        rdfs:label "buildMeta" ;
        rdfs:comment "A reference build metadata related to a published package."@en .

    <https://spdx.org/rdf/3.0.1/terms/Core/ExternalRefType/buildSystem> a owl:NamedIndividual,
            ns1:ExternalRefType ;
        rdfs:label "buildSystem" ;
        rdfs:comment "A reference build system used to create or publish the package."@en .

    <https://spdx.org/rdf/3.0.1/terms/Core/ExternalRefType/certificationReport> a owl:NamedIndividual,
            ns1:ExternalRefType ;
        rdfs:label "certificationReport" ;
        rdfs:comment "A reference to a certification report for a package from an accredited/independent body."@en .

    <https://spdx.org/rdf/3.0.1/terms/Core/ExternalRefType/chat> a owl:NamedIndividual,
            ns1:ExternalRefType ;
        rdfs:label "chat" ;
        rdfs:comment "A reference to the instant messaging system used by the maintainer for a package."@en .

    <https://spdx.org/rdf/3.0.1/terms/Core/ExternalRefType/componentAnalysisReport> a owl:NamedIndividual,
            ns1:ExternalRefType ;
        rdfs:label "componentAnalysisReport" ;
        rdfs:comment "A reference to a Software Composition Analysis (SCA) report."@en .

    <https://spdx.org/rdf/3.0.1/terms/Core/ExternalRefType/cwe> a owl:NamedIndividual,
            ns1:ExternalRefType ;
        rdfs:label "cwe" ;
        rdfs:comment "[Common Weakness Enumeration](https://csrc.nist.gov/glossary/term/common_weakness_enumeration). A reference to a source of software flaw defined within the official [CWE List](https://cwe.mitre.org/data/) that conforms to the [CWE specification](https://cwe.mitre.org/)."@en .

    <https://spdx.org/rdf/3.0.1/terms/Core/ExternalRefType/documentation> a owl:NamedIndividual,
            ns1:ExternalRefType ;
        rdfs:label "documentation" ;
        rdfs:comment "A reference to the documentation for a package."@en .

    <https://spdx.org/rdf/3.0.1/terms/Core/ExternalRefType/dynamicAnalysisReport> a owl:NamedIndividual,
            ns1:ExternalRefType ;
        rdfs:label "dynamicAnalysisReport" ;
        rdfs:comment "A reference to a dynamic analysis report for a package."@en .

    <https://spdx.org/rdf/3.0.1/terms/Core/ExternalRefType/eolNotice> a owl:NamedIndividual,
            ns1:ExternalRefType ;
        rdfs:label "eolNotice" ;
        rdfs:comment "A reference to the End Of Sale (EOS) and/or End Of Life (EOL) information related to a package."@en .

    <https://spdx.org/rdf/3.0.1/terms/Core/ExternalRefType/exportControlAssessment> a owl:NamedIndividual,
            ns1:ExternalRefType ;
        rdfs:label "exportControlAssessment" ;
        rdfs:comment "A reference to a export control assessment for a package."@en .

    <https://spdx.org/rdf/3.0.1/terms/Core/ExternalRefType/funding> a owl:NamedIndividual,
            ns1:ExternalRefType ;
        rdfs:label "funding" ;
        rdfs:comment "A reference to funding information related to a package."@en .

    <https://spdx.org/rdf/3.0.1/terms/Core/ExternalRefType/issueTracker> a owl:NamedIndividual,
            ns1:ExternalRefType ;
        rdfs:label "issueTracker" ;
        rdfs:comment "A reference to the issue tracker for a package."@en .

    <https://spdx.org/rdf/3.0.1/terms/Core/ExternalRefType/license> a owl:NamedIndividual,
            ns1:ExternalRefType ;
        rdfs:label "license" ;
        rdfs:comment "A reference to additional license information related to an artifact."@en .

    <https://spdx.org/rdf/3.0.1/terms/Core/ExternalRefType/mailingList> a owl:NamedIndividual,
            ns1:ExternalRefType ;
        rdfs:label "mailingList" ;
        rdfs:comment "A reference to the mailing list used by the maintainer for a package."@en .

    <https://spdx.org/rdf/3.0.1/terms/Core/ExternalRefType/mavenCentral> a owl:NamedIndividual,
            ns1:ExternalRefType ;
        rdfs:label "mavenCentral" ;
        rdfs:comment "A reference to a Maven repository artifact. The artifact locator format is defined in the [Maven documentation](https://maven.apache.org/guides/mini/guide-naming-conventions.html) and looks like `groupId:artifactId[:version]`."@en .

    <https://spdx.org/rdf/3.0.1/terms/Core/ExternalRefType/metrics> a owl:NamedIndividual,
            ns1:ExternalRefType ;
        rdfs:label "metrics" ;
        rdfs:comment "A reference to metrics related to package such as OpenSSF scorecards."@en .

    <https://spdx.org/rdf/3.0.1/terms/Core/ExternalRefType/npm> a owl:NamedIndividual,
            ns1:ExternalRefType ;
        rdfs:label "npm" ;
        rdfs:comment "A reference to an npm package. The package locator format is defined in the [npm documentation](https://docs.npmjs.com/cli/v10/configuring-npm/package-json) and looks like `package@version`."@en .

    <https://spdx.org/rdf/3.0.1/terms/Core/ExternalRefType/nuget> a owl:NamedIndividual,
            ns1:ExternalRefType ;
        rdfs:label "nuget" ;
        rdfs:comment "A reference to a NuGet package. The package locator format is defined in the [NuGet documentation](https://docs.nuget.org) and looks like `package/version`."@en .

    <https://spdx.org/rdf/3.0.1/terms/Core/ExternalRefType/other> a owl:NamedIndividual,
            ns1:ExternalRefType ;
        rdfs:label "other" ;
        rdfs:comment "Used when the type does not match any of the other options."@en .

    <https://spdx.org/rdf/3.0.1/terms/Core/ExternalRefType/privacyAssessment> a owl:NamedIndividual,
            ns1:ExternalRefType ;
        rdfs:label "privacyAssessment" ;
        rdfs:comment "A reference to a privacy assessment for a package."@en .

    <https://spdx.org/rdf/3.0.1/terms/Core/ExternalRefType/productMetadata> a owl:NamedIndividual,
            ns1:ExternalRefType ;
        rdfs:label "productMetadata" ;
        rdfs:comment "A reference to additional product metadata such as reference within organization's product catalog."@en .

    <https://spdx.org/rdf/3.0.1/terms/Core/ExternalRefType/purchaseOrder> a owl:NamedIndividual,
            ns1:ExternalRefType ;
        rdfs:label "purchaseOrder" ;
        rdfs:comment "A reference to a purchase order for a package."@en .

    <https://spdx.org/rdf/3.0.1/terms/Core/ExternalRefType/qualityAssessmentReport> a owl:NamedIndividual,
            ns1:ExternalRefType ;
        rdfs:label "qualityAssessmentReport" ;
        rdfs:comment "A reference to a quality assessment for a package."@en .

    <https://spdx.org/rdf/3.0.1/terms/Core/ExternalRefType/releaseHistory> a owl:NamedIndividual,
            ns1:ExternalRefType ;
        rdfs:label "releaseHistory" ;
        rdfs:comment "A reference to a published list of releases for a package."@en .

    <https://spdx.org/rdf/3.0.1/terms/Core/ExternalRefType/releaseNotes> a owl:NamedIndividual,
            ns1:ExternalRefType ;
        rdfs:label "releaseNotes" ;
        rdfs:comment "A reference to the release notes for a package."@en .

    <https://spdx.org/rdf/3.0.1/terms/Core/ExternalRefType/riskAssessment> a owl:NamedIndividual,
            ns1:ExternalRefType ;
        rdfs:label "riskAssessment" ;
        rdfs:comment "A reference to a risk assessment for a package."@en .

    <https://spdx.org/rdf/3.0.1/terms/Core/ExternalRefType/runtimeAnalysisReport> a owl:NamedIndividual,
            ns1:ExternalRefType ;
        rdfs:label "runtimeAnalysisReport" ;
        rdfs:comment "A reference to a runtime analysis report for a package."@en .

    <https://spdx.org/rdf/3.0.1/terms/Core/ExternalRefType/secureSoftwareAttestation> a owl:NamedIndividual,
            ns1:ExternalRefType ;
        rdfs:label "secureSoftwareAttestation" ;
        rdfs:comment "A reference to information assuring that the software is developed using security practices as defined by [NIST SP 800-218 Secure Software Development Framework (SSDF) Version 1.1](https://csrc.nist.gov/pubs/sp/800/218/final) or [CISA Secure Software Development Attestation Form](https://www.cisa.gov/resources-tools/resources/secure-software-development-attestation-form)."@en .

    <https://spdx.org/rdf/3.0.1/terms/Core/ExternalRefType/securityAdversaryModel> a owl:NamedIndividual,
            ns1:ExternalRefType ;
        rdfs:label "securityAdversaryModel" ;
        rdfs:comment "A reference to the security adversary model for a package."@en .

    <https://spdx.org/rdf/3.0.1/terms/Core/ExternalRefType/securityAdvisory> a owl:NamedIndividual,
            ns1:ExternalRefType ;
        rdfs:label "securityAdvisory" ;
        rdfs:comment "A reference to a published security advisory (where advisory as defined per [ISO 29147:2018](https://www.iso.org/standard/72311.html)) that may affect one or more elements, e.g., vendor advisories or specific NVD entries."@en .

    <https://spdx.org/rdf/3.0.1/terms/Core/ExternalRefType/securityFix> a owl:NamedIndividual,
            ns1:ExternalRefType ;
        rdfs:label "securityFix" ;
        rdfs:comment "A reference to the patch or source code that fixes a vulnerability."@en .

    <https://spdx.org/rdf/3.0.1/terms/Core/ExternalRefType/securityOther> a owl:NamedIndividual,
            ns1:ExternalRefType ;
        rdfs:label "securityOther" ;
        rdfs:comment "A reference to related security information of unspecified type."@en .

    <https://spdx.org/rdf/3.0.1/terms/Core/ExternalRefType/securityPenTestReport> a owl:NamedIndividual,
            ns1:ExternalRefType ;
        rdfs:label "securityPenTestReport" ;
        rdfs:comment "A reference to a [penetration test](https://en.wikipedia.org/wiki/Penetration_test) report for a package."@en .

    <https://spdx.org/rdf/3.0.1/terms/Core/ExternalRefType/securityPolicy> a owl:NamedIndividual,
            ns1:ExternalRefType ;
        rdfs:label "securityPolicy" ;
        rdfs:comment "A reference to instructions for reporting newly discovered security vulnerabilities for a package."@en .

    <https://spdx.org/rdf/3.0.1/terms/Core/ExternalRefType/securityThreatModel> a owl:NamedIndividual,
            ns1:ExternalRefType ;
        rdfs:label "securityThreatModel" ;
        rdfs:comment "A reference the [security threat model](https://en.wikipedia.org/wiki/Threat_model) for a package."@en .

    <https://spdx.org/rdf/3.0.1/terms/Core/ExternalRefType/socialMedia> a owl:NamedIndividual,
            ns1:ExternalRefType ;
        rdfs:label "socialMedia" ;
        rdfs:comment "A reference to a social media channel for a package."@en .

    <https://spdx.org/rdf/3.0.1/terms/Core/ExternalRefType/sourceArtifact> a owl:NamedIndividual,
            ns1:ExternalRefType ;
        rdfs:label "sourceArtifact" ;
        rdfs:comment "A reference to an artifact containing the sources for a package."@en .

    <https://spdx.org/rdf/3.0.1/terms/Core/ExternalRefType/staticAnalysisReport> a owl:NamedIndividual,
            ns1:ExternalRefType ;
        rdfs:label "staticAnalysisReport" ;
        rdfs:comment "A reference to a static analysis report for a package."@en .

    <https://spdx.org/rdf/3.0.1/terms/Core/ExternalRefType/support> a owl:NamedIndividual,
            ns1:ExternalRefType ;
        rdfs:label "support" ;
        rdfs:comment "A reference to the software support channel or other support information for a package."@en .

    <https://spdx.org/rdf/3.0.1/terms/Core/ExternalRefType/vcs> a owl:NamedIndividual,
            ns1:ExternalRefType ;
        rdfs:label "vcs" ;
        rdfs:comment "A reference to a version control system related to a software artifact."@en .

    <https://spdx.org/rdf/3.0.1/terms/Core/ExternalRefType/vulnerabilityDisclosureReport> a owl:NamedIndividual,
            ns1:ExternalRefType ;
        rdfs:label "vulnerabilityDisclosureReport" ;
        rdfs:comment "A reference to a Vulnerability Disclosure Report (VDR) which provides the software supplier's analysis and findings describing the impact (or lack of impact) that reported vulnerabilities have on packages or products in the supplier's SBOM as defined in [NIST SP 800-161 Cybersecurity Supply Chain Risk Management Practices for Systems and Organizations](https://csrc.nist.gov/pubs/sp/800/161/r1/final)."@en .

    <https://spdx.org/rdf/3.0.1/terms/Core/ExternalRefType/vulnerabilityExploitabilityAssessment> a owl:NamedIndividual,
            ns1:ExternalRefType ;
        rdfs:label "vulnerabilityExploitabilityAssessment" ;
        rdfs:comment "A reference to a Vulnerability Exploitability eXchange (VEX) statement which provides information on whether a product is impacted by a specific vulnerability in an included package and, if affected, whether there are actions recommended to remediate. See also [NTIA VEX one-page summary](https://ntia.gov/files/ntia/publications/vex_one-page_summary.pdf)."@en .

    <https://spdx.org/rdf/3.0.1/terms/Core/LifecycleScopeType/build> a owl:NamedIndividual,
            ns1:LifecycleScopeType ;
        rdfs:label "build" ;
        rdfs:comment "A relationship has specific context implications during an element's build phase, during development."@en .

    <https://spdx.org/rdf/3.0.1/terms/Core/LifecycleScopeType/design> a owl:NamedIndividual,
            ns1:LifecycleScopeType ;
        rdfs:label "design" ;
        rdfs:comment "A relationship has specific context implications during an element's design."@en .

    <https://spdx.org/rdf/3.0.1/terms/Core/LifecycleScopeType/development> a owl:NamedIndividual,
            ns1:LifecycleScopeType ;
        rdfs:label "development" ;
        rdfs:comment "A relationship has specific context implications during development phase of an element."@en .

    <https://spdx.org/rdf/3.0.1/terms/Core/LifecycleScopeType/other> a owl:NamedIndividual,
            ns1:LifecycleScopeType ;
        rdfs:label "other" ;
        rdfs:comment "A relationship has other specific context information necessary to capture that the above set of enumerations does not handle."@en .

    <https://spdx.org/rdf/3.0.1/terms/Core/LifecycleScopeType/runtime> a owl:NamedIndividual,
            ns1:LifecycleScopeType ;
        rdfs:label "runtime" ;
        rdfs:comment "A relationship has specific context implications during the execution phase of an element."@en .

    <https://spdx.org/rdf/3.0.1/terms/Core/LifecycleScopeType/test> a owl:NamedIndividual,
            ns1:LifecycleScopeType ;
        rdfs:label "test" ;
        rdfs:comment "A relationship has specific context implications during an element's testing phase, during development."@en .

    ns1:Organization a owl:Class ;
        rdfs:comment "A group of people who work together in an organized way for a shared purpose."@en ;
        rdfs:subClassOf ns1:Agent ;
        sh:nodeKind sh:IRI .

    <https://spdx.org/rdf/3.0.1/terms/Core/ProfileIdentifierType/ai> a owl:NamedIndividual,
            ns1:ProfileIdentifierType ;
        rdfs:label "ai" ;
        rdfs:comment "the element follows the AI profile specification"@en .

    <https://spdx.org/rdf/3.0.1/terms/Core/ProfileIdentifierType/build> a owl:NamedIndividual,
            ns1:ProfileIdentifierType ;
        rdfs:label "build" ;
        rdfs:comment "the element follows the Build profile specification"@en .

    <https://spdx.org/rdf/3.0.1/terms/Core/ProfileIdentifierType/core> a owl:NamedIndividual,
            ns1:ProfileIdentifierType ;
        rdfs:label "core" ;
        rdfs:comment "the element follows the Core profile specification"@en .

    <https://spdx.org/rdf/3.0.1/terms/Core/ProfileIdentifierType/dataset> a owl:NamedIndividual,
            ns1:ProfileIdentifierType ;
        rdfs:label "dataset" ;
        rdfs:comment "the element follows the Dataset profile specification"@en .

    <https://spdx.org/rdf/3.0.1/terms/Core/ProfileIdentifierType/expandedLicensing> a owl:NamedIndividual,
            ns1:ProfileIdentifierType ;
        rdfs:label "expandedLicensing" ;
        rdfs:comment "the element follows the ExpandedLicensing profile specification"@en .

    <https://spdx.org/rdf/3.0.1/terms/Core/ProfileIdentifierType/extension> a owl:NamedIndividual,
            ns1:ProfileIdentifierType ;
        rdfs:label "extension" ;
        rdfs:comment "the element follows the Extension profile specification"@en .

    <https://spdx.org/rdf/3.0.1/terms/Core/ProfileIdentifierType/lite> a owl:NamedIndividual,
            ns1:ProfileIdentifierType ;
        rdfs:label "lite" ;
        rdfs:comment "the element follows the Lite profile specification"@en .

    <https://spdx.org/rdf/3.0.1/terms/Core/ProfileIdentifierType/security> a owl:NamedIndividual,
            ns1:ProfileIdentifierType ;
        rdfs:label "security" ;
        rdfs:comment "the element follows the Security profile specification"@en .

    <https://spdx.org/rdf/3.0.1/terms/Core/ProfileIdentifierType/simpleLicensing> a owl:NamedIndividual,
            ns1:ProfileIdentifierType ;
        rdfs:label "simpleLicensing" ;
        rdfs:comment "the element follows the SimpleLicensing profile specification"@en .

    <https://spdx.org/rdf/3.0.1/terms/Core/ProfileIdentifierType/software> a owl:NamedIndividual,
            ns1:ProfileIdentifierType ;
        rdfs:label "software" ;
        rdfs:comment "the element follows the Software profile specification"@en .

    <https://spdx.org/rdf/3.0.1/terms/Core/RelationshipCompleteness/complete> a owl:NamedIndividual,
            ns1:RelationshipCompleteness ;
        rdfs:label "complete" ;
        rdfs:comment "The relationship is known to be exhaustive."@en .

    <https://spdx.org/rdf/3.0.1/terms/Core/RelationshipCompleteness/incomplete> a owl:NamedIndividual,
            ns1:RelationshipCompleteness ;
        rdfs:label "incomplete" ;
        rdfs:comment "The relationship is known not to be exhaustive."@en .

    <https://spdx.org/rdf/3.0.1/terms/Core/RelationshipCompleteness/noAssertion> a owl:NamedIndividual,
            ns1:RelationshipCompleteness ;
        rdfs:label "noAssertion" ;
        rdfs:comment "No assertion can be made about the completeness of the relationship."@en .

    <https://spdx.org/rdf/3.0.1/terms/Core/RelationshipType/affects> a owl:NamedIndividual,
            ns1:RelationshipType ;
        rdfs:label "affects" ;
        rdfs:comment "The `from` Vulnerability affects each `to` Element. The use of the `affects` type is constrained to `VexAffectedVulnAssessmentRelationship` classed relationships."@en .

    <https://spdx.org/rdf/3.0.1/terms/Core/RelationshipType/amendedBy> a owl:NamedIndividual,
            ns1:RelationshipType ;
        rdfs:label "amendedBy" ;
        rdfs:comment "The `from` Element is amended by each `to` Element."@en .

    <https://spdx.org/rdf/3.0.1/terms/Core/RelationshipType/ancestorOf> a owl:NamedIndividual,
            ns1:RelationshipType ;
        rdfs:label "ancestorOf" ;
        rdfs:comment "The `from` Element is an ancestor of each `to` Element."@en .

    <https://spdx.org/rdf/3.0.1/terms/Core/RelationshipType/availableFrom> a owl:NamedIndividual,
            ns1:RelationshipType ;
        rdfs:label "availableFrom" ;
        rdfs:comment "The `from` Element is available from the additional supplier described by each `to` Element."@en .

    <https://spdx.org/rdf/3.0.1/terms/Core/RelationshipType/configures> a owl:NamedIndividual,
            ns1:RelationshipType ;
        rdfs:label "configures" ;
        rdfs:comment "The `from` Element is a configuration applied to each `to` Element, during a LifecycleScopeType period."@en .

    <https://spdx.org/rdf/3.0.1/terms/Core/RelationshipType/contains> a owl:NamedIndividual,
            ns1:RelationshipType ;
        rdfs:label "contains" ;
        rdfs:comment "The `from` Element contains each `to` Element."@en .

    <https://spdx.org/rdf/3.0.1/terms/Core/RelationshipType/coordinatedBy> a owl:NamedIndividual,
            ns1:RelationshipType ;
        rdfs:label "coordinatedBy" ;
        rdfs:comment "The `from` Vulnerability is coordinatedBy the `to` Agent(s) (vendor, researcher, or consumer agent)."@en .

    <https://spdx.org/rdf/3.0.1/terms/Core/RelationshipType/copiedTo> a owl:NamedIndividual,
            ns1:RelationshipType ;
        rdfs:label "copiedTo" ;
        rdfs:comment "The `from` Element has been copied to each `to` Element."@en .

    <https://spdx.org/rdf/3.0.1/terms/Core/RelationshipType/delegatedTo> a owl:NamedIndividual,
            ns1:RelationshipType ;
        rdfs:label "delegatedTo" ;
        rdfs:comment "The `from` Agent is delegating an action to the Agent of the `to` Relationship (which must be of type invokedBy), during a LifecycleScopeType (e.g. the `to` invokedBy Relationship is being done on behalf of `from`)."@en .

    <https://spdx.org/rdf/3.0.1/terms/Core/RelationshipType/dependsOn> a owl:NamedIndividual,
            ns1:RelationshipType ;
        rdfs:label "dependsOn" ;
        rdfs:comment "The `from` Element depends on each `to` Element, during a LifecycleScopeType period."@en .

    <https://spdx.org/rdf/3.0.1/terms/Core/RelationshipType/descendantOf> a owl:NamedIndividual,
            ns1:RelationshipType ;
        rdfs:label "descendantOf" ;
        rdfs:comment "The `from` Element is a descendant of each `to` Element."@en .

    <https://spdx.org/rdf/3.0.1/terms/Core/RelationshipType/describes> a owl:NamedIndividual,
            ns1:RelationshipType ;
        rdfs:label "describes" ;
        rdfs:comment "The `from` Element describes each `to` Element. To denote the root(s) of a tree of elements in a collection, the rootElement property should be used."@en .

    <https://spdx.org/rdf/3.0.1/terms/Core/RelationshipType/doesNotAffect> a owl:NamedIndividual,
            ns1:RelationshipType ;
        rdfs:label "doesNotAffect" ;
        rdfs:comment "The `from` Vulnerability has no impact on each `to` Element. The use of the `doesNotAffect` is constrained to `VexNotAffectedVulnAssessmentRelationship` classed relationships."@en .

    <https://spdx.org/rdf/3.0.1/terms/Core/RelationshipType/expandsTo> a owl:NamedIndividual,
            ns1:RelationshipType ;
        rdfs:label "expandsTo" ;
        rdfs:comment "The `from` archive expands out as an artifact described by each `to` Element."@en .

    <https://spdx.org/rdf/3.0.1/terms/Core/RelationshipType/exploitCreatedBy> a owl:NamedIndividual,
            ns1:RelationshipType ;
        rdfs:label "exploitCreatedBy" ;
        rdfs:comment "The `from` Vulnerability has had an exploit created against it by each `to` Agent."@en .

    <https://spdx.org/rdf/3.0.1/terms/Core/RelationshipType/fixedBy> a owl:NamedIndividual,
            ns1:RelationshipType ;
        rdfs:label "fixedBy" ;
        rdfs:comment "Designates a `from` Vulnerability has been fixed by the `to` Agent(s)."@en .

    <https://spdx.org/rdf/3.0.1/terms/Core/RelationshipType/fixedIn> a owl:NamedIndividual,
            ns1:RelationshipType ;
        rdfs:label "fixedIn" ;
        rdfs:comment "A `from` Vulnerability has been fixed in each `to` Element. The use of the `fixedIn` type is constrained to `VexFixedVulnAssessmentRelationship` classed relationships."@en .

    <https://spdx.org/rdf/3.0.1/terms/Core/RelationshipType/foundBy> a owl:NamedIndividual,
            ns1:RelationshipType ;
        rdfs:label "foundBy" ;
        rdfs:comment "Designates a `from` Vulnerability was originally discovered by the `to` Agent(s)."@en .

    <https://spdx.org/rdf/3.0.1/terms/Core/RelationshipType/generates> a owl:NamedIndividual,
            ns1:RelationshipType ;
        rdfs:label "generates" ;
        rdfs:comment "The `from` Element generates each `to` Element."@en .

    <https://spdx.org/rdf/3.0.1/terms/Core/RelationshipType/hasAddedFile> a owl:NamedIndividual,
            ns1:RelationshipType ;
        rdfs:label "hasAddedFile" ;
        rdfs:comment "Every `to` Element is a file added to the `from` Element (`from` hasAddedFile `to`)."@en .

    <https://spdx.org/rdf/3.0.1/terms/Core/RelationshipType/hasAssessmentFor> a owl:NamedIndividual,
            ns1:RelationshipType ;
        rdfs:label "hasAssessmentFor" ;
        rdfs:comment "Relates a `from` Vulnerability and each `to` Element with a security assessment. To be used with `VulnAssessmentRelationship` types."@en .

    <https://spdx.org/rdf/3.0.1/terms/Core/RelationshipType/hasAssociatedVulnerability> a owl:NamedIndividual,
            ns1:RelationshipType ;
        rdfs:label "hasAssociatedVulnerability" ;
        rdfs:comment "Used to associate a `from` Artifact with each `to` Vulnerability."@en .

    <https://spdx.org/rdf/3.0.1/terms/Core/RelationshipType/hasConcludedLicense> a owl:NamedIndividual,
            ns1:RelationshipType ;
        rdfs:label "hasConcludedLicense" ;
        rdfs:comment "The `from` SoftwareArtifact is concluded by the SPDX data creator to be governed by each `to` license."@en .

    <https://spdx.org/rdf/3.0.1/terms/Core/RelationshipType/hasDataFile> a owl:NamedIndividual,
            ns1:RelationshipType ;
        rdfs:label "hasDataFile" ;
        rdfs:comment "The `from` Element treats each `to` Element as a data file. A data file is an artifact that stores data required or optional for the `from` Element's functionality. A data file can be a database file, an index file, a log file, an AI model file, a calibration data file, a temporary file, a backup file, and more. For AI training dataset, test dataset, test artifact, configuration data, build input data, and build output data, please consider using the more specific relationship types: `trainedOn`, `testedOn`, `hasTest`, `configures`, `hasInput`, and `hasOutput`, respectively. This relationship does not imply dependency."@en .

    <https://spdx.org/rdf/3.0.1/terms/Core/RelationshipType/hasDeclaredLicense> a owl:NamedIndividual,
            ns1:RelationshipType ;
        rdfs:label "hasDeclaredLicense" ;
        rdfs:comment "The `from` SoftwareArtifact was discovered to actually contain each `to` license, for example as detected by use of automated tooling."@en .

    <https://spdx.org/rdf/3.0.1/terms/Core/RelationshipType/hasDeletedFile> a owl:NamedIndividual,
            ns1:RelationshipType ;
        rdfs:label "hasDeletedFile" ;
        rdfs:comment "Every `to` Element is a file deleted from the `from` Element (`from` hasDeletedFile `to`)."@en .

    <https://spdx.org/rdf/3.0.1/terms/Core/RelationshipType/hasDependencyManifest> a owl:NamedIndividual,
            ns1:RelationshipType ;
        rdfs:label "hasDependencyManifest" ;
        rdfs:comment "The `from` Element has manifest files that contain dependency information in each `to` Element."@en .

    <https://spdx.org/rdf/3.0.1/terms/Core/RelationshipType/hasDistributionArtifact> a owl:NamedIndividual,
            ns1:RelationshipType ;
        rdfs:label "hasDistributionArtifact" ;
        rdfs:comment "The `from` Element is distributed as an artifact in each `to` Element (e.g. an RPM or archive file)."@en .

    <https://spdx.org/rdf/3.0.1/terms/Core/RelationshipType/hasDocumentation> a owl:NamedIndividual,
            ns1:RelationshipType ;
        rdfs:label "hasDocumentation" ;
        rdfs:comment "The `from` Element is documented by each `to` Element."@en .

    <https://spdx.org/rdf/3.0.1/terms/Core/RelationshipType/hasDynamicLink> a owl:NamedIndividual,
            ns1:RelationshipType ;
        rdfs:label "hasDynamicLink" ;
        rdfs:comment "The `from` Element dynamically links in each `to` Element, during a LifecycleScopeType period."@en .

    <https://spdx.org/rdf/3.0.1/terms/Core/RelationshipType/hasEvidence> a owl:NamedIndividual,
            ns1:RelationshipType ;
        rdfs:label "hasEvidence" ;
        rdfs:comment "Every `to` Element is considered as evidence for the `from` Element (`from` hasEvidence `to`)."@en .

    <https://spdx.org/rdf/3.0.1/terms/Core/RelationshipType/hasExample> a owl:NamedIndividual,
            ns1:RelationshipType ;
        rdfs:label "hasExample" ;
        rdfs:comment "Every `to` Element is an example for the `from` Element (`from` hasExample `to`)."@en .

    <https://spdx.org/rdf/3.0.1/terms/Core/RelationshipType/hasHost> a owl:NamedIndividual,
            ns1:RelationshipType ;
        rdfs:label "hasHost" ;
        rdfs:comment "The `from` Build was run on the `to` Element during a LifecycleScopeType period (e.g. the host that the build runs on)."@en .

    <https://spdx.org/rdf/3.0.1/terms/Core/RelationshipType/hasInput> a owl:NamedIndividual,
            ns1:RelationshipType ;
        rdfs:label "hasInput" ;
        rdfs:comment "The `from` Build has each `to` Element as an input, during a LifecycleScopeType period."@en .

    <https://spdx.org/rdf/3.0.1/terms/Core/RelationshipType/hasMetadata> a owl:NamedIndividual,
            ns1:RelationshipType ;
        rdfs:label "hasMetadata" ;
        rdfs:comment "Every `to` Element is metadata about the `from` Element (`from` hasMetadata `to`)."@en .

    <https://spdx.org/rdf/3.0.1/terms/Core/RelationshipType/hasOptionalComponent> a owl:NamedIndividual,
            ns1:RelationshipType ;
        rdfs:label "hasOptionalComponent" ;
        rdfs:comment "Every `to` Element is an optional component of the `from` Element (`from` hasOptionalComponent `to`)."@en .

    <https://spdx.org/rdf/3.0.1/terms/Core/RelationshipType/hasOptionalDependency> a owl:NamedIndividual,
            ns1:RelationshipType ;
        rdfs:label "hasOptionalDependency" ;
        rdfs:comment "The `from` Element optionally depends on each `to` Element, during a LifecycleScopeType period."@en .

    <https://spdx.org/rdf/3.0.1/terms/Core/RelationshipType/hasOutput> a owl:NamedIndividual,
            ns1:RelationshipType ;
        rdfs:label "hasOutput" ;
        rdfs:comment "The `from` Build element generates each `to` Element as an output, during a LifecycleScopeType period."@en .

    <https://spdx.org/rdf/3.0.1/terms/Core/RelationshipType/hasPrerequisite> a owl:NamedIndividual,
            ns1:RelationshipType ;
        rdfs:label "hasPrerequisite" ;
        rdfs:comment "The `from` Element has a prerequisite on each `to` Element, during a LifecycleScopeType period."@en .

    <https://spdx.org/rdf/3.0.1/terms/Core/RelationshipType/hasProvidedDependency> a owl:NamedIndividual,
            ns1:RelationshipType ;
        rdfs:label "hasProvidedDependency" ;
        rdfs:comment "The `from` Element has a dependency on each `to` Element, dependency is not in the distributed artifact, but assumed to be provided, during a LifecycleScopeType period."@en .

    <https://spdx.org/rdf/3.0.1/terms/Core/RelationshipType/hasRequirement> a owl:NamedIndividual,
            ns1:RelationshipType ;
        rdfs:label "hasRequirement" ;
        rdfs:comment "The `from` Element has a requirement on each `to` Element, during a LifecycleScopeType period."@en .

    <https://spdx.org/rdf/3.0.1/terms/Core/RelationshipType/hasSpecification> a owl:NamedIndividual,
            ns1:RelationshipType ;
        rdfs:label "hasSpecification" ;
        rdfs:comment "Every `to` Element is a specification for the `from` Element (`from` hasSpecification `to`), during a LifecycleScopeType period."@en .

    <https://spdx.org/rdf/3.0.1/terms/Core/RelationshipType/hasStaticLink> a owl:NamedIndividual,
            ns1:RelationshipType ;
        rdfs:label "hasStaticLink" ;
        rdfs:comment "The `from` Element statically links in each `to` Element, during a LifecycleScopeType period."@en .

    <https://spdx.org/rdf/3.0.1/terms/Core/RelationshipType/hasTest> a owl:NamedIndividual,
            ns1:RelationshipType ;
        rdfs:label "hasTest" ;
        rdfs:comment "Every `to` Element is a test artifact for the `from` Element (`from` hasTest `to`), during a LifecycleScopeType period."@en .

    <https://spdx.org/rdf/3.0.1/terms/Core/RelationshipType/hasTestCase> a owl:NamedIndividual,
            ns1:RelationshipType ;
        rdfs:label "hasTestCase" ;
        rdfs:comment "Every `to` Element is a test case for the `from` Element (`from` hasTestCase `to`)."@en .

    <https://spdx.org/rdf/3.0.1/terms/Core/RelationshipType/hasVariant> a owl:NamedIndividual,
            ns1:RelationshipType ;
        rdfs:label "hasVariant" ;
        rdfs:comment "Every `to` Element is a variant the `from` Element (`from` hasVariant `to`)."@en .

    <https://spdx.org/rdf/3.0.1/terms/Core/RelationshipType/invokedBy> a owl:NamedIndividual,
            ns1:RelationshipType ;
        rdfs:label "invokedBy" ;
        rdfs:comment "The `from` Element was invoked by the `to` Agent, during a LifecycleScopeType period (for example, a Build element that describes a build step)."@en .

    <https://spdx.org/rdf/3.0.1/terms/Core/RelationshipType/modifiedBy> a owl:NamedIndividual,
            ns1:RelationshipType ;
        rdfs:label "modifiedBy" ;
        rdfs:comment "The `from` Element is modified by each `to` Element."@en .

    <https://spdx.org/rdf/3.0.1/terms/Core/RelationshipType/other> a owl:NamedIndividual,
            ns1:RelationshipType ;
        rdfs:label "other" ;
        rdfs:comment "Every `to` Element is related to the `from` Element where the relationship type is not described by any of the SPDX relationship types (this relationship is directionless)."@en .

    <https://spdx.org/rdf/3.0.1/terms/Core/RelationshipType/packagedBy> a owl:NamedIndividual,
            ns1:RelationshipType ;
        rdfs:label "packagedBy" ;
        rdfs:comment "Every `to` Element is a packaged instance of the `from` Element (`from` packagedBy `to`)."@en .

    <https://spdx.org/rdf/3.0.1/terms/Core/RelationshipType/patchedBy> a owl:NamedIndividual,
            ns1:RelationshipType ;
        rdfs:label "patchedBy" ;
        rdfs:comment "Every `to` Element is a patch for the `from` Element (`from` patchedBy `to`)."@en .

    <https://spdx.org/rdf/3.0.1/terms/Core/RelationshipType/publishedBy> a owl:NamedIndividual,
            ns1:RelationshipType ;
        rdfs:label "publishedBy" ;
        rdfs:comment "Designates a `from` Vulnerability was made available for public use or reference by each `to` Agent."@en .

    <https://spdx.org/rdf/3.0.1/terms/Core/RelationshipType/reportedBy> a owl:NamedIndividual,
            ns1:RelationshipType ;
        rdfs:label "reportedBy" ;
        rdfs:comment "Designates a `from` Vulnerability was first reported to a project, vendor, or tracking database for formal identification by each `to` Agent."@en .

    <https://spdx.org/rdf/3.0.1/terms/Core/RelationshipType/republishedBy> a owl:NamedIndividual,
            ns1:RelationshipType ;
        rdfs:label "republishedBy" ;
        rdfs:comment "Designates a `from` Vulnerability's details were tracked, aggregated, and/or enriched to improve context (i.e. NVD) by each `to` Agent."@en .

    <https://spdx.org/rdf/3.0.1/terms/Core/RelationshipType/serializedInArtifact> a owl:NamedIndividual,
            ns1:RelationshipType ;
        rdfs:label "serializedInArtifact" ;
        rdfs:comment "The `from` SpdxDocument can be found in a serialized form in each `to` Artifact."@en .

    <https://spdx.org/rdf/3.0.1/terms/Core/RelationshipType/testedOn> a owl:NamedIndividual,
            ns1:RelationshipType ;
        rdfs:label "testedOn" ;
        rdfs:comment "The `from` Element has been tested on the `to` Element(s)."@en .

    <https://spdx.org/rdf/3.0.1/terms/Core/RelationshipType/trainedOn> a owl:NamedIndividual,
            ns1:RelationshipType ;
        rdfs:label "trainedOn" ;
        rdfs:comment "The `from` Element has been trained on the `to` Element(s)."@en .

    <https://spdx.org/rdf/3.0.1/terms/Core/RelationshipType/underInvestigationFor> a owl:NamedIndividual,
            ns1:RelationshipType ;
        rdfs:label "underInvestigationFor" ;
        rdfs:comment "The `from` Vulnerability impact is being investigated for each `to` Element. The use of the `underInvestigationFor` type is constrained to `VexUnderInvestigationVulnAssessmentRelationship` classed relationships."@en .

    <https://spdx.org/rdf/3.0.1/terms/Core/RelationshipType/usesTool> a owl:NamedIndividual,
            ns1:RelationshipType ;
        rdfs:label "usesTool" ;
        rdfs:comment "The `from` Element uses each `to` Element as a tool, during a LifecycleScopeType period."@en .

    <https://spdx.org/rdf/3.0.1/terms/Core/SupportType/deployed> a owl:NamedIndividual,
            ns1:SupportType ;
        rdfs:label "deployed" ;
        rdfs:comment "in addition to being supported by the supplier, the software is known to have been deployed and is in use.  For a software as a service provider, this implies the software is now available as a service."@en .

    <https://spdx.org/rdf/3.0.1/terms/Core/SupportType/development> a owl:NamedIndividual,
            ns1:SupportType ;
        rdfs:label "development" ;
        rdfs:comment "the artifact is in active development and is not considered ready for formal support from the supplier."@en .

    <https://spdx.org/rdf/3.0.1/terms/Core/SupportType/endOfSupport> a owl:NamedIndividual,
            ns1:SupportType ;
        rdfs:label "endOfSupport" ;
        rdfs:comment "there is a defined end of support for the artifact from the supplier.  This may also be referred to as end of life. There is a validUntilDate that can be used to signal when support ends for the artifact."@en .

    <https://spdx.org/rdf/3.0.1/terms/Core/SupportType/limitedSupport> a owl:NamedIndividual,
            ns1:SupportType ;
        rdfs:label "limitedSupport" ;
        rdfs:comment "the artifact has been released, and there is limited support available from the supplier. There is a validUntilDate that can provide additional information about the duration of support."@en .

    <https://spdx.org/rdf/3.0.1/terms/Core/SupportType/noAssertion> a owl:NamedIndividual,
            ns1:SupportType ;
        rdfs:label "noAssertion" ;
        rdfs:comment "no assertion about the type of support is made.   This is considered the default if no other support type is used."@en .

    <https://spdx.org/rdf/3.0.1/terms/Core/SupportType/noSupport> a owl:NamedIndividual,
            ns1:SupportType ;
        rdfs:label "noSupport" ;
        rdfs:comment "there is no support for the artifact from the supplier, consumer assumes any support obligations."@en .

    <https://spdx.org/rdf/3.0.1/terms/Core/SupportType/support> a owl:NamedIndividual,
            ns1:SupportType ;
        rdfs:label "support" ;
        rdfs:comment "the artifact has been released, and is supported from the supplier.   There is a validUntilDate that can provide additional information about the duration of support."@en .

    ns1:annotationType a owl:ObjectProperty ;
        rdfs:comment "Describes the type of annotation."@en ;
        rdfs:range ns1:AnnotationType .

    ns1:beginIntegerRange a owl:DatatypeProperty ;
        rdfs:comment "Defines the beginning of a range."@en ;
        rdfs:range xsd:positiveInteger .

    ns1:builtTime a owl:DatatypeProperty ;
        rdfs:comment "Specifies the time an artifact was built."@en ;
        rdfs:range xsd:dateTimeStamp .

    ns1:completeness a owl:ObjectProperty ;
        rdfs:comment "Provides information about the completeness of relationships."@en ;
        rdfs:range ns1:RelationshipCompleteness .

    ns1:context a owl:DatatypeProperty ;
        rdfs:comment """Gives information about the circumstances or unifying properties
that Elements of the bundle have been assembled under."""@en ;
        rdfs:range xsd:string .

    ns1:created a owl:DatatypeProperty ;
        rdfs:comment "Identifies when the Element was originally created."@en ;
        rdfs:range xsd:dateTimeStamp .

    ns1:createdBy a owl:ObjectProperty ;
        rdfs:comment "Identifies who or what created the Element."@en ;
        rdfs:range ns1:Agent .

    ns1:createdUsing a owl:ObjectProperty ;
        rdfs:comment "Identifies the tooling that was used during the creation of the Element."@en ;
        rdfs:range ns1:Tool .

    ns1:creationInfo a owl:ObjectProperty ;
        rdfs:comment "Provides information about the creation of the Element."@en ;
        rdfs:range ns1:CreationInfo .

    ns1:dataLicense a owl:ObjectProperty ;
        rdfs:comment """Provides the license under which the SPDX documentation of the Element can be
used."""@en ;
        rdfs:range <https://spdx.org/rdf/3.0.1/terms/SimpleLicensing/AnyLicenseInfo> .

    ns1:definingArtifact a owl:ObjectProperty ;
        rdfs:comment """Artifact representing a serialization instance of SPDX data containing the
definition of a particular Element."""@en ;
        rdfs:range ns1:Artifact .

    ns1:description a owl:DatatypeProperty ;
        rdfs:comment "Provides a detailed description of the Element."@en ;
        rdfs:range xsd:string .

    ns1:element a owl:ObjectProperty ;
        rdfs:comment "Refers to one or more Elements that are part of an ElementCollection."@en ;
        rdfs:range ns1:Element .

    ns1:endIntegerRange a owl:DatatypeProperty ;
        rdfs:comment "Defines the end of a range."@en ;
        rdfs:range xsd:positiveInteger .

    ns1:endTime a owl:DatatypeProperty ;
        rdfs:comment "Specifies the time from which an element is no longer applicable / valid."@en ;
        rdfs:range xsd:dateTimeStamp .

    ns1:extension a owl:ObjectProperty ;
        rdfs:comment "Specifies an Extension characterization of some aspect of an Element."@en ;
        rdfs:range <https://spdx.org/rdf/3.0.1/terms/Extension/Extension> .

    ns1:externalIdentifier a owl:ObjectProperty ;
        rdfs:comment """Provides a reference to a resource outside the scope of SPDX-3.0 content
that uniquely identifies an Element."""@en ;
        rdfs:range ns1:ExternalIdentifier .

    ns1:externalIdentifierType a owl:ObjectProperty ;
        rdfs:comment "Specifies the type of the external identifier."@en ;
        rdfs:range ns1:ExternalIdentifierType .

    ns1:externalRef a owl:ObjectProperty ;
        rdfs:comment """Points to a resource outside the scope of the SPDX-3.0 content
that provides additional characteristics of an Element."""@en ;
        rdfs:range ns1:ExternalRef .

    ns1:externalRefType a owl:ObjectProperty ;
        rdfs:comment "Specifies the type of the external reference."@en ;
        rdfs:range ns1:ExternalRefType .

    ns1:externalSpdxId a owl:DatatypeProperty ;
        rdfs:comment """Identifies an external Element used within an SpdxDocument but defined
external to that SpdxDocument."""@en ;
        rdfs:range xsd:anyURI .

    ns1:from a owl:ObjectProperty ;
        rdfs:comment "References the Element on the left-hand side of a relationship."@en ;
        rdfs:range ns1:Element .

    ns1:identifier a owl:DatatypeProperty ;
        rdfs:comment "Uniquely identifies an external element."@en ;
        rdfs:range xsd:string .

    ns1:identifierLocator a owl:DatatypeProperty ;
        rdfs:comment "Provides the location for more information regarding an external identifier."@en ;
        rdfs:range xsd:anyURI .

    ns1:import a owl:ObjectProperty ;
        rdfs:comment "Provides an ExternalMap of Element identifiers."@en ;
        rdfs:range ns1:ExternalMap .

    ns1:issuingAuthority a owl:DatatypeProperty ;
        rdfs:comment "An entity that is authorized to issue identification credentials."@en ;
        rdfs:range xsd:string .

    ns1:key a owl:DatatypeProperty ;
        rdfs:comment "A key used in a generic key-value pair."@en ;
        rdfs:range xsd:string .

    ns1:locationHint a owl:DatatypeProperty ;
        rdfs:comment "Provides an indication of where to retrieve an external Element."@en ;
        rdfs:range xsd:anyURI .

    ns1:locator a owl:DatatypeProperty ;
        rdfs:comment "Provides the location of an external reference."@en ;
        rdfs:range xsd:string .

    ns1:name a owl:DatatypeProperty ;
        rdfs:comment "Identifies the name of an Element as designated by the creator."@en ;
        rdfs:range xsd:string .

    ns1:namespace a owl:DatatypeProperty ;
        rdfs:comment """Provides an unambiguous mechanism for conveying a URI fragment portion of an
Element ID."""@en ;
        rdfs:range xsd:anyURI .

    ns1:namespaceMap a owl:ObjectProperty ;
        rdfs:comment "Provides a NamespaceMap of prefixes and associated namespace partial URIs applicable to an SpdxDocument and independent of any specific serialization format or instance."@en ;
        rdfs:range ns1:NamespaceMap .

    ns1:originatedBy a owl:ObjectProperty ;
        rdfs:comment "Identifies from where or whom the Element originally came."@en ;
        rdfs:range ns1:Agent .

    ns1:packageVerificationCodeExcludedFile a owl:DatatypeProperty ;
        rdfs:comment """The relative file name of a file to be excluded from the
`PackageVerificationCode`."""@en ;
        rdfs:range xsd:string .

    ns1:prefix a owl:DatatypeProperty ;
        rdfs:comment "A substitute for a URI."@en ;
        rdfs:range xsd:string .

    ns1:profileConformance a owl:ObjectProperty ;
        rdfs:comment """Describes one a profile which the creator of this ElementCollection intends to
conform to."""@en ;
        rdfs:range ns1:ProfileIdentifierType .

    ns1:relationshipType a owl:ObjectProperty ;
        rdfs:comment "Information about the relationship between two Elements."@en ;
        rdfs:range ns1:RelationshipType .

    ns1:releaseTime a owl:DatatypeProperty ;
        rdfs:comment "Specifies the time an artifact was released."@en ;
        rdfs:range xsd:dateTimeStamp .

    ns1:rootElement a owl:ObjectProperty ;
        rdfs:comment "This property is used to denote the root Element(s) of a tree of elements contained in a BOM."@en ;
        rdfs:range ns1:Element .

    ns1:scope a owl:ObjectProperty ;
        rdfs:comment "Capture the scope of information about a specific relationship between elements."@en ;
        rdfs:range ns1:LifecycleScopeType .

    ns1:specVersion a owl:DatatypeProperty ;
        rdfs:comment """Provides a reference number that can be used to understand how to parse and
interpret an Element."""@en ;
        rdfs:range xsd:string .

    ns1:standardName a owl:DatatypeProperty ;
        rdfs:comment "The name of a relevant standard that may apply to an artifact."@en ;
        rdfs:range xsd:string .

    ns1:startTime a owl:DatatypeProperty ;
        rdfs:comment "Specifies the time from which an element is applicable / valid."@en ;
        rdfs:range xsd:dateTimeStamp .

    ns1:statement a owl:DatatypeProperty ;
        rdfs:comment "Commentary on an assertion that an annotator has made."@en ;
        rdfs:range xsd:string .

    ns1:subject a owl:ObjectProperty ;
        rdfs:comment "An Element an annotator has made an assertion about."@en ;
        rdfs:range ns1:Element .

    ns1:summary a owl:DatatypeProperty ;
        rdfs:comment "A short description of an Element."@en ;
        rdfs:range xsd:string .

    ns1:supportLevel a owl:ObjectProperty ;
        rdfs:comment "Specifies the level of support associated with an artifact."@en ;
        rdfs:range ns1:SupportType .

    ns1:to a owl:ObjectProperty ;
        rdfs:comment "References an Element on the right-hand side of a relationship."@en ;
        rdfs:range ns1:Element .

    ns1:validUntilTime a owl:DatatypeProperty ;
        rdfs:comment """Specifies until when the artifact can be used before its usage needs to be
reassessed."""@en ;
        rdfs:range xsd:dateTimeStamp .

    ns1:value a owl:DatatypeProperty ;
        rdfs:comment "A value used in a generic key-value pair."@en ;
        rdfs:range xsd:string .

    <https://spdx.org/rdf/3.0.1/terms/Dataset/ConfidentialityLevelType/amber> a owl:NamedIndividual,
            ns6:ConfidentialityLevelType ;
        rdfs:label "amber" ;
        rdfs:comment "Data points in the dataset can be shared only with specific organizations and their clients on a need to know basis."@en .

    <https://spdx.org/rdf/3.0.1/terms/Dataset/ConfidentialityLevelType/clear> a owl:NamedIndividual,
            ns6:ConfidentialityLevelType ;
        rdfs:label "clear" ;
        rdfs:comment "Dataset may be distributed freely, without restriction."@en .

    <https://spdx.org/rdf/3.0.1/terms/Dataset/ConfidentialityLevelType/green> a owl:NamedIndividual,
            ns6:ConfidentialityLevelType ;
        rdfs:label "green" ;
        rdfs:comment "Dataset can be shared within a community of peers and partners."@en .

    <https://spdx.org/rdf/3.0.1/terms/Dataset/ConfidentialityLevelType/red> a owl:NamedIndividual,
            ns6:ConfidentialityLevelType ;
        rdfs:label "red" ;
        rdfs:comment "Data points in the dataset are highly confidential and can only be shared with named recipients."@en .

    <https://spdx.org/rdf/3.0.1/terms/Dataset/DatasetAvailabilityType/clickthrough> a owl:NamedIndividual,
            ns6:DatasetAvailabilityType ;
        rdfs:label "clickthrough" ;
        rdfs:comment "the dataset is not publicly available and can only be accessed after affirmatively accepting terms on a clickthrough webpage."@en .

    <https://spdx.org/rdf/3.0.1/terms/Dataset/DatasetAvailabilityType/directDownload> a owl:NamedIndividual,
            ns6:DatasetAvailabilityType ;
        rdfs:label "directDownload" ;
        rdfs:comment "the dataset is publicly available and can be downloaded directly."@en .

    <https://spdx.org/rdf/3.0.1/terms/Dataset/DatasetAvailabilityType/query> a owl:NamedIndividual,
            ns6:DatasetAvailabilityType ;
        rdfs:label "query" ;
        rdfs:comment "the dataset is publicly available, but not all at once, and can only be accessed through queries which return parts of the dataset."@en .

    <https://spdx.org/rdf/3.0.1/terms/Dataset/DatasetAvailabilityType/registration> a owl:NamedIndividual,
            ns6:DatasetAvailabilityType ;
        rdfs:label "registration" ;
        rdfs:comment "the dataset is not publicly available and an email registration is required before accessing the dataset, although without an affirmative acceptance of terms."@en .

    <https://spdx.org/rdf/3.0.1/terms/Dataset/DatasetAvailabilityType/scrapingScript> a owl:NamedIndividual,
            ns6:DatasetAvailabilityType ;
        rdfs:label "scrapingScript" ;
        rdfs:comment "the dataset provider is not making available the underlying data and the dataset must be reassembled, typically using the provided script for scraping the data."@en .

    <https://spdx.org/rdf/3.0.1/terms/Dataset/DatasetType/audio> a owl:NamedIndividual,
            ns6:DatasetType ;
        rdfs:label "audio" ;
        rdfs:comment "data is audio based, such as a collection of music from the 80s."@en .

    <https://spdx.org/rdf/3.0.1/terms/Dataset/DatasetType/categorical> a owl:NamedIndividual,
            ns6:DatasetType ;
        rdfs:label "categorical" ;
        rdfs:comment "data that is classified into a discrete number of categories, such as the eye color of a population of people."@en .

    <https://spdx.org/rdf/3.0.1/terms/Dataset/DatasetType/graph> a owl:NamedIndividual,
            ns6:DatasetType ;
        rdfs:label "graph" ;
        rdfs:comment "data is in the form of a graph where entries are somehow related to each other through edges, such a social network of friends."@en .

    <https://spdx.org/rdf/3.0.1/terms/Dataset/DatasetType/image> a owl:NamedIndividual,
            ns6:DatasetType ;
        rdfs:label "image" ;
        rdfs:comment "data is a collection of images such as pictures of animals."@en .

    <https://spdx.org/rdf/3.0.1/terms/Dataset/DatasetType/noAssertion> a owl:NamedIndividual,
            ns6:DatasetType ;
        rdfs:label "noAssertion" ;
        rdfs:comment "data type is not known."@en .

    <https://spdx.org/rdf/3.0.1/terms/Dataset/DatasetType/numeric> a owl:NamedIndividual,
            ns6:DatasetType ;
        rdfs:label "numeric" ;
        rdfs:comment "data consists only of numeric entries."@en .

    <https://spdx.org/rdf/3.0.1/terms/Dataset/DatasetType/other> a owl:NamedIndividual,
            ns6:DatasetType ;
        rdfs:label "other" ;
        rdfs:comment "data is of a type not included in this list."@en .

    <https://spdx.org/rdf/3.0.1/terms/Dataset/DatasetType/sensor> a owl:NamedIndividual,
            ns6:DatasetType ;
        rdfs:label "sensor" ;
        rdfs:comment "data is recorded from a physical sensor, such as a thermometer reading or biometric device."@en .

    <https://spdx.org/rdf/3.0.1/terms/Dataset/DatasetType/structured> a owl:NamedIndividual,
            ns6:DatasetType ;
        rdfs:label "structured" ;
        rdfs:comment "data is stored in tabular format or retrieved from a relational database."@en .

    <https://spdx.org/rdf/3.0.1/terms/Dataset/DatasetType/syntactic> a owl:NamedIndividual,
            ns6:DatasetType ;
        rdfs:label "syntactic" ;
        rdfs:comment "data describes the syntax or semantics of a language or text, such as a parse tree used for natural language processing."@en .

    <https://spdx.org/rdf/3.0.1/terms/Dataset/DatasetType/text> a owl:NamedIndividual,
            ns6:DatasetType ;
        rdfs:label "text" ;
        rdfs:comment "data consists of unstructured text, such as a book, Wikipedia article (without images), or transcript."@en .

    <https://spdx.org/rdf/3.0.1/terms/Dataset/DatasetType/timeseries> a owl:NamedIndividual,
            ns6:DatasetType ;
        rdfs:label "timeseries" ;
        rdfs:comment "data is recorded in an ordered sequence of timestamped entries, such as the price of a stock over the course of a day."@en .

    <https://spdx.org/rdf/3.0.1/terms/Dataset/DatasetType/timestamp> a owl:NamedIndividual,
            ns6:DatasetType ;
        rdfs:label "timestamp" ;
        rdfs:comment "data is recorded with a timestamp for each entry, but not necessarily ordered or at specific intervals, such as when a taxi ride starts and ends."@en .

    <https://spdx.org/rdf/3.0.1/terms/Dataset/DatasetType/video> a owl:NamedIndividual,
            ns6:DatasetType ;
        rdfs:label "video" ;
        rdfs:comment "data is video based, such as a collection of movie clips featuring Tom Hanks."@en .

    ns6:anonymizationMethodUsed a owl:DatatypeProperty ;
        rdfs:comment "Describes the anonymization methods used."@en ;
        rdfs:range xsd:string .

    ns6:confidentialityLevel a owl:ObjectProperty ;
        rdfs:comment "Describes the confidentiality level of the data points contained in the dataset."@en ;
        rdfs:range ns6:ConfidentialityLevelType .

    ns6:dataCollectionProcess a owl:DatatypeProperty ;
        rdfs:comment "Describes how the dataset was collected."@en ;
        rdfs:range xsd:string .

    ns6:dataPreprocessing a owl:DatatypeProperty ;
        rdfs:comment "Describes the preprocessing steps that were applied to the raw data to create the given dataset."@en ;
        rdfs:range xsd:string .

    ns6:datasetAvailability a owl:ObjectProperty ;
        rdfs:comment "The field describes the availability of a dataset."@en ;
        rdfs:range ns6:DatasetAvailabilityType .

    ns6:datasetNoise a owl:DatatypeProperty ;
        rdfs:comment "Describes potentially noisy elements of the dataset."@en ;
        rdfs:range xsd:string .

    ns6:datasetSize a owl:DatatypeProperty ;
        rdfs:comment "Captures the size of the dataset."@en ;
        rdfs:range xsd:nonNegativeInteger .

    ns6:datasetType a owl:ObjectProperty ;
        rdfs:comment "Describes the type of the given dataset."@en ;
        rdfs:range ns6:DatasetType .

    ns6:datasetUpdateMechanism a owl:DatatypeProperty ;
        rdfs:comment "Describes a mechanism to update the dataset."@en ;
        rdfs:range xsd:string .

    ns6:hasSensitivePersonalInformation a owl:ObjectProperty ;
        rdfs:comment "Describes if any sensitive personal information is present in the dataset."@en ;
        rdfs:range ns1:PresenceType .

    ns6:intendedUse a owl:DatatypeProperty ;
        rdfs:comment "Describes what the given dataset should be used for."@en ;
        rdfs:range xsd:string .

    ns6:knownBias a owl:DatatypeProperty ;
        rdfs:comment "Records the biases that the dataset is known to encompass."@en ;
        rdfs:range xsd:string .

    ns6:sensor a owl:ObjectProperty ;
        rdfs:comment "Describes a sensor used for collecting the data."@en ;
        rdfs:range ns1:DictionaryEntry .

    ns5:additionText a owl:DatatypeProperty ;
        rdfs:comment "Identifies the full text of a LicenseAddition."@en ;
        rdfs:range xsd:string .

    ns5:isDeprecatedAdditionId a owl:DatatypeProperty ;
        rdfs:comment "Specifies whether an additional text identifier has been marked as deprecated."@en ;
        rdfs:range xsd:boolean .

    ns5:isDeprecatedLicenseId a owl:DatatypeProperty ;
        rdfs:comment """Specifies whether a license or additional text identifier has been marked as
deprecated."""@en ;
        rdfs:range xsd:boolean .

    ns5:isFsfLibre a owl:DatatypeProperty ;
        rdfs:comment """Specifies whether the License is listed as free by the
Free Software Foundation (FSF)."""@en ;
        rdfs:range xsd:boolean .

    ns5:isOsiApproved a owl:DatatypeProperty ;
        rdfs:comment """Specifies whether the License is listed as approved by the
Open Source Initiative (OSI)."""@en ;
        rdfs:range xsd:boolean .

    ns5:standardAdditionTemplate a owl:DatatypeProperty ;
        rdfs:comment "Identifies the full text of a LicenseAddition, in SPDX templating format."@en ;
        rdfs:range xsd:string .

    ns5:standardLicenseHeader a owl:DatatypeProperty ;
        rdfs:comment """Provides a License author's preferred text to indicate that a file is covered
by the License."""@en ;
        rdfs:range xsd:string .

    ns5:standardLicenseTemplate a owl:DatatypeProperty ;
        rdfs:comment "Identifies the full text of a License, in SPDX templating format."@en ;
        rdfs:range xsd:string .

    ns5:subjectAddition a owl:ObjectProperty ;
        rdfs:comment "A LicenseAddition participating in a 'with addition' model."@en ;
        rdfs:range ns5:LicenseAddition .

    ns5:subjectExtendableLicense a owl:ObjectProperty ;
        rdfs:comment "A License participating in a 'with addition' model."@en ;
        rdfs:range ns5:ExtendableLicense .

    ns5:subjectLicense a owl:ObjectProperty ;
        rdfs:comment "A License participating in an 'or later' model."@en ;
        rdfs:range ns5:License .

    <https://spdx.org/rdf/3.0.1/terms/Extension/cdxPropName> a owl:DatatypeProperty ;
        rdfs:comment "A name used in a CdxPropertyEntry name-value pair."@en ;
        rdfs:range xsd:string .

    <https://spdx.org/rdf/3.0.1/terms/Extension/cdxPropValue> a owl:DatatypeProperty ;
        rdfs:comment "A value used in a CdxPropertyEntry name-value pair."@en ;
        rdfs:range xsd:string .

    <https://spdx.org/rdf/3.0.1/terms/Extension/cdxProperty> a owl:ObjectProperty ;
        rdfs:comment "Provides a map of a property names to a values."@en ;
        rdfs:range <https://spdx.org/rdf/3.0.1/terms/Extension/CdxPropertyEntry> .

    <https://spdx.org/rdf/3.0.1/terms/Security/ExploitCatalogType/kev> a owl:NamedIndividual,
            ns4:ExploitCatalogType ;
        rdfs:label "kev" ;
        rdfs:comment "CISA's Known Exploited Vulnerability (KEV) Catalog"@en .

    <https://spdx.org/rdf/3.0.1/terms/Security/ExploitCatalogType/other> a owl:NamedIndividual,
            ns4:ExploitCatalogType ;
        rdfs:label "other" ;
        rdfs:comment "Other exploit catalogs"@en .

    <https://spdx.org/rdf/3.0.1/terms/Security/SsvcDecisionType/act> a owl:NamedIndividual,
            ns4:SsvcDecisionType ;
        rdfs:label "act" ;
        rdfs:comment "The vulnerability requires attention from the organization's internal, supervisory-level and leadership-level individuals. Necessary actions include requesting assistance or information about the vulnerability, as well as publishing a notification either internally and/or externally. Typically, internal groups would meet to determine the overall response and then execute agreed upon actions. CISA recommends remediating Act vulnerabilities as soon as possible."@en .

    <https://spdx.org/rdf/3.0.1/terms/Security/SsvcDecisionType/attend> a owl:NamedIndividual,
            ns4:SsvcDecisionType ;
        rdfs:label "attend" ;
        rdfs:comment "The vulnerability requires attention from the organization's internal, supervisory-level individuals. Necessary actions include requesting assistance or information about the vulnerability, and may involve publishing a notification either internally and/or externally. CISA recommends remediating Attend vulnerabilities sooner than standard update timelines."@en .

    <https://spdx.org/rdf/3.0.1/terms/Security/SsvcDecisionType/track> a owl:NamedIndividual,
            ns4:SsvcDecisionType ;
        rdfs:label "track" ;
        rdfs:comment "The vulnerability does not require action at this time. The organization would continue to track the vulnerability and reassess it if new information becomes available. CISA recommends remediating Track vulnerabilities within standard update timelines."@en .

    <https://spdx.org/rdf/3.0.1/terms/Security/SsvcDecisionType/trackStar> a owl:NamedIndividual,
            ns4:SsvcDecisionType ;
        rdfs:label "trackStar" ;
        rdfs:comment "(\"Track\\*\" in the SSVC spec) The vulnerability contains specific characteristics that may require closer monitoring for changes. CISA recommends remediating Track\\* vulnerabilities within standard update timelines."@en .

    <https://spdx.org/rdf/3.0.1/terms/Security/VexJustificationType/componentNotPresent> a owl:NamedIndividual,
            ns4:VexJustificationType ;
        rdfs:label "componentNotPresent" ;
        rdfs:comment "The software is not affected because the vulnerable component is not in the product."@en .

    <https://spdx.org/rdf/3.0.1/terms/Security/VexJustificationType/inlineMitigationsAlreadyExist> a owl:NamedIndividual,
            ns4:VexJustificationType ;
        rdfs:label "inlineMitigationsAlreadyExist" ;
        rdfs:comment "Built-in inline controls or mitigations prevent an adversary from leveraging the vulnerability."@en .

    <https://spdx.org/rdf/3.0.1/terms/Security/VexJustificationType/vulnerableCodeCannotBeControlledByAdversary> a owl:NamedIndividual,
            ns4:VexJustificationType ;
        rdfs:label "vulnerableCodeCannotBeControlledByAdversary" ;
        rdfs:comment "The vulnerable component is present, and the component contains the vulnerable code. However, vulnerable code is used in such a way that an attacker cannot mount any anticipated attack."@en .

    <https://spdx.org/rdf/3.0.1/terms/Security/VexJustificationType/vulnerableCodeNotInExecutePath> a owl:NamedIndividual,
            ns4:VexJustificationType ;
        rdfs:label "vulnerableCodeNotInExecutePath" ;
        rdfs:comment "The affected code is not reachable through the execution of the code, including non-anticipated states of the product."@en .

    <https://spdx.org/rdf/3.0.1/terms/Security/VexJustificationType/vulnerableCodeNotPresent> a owl:NamedIndividual,
            ns4:VexJustificationType ;
        rdfs:label "vulnerableCodeNotPresent" ;
        rdfs:comment "The product is not affected because the code underlying the vulnerability is not present in the product."@en .

    ns4:actionStatement a owl:DatatypeProperty ;
        rdfs:comment """Provides advise on how to mitigate or remediate a vulnerability when a VEX product
is affected by it."""@en ;
        rdfs:range xsd:string .

    ns4:actionStatementTime a owl:DatatypeProperty ;
        rdfs:comment """Records the time when a recommended action was communicated in a VEX statement
to mitigate a vulnerability."""@en ;
        rdfs:range xsd:dateTimeStamp .

    ns4:assessedElement a owl:ObjectProperty ;
        rdfs:comment """Specifies an Element contained in a piece of software where a vulnerability was
found."""@en ;
        rdfs:range ns3:SoftwareArtifact .

    ns4:catalogType a owl:ObjectProperty ;
        rdfs:comment "Specifies the exploit catalog type."@en ;
        rdfs:range ns4:ExploitCatalogType .

    ns4:decisionType a owl:ObjectProperty ;
        rdfs:comment """Provide the enumeration of possible decisions in the
[Stakeholder-Specific Vulnerability Categorization (SSVC) decision tree](https://www.cisa.gov/stakeholder-specific-vulnerability-categorization-ssvc)."""@en ;
        rdfs:range ns4:SsvcDecisionType .

    ns4:exploited a owl:DatatypeProperty ;
        rdfs:comment "Describe that a CVE is known to have an exploit because it's been listed in an exploit catalog."@en ;
        rdfs:range xsd:boolean .

    ns4:impactStatement a owl:DatatypeProperty ;
        rdfs:comment """Explains why a VEX product is not affected by a vulnerability. It is an
alternative in VexNotAffectedVulnAssessmentRelationship to the machine-readable
justification label."""@en ;
        rdfs:range xsd:string .

    ns4:impactStatementTime a owl:DatatypeProperty ;
        rdfs:comment "Timestamp of impact statement."@en ;
        rdfs:range xsd:dateTimeStamp .

    ns4:justificationType a owl:ObjectProperty ;
        rdfs:comment """Impact justification label to be used when linking a vulnerability to an element
representing a VEX product with a VexNotAffectedVulnAssessmentRelationship
relationship."""@en ;
        rdfs:range ns4:VexJustificationType .

    ns4:locator a owl:DatatypeProperty ;
        rdfs:comment "Provides the location of an exploit catalog."@en ;
        rdfs:range xsd:anyURI .

    ns4:percentile a owl:DatatypeProperty ;
        rdfs:comment "The percentile of the current probability score."@en ;
        rdfs:range xsd:decimal .

    ns4:probability a owl:DatatypeProperty ;
        rdfs:comment "A probability score between 0 and 1 of a vulnerability being exploited."@en ;
        rdfs:range xsd:decimal .

    ns4:statusNotes a owl:DatatypeProperty ;
        rdfs:comment "Conveys information about how VEX status was determined."@en ;
        rdfs:range xsd:string .

    ns4:vexVersion a owl:DatatypeProperty ;
        rdfs:comment "Specifies the version of a VEX statement."@en ;
        rdfs:range xsd:string .

    <https://spdx.org/rdf/3.0.1/terms/SimpleLicensing/customIdToUri> a owl:ObjectProperty ;
        rdfs:comment """Maps a LicenseRef or AdditionRef string for a Custom License or a Custom
License Addition to its URI ID."""@en ;
        rdfs:range ns1:DictionaryEntry .

    <https://spdx.org/rdf/3.0.1/terms/SimpleLicensing/licenseExpression> a owl:DatatypeProperty ;
        rdfs:comment "A string in the license expression format."@en ;
        rdfs:range xsd:string .

    <https://spdx.org/rdf/3.0.1/terms/SimpleLicensing/licenseListVersion> a owl:DatatypeProperty ;
        rdfs:comment "The version of the SPDX License List used in the license expression."@en ;
        rdfs:range xsd:string .

    <https://spdx.org/rdf/3.0.1/terms/Software/ContentIdentifierType/gitoid> a owl:NamedIndividual,
            ns3:ContentIdentifierType ;
        rdfs:label "gitoid" ;
        rdfs:comment "[Gitoid](https://www.iana.org/assignments/uri-schemes/prov/gitoid), stands for [Git Object ID](https://git-scm.com/book/en/v2/Git-Internals-Git-Objects). A gitoid of type blob is a unique hash of a binary artifact. A gitoid may represent either an [Artifact Identifier](https://github.com/omnibor/spec/blob/eb1ee5c961c16215eb8709b2975d193a2007a35d/spec/SPEC.md#artifact-identifier-types) for the software artifact or an [Input Manifest Identifier](https://github.com/omnibor/spec/blob/eb1ee5c961c16215eb8709b2975d193a2007a35d/spec/SPEC.md#input-manifest-identifier) for the software artifact's associated [Artifact Input Manifest](https://github.com/omnibor/spec/blob/eb1ee5c961c16215eb8709b2975d193a2007a35d/spec/SPEC.md#artifact-input-manifest); this ambiguity exists because the Artifact Input Manifest is itself an artifact, and the gitoid of that artifact is its valid identifier. Gitoids calculated on software artifacts (Snippet, File, or Package Elements) should be recorded in the SPDX 3.0 SoftwareArtifact's contentIdentifier property. Gitoids calculated on the Artifact Input Manifest (Input Manifest Identifier) should be recorded in the SPDX 3.0 Element's externalIdentifier property. See [OmniBOR Specification](https://github.com/omnibor/spec/), a minimalistic specification for describing software [Artifact Dependency Graphs](https://github.com/omnibor/spec/blob/eb1ee5c961c16215eb8709b2975d193a2007a35d/spec/SPEC.md#artifact-dependency-graph-adg)."@en .

    <https://spdx.org/rdf/3.0.1/terms/Software/ContentIdentifierType/swhid> a owl:NamedIndividual,
            ns3:ContentIdentifierType ;
        rdfs:label "swhid" ;
        rdfs:comment "SoftWare Hash IDentifier, a persistent intrinsic identifier for digital artifacts, such as files, trees (also known as directories or folders), commits, and other objects typically found in version control systems. The format of the identifiers is defined in the [SWHID specification](https://www.swhid.org/specification/v1.1/4.Syntax) (ISO/IEC DIS 18670). They typically look like `swh:1:cnt:94a9ed024d3859793618152ea559a168bbcbb5e2`."@en .

    <https://spdx.org/rdf/3.0.1/terms/Software/FileKindType/directory> a owl:NamedIndividual,
            ns3:FileKindType ;
        rdfs:label "directory" ;
        rdfs:comment "The file represents a directory and all content stored in that directory."@en .

    <https://spdx.org/rdf/3.0.1/terms/Software/FileKindType/file> a owl:NamedIndividual,
            ns3:FileKindType ;
        rdfs:label "file" ;
        rdfs:comment "The file represents a single file (default)."@en .

    <https://spdx.org/rdf/3.0.1/terms/Software/SbomType/analyzed> a owl:NamedIndividual,
            ns3:SbomType ;
        rdfs:label "analyzed" ;
        rdfs:comment "SBOM generated through analysis of artifacts (e.g., executables, packages, containers, and virtual machine images) after its build. Such analysis generally requires a variety of heuristics. In some contexts, this may also be referred to as a \"3rd party\" SBOM."@en .

    <https://spdx.org/rdf/3.0.1/terms/Software/SbomType/build> a owl:NamedIndividual,
            ns3:SbomType ;
        rdfs:label "build" ;
        rdfs:comment "SBOM generated as part of the process of building the software to create a releasable artifact (e.g., executable or package) from data such as source files, dependencies, built components, build process ephemeral data, and other SBOMs."@en .

    <https://spdx.org/rdf/3.0.1/terms/Software/SbomType/deployed> a owl:NamedIndividual,
            ns3:SbomType ;
        rdfs:label "deployed" ;
        rdfs:comment "SBOM provides an inventory of software that is present on a system. This may be an assembly of other SBOMs that combines analysis of configuration options, and examination of execution behavior in a (potentially simulated) deployment environment."@en .

    <https://spdx.org/rdf/3.0.1/terms/Software/SbomType/design> a owl:NamedIndividual,
            ns3:SbomType ;
        rdfs:label "design" ;
        rdfs:comment "SBOM of intended, planned software project or product with included components (some of which may not yet exist) for a new software artifact."@en .

    <https://spdx.org/rdf/3.0.1/terms/Software/SbomType/runtime> a owl:NamedIndividual,
            ns3:SbomType ;
        rdfs:label "runtime" ;
        rdfs:comment "SBOM generated through instrumenting the system running the software, to capture only components present in the system, as well as external call-outs or dynamically loaded components. In some contexts, this may also be referred to as an \"Instrumented\" or \"Dynamic\" SBOM."@en .

    <https://spdx.org/rdf/3.0.1/terms/Software/SbomType/source> a owl:NamedIndividual,
            ns3:SbomType ;
        rdfs:label "source" ;
        rdfs:comment "SBOM created directly from the development environment, source files, and included dependencies used to build an product artifact."@en .

    ns3:additionalPurpose a owl:ObjectProperty ;
        rdfs:comment "Provides additional purpose information of the software artifact."@en ;
        rdfs:range ns3:SoftwarePurpose .

    ns3:attributionText a owl:DatatypeProperty ;
        rdfs:comment """Provides a place for the SPDX data creator to record acknowledgement text for
a software Package, File or Snippet."""@en ;
        rdfs:range xsd:string .

    ns3:byteRange a owl:DatatypeProperty ;
        rdfs:comment """Defines the byte range in the original host file that the snippet information
applies to."""@en ;
        rdfs:range ns1:PositiveIntegerRange .

    ns3:contentIdentifier a owl:DatatypeProperty ;
        rdfs:comment """A canonical, unique, immutable identifier of the artifact content, that may be
used for verifying its identity and/or integrity."""@en ;
        rdfs:range ns3:ContentIdentifier .

    ns3:contentIdentifierType a owl:ObjectProperty ;
        rdfs:comment "Specifies the type of the content identifier."@en ;
        rdfs:range ns3:ContentIdentifierType .

    ns3:contentIdentifierValue a owl:DatatypeProperty ;
        rdfs:comment "Specifies the value of the content identifier."@en ;
        rdfs:range xsd:anyURI .

    ns3:copyrightText a owl:DatatypeProperty ;
        rdfs:comment """Identifies the text of one or more copyright notices for a software Package,
File or Snippet, if any."""@en ;
        rdfs:range xsd:string .

    ns3:downloadLocation a owl:DatatypeProperty ;
        rdfs:comment """Identifies the download Uniform Resource Identifier for the package at the time
that the document was created."""@en ;
        rdfs:range xsd:anyURI .

    ns3:fileKind a owl:ObjectProperty ;
        rdfs:comment "Describes if a given file is a directory or non-directory kind of file."@en ;
        rdfs:range ns3:FileKindType .

    ns3:homePage a owl:DatatypeProperty ;
        rdfs:comment """A place for the SPDX document creator to record a website that serves as the
package's home page."""@en ;
        rdfs:range xsd:anyURI .

    ns3:lineRange a owl:DatatypeProperty ;
        rdfs:comment """Defines the line range in the original host file that the snippet information
applies to."""@en ;
        rdfs:range ns1:PositiveIntegerRange .

    ns3:packageUrl a owl:DatatypeProperty ;
        rdfs:comment """Provides a place for the SPDX data creator to record the package URL string
(in accordance with the Package URL specification) for a software Package."""@en ;
        rdfs:range xsd:anyURI .

    ns3:packageVersion a owl:DatatypeProperty ;
        rdfs:comment "Identify the version of a package."@en ;
        rdfs:range xsd:string .

    ns3:primaryPurpose a owl:ObjectProperty ;
        rdfs:comment "Provides information about the primary purpose of the software artifact."@en ;
        rdfs:range ns3:SoftwarePurpose .

    ns3:sbomType a owl:ObjectProperty ;
        rdfs:comment "Provides information about the type of an SBOM."@en ;
        rdfs:range ns3:SbomType .

    ns3:snippetFromFile a owl:ObjectProperty ;
        rdfs:comment "Defines the original host file that the snippet information applies to."@en ;
        rdfs:range ns3:File .

    ns3:sourceInfo a owl:DatatypeProperty ;
        rdfs:comment """Records any relevant background information or additional comments
about the origin of the package."""@en ;
        rdfs:range xsd:string .

    ns2:EnergyConsumption a owl:Class,
            sh:NodeShape ;
        rdfs:comment """A class for describing the energy consumption incurred by an AI model in
different stages of its lifecycle."""@en ;
        sh:nodeKind sh:BlankNodeOrIRI ;
        sh:property _:N363c77746fe14d01b9156613c76390e7,
            _:N49fc85ac4b3e4255965bec1092f3b0bf,
            _:Nd69ae884faaa40898d49c158f8a742fb .

    ns1:ExternalIdentifier a owl:Class,
            sh:NodeShape ;
        rdfs:comment "A reference to a resource identifier defined outside the scope of SPDX-3.0 content that uniquely identifies an Element."@en ;
        sh:nodeKind sh:BlankNodeOrIRI ;
        sh:property _:N10108a0536bb489f88b2fe61aae33caa,
            _:N51eef082985242c7aad70e82f553a639,
            _:N6097953061744c33b80298571399ff7c,
            _:Nb231c2e250ea41fa9d72b8605352f378,
            _:Nbba9abfd6a68448dbef334e60ce75826 .

    ns1:ExternalMap a owl:Class,
            sh:NodeShape ;
        rdfs:comment """A map of Element identifiers that are used within an SpdxDocument but defined
external to that SpdxDocument."""@en ;
        sh:nodeKind sh:BlankNodeOrIRI ;
        sh:property _:N0424b2581a0d4d4aabfbe49ee71c6de7,
            _:N3f1160e3da0e48f5a7f879d3089bc895,
            _:Na360199da8ee498c93cf88f92c327427,
            _:Nf25c1da35dd24967a70cec4affc61874 .

    ns1:ExternalRef a owl:Class,
            sh:NodeShape ;
        rdfs:comment "A reference to a resource outside the scope of SPDX-3.0 content related to an Element."@en ;
        sh:nodeKind sh:BlankNodeOrIRI ;
        sh:property _:N0921a60ce67049798ca7d56bcdec6dab,
            _:N46c085d9b83f4ef3b53633491f4e362a,
            _:N5c84929041474695a6ed261ce7b4ad19,
            _:N8114becca8804d67bed986f971629c1c .

    ns1:Hash a owl:Class,
            sh:NodeShape ;
        rdfs:comment "A mathematically calculated representation of a grouping of data."@en ;
        rdfs:subClassOf ns1:IntegrityMethod ;
        sh:nodeKind sh:BlankNodeOrIRI ;
        sh:property _:Nb3de9ed0037c4b249b07b05a9af68f5b,
            _:Ne6b4111dd98f4642bdc8313bb4485ac4 .

    <https://spdx.org/rdf/3.0.1/terms/Core/HashAlgorithm/adler32> a owl:NamedIndividual,
            ns1:HashAlgorithm ;
        rdfs:label "adler32" ;
        rdfs:comment "Adler-32 checksum is part of the widely used zlib compression library as defined in [RFC 1950](https://datatracker.ietf.org/doc/rfc1950/) Section 2.3."@en .

    <https://spdx.org/rdf/3.0.1/terms/Core/HashAlgorithm/blake2b256> a owl:NamedIndividual,
            ns1:HashAlgorithm ;
        rdfs:label "blake2b256" ;
        rdfs:comment "BLAKE2b algorithm with a digest size of 256, as defined in [RFC 7693](https://datatracker.ietf.org/doc/rfc7693/) Section 4."@en .

    <https://spdx.org/rdf/3.0.1/terms/Core/HashAlgorithm/blake2b384> a owl:NamedIndividual,
            ns1:HashAlgorithm ;
        rdfs:label "blake2b384" ;
        rdfs:comment "BLAKE2b algorithm with a digest size of 384, as defined in [RFC 7693](https://datatracker.ietf.org/doc/rfc7693/) Section 4."@en .

    <https://spdx.org/rdf/3.0.1/terms/Core/HashAlgorithm/blake2b512> a owl:NamedIndividual,
            ns1:HashAlgorithm ;
        rdfs:label "blake2b512" ;
        rdfs:comment "BLAKE2b algorithm with a digest size of 512, as defined in [RFC 7693](https://datatracker.ietf.org/doc/rfc7693/) Section 4."@en .

    <https://spdx.org/rdf/3.0.1/terms/Core/HashAlgorithm/blake3> a owl:NamedIndividual,
            ns1:HashAlgorithm ;
        rdfs:label "blake3" ;
        rdfs:comment "[BLAKE3](https://github.com/BLAKE3-team/BLAKE3-specs/blob/master/blake3.pdf)"@en .

    <https://spdx.org/rdf/3.0.1/terms/Core/HashAlgorithm/crystalsDilithium> a owl:NamedIndividual,
            ns1:HashAlgorithm ;
        rdfs:label "crystalsDilithium" ;
        rdfs:comment "[Dilithium](https://pq-crystals.org/dilithium/)"@en .

    <https://spdx.org/rdf/3.0.1/terms/Core/HashAlgorithm/crystalsKyber> a owl:NamedIndividual,
            ns1:HashAlgorithm ;
        rdfs:label "crystalsKyber" ;
        rdfs:comment "[Kyber](https://pq-crystals.org/kyber/)"@en .

    <https://spdx.org/rdf/3.0.1/terms/Core/HashAlgorithm/falcon> a owl:NamedIndividual,
            ns1:HashAlgorithm ;
        rdfs:label "falcon" ;
        rdfs:comment "[FALCON](https://falcon-sign.info/falcon.pdf)"@en .

    <https://spdx.org/rdf/3.0.1/terms/Core/HashAlgorithm/md2> a owl:NamedIndividual,
            ns1:HashAlgorithm ;
        rdfs:label "md2" ;
        rdfs:comment "MD2 message-digest algorithm, as defined in [RFC 1319](https://datatracker.ietf.org/doc/rfc1319/)."@en .

    <https://spdx.org/rdf/3.0.1/terms/Core/HashAlgorithm/md4> a owl:NamedIndividual,
            ns1:HashAlgorithm ;
        rdfs:label "md4" ;
        rdfs:comment "MD4 message-digest algorithm, as defined in [RFC 1186](https://datatracker.ietf.org/doc/rfc1186/)."@en .

    <https://spdx.org/rdf/3.0.1/terms/Core/HashAlgorithm/md5> a owl:NamedIndividual,
            ns1:HashAlgorithm ;
        rdfs:label "md5" ;
        rdfs:comment "MD5 message-digest algorithm, as defined in [RFC 1321](https://datatracker.ietf.org/doc/rfc1321/)."@en .

    <https://spdx.org/rdf/3.0.1/terms/Core/HashAlgorithm/md6> a owl:NamedIndividual,
            ns1:HashAlgorithm ;
        rdfs:label "md6" ;
        rdfs:comment "[MD6 hash function](https://people.csail.mit.edu/rivest/pubs/RABCx08.pdf)"@en .

    <https://spdx.org/rdf/3.0.1/terms/Core/HashAlgorithm/other> a owl:NamedIndividual,
            ns1:HashAlgorithm ;
        rdfs:label "other" ;
        rdfs:comment "any hashing algorithm that does not exist in this list of entries"@en .

    <https://spdx.org/rdf/3.0.1/terms/Core/HashAlgorithm/sha1> a owl:NamedIndividual,
            ns1:HashAlgorithm ;
        rdfs:label "sha1" ;
        rdfs:comment "SHA-1, a secure hashing algorithm, as defined in [RFC 3174](https://datatracker.ietf.org/doc/rfc3174/)."@en .

    <https://spdx.org/rdf/3.0.1/terms/Core/HashAlgorithm/sha224> a owl:NamedIndividual,
            ns1:HashAlgorithm ;
        rdfs:label "sha224" ;
        rdfs:comment "SHA-2 with a digest length of 224, as defined in [RFC 3874](https://datatracker.ietf.org/doc/rfc3874/)."@en .

    <https://spdx.org/rdf/3.0.1/terms/Core/HashAlgorithm/sha256> a owl:NamedIndividual,
            ns1:HashAlgorithm ;
        rdfs:label "sha256" ;
        rdfs:comment "SHA-2 with a digest length of 256, as defined in [RFC 6234](https://datatracker.ietf.org/doc/rfc6234/)."@en .

    <https://spdx.org/rdf/3.0.1/terms/Core/HashAlgorithm/sha384> a owl:NamedIndividual,
            ns1:HashAlgorithm ;
        rdfs:label "sha384" ;
        rdfs:comment "SHA-2 with a digest length of 384, as defined in [RFC 6234](https://datatracker.ietf.org/doc/rfc6234/)."@en .

    <https://spdx.org/rdf/3.0.1/terms/Core/HashAlgorithm/sha3_224> a owl:NamedIndividual,
            ns1:HashAlgorithm ;
        rdfs:label "sha3_224" ;
        rdfs:comment "SHA-3 with a digest length of 224, as defined in [FIPS 202](https://csrc.nist.gov/pubs/fips/202/final)."@en .

    <https://spdx.org/rdf/3.0.1/terms/Core/HashAlgorithm/sha3_256> a owl:NamedIndividual,
            ns1:HashAlgorithm ;
        rdfs:label "sha3_256" ;
        rdfs:comment "SHA-3 with a digest length of 256, as defined in [FIPS 202](https://csrc.nist.gov/pubs/fips/202/final)."@en .

    <https://spdx.org/rdf/3.0.1/terms/Core/HashAlgorithm/sha3_384> a owl:NamedIndividual,
            ns1:HashAlgorithm ;
        rdfs:label "sha3_384" ;
        rdfs:comment "SHA-3 with a digest length of 384, as defined in [FIPS 202](https://csrc.nist.gov/pubs/fips/202/final)."@en .

    <https://spdx.org/rdf/3.0.1/terms/Core/HashAlgorithm/sha3_512> a owl:NamedIndividual,
            ns1:HashAlgorithm ;
        rdfs:label "sha3_512" ;
        rdfs:comment "SHA-3 with a digest length of 512, as defined in [FIPS 202](https://csrc.nist.gov/pubs/fips/202/final)."@en .

    <https://spdx.org/rdf/3.0.1/terms/Core/HashAlgorithm/sha512> a owl:NamedIndividual,
            ns1:HashAlgorithm ;
        rdfs:label "sha512" ;
        rdfs:comment "SHA-2 with a digest length of 512, as defined in [RFC 6234](https://datatracker.ietf.org/doc/rfc6234/)."@en .

    ns1:IndividualElement a owl:Class ;
        rdfs:comment """A concrete subclass of Element used by Individuals in the
Core profile."""@en ;
        rdfs:subClassOf ns1:Element ;
        sh:nodeKind sh:IRI .

    ns1:NamespaceMap a owl:Class,
            sh:NodeShape ;
        rdfs:comment "A mapping between prefixes and namespace partial URIs."@en ;
        sh:nodeKind sh:BlankNodeOrIRI ;
        sh:property _:N552625ddd9864602a0ee19418b5be3ad,
            _:N9f51729e24eb42d4965a4a74fe302d3a .

    ns1:Relationship a owl:Class,
            sh:NodeShape ;
        rdfs:comment "Describes a relationship between one or more elements."@en ;
        rdfs:subClassOf ns1:Element ;
        sh:nodeKind sh:IRI ;
        sh:property _:N2d48f33c49aa4655a422188c69928cd8,
            _:N45063856b753439d8cf82d7fee02490e,
            _:N51e95bcda10e477fb13d33c114b9440e,
            _:N54056810820d48cf8ab5b16acee5b46e,
            _:N5c04e2eaeb8d44b48535608e5aed9b28,
            _:Nc7934e8be9ac4597a30ceb464f3d5037 .

    ns1:Tool a owl:Class ;
        rdfs:comment "An element of hardware and/or software utilized to carry out a particular function."@en ;
        rdfs:subClassOf ns1:Element ;
        sh:nodeKind sh:IRI .

    ns1:algorithm a owl:ObjectProperty ;
        rdfs:comment "Specifies the algorithm used for calculating the hash value."@en ;
        rdfs:range ns1:HashAlgorithm .

    ns1:hashValue a owl:DatatypeProperty ;
        rdfs:comment "The result of applying a hash algorithm to an Element."@en ;
        rdfs:range xsd:string .

    ns1:suppliedBy a owl:ObjectProperty ;
        rdfs:comment """Identifies who or what supplied the artifact or VulnAssessmentRelationship
referenced by the Element."""@en ;
        rdfs:range ns1:Agent .

    ns1:verifiedUsing a owl:ObjectProperty ;
        rdfs:comment """Provides an IntegrityMethod with which the integrity of an Element can be
asserted."""@en ;
        rdfs:range ns1:IntegrityMethod .

    ns5:IndividualLicensingInfo a owl:Class ;
        rdfs:comment """A concrete subclass of AnyLicenseInfo used by Individuals in the
ExpandedLicensing profile."""@en ;
        rdfs:subClassOf <https://spdx.org/rdf/3.0.1/terms/SimpleLicensing/AnyLicenseInfo> ;
        sh:nodeKind sh:IRI .

    ns5:deprecatedVersion a owl:DatatypeProperty ;
        rdfs:comment """Specifies the SPDX License List version in which this license or exception
identifier was deprecated."""@en ;
        rdfs:range xsd:string .

    ns5:licenseXml a owl:DatatypeProperty ;
        rdfs:comment """Identifies all the text and metadata associated with a license in the license
XML format."""@en ;
        rdfs:range xsd:string .

    ns5:listVersionAdded a owl:DatatypeProperty ;
        rdfs:comment """Specifies the SPDX License List version in which this ListedLicense or
ListedLicenseException identifier was first added."""@en ;
        rdfs:range xsd:string .

    ns5:member a owl:ObjectProperty ;
        rdfs:comment "A license expression participating in a license set."@en ;
        rdfs:range <https://spdx.org/rdf/3.0.1/terms/SimpleLicensing/AnyLicenseInfo> .

    ns5:obsoletedBy a owl:DatatypeProperty ;
        rdfs:comment """Specifies the licenseId that is preferred to be used in place of a deprecated
License or LicenseAddition."""@en ;
        rdfs:range xsd:string .

    ns5:seeAlso a owl:DatatypeProperty ;
        rdfs:comment "Contains a URL where the License or LicenseAddition can be found in use."@en ;
        rdfs:range xsd:anyURI .

    <https://spdx.org/rdf/3.0.1/terms/Extension/CdxPropertyEntry> a owl:Class,
            sh:NodeShape ;
        rdfs:comment "A property name with an associated value."@en ;
        sh:nodeKind sh:BlankNodeOrIRI ;
        sh:property _:N1eceff509a414ae0a364c00261c99d82,
            _:N6b07fbd78cf44270865f58743c1d4717 .

    <https://spdx.org/rdf/3.0.1/terms/Security/CvssSeverityType/critical> a owl:NamedIndividual,
            ns4:CvssSeverityType ;
        rdfs:label "critical" ;
        rdfs:comment "When a CVSS score is between 9.0 - 10.0"@en .

    <https://spdx.org/rdf/3.0.1/terms/Security/CvssSeverityType/high> a owl:NamedIndividual,
            ns4:CvssSeverityType ;
        rdfs:label "high" ;
        rdfs:comment "When a CVSS score is between 7.0 - 8.9"@en .

    <https://spdx.org/rdf/3.0.1/terms/Security/CvssSeverityType/low> a owl:NamedIndividual,
            ns4:CvssSeverityType ;
        rdfs:label "low" ;
        rdfs:comment "When a CVSS score is between 0.1 - 3.9"@en .

    <https://spdx.org/rdf/3.0.1/terms/Security/CvssSeverityType/medium> a owl:NamedIndividual,
            ns4:CvssSeverityType ;
        rdfs:label "medium" ;
        rdfs:comment "When a CVSS score is between 4.0 - 6.9"@en .

    <https://spdx.org/rdf/3.0.1/terms/Security/CvssSeverityType/none> a owl:NamedIndividual,
            ns4:CvssSeverityType ;
        rdfs:label "none" ;
        rdfs:comment "When a CVSS score is 0.0"@en .

    ns4:modifiedTime a owl:DatatypeProperty ;
        rdfs:comment "Specifies a time when a vulnerability assessment was modified"@en ;
        rdfs:range xsd:dateTimeStamp .

    ns4:publishedTime a owl:DatatypeProperty ;
        rdfs:comment "Specifies the time when a vulnerability was published."@en ;
        rdfs:range xsd:dateTimeStamp .

    ns4:severity a owl:ObjectProperty ;
        rdfs:comment "Specifies the CVSS qualitative severity rating of a vulnerability in relation to a piece of software."@en ;
        rdfs:range ns4:CvssSeverityType .

    ns4:withdrawnTime a owl:DatatypeProperty ;
        rdfs:comment "Specified the time and date when a vulnerability was withdrawn."@en ;
        rdfs:range xsd:dateTimeStamp .

    <https://spdx.org/rdf/3.0.1/terms/SimpleLicensing/licenseText> a owl:DatatypeProperty ;
        rdfs:comment "Identifies the full text of a License or Addition."@en ;
        rdfs:range xsd:string .

    ns3:ContentIdentifier a owl:Class,
            sh:NodeShape ;
        rdfs:comment "A canonical, unique, immutable identifier"@en ;
        rdfs:subClassOf ns1:IntegrityMethod ;
        sh:nodeKind sh:BlankNodeOrIRI ;
        sh:property _:N2f453dff5c3d4aeb9eeca1c273089f5d,
            _:N6bd1a6d665974f37b6330aee72463c40 .

    ns3:File a owl:Class,
            sh:NodeShape ;
        rdfs:comment "Refers to any object that stores content on a computer."@en ;
        rdfs:subClassOf ns3:SoftwareArtifact ;
        sh:nodeKind sh:IRI ;
        sh:property _:N2c00f81f03274496b7c4c8ab8bf09b2a,
            _:N77cfd96960c54e7da88fac7740281ef5 .

    ns3:Package a owl:Class,
            sh:NodeShape ;
        rdfs:comment """Refers to any unit of content that can be associated with a distribution of
software."""@en ;
        rdfs:subClassOf ns3:SoftwareArtifact ;
        sh:nodeKind sh:IRI ;
        sh:property _:N7bb26512f3b246a189e3c1caf404b878,
            _:N9067cfbcf2ce44789dab84e7b2d41316,
            _:Nb63b9b48ace04747b731a24ec5937acf,
            _:Nf456142b643f465ba3425afbe9dc23e9,
            _:Nf79a3a3329be4b8fbccf847359371718 .

    <https://spdx.org/rdf/3.0.1/terms/Software/SoftwarePurpose/application> a owl:NamedIndividual,
            ns3:SoftwarePurpose ;
        rdfs:label "application" ;
        rdfs:comment "The Element is a software application."@en .

    <https://spdx.org/rdf/3.0.1/terms/Software/SoftwarePurpose/archive> a owl:NamedIndividual,
            ns3:SoftwarePurpose ;
        rdfs:label "archive" ;
        rdfs:comment "The Element is an archived collection of one or more files (.tar, .zip, etc.)."@en .

    <https://spdx.org/rdf/3.0.1/terms/Software/SoftwarePurpose/bom> a owl:NamedIndividual,
            ns3:SoftwarePurpose ;
        rdfs:label "bom" ;
        rdfs:comment "The Element is a bill of materials."@en .

    <https://spdx.org/rdf/3.0.1/terms/Software/SoftwarePurpose/configuration> a owl:NamedIndividual,
            ns3:SoftwarePurpose ;
        rdfs:label "configuration" ;
        rdfs:comment "The Element is configuration data."@en .

    <https://spdx.org/rdf/3.0.1/terms/Software/SoftwarePurpose/container> a owl:NamedIndividual,
            ns3:SoftwarePurpose ;
        rdfs:label "container" ;
        rdfs:comment "The Element is a container image which can be used by a container runtime application."@en .

    <https://spdx.org/rdf/3.0.1/terms/Software/SoftwarePurpose/data> a owl:NamedIndividual,
            ns3:SoftwarePurpose ;
        rdfs:label "data" ;
        rdfs:comment "The Element is data."@en .

    <https://spdx.org/rdf/3.0.1/terms/Software/SoftwarePurpose/device> a owl:NamedIndividual,
            ns3:SoftwarePurpose ;
        rdfs:label "device" ;
        rdfs:comment "The Element refers to a chipset, processor, or electronic board."@en .

    <https://spdx.org/rdf/3.0.1/terms/Software/SoftwarePurpose/deviceDriver> a owl:NamedIndividual,
            ns3:SoftwarePurpose ;
        rdfs:label "deviceDriver" ;
        rdfs:comment "The Element represents software that controls hardware devices."@en .

    <https://spdx.org/rdf/3.0.1/terms/Software/SoftwarePurpose/diskImage> a owl:NamedIndividual,
            ns3:SoftwarePurpose ;
        rdfs:label "diskImage" ;
        rdfs:comment "The Element refers to a disk image that can be written to a disk, booted in a VM, etc. A disk image typically contains most or all of the components necessary to boot, such as bootloaders, kernels, firmware, userspace, etc."@en .

    <https://spdx.org/rdf/3.0.1/terms/Software/SoftwarePurpose/documentation> a owl:NamedIndividual,
            ns3:SoftwarePurpose ;
        rdfs:label "documentation" ;
        rdfs:comment "The Element is documentation."@en .

    <https://spdx.org/rdf/3.0.1/terms/Software/SoftwarePurpose/evidence> a owl:NamedIndividual,
            ns3:SoftwarePurpose ;
        rdfs:label "evidence" ;
        rdfs:comment "The Element is the evidence that a specification or requirement has been fulfilled."@en .

    <https://spdx.org/rdf/3.0.1/terms/Software/SoftwarePurpose/executable> a owl:NamedIndividual,
            ns3:SoftwarePurpose ;
        rdfs:label "executable" ;
        rdfs:comment "The Element is an Artifact that can be run on a computer."@en .

    <https://spdx.org/rdf/3.0.1/terms/Software/SoftwarePurpose/file> a owl:NamedIndividual,
            ns3:SoftwarePurpose ;
        rdfs:label "file" ;
        rdfs:comment "The Element is a single file which can be independently distributed (configuration file, statically linked binary, Kubernetes deployment, etc.)."@en .

    <https://spdx.org/rdf/3.0.1/terms/Software/SoftwarePurpose/filesystemImage> a owl:NamedIndividual,
            ns3:SoftwarePurpose ;
        rdfs:label "filesystemImage" ;
        rdfs:comment "The Element is a file system image that can be written to a disk (or virtual) partition."@en .

    <https://spdx.org/rdf/3.0.1/terms/Software/SoftwarePurpose/firmware> a owl:NamedIndividual,
            ns3:SoftwarePurpose ;
        rdfs:label "firmware" ;
        rdfs:comment "The Element provides low level control over a device's hardware."@en .

    <https://spdx.org/rdf/3.0.1/terms/Software/SoftwarePurpose/framework> a owl:NamedIndividual,
            ns3:SoftwarePurpose ;
        rdfs:label "framework" ;
        rdfs:comment "The Element is a software framework."@en .

    <https://spdx.org/rdf/3.0.1/terms/Software/SoftwarePurpose/install> a owl:NamedIndividual,
            ns3:SoftwarePurpose ;
        rdfs:label "install" ;
        rdfs:comment "The Element is used to install software on disk."@en .

    <https://spdx.org/rdf/3.0.1/terms/Software/SoftwarePurpose/library> a owl:NamedIndividual,
            ns3:SoftwarePurpose ;
        rdfs:label "library" ;
        rdfs:comment "The Element is a software library."@en .

    <https://spdx.org/rdf/3.0.1/terms/Software/SoftwarePurpose/manifest> a owl:NamedIndividual,
            ns3:SoftwarePurpose ;
        rdfs:label "manifest" ;
        rdfs:comment "The Element is a software manifest."@en .

    <https://spdx.org/rdf/3.0.1/terms/Software/SoftwarePurpose/model> a owl:NamedIndividual,
            ns3:SoftwarePurpose ;
        rdfs:label "model" ;
        rdfs:comment "The Element is a machine learning or artificial intelligence model."@en .

    <https://spdx.org/rdf/3.0.1/terms/Software/SoftwarePurpose/module> a owl:NamedIndividual,
            ns3:SoftwarePurpose ;
        rdfs:label "module" ;
        rdfs:comment "The Element is a module of a piece of software."@en .

    <https://spdx.org/rdf/3.0.1/terms/Software/SoftwarePurpose/operatingSystem> a owl:NamedIndividual,
            ns3:SoftwarePurpose ;
        rdfs:label "operatingSystem" ;
        rdfs:comment "The Element is an operating system."@en .

    <https://spdx.org/rdf/3.0.1/terms/Software/SoftwarePurpose/other> a owl:NamedIndividual,
            ns3:SoftwarePurpose ;
        rdfs:label "other" ;
        rdfs:comment "The Element doesn't fit into any of the other categories."@en .

    <https://spdx.org/rdf/3.0.1/terms/Software/SoftwarePurpose/patch> a owl:NamedIndividual,
            ns3:SoftwarePurpose ;
        rdfs:label "patch" ;
        rdfs:comment "The Element contains a set of changes to update, fix, or improve another Element."@en .

    <https://spdx.org/rdf/3.0.1/terms/Software/SoftwarePurpose/platform> a owl:NamedIndividual,
            ns3:SoftwarePurpose ;
        rdfs:label "platform" ;
        rdfs:comment "The Element represents a runtime environment."@en .

    <https://spdx.org/rdf/3.0.1/terms/Software/SoftwarePurpose/requirement> a owl:NamedIndividual,
            ns3:SoftwarePurpose ;
        rdfs:label "requirement" ;
        rdfs:comment "The Element provides a requirement needed as input for another Element."@en .

    <https://spdx.org/rdf/3.0.1/terms/Software/SoftwarePurpose/source> a owl:NamedIndividual,
            ns3:SoftwarePurpose ;
        rdfs:label "source" ;
        rdfs:comment "The Element is a single or a collection of source files."@en .

    <https://spdx.org/rdf/3.0.1/terms/Software/SoftwarePurpose/specification> a owl:NamedIndividual,
            ns3:SoftwarePurpose ;
        rdfs:label "specification" ;
        rdfs:comment "The Element is a plan, guideline or strategy how to create, perform or analyze an application."@en .

    <https://spdx.org/rdf/3.0.1/terms/Software/SoftwarePurpose/test> a owl:NamedIndividual,
            ns3:SoftwarePurpose ;
        rdfs:label "test" ;
        rdfs:comment "The Element is a test used to verify functionality on an software element."@en .

    ns1:ElementCollection a owl:Class,
            sh:NodeShape ;
        rdfs:comment "A collection of Elements, not necessarily with unifying context."@en ;
        rdfs:subClassOf ns1:Element ;
        sh:nodeKind sh:IRI ;
        sh:property _:N04198a73e7ea442393c03cfc23850af1,
            _:N482bb00385844dc6b842a414c6156a37,
            _:N56610830d7ac4b88becc196329620d76,
            _:N8ec3a357913b4e8f9be6010fede1f88b .

    <https://spdx.org/rdf/3.0.1/terms/Core/PresenceType/no> a owl:NamedIndividual,
            ns1:PresenceType ;
        rdfs:label "no" ;
        rdfs:comment "Indicates absence of the field."@en .

    <https://spdx.org/rdf/3.0.1/terms/Core/PresenceType/noAssertion> a owl:NamedIndividual,
            ns1:PresenceType ;
        rdfs:label "noAssertion" ;
        rdfs:comment "Makes no assertion about the field."@en .

    <https://spdx.org/rdf/3.0.1/terms/Core/PresenceType/yes> a owl:NamedIndividual,
            ns1:PresenceType ;
        rdfs:label "yes" ;
        rdfs:comment "Indicates presence of the field."@en .

    ns1:contentType a owl:DatatypeProperty ;
        rdfs:comment "Provides information about the content type of an Element or a Property."@en ;
        rdfs:range xsd:string .

    ns4:score a owl:DatatypeProperty ;
        rdfs:comment "Provides a numerical (0-10) representation of the severity of a vulnerability."@en ;
        rdfs:range xsd:decimal .

    ns4:vectorString a owl:DatatypeProperty ;
        rdfs:comment "Specifies the CVSS vector string for a vulnerability."@en ;
        rdfs:range xsd:string .

    ns1:AnnotationType a owl:Class ;
        rdfs:comment "Specifies the type of an annotation."@en .

    ns1:PositiveIntegerRange a owl:Class,
            sh:NodeShape ;
        rdfs:comment "A tuple of two positive integers that define a range."@en ;
        sh:nodeKind sh:BlankNodeOrIRI ;
        sh:property _:Nd6f96cdb35ca487ebe5f0c1ef4d318eb,
            _:Ne72021f629d34d889aa64dd671270777 .

    <https://spdx.org/rdf/3.0.1/terms/Extension/Extension> a owl:Class ;
        rdfs:comment "A characterization of some aspect of an Element that is associated with the Element in a generalized fashion."@en ;
        sh:nodeKind sh:BlankNodeOrIRI ;
        sh:property _:N5d3cfef88942468f8626584333640c31 .

    ns4:ExploitCatalogType a owl:Class ;
        rdfs:comment "Specifies the exploit catalog type."@en .

    ns3:ContentIdentifierType a owl:Class ;
        rdfs:comment "Specifies the type of a content identifier."@en .

    ns3:FileKindType a owl:Class ;
        rdfs:comment "Enumeration of the different kinds of SPDX file."@en .

    ns2:EnergyUnitType a owl:Class ;
        rdfs:comment "Specifies the unit of energy consumption."@en .

    ns1:Artifact a owl:Class,
            sh:NodeShape ;
        rdfs:comment "A distinct article or unit within the digital domain."@en ;
        rdfs:subClassOf ns1:Element ;
        sh:nodeKind sh:IRI ;
        sh:property _:N41c9b9a507de47d4a519c0b6be4c3019,
            _:N672fab4a7fc044949e885d5809f89577,
            _:N69f1d00a23cc4b8e8a94de780133c16f,
            _:N7cd9750385bc4a599bec4444bf204571,
            _:N83e7170013b548ba92e291f418b50a47,
            _:Nc045fbbe74684a038b56bd5c153fdabf,
            _:Nc05a6979941045b19ff160e0990b67c9,
            _:Ne69badf11b7147abb2046a897c76c730 .

    ns1:RelationshipCompleteness a owl:Class ;
        rdfs:comment "Indicates whether a relationship is known to be complete, incomplete, or if no assertion is made with respect to relationship completeness."@en .

    ns1:SpdxOrganization a owl:NamedIndividual,
            ns1:Organization ;
        rdfs:comment "An Organization representing the SPDX Project."@en ;
        owl:sameAs <https://spdx.org/> ;
        ns1:creationInfo <https://spdx.org/rdf/3.0.1/creationInfo_SpdxOrganization> .

    ns1:comment a owl:DatatypeProperty ;
        rdfs:comment """Provide consumers with comments by the creator of the Element about the
Element."""@en ;
        rdfs:range xsd:string .

    ns5:ExtendableLicense a owl:Class ;
        rdfs:comment "Abstract class representing a License or an OrLaterOperator."@en ;
        rdfs:subClassOf <https://spdx.org/rdf/3.0.1/terms/SimpleLicensing/AnyLicenseInfo> ;
        sh:nodeKind sh:IRI ;
        sh:property _:N389d3e9e81e74e3797b180d81edca2e0 .

    ns5:License a owl:Class,
            sh:NodeShape ;
        rdfs:comment "Abstract class for the portion of an AnyLicenseInfo representing a license."@en ;
        rdfs:subClassOf ns5:ExtendableLicense ;
        sh:nodeKind sh:IRI ;
        sh:property _:N3e29af3bed3d478b8963ae1822aa1c32,
            _:N4917b1e13e4948c3ba296ae65637fe94,
            _:N5cddeb9dcb2146139887c2fd1e84cfa9,
            _:N648f9ffbb9ba43b6aab8f8d5f154cc28,
            _:N6c7a51ed84ac4676a3ba3d01dc04d315,
            _:N9b60d6fcf46f4094acac3c7d16abd05f,
            _:Nb0cacc9c6dba43949be9de7002ca8e9d,
            _:Ndae7379c02584fffb6506e7a8828e22a,
            _:Nf6895f10a25a4c93bebd86ffcf1880aa,
            _:Nfa471bceb89b4edaa32262f73d08f93f .

    ns5:LicenseAddition a owl:Class,
            sh:NodeShape ;
        rdfs:comment """Abstract class for additional text intended to be added to a License, but
which is not itself a standalone License."""@en ;
        rdfs:subClassOf ns1:Element ;
        sh:nodeKind sh:IRI ;
        sh:property _:N0d31a389bc9143c3bafe54fa421e0341,
            _:N4589bfc7dc3f4233a4abb115ddaef820,
            _:N83d1d8ce6a5f4da29db196af54f27038,
            _:Nb20751516ec94669b1cd6f091b402af8,
            _:Nc40a347af0ca48028766e58ea8649917,
            _:Nd572e06c587345cd87d1d4094ca0fadb,
            _:Nda712abeccdd49c09c5c2bc685e05ee4 .

    ns4:VexVulnAssessmentRelationship a owl:Class,
            sh:NodeShape ;
        rdfs:comment "Abstract ancestor class for all VEX relationships"@en ;
        rdfs:subClassOf ns4:VulnAssessmentRelationship ;
        sh:nodeKind sh:IRI ;
        sh:property _:N827d4765f14f49ed9f7cc0b184462699,
            _:N86fa428dffca47ed9477433da6de995f,
            _:Ne85767bf657647678f43e419fe3d7b41 .

    ns2:EnergyConsumptionDescription a owl:Class,
            sh:NodeShape ;
        rdfs:comment """The class that helps note down the quantity of energy consumption and the unit
used for measurement."""@en ;
        sh:nodeKind sh:BlankNodeOrIRI ;
        sh:property _:N49573a6d817241a29c43c15a2355169a,
            _:Nf56f6c0a984245cebdfaf7de7413c7fa .

    ns2:SafetyRiskAssessmentType a owl:Class ;
        rdfs:comment "Specifies the safety risk level."@en .

    ns6:ConfidentialityLevelType a owl:Class ;
        rdfs:comment "Categories of confidentiality level."@en .

    ns4:SsvcDecisionType a owl:Class ;
        rdfs:comment "Specifies the SSVC decision type."@en .

    ns3:SoftwareArtifact a owl:Class,
            sh:NodeShape ;
        rdfs:comment "A distinct article or unit related to Software."@en ;
        rdfs:subClassOf ns1:Artifact ;
        sh:nodeKind sh:IRI ;
        sh:property _:N2d6f29ae54bf4063ae6b902a9d9d0e65,
            _:N30278794a47b432991916e0f8b7edd43,
            _:N369dde9853ee441baf76508a7b5b2087,
            _:N3cb59368bd5246eb9331b056be55010f,
            _:Nce85940987124e80ab8a09c3b530105f,
            _:Ne7bb452ea72c40559a74147d8436b910 .

    ns1:CreationInfo a owl:Class,
            sh:NodeShape ;
        rdfs:comment "Provides information about the creation of the Element."@en ;
        sh:nodeKind sh:BlankNodeOrIRI ;
        sh:property _:N142a867c450d484d86db550e64996345,
            _:N7731592841b44d1f9105c81c87ead7bb,
            _:N826a427a992d4c63a9b10b25d7bb37d2,
            _:Nabdb0a76ad4947e4993004af784ba9b7,
            _:Nb358c8f5280a4bcb8f424632e755e642 .

    ns1:IntegrityMethod a owl:Class,
            sh:NodeShape ;
        rdfs:comment "Provides an independently reproducible mechanism that permits verification of a specific Element."@en ;
        sh:nodeKind sh:BlankNodeOrIRI ;
        sh:property _:N236de371a7df48ee905f0267cb6ca760,
            _:N44f85a5a2d544ce2ac794e36c7150f73 .

    ns6:DatasetAvailabilityType a owl:Class ;
        rdfs:comment "Availability of dataset."@en .

    ns4:VexJustificationType a owl:Class ;
        rdfs:comment "Specifies the VEX justification type."@en .

    ns1:LifecycleScopeType a owl:Class ;
        rdfs:comment "Provide an enumerated set of lifecycle phases that can provide context to relationships."@en .

    ns4:CvssSeverityType a owl:Class ;
        rdfs:comment "Specifies the CVSS base, temporal, threat, or environmental severity type."@en .

    ns4:VulnAssessmentRelationship a owl:Class,
            sh:NodeShape ;
        rdfs:comment "Abstract ancestor class for all vulnerability assessments"@en ;
        rdfs:subClassOf ns1:Relationship ;
        sh:nodeKind sh:IRI ;
        sh:property _:N1668119826b547d294ab973a0b1f44fa,
            _:N4378898d7a4e45aba687da8f75c50a03,
            _:N50ac56aefa494b28ac37f9f5f9fe85c9,
            _:Nb3940c1a89ea40fd93067b312aa7ec47,
            _:Nb926c51e6e424f4d91bff7da1f5c5f5d,
            _:Nd02644afb1dc49c1a5d3579aee9238e5 .

    ns3:SbomType a owl:Class ;
        rdfs:comment """Provides a set of values to be used to describe the common types of SBOMs that
tools may create."""@en .

    ns1:PresenceType a owl:Class ;
        rdfs:comment "Categories of presence or absence."@en .

    ns1:SupportType a owl:Class ;
        rdfs:comment "Indicates the type of support that is associated with an artifact."@en .

    ns1:Agent a owl:Class ;
        rdfs:comment "Agent represents anything with the potential to act on a system."@en ;
        rdfs:subClassOf ns1:Element ;
        sh:nodeKind sh:IRI .

    ns1:ProfileIdentifierType a owl:Class ;
        rdfs:comment "Enumeration of the valid profiles."@en .

    <https://spdx.org/rdf/3.0.1/terms/SimpleLicensing/AnyLicenseInfo> a owl:Class ;
        rdfs:comment "Abstract class representing a license combination consisting of one or more licenses."@en ;
        rdfs:subClassOf ns1:Element ;
        sh:nodeKind sh:IRI ;
        sh:property _:N34abe76a351f47099af1b04cc4cfd9c5 .

    ns1:ExternalIdentifierType a owl:Class ;
        rdfs:comment "Specifies the type of an external identifier."@en .

    ns1:DictionaryEntry a owl:Class,
            sh:NodeShape ;
        rdfs:comment "A key with an associated value."@en ;
        sh:nodeKind sh:BlankNodeOrIRI ;
        sh:property _:N11cf77d03f2047b6a91de3d4c0a81bf3,
            _:Na3ccc8a5475e4877bc9d318834c95e4e .

    ns6:DatasetType a owl:Class ;
        rdfs:comment "Enumeration of dataset types."@en .

    ns1:Element a owl:Class,
            sh:NodeShape ;
        rdfs:comment "Base domain class from which all other SPDX-3.0 domain classes derive."@en ;
        sh:nodeKind sh:IRI ;
        sh:property _:N066a871ed8d14e67989e39b2bd55c848,
            _:N1732a010a6e64fbbb5091d00bdf2e390,
            _:N3198c8321a1240af8c99caf34a2348ae,
            _:N5062d561da4648989b12854ee210a870,
            _:N6d18b467590e4ae986b20549403ebfc4,
            _:Naba532c8417a4c379b511d2a06a9d2fe,
            _:Nb873ceb870fd443ea791544deae8e0ea,
            _:Ncae5f5c7bcc644478c0d7931eff17663,
            _:Ndf3547c4313b46d5a449051395fdc15f,
            _:Nfc923ccf1ea740df81bd77a3cddf7027 .

    ns1:HashAlgorithm a owl:Class ;
        rdfs:comment "A mathematical algorithm that maps data of arbitrary size to a bit string."@en .

    ns3:SoftwarePurpose a owl:Class ;
        rdfs:comment "Provides information about the primary purpose of an Element."@en .

    ns1:ExternalRefType a owl:Class ;
        rdfs:comment "Specifies the type of an external reference."@en .

    ns1:RelationshipType a owl:Class ;
        rdfs:comment "Information about the relationship between two Elements."@en .

    _:N0055f76237eb4d249deebcb85dc89088 rdf:first <https://spdx.org/rdf/3.0.1/terms/Software/SoftwarePurpose/file> ;
        rdf:rest _:Ncd1772ea8f2143b89f9aeaa4912b5ca1 .

    _:N00a75e275a744df5ad99e30ebba988d0 rdf:first <https://spdx.org/rdf/3.0.1/terms/Core/ExternalRefType/documentation> ;
        rdf:rest _:Ncaf5eb2ed5ff4a08aa3c180f3cf81900 .

    _:N015d5660aba34b1ca246001ab6fc6ef7 rdf:first <https://spdx.org/rdf/3.0.1/terms/Core/LifecycleScopeType/test> ;
        rdf:rest _:Nb70a709fefb24fcf8edc194e9535bbe1 .

    _:N04198a73e7ea442393c03cfc23850af1 sh:class ns1:ProfileIdentifierType ;
        sh:in _:N49fb499038de43bcb9ef8aceac34740e ;
        sh:nodeKind sh:IRI ;
        sh:path ns1:profileConformance .

    _:N0424b2581a0d4d4aabfbe49ee71c6de7 sh:class ns1:IntegrityMethod ;
        sh:nodeKind sh:BlankNodeOrIRI ;
        sh:path ns1:verifiedUsing .

    _:N04fbf9eb972a43e08f04e6eee07296c3 rdf:first <https://spdx.org/rdf/3.0.1/terms/Core/HashAlgorithm/sha3_384> ;
        rdf:rest _:N58e74d9233994aba923e2ff87f590d6c .

    _:N058f54e17ad24bb188ce1059e8fb8749 rdf:first <https://spdx.org/rdf/3.0.1/terms/Dataset/DatasetAvailabilityType/directDownload> ;
        rdf:rest _:Nae4301a313374dd297ef6012748ea2da .

    _:N066a871ed8d14e67989e39b2bd55c848 sh:datatype xsd:string ;
        sh:maxCount 1 ;
        sh:nodeKind sh:Literal ;
        sh:path ns1:description .

    _:N077c921cc7f44e75920b8add30c76513 rdf:first <https://spdx.org/rdf/3.0.1/terms/Security/CvssSeverityType/high> ;
        rdf:rest _:Ncb100fcbde1f40d78a139ebc861c1dc3 .

    _:N07b0761fa8a5417ebb12637ce7c825a3 rdf:first <https://spdx.org/rdf/3.0.1/terms/Software/SoftwarePurpose/documentation> ;
        rdf:rest _:Na7e4738fe27648738164082e104e7554 .

    _:N07b7170e552e4a4796c656e12821a04e rdf:first <https://spdx.org/rdf/3.0.1/terms/Security/CvssSeverityType/low> ;
        rdf:rest _:Nd9e9103cee9c41ea980d92b72d415fa7 .

    _:N07f2acb5ed1f4a24bc28f6fc41863899 rdf:first <https://spdx.org/rdf/3.0.1/terms/Core/ExternalRefType/buildSystem> ;
        rdf:rest _:N2b01dd2f246a421a99790003422f7bf5 .

    _:N08c8d3c9a7fb4e99847505287f582007 rdf:first <https://spdx.org/rdf/3.0.1/terms/Core/LifecycleScopeType/development> ;
        rdf:rest _:N5bcf96480af248baace930d2e86442eb .

    _:N0921a60ce67049798ca7d56bcdec6dab sh:datatype xsd:string ;
        sh:maxCount 1 ;
        sh:nodeKind sh:Literal ;
        sh:path ns1:comment .

    _:N09b7681fb0c84e70b5e00f3f608f8a57 rdf:first <https://spdx.org/rdf/3.0.1/terms/Core/RelationshipType/foundBy> ;
        rdf:rest _:N77174bb20392458ca2d4327110d21509 .

    _:N0c13a3aec38c42dc9974cb19f9083ffa rdf:first <https://spdx.org/rdf/3.0.1/terms/Software/SoftwarePurpose/other> ;
        rdf:rest _:N64f93ff472734041b10fdc6d28dfa4fb .

    _:N0ce73a98987540c29f974f5ff5da483f rdf:first <https://spdx.org/rdf/3.0.1/terms/Core/PresenceType/no> ;
        rdf:rest _:Nb0268a8c77ec4002a3462358e1880e18 .

    _:N0d31a389bc9143c3bafe54fa421e0341 sh:datatype xsd:string ;
        sh:maxCount 1 ;
        sh:nodeKind sh:Literal ;
        sh:path ns5:licenseXml .

    _:N0d825a0c45ee44bca0cb57c439a3a445 sh:datatype xsd:dateTimeStamp ;
        sh:maxCount 1 ;
        sh:nodeKind sh:Literal ;
        sh:path ns4:impactStatementTime ;
        sh:pattern "^\\d\\d\\d\\d-\\d\\d-\\d\\dT\\d\\d:\\d\\d:\\d\\dZ$" .

    _:N0db09bc77e6147aaa587b2360854742c rdf:first <https://spdx.org/rdf/3.0.1/terms/Core/ExternalRefType/metrics> ;
        rdf:rest _:Nea67e787267c4806a636ab1b755ac4c2 .

    _:N0de811ecc9ec4518b617ae1b51981680 rdf:first <https://spdx.org/rdf/3.0.1/terms/Core/HashAlgorithm/sha3_224> ;
        rdf:rest _:N1211087f69bf40c6bf514935852d9b2e .

    _:N0e1da744a23f43e19fc21d07c44f8dbc rdf:first <https://spdx.org/rdf/3.0.1/terms/Core/HashAlgorithm/falcon> ;
        rdf:rest _:Nf3b79d08d7a146179b7b5d74e752f9e9 .

    _:N0e42e2b59c914ea49f056fa11e0247af sh:class ns6:ConfidentialityLevelType ;
        sh:in _:N3db69ed93b0e4a72a55385089dcfdb33 ;
        sh:maxCount 1 ;
        sh:nodeKind sh:IRI ;
        sh:path ns6:confidentialityLevel .

    _:N0e59217e851a4ed5aa13df590bab757a rdf:first <https://spdx.org/rdf/3.0.1/terms/Software/SoftwarePurpose/test> ;
        rdf:rest () .

    _:N0ef2938545be4fd1ae2cb24839f79535 rdf:first <https://spdx.org/rdf/3.0.1/terms/Software/SoftwarePurpose/requirement> ;
        rdf:rest _:Nf91ae204c3344f3dbfe89daa20fec99d .

    _:N10108a0536bb489f88b2fe61aae33caa sh:datatype xsd:string ;
        sh:maxCount 1 ;
        sh:nodeKind sh:Literal ;
        sh:path ns1:comment .

    _:N11bf493c9a9d45a5a782561a62bededf rdf:first <https://spdx.org/rdf/3.0.1/terms/Software/SoftwarePurpose/patch> ;
        rdf:rest _:N2aef0b5e25944c678ead8271018a992d .

    _:N11cf77d03f2047b6a91de3d4c0a81bf3 sh:datatype xsd:string ;
        sh:maxCount 1 ;
        sh:nodeKind sh:Literal ;
        sh:path ns1:value .

    _:N1211087f69bf40c6bf514935852d9b2e rdf:first <https://spdx.org/rdf/3.0.1/terms/Core/HashAlgorithm/sha3_256> ;
        rdf:rest _:N5cb5df020da54023a0414a7b6630c2dc .

    _:N12bda6abdf98496c9a1d5833ce99465e rdf:first <https://spdx.org/rdf/3.0.1/terms/Dataset/DatasetType/sensor> ;
        rdf:rest _:N37da02b57bb245d2b3edacd9f6c17290 .

    _:N13ceb50f498b427f8678e0084e8f5ace sh:hasValue <https://spdx.org/rdf/3.0.1/terms/Extension/Extension> .

    _:N142a867c450d484d86db550e64996345 sh:datatype xsd:dateTimeStamp ;
        sh:maxCount 1 ;
        sh:minCount 1 ;
        sh:nodeKind sh:Literal ;
        sh:path ns1:created ;
        sh:pattern "^\\d\\d\\d\\d-\\d\\d-\\d\\dT\\d\\d:\\d\\d:\\d\\dZ$" .

    _:N143985a756e44389b9f2dd3a852b8a0b rdf:first <https://spdx.org/rdf/3.0.1/terms/Core/ExternalIdentifierType/email> ;
        rdf:rest _:N54e5abc4b90c409dad8d267544c234b8 .

    _:N144fb0311d3c4636853d832cd22c617d rdf:first <https://spdx.org/rdf/3.0.1/terms/Software/SoftwarePurpose/deviceDriver> ;
        rdf:rest _:Neddd67434de24b47b73290d608b6f7fe .

    _:N145fd66cc8f7451a9314fd48034adb1a rdf:first <https://spdx.org/rdf/3.0.1/terms/Core/ExternalRefType/securityAdvisory> ;
        rdf:rest _:N9c4632e5374e4c0e943bd16b59a9edd3 .

    _:N15137679a21c43828dd693e3a1badc84 rdf:first <https://spdx.org/rdf/3.0.1/terms/AI/EnergyUnitType/megajoule> ;
        rdf:rest _:N88a5ef940b0c4ebbbcdc22280bec27ce .

    _:N15521aa0152f4af5a3545aa71f2c4b78 sh:datatype xsd:dateTimeStamp ;
        sh:maxCount 1 ;
        sh:nodeKind sh:Literal ;
        sh:path <https://spdx.org/rdf/3.0.1/terms/Build/buildEndTime> ;
        sh:pattern "^\\d\\d\\d\\d-\\d\\d-\\d\\dT\\d\\d:\\d\\d:\\d\\dZ$" .

    _:N1599c92508f549eeadacc4250040a171 sh:class ns1:AnnotationType ;
        sh:in _:Nf2f53884af9d4eb2a1400a9c7c189a80 ;
        sh:maxCount 1 ;
        sh:minCount 1 ;
        sh:nodeKind sh:IRI ;
        sh:path ns1:annotationType .

    _:N15b8d7dbed8a4fe19ecbbc9433b7daf2 rdf:first <https://spdx.org/rdf/3.0.1/terms/Software/SoftwarePurpose/platform> ;
        rdf:rest _:N0ef2938545be4fd1ae2cb24839f79535 .

    _:N1668119826b547d294ab973a0b1f44fa sh:datatype xsd:dateTimeStamp ;
        sh:maxCount 1 ;
        sh:nodeKind sh:Literal ;
        sh:path ns4:withdrawnTime ;
        sh:pattern "^\\d\\d\\d\\d-\\d\\d-\\d\\dT\\d\\d:\\d\\d:\\d\\dZ$" .

    _:N1717d17447d649a2b154d555a39a5bd1 rdf:first <https://spdx.org/rdf/3.0.1/terms/Core/RelationshipType/hasEvidence> ;
        rdf:rest _:N591e1d014a0149b78d304cb4bee48359 .

    _:N1732a010a6e64fbbb5091d00bdf2e390 sh:class ns1:ExternalIdentifier ;
        sh:nodeKind sh:BlankNodeOrIRI ;
        sh:path ns1:externalIdentifier .

    _:N17835996c18345acb753167a8e04a7e7 rdf:first <https://spdx.org/rdf/3.0.1/terms/Dataset/DatasetType/text> ;
        rdf:rest _:N737b16f66b5e4fa4bb411e7725fd81ff .

    _:N17b11e9782cb42ceba98928679b0f78b sh:datatype xsd:anyURI ;
        sh:maxCount 1 ;
        sh:minCount 1 ;
        sh:nodeKind sh:Literal ;
        sh:path <https://spdx.org/rdf/3.0.1/terms/Build/buildType> .

    _:N19ca4558cdb341ee9c37bfe7dbd5725f sh:datatype xsd:string ;
        sh:nodeKind sh:Literal ;
        sh:path ns2:typeOfModel .

    _:N1a67920cb6604510b2f1857dabdf44c4 sh:hasValue ns1:IntegrityMethod .

    _:N1a98fafcbfca426eb77dc5e8d4edfe45 rdf:first <https://spdx.org/rdf/3.0.1/terms/Core/HashAlgorithm/adler32> ;
        rdf:rest _:Ne761637246cf43209f897d0766c1ff4b .

    _:N1acf963fc18642aeb4fd5e352a34b64a rdf:first <https://spdx.org/rdf/3.0.1/terms/Security/VexJustificationType/vulnerableCodeNotInExecutePath> ;
        rdf:rest _:Nb93310f68d2e4dd79db3e0e8f3d9faec .

    _:N1ae6ad8ea0d143daba2c967f177264a0 rdf:first <https://spdx.org/rdf/3.0.1/terms/Core/RelationshipType/fixedIn> ;
        rdf:rest _:N09b7681fb0c84e70b5e00f3f608f8a57 .

    _:N1b70e585aedf4769b01c68baae40b4f4 rdf:first <https://spdx.org/rdf/3.0.1/terms/Dataset/DatasetAvailabilityType/registration> ;
        rdf:rest _:N6254eb0c38204b3b809ee94f2ea1e3f1 .

    _:N1be37168f2354f8aa16fac868e264502 rdf:first <https://spdx.org/rdf/3.0.1/terms/Software/SbomType/build> ;
        rdf:rest _:N69d74818048847a386ab183dd27d4165 .

    _:N1d060b61efbb4904bb56b16b3884b365 rdf:first <https://spdx.org/rdf/3.0.1/terms/Core/ExternalRefType/mailingList> ;
        rdf:rest _:Nc0140fcc182b4ab38eff7add9d74a59f .

    _:N1d0f7a3442d1402692990d48696cca6e rdf:first <https://spdx.org/rdf/3.0.1/terms/Core/ExternalRefType/staticAnalysisReport> ;
        rdf:rest _:N785dc2563b5b478aa13fdc122753beea .

    _:N1e9da875ffa041578e3c8769129e85f2 rdf:first <https://spdx.org/rdf/3.0.1/terms/Core/HashAlgorithm/md5> ;
        rdf:rest _:Nbb9bd3c264b5448dad629d6045fe3eaf .

    _:N1eceff509a414ae0a364c00261c99d82 sh:datatype xsd:string ;
        sh:maxCount 1 ;
        sh:minCount 1 ;
        sh:nodeKind sh:Literal ;
        sh:path <https://spdx.org/rdf/3.0.1/terms/Extension/cdxPropName> .

    _:N1f22a6fa2025402ebb1d66bae0bbfd63 sh:datatype xsd:string ;
        sh:nodeKind sh:Literal ;
        sh:path ns2:modelDataPreprocessing .

    _:N1f7ae52072c64db5a97e800f01cabe74 rdf:first <https://spdx.org/rdf/3.0.1/terms/Core/RelationshipType/hasOutput> ;
        rdf:rest _:N96974ebfb89648cb9f4323f638c46390 .

    _:N23238f039f16407faa4dfddc2d622573 sh:class <https://spdx.org/rdf/3.0.1/terms/SimpleLicensing/AnyLicenseInfo> ;
        sh:minCount 2 ;
        sh:nodeKind sh:IRI ;
        sh:path ns5:member .

    _:N236de371a7df48ee905f0267cb6ca760 sh:message "https://spdx.org/rdf/3.0.1/terms/Core/IntegrityMethod is an abstract class and should not be instantiated directly. Instantiate a subclass instead."@en ;
        sh:not _:N1a67920cb6604510b2f1857dabdf44c4 ;
        sh:path rdf:type .

    _:N241832593c8748c0b8e5815721925b63 rdf:first <https://spdx.org/rdf/3.0.1/terms/Core/RelationshipType/testedOn> ;
        rdf:rest _:Nff823a63d7084b458218a829ce330580 .

    _:N2591b91740354a0ead11f5294ea11e44 rdf:first <https://spdx.org/rdf/3.0.1/terms/Core/RelationshipType/hasDynamicLink> ;
        rdf:rest _:N1717d17447d649a2b154d555a39a5bd1 .

    _:N25f14b85810e4dfcb200429bde931173 rdf:first <https://spdx.org/rdf/3.0.1/terms/Core/ExternalRefType/altDownloadLocation> ;
        rdf:rest _:Ncb08ebb7079c43059ae88abc8e6192ba .

    _:N264db893a85d4367bd49adef5d62f643 rdf:first <https://spdx.org/rdf/3.0.1/terms/Core/HashAlgorithm/crystalsKyber> ;
        rdf:rest _:N43db92f0924e475f9d2e9ab9239650de .

    _:N265fe36ac5d944b0975defd743c05a30 rdf:first <https://spdx.org/rdf/3.0.1/terms/Core/HashAlgorithm/md5> ;
        rdf:rest _:N8e47b331646c4f46b0249c7d7101ed4a .

    _:N27000931246a42d2886129c31ac2dcc7 rdf:first <https://spdx.org/rdf/3.0.1/terms/Core/ExternalRefType/securityOther> ;
        rdf:rest _:N91d59f3e252f4ccfacb8cf348a59dca2 .

    _:N277e37dd63f24c76a29e15a02660e003 sh:class ns5:ExtendableLicense ;
        sh:maxCount 1 ;
        sh:minCount 1 ;
        sh:nodeKind sh:IRI ;
        sh:path ns5:subjectExtendableLicense .

    _:N286dd473156f45b1bed255af1c1ce34e rdf:first <https://spdx.org/rdf/3.0.1/terms/Core/ExternalRefType/securityPolicy> ;
        rdf:rest _:N2c358c96db174e829d5360e861b9e429 .

    _:N28a0bff75a6a4d848f221f7c6e6c333e rdf:first <https://spdx.org/rdf/3.0.1/terms/Dataset/ConfidentialityLevelType/amber> ;
        rdf:rest _:N8bedee90de324e0ca9f0bf438f29e49d .

    _:N2941fbec200e4a24a6b288efdccf9f61 rdf:first <https://spdx.org/rdf/3.0.1/terms/Software/SbomType/design> ;
        rdf:rest _:N9923bb8ce2714e80aed0235ac5044f48 .

    _:N29cee72ea302413db6fb90c4cf46a270 rdf:first <https://spdx.org/rdf/3.0.1/terms/Software/SoftwarePurpose/module> ;
        rdf:rest _:N48c89febf7304b21992546e6b7c521e2 .

    _:N29eb269c4389443f8ded26f8ac3ba6b6 sh:class ns1:DictionaryEntry ;
        sh:nodeKind sh:BlankNodeOrIRI ;
        sh:path ns2:metricDecisionThreshold .

    _:N2aca376e7fa643248d0ae1615af9bc14 sh:datatype xsd:string ;
        sh:maxCount 1 ;
        sh:nodeKind sh:Literal ;
        sh:path ns5:deprecatedVersion .

    _:N2aef0b5e25944c678ead8271018a992d rdf:first <https://spdx.org/rdf/3.0.1/terms/Software/SoftwarePurpose/platform> ;
        rdf:rest _:Nd7fa1d4fbb0a46e39831eeb358241747 .

    _:N2b01dd2f246a421a99790003422f7bf5 rdf:first <https://spdx.org/rdf/3.0.1/terms/Core/ExternalRefType/chat> ;
        rdf:rest _:N8f02949295a84de8b9950130e13d33e2 .

    _:N2c00f81f03274496b7c4c8ab8bf09b2a sh:datatype xsd:string ;
        sh:maxCount 1 ;
        sh:nodeKind sh:Literal ;
        sh:path ns1:contentType ;
        sh:pattern "^[^\\/]+\\/[^\\/]+$" .

    _:N2c30cc006c0c4e83beca0905093f5d8a rdf:first <https://spdx.org/rdf/3.0.1/terms/Core/RelationshipType/copiedTo> ;
        rdf:rest _:Nc83c7ff0a3a746feab4b5250822afaad .

    _:N2c358c96db174e829d5360e861b9e429 rdf:first <https://spdx.org/rdf/3.0.1/terms/Core/ExternalRefType/securityThreatModel> ;
        rdf:rest _:N90beb5cae77044a7865d4fa65f54cadb .

    _:N2c39a98a694448f6aa6a7b9a28962f36 rdf:first <https://spdx.org/rdf/3.0.1/terms/Core/HashAlgorithm/sha384> ;
        rdf:rest _:Ne81a57a701844ae68d91471cca52a8d2 .

    _:N2d48f33c49aa4655a422188c69928cd8 sh:class ns1:Element ;
        sh:minCount 1 ;
        sh:nodeKind sh:IRI ;
        sh:path ns1:to .

    _:N2d6f29ae54bf4063ae6b902a9d9d0e65 sh:class ns3:SoftwarePurpose ;
        sh:in _:Na28e863b0b24448aaf988665801a3d38 ;
        sh:nodeKind sh:IRI ;
        sh:path ns3:additionalPurpose .

    _:N2f234aa991c24d8d8673af6d5de553f9 rdf:first <https://spdx.org/rdf/3.0.1/terms/Security/CvssSeverityType/critical> ;
        rdf:rest _:N077c921cc7f44e75920b8add30c76513 .

    _:N2f453dff5c3d4aeb9eeca1c273089f5d sh:class ns3:ContentIdentifierType ;
        sh:in _:N81e6654c1a534dc8b23f469162487360 ;
        sh:maxCount 1 ;
        sh:minCount 1 ;
        sh:nodeKind sh:IRI ;
        sh:path ns3:contentIdentifierType .

    _:N2f649d29104c43b194e0945809fea0bb rdf:first <https://spdx.org/rdf/3.0.1/terms/Core/RelationshipType/coordinatedBy> ;
        rdf:rest _:N2c30cc006c0c4e83beca0905093f5d8a .

    _:N30278794a47b432991916e0f8b7edd43 sh:message "https://spdx.org/rdf/3.0.1/terms/Software/SoftwareArtifact is an abstract class and should not be instantiated directly. Instantiate a subclass instead."@en ;
        sh:not _:Nb8cfa0626ffe40b4bf076a3698bb7221 ;
        sh:path rdf:type .

    _:N308ac8913c6440c68ef5331eaaef0508 sh:datatype xsd:string ;
        sh:maxCount 1 ;
        sh:nodeKind sh:Literal ;
        sh:path ns6:dataCollectionProcess .

    _:N315f408bdbab45dab111243059344360 rdf:first <https://spdx.org/rdf/3.0.1/terms/Core/RelationshipType/hasAddedFile> ;
        rdf:rest _:N4104c04bd5fa4771893e092c07799fa5 .

    _:N3198c8321a1240af8c99caf34a2348ae sh:datatype xsd:string ;
        sh:maxCount 1 ;
        sh:nodeKind sh:Literal ;
        sh:path ns1:comment .

    _:N32ea05029eca4d0cb9b3191393efdb1c sh:class ns1:PresenceType ;
        sh:in _:N93d18c08169a49b08ba0231691a7a086 ;
        sh:maxCount 1 ;
        sh:nodeKind sh:IRI ;
        sh:path ns2:useSensitivePersonalInformation .

    _:N335cac8b2f044be299cfb9d7abd78951 rdf:first <https://spdx.org/rdf/3.0.1/terms/Core/RelationshipType/hasSpecification> ;
        rdf:rest _:N83403ff4e6134ab283336f5b2abf62bb .

    _:N341b65da06ac49e990a60307d9c787ac rdf:first <https://spdx.org/rdf/3.0.1/terms/Core/ExternalIdentifierType/cpe22> ;
        rdf:rest _:Ndb95de258758441cb6ae88d3925e8f63 .

    _:N34851da2662f43dfba6075ee0badd951 rdf:first <https://spdx.org/rdf/3.0.1/terms/Security/SsvcDecisionType/track> ;
        rdf:rest _:N7bc39608ff4147fbb303dec6bc5b0c7a .

    _:N34abe76a351f47099af1b04cc4cfd9c5 sh:message "https://spdx.org/rdf/3.0.1/terms/SimpleLicensing/AnyLicenseInfo is an abstract class and should not be instantiated directly. Instantiate a subclass instead."@en ;
        sh:not _:N5c04428de4e14d74824de2780dc99cbb ;
        sh:path rdf:type .

    _:N3523f55fb2c04444a15f8bf5108e4f4d rdf:first <https://spdx.org/rdf/3.0.1/terms/Core/ExternalRefType/funding> ;
        rdf:rest _:N6dfda762ba7a4348b0dfbb53ab48e812 .

    _:N354ff8b540a0427a97dc3c7fe3fcaba2 sh:datatype xsd:string ;
        sh:maxCount 1 ;
        sh:nodeKind sh:Literal ;
        sh:path ns5:deprecatedVersion .

    _:N363c77746fe14d01b9156613c76390e7 sh:class ns2:EnergyConsumptionDescription ;
        sh:nodeKind sh:BlankNodeOrIRI ;
        sh:path ns2:inferenceEnergyConsumption .

    _:N369dde9853ee441baf76508a7b5b2087 sh:class ns3:ContentIdentifier ;
        sh:nodeKind sh:BlankNodeOrIRI ;
        sh:path ns3:contentIdentifier .

    _:N370ed73a1c1e4ff09d768ae422e135dd sh:datatype xsd:string ;
        sh:maxCount 1 ;
        sh:nodeKind sh:Literal ;
        sh:path ns2:informationAboutTraining .

    _:N37da02b57bb245d2b3edacd9f6c17290 rdf:first <https://spdx.org/rdf/3.0.1/terms/Dataset/DatasetType/structured> ;
        rdf:rest _:Ne3190c214db5431e89558087e85a5b81 .

    _:N37db31524a794bbd8b57460903c356d7 rdf:first <https://spdx.org/rdf/3.0.1/terms/Core/RelationshipType/hasInput> ;
        rdf:rest _:Nb28b73f573b7440bbbbf82e84e8e8b21 .

    _:N37ea1088bfd243d5a54936253404904a rdf:first <https://spdx.org/rdf/3.0.1/terms/Core/HashAlgorithm/sha256> ;
        rdf:rest _:Nd79c9dbb4e544a9d890ab2c44df9dc6d .

    _:N3823ee9f07c34e0ca71f9c6c5354ad8d rdf:first <https://spdx.org/rdf/3.0.1/terms/Software/SoftwarePurpose/data> ;
        rdf:rest _:Nd3bbfec37f114f2ba626d3e104fe8b99 .

    _:N389d3e9e81e74e3797b180d81edca2e0 sh:message "https://spdx.org/rdf/3.0.1/terms/ExpandedLicensing/ExtendableLicense is an abstract class and should not be instantiated directly. Instantiate a subclass instead."@en ;
        sh:not _:Nba9d94c6ccef43378e341caf081b2205 ;
        sh:path rdf:type .

    _:N392736ad660c4444b162925f2f85a971 sh:datatype xsd:decimal ;
        sh:maxCount 1 ;
        sh:minCount 1 ;
        sh:nodeKind sh:Literal ;
        sh:path ns4:score .

    _:N3963aaabe6d3491399d37f148c43248a rdf:first <https://spdx.org/rdf/3.0.1/terms/Software/SoftwarePurpose/deviceDriver> ;
        rdf:rest _:N07b0761fa8a5417ebb12637ce7c825a3 .

    _:N39c989915c2d4c92b69c3a9dedcf3c7a rdf:first <https://spdx.org/rdf/3.0.1/terms/Core/ProfileIdentifierType/lite> ;
        rdf:rest () .

    _:N3aa7cebacf8742c3893b955cd12bf58c rdf:first <https://spdx.org/rdf/3.0.1/terms/Core/AnnotationType/review> ;
        rdf:rest () .

    _:N3cb59368bd5246eb9331b056be55010f sh:datatype xsd:string ;
        sh:nodeKind sh:Literal ;
        sh:path ns3:attributionText .

    _:N3ce7cee25ad3415e976ed9d7b79b0394 rdf:first <https://spdx.org/rdf/3.0.1/terms/Security/VexJustificationType/vulnerableCodeCannotBeControlledByAdversary> ;
        rdf:rest _:N1acf963fc18642aeb4fd5e352a34b64a .

    _:N3cf836c0e1cc41a780ab94e0d629cfc8 sh:class ns1:Hash ;
        sh:nodeKind sh:BlankNodeOrIRI ;
        sh:path <https://spdx.org/rdf/3.0.1/terms/Build/configSourceDigest> .

    _:N3d3db55210ce441eb305cdf967d96a2d sh:datatype xsd:anyURI ;
        sh:nodeKind sh:Literal ;
        sh:path <https://spdx.org/rdf/3.0.1/terms/Build/configSourceUri> .

    _:N3db69ed93b0e4a72a55385089dcfdb33 rdf:first <https://spdx.org/rdf/3.0.1/terms/Dataset/ConfidentialityLevelType/red> ;
        rdf:rest _:N28a0bff75a6a4d848f221f7c6e6c333e .

    _:N3e29af3bed3d478b8963ae1822aa1c32 sh:datatype xsd:boolean ;
        sh:maxCount 1 ;
        sh:nodeKind sh:Literal ;
        sh:path ns5:isDeprecatedLicenseId .

    _:N3f1160e3da0e48f5a7f879d3089bc895 sh:datatype xsd:anyURI ;
        sh:maxCount 1 ;
        sh:nodeKind sh:Literal ;
        sh:path ns1:locationHint .

    _:N40fa50df7da84543bc78883423152ecb rdf:first <https://spdx.org/rdf/3.0.1/terms/Core/HashAlgorithm/blake2b256> ;
        rdf:rest _:N4beef7ef5ea448f3a28d449ca84cb60f .

    _:N4104c04bd5fa4771893e092c07799fa5 rdf:first <https://spdx.org/rdf/3.0.1/terms/Core/RelationshipType/hasAssessmentFor> ;
        rdf:rest _:N5f5c21c2ca56420e9b21ac77bfae6cb9 .

    _:N419d1972d24c46fd83927a9917e8ca7d rdf:first <https://spdx.org/rdf/3.0.1/terms/Security/SsvcDecisionType/act> ;
        rdf:rest _:N6b000a1e4c674af7918e4f41aabac3e5 .

    _:N41c9b9a507de47d4a519c0b6be4c3019 sh:datatype xsd:dateTimeStamp ;
        sh:maxCount 1 ;
        sh:nodeKind sh:Literal ;
        sh:path ns1:releaseTime ;
        sh:pattern "^\\d\\d\\d\\d-\\d\\d-\\d\\dT\\d\\d:\\d\\d:\\d\\dZ$" .

    _:N42136f4bf09e450cba628f5056116c44 rdf:first <https://spdx.org/rdf/3.0.1/terms/Software/SoftwarePurpose/manifest> ;
        rdf:rest _:Na6c5560266a54e1ba3c5fff179ece5c0 .

    _:N424a5985e65648579f3f351d5ddcbe9a sh:datatype xsd:string ;
        sh:maxCount 1 ;
        sh:nodeKind sh:Literal ;
        sh:path ns5:listVersionAdded .

    _:N434acd04bf4f4e8e98eb06fc4e5a571e rdf:first <https://spdx.org/rdf/3.0.1/terms/Core/HashAlgorithm/crystalsDilithium> ;
        rdf:rest _:N4dcfce52954c4b5bab377b22afbe3f58 .

    _:N4378898d7a4e45aba687da8f75c50a03 sh:class ns1:Agent ;
        sh:maxCount 1 ;
        sh:nodeKind sh:IRI ;
        sh:path ns1:suppliedBy .

    _:N43db92f0924e475f9d2e9ab9239650de rdf:first <https://spdx.org/rdf/3.0.1/terms/Core/HashAlgorithm/falcon> ;
        rdf:rest _:N866ac4b0ae744cccbb182a6c431cf182 .

    _:N445a5c48a1f14e23b5b70e2bfbc3948b rdf:first <https://spdx.org/rdf/3.0.1/terms/Core/RelationshipType/hasOptionalDependency> ;
        rdf:rest _:N1f7ae52072c64db5a97e800f01cabe74 .

    _:N44f85a5a2d544ce2ac794e36c7150f73 sh:datatype xsd:string ;
        sh:maxCount 1 ;
        sh:nodeKind sh:Literal ;
        sh:path ns1:comment .

    _:N45063856b753439d8cf82d7fee02490e sh:class ns1:RelationshipType ;
        sh:in _:N5a131180d5ee42c6924c671e204fea68 ;
        sh:maxCount 1 ;
        sh:minCount 1 ;
        sh:nodeKind sh:IRI ;
        sh:path ns1:relationshipType .

    _:N456a031dc13e4a0e956d1c1983fc6234 rdf:first <https://spdx.org/rdf/3.0.1/terms/Core/RelationshipType/hasProvidedDependency> ;
        rdf:rest _:N4ff568b72cd848bbaddc66ccfba4d839 .

    _:N4589bfc7dc3f4233a4abb115ddaef820 sh:message "https://spdx.org/rdf/3.0.1/terms/ExpandedLicensing/LicenseAddition is an abstract class and should not be instantiated directly. Instantiate a subclass instead."@en ;
        sh:not _:N833037d94cbe4a28b7d115fbffced3f7 ;
        sh:path rdf:type .

    _:N45c6754475234fb3981040e1eb691220 sh:datatype xsd:string ;
        sh:maxCount 1 ;
        sh:nodeKind sh:Literal ;
        sh:path ns4:impactStatement .

    _:N46c085d9b83f4ef3b53633491f4e362a sh:datatype xsd:string ;
        sh:maxCount 1 ;
        sh:nodeKind sh:Literal ;
        sh:path ns1:contentType ;
        sh:pattern "^[^\\/]+\\/[^\\/]+$" .

    _:N471e042c9abf46e69e190e4a59ac0d24 rdf:first <https://spdx.org/rdf/3.0.1/terms/Software/SoftwarePurpose/bom> ;
        rdf:rest _:Nc461500b62594ca3bda4bc0a9780673b .

    _:N477d8d78964845ceba553659dc2db168 rdf:first <https://spdx.org/rdf/3.0.1/terms/Core/RelationshipType/hasTestCase> ;
        rdf:rest _:N7459ec882b2e4d8e802d52e7a2b74ef9 .

    _:N47fb54a94ed9447280f7321c48e2982b sh:class ns1:PresenceType ;
        sh:in _:Na4040cdcb4ed4696ad904d1a44fe4aec ;
        sh:maxCount 1 ;
        sh:nodeKind sh:IRI ;
        sh:path ns2:autonomyType .

    _:N482bb00385844dc6b842a414c6156a37 sh:message "https://spdx.org/rdf/3.0.1/terms/Core/ElementCollection is an abstract class and should not be instantiated directly. Instantiate a subclass instead."@en ;
        sh:not _:Nc9e50174e3d448448737206a174eb9e1 ;
        sh:path rdf:type .

    _:N48c89febf7304b21992546e6b7c521e2 rdf:first <https://spdx.org/rdf/3.0.1/terms/Software/SoftwarePurpose/operatingSystem> ;
        rdf:rest _:N0c13a3aec38c42dc9974cb19f9083ffa .

    _:N4917b1e13e4948c3ba296ae65637fe94 sh:datatype xsd:boolean ;
        sh:maxCount 1 ;
        sh:nodeKind sh:Literal ;
        sh:path ns5:isOsiApproved .

    _:N49255f1d76a848aa802391a2afe0cbe1 sh:class ns1:PositiveIntegerRange ;
        sh:maxCount 1 ;
        sh:nodeKind sh:BlankNodeOrIRI ;
        sh:path ns3:lineRange .

    _:N49573a6d817241a29c43c15a2355169a sh:datatype xsd:decimal ;
        sh:maxCount 1 ;
        sh:minCount 1 ;
        sh:nodeKind sh:Literal ;
        sh:path ns2:energyQuantity .

    _:N49fb499038de43bcb9ef8aceac34740e rdf:first <https://spdx.org/rdf/3.0.1/terms/Core/ProfileIdentifierType/core> ;
        rdf:rest _:N5813afc202be42548985f66dd533b449 .

    _:N49fc85ac4b3e4255965bec1092f3b0bf sh:class ns2:EnergyConsumptionDescription ;
        sh:nodeKind sh:BlankNodeOrIRI ;
        sh:path ns2:finetuningEnergyConsumption .

    _:N4a2164f0942e45a196c2f32e1eb124aa rdf:first <https://spdx.org/rdf/3.0.1/terms/Core/ExternalRefType/riskAssessment> ;
        rdf:rest _:Nbf306a0291d44bd6b1f42fc2c74225df .

    _:N4a711386f320400fa625658b20fcaece rdf:first <https://spdx.org/rdf/3.0.1/terms/Core/ProfileIdentifierType/simpleLicensing> ;
        rdf:rest _:Ncffed33ec761432298dbbe9a975cab49 .

    _:N4aa50d0271014a36b5d3cbddad0a30f3 rdf:first <https://spdx.org/rdf/3.0.1/terms/Security/CvssSeverityType/critical> ;
        rdf:rest _:Nc7472f25ff1a48419a5476b02e425121 .

    _:N4acbfeca863a47f48ea0ccfc2d69b6c6 sh:datatype xsd:string ;
        sh:maxCount 1 ;
        sh:nodeKind sh:Literal ;
        sh:path ns6:intendedUse .

    _:N4ae21911384f4b8ba646f7789dce9351 rdf:first <https://spdx.org/rdf/3.0.1/terms/Core/RelationshipType/hasConcludedLicense> ;
        rdf:rest _:Nd270bd036dc54b30ae14d2e15e4efc18 .

    _:N4beef7ef5ea448f3a28d449ca84cb60f rdf:first <https://spdx.org/rdf/3.0.1/terms/Core/HashAlgorithm/blake2b384> ;
        rdf:rest _:N5ad39dcdd3c84f519f77a0cca2985866 .

    _:N4dcfce52954c4b5bab377b22afbe3f58 rdf:first <https://spdx.org/rdf/3.0.1/terms/Core/HashAlgorithm/crystalsKyber> ;
        rdf:rest _:N0e1da744a23f43e19fc21d07c44f8dbc .

    _:N4f0b7830361d4b38bff91506e120cb77 sh:class ns4:SsvcDecisionType ;
        sh:in _:N419d1972d24c46fd83927a9917e8ca7d ;
        sh:maxCount 1 ;
        sh:minCount 1 ;
        sh:nodeKind sh:IRI ;
        sh:path ns4:decisionType .

    _:N4fc5b94e528a42f7afe6c41473174094 sh:datatype xsd:string ;
        sh:nodeKind sh:Literal ;
        sh:path ns1:packageVerificationCodeExcludedFile .

    _:N4ff24d426d9d4742af402bb81fac3595 rdf:first <https://spdx.org/rdf/3.0.1/terms/Software/SoftwarePurpose/evidence> ;
        rdf:rest _:N8aa30e7bba764b98a907f64507d46c15 .

    _:N4ff568b72cd848bbaddc66ccfba4d839 rdf:first <https://spdx.org/rdf/3.0.1/terms/Core/RelationshipType/hasRequirement> ;
        rdf:rest _:N335cac8b2f044be299cfb9d7abd78951 .

    _:N5062d561da4648989b12854ee210a870 sh:class ns1:IntegrityMethod ;
        sh:nodeKind sh:BlankNodeOrIRI ;
        sh:path ns1:verifiedUsing .

    _:N50ac56aefa494b28ac37f9f5f9fe85c9 sh:message "https://spdx.org/rdf/3.0.1/terms/Security/VulnAssessmentRelationship is an abstract class and should not be instantiated directly. Instantiate a subclass instead."@en ;
        sh:not _:N87ae6f2c35244fb3828abd80ac3d36af ;
        sh:path rdf:type .

    _:N51872cae29bf4b38b2304fa980844191 rdf:first <https://spdx.org/rdf/3.0.1/terms/Core/HashAlgorithm/other> ;
        rdf:rest _:N6176b4e9374646ff969084bff63ba5d8 .

    _:N51aef2d74cdd4cacb76c17b047be429e rdf:first <https://spdx.org/rdf/3.0.1/terms/Software/SoftwarePurpose/diskImage> ;
        rdf:rest _:N144fb0311d3c4636853d832cd22c617d .

    _:N51e95bcda10e477fb13d33c114b9440e sh:class ns1:RelationshipCompleteness ;
        sh:in _:Nb45b5d6cdcf54be991e8c990a24f18f1 ;
        sh:maxCount 1 ;
        sh:nodeKind sh:IRI ;
        sh:path ns1:completeness .

    _:N51eef082985242c7aad70e82f553a639 sh:datatype xsd:string ;
        sh:maxCount 1 ;
        sh:nodeKind sh:Literal ;
        sh:path ns1:issuingAuthority .

    _:N52681db5aa364b8bb16f1726e4656eb3 rdf:first <https://spdx.org/rdf/3.0.1/terms/Core/SupportType/support> ;
        rdf:rest _:Ndd5dcc6f3a544027a8a159152e96038b .

    _:N5351eb3f50eb48b394de1195b7ab0833 rdf:first <https://spdx.org/rdf/3.0.1/terms/Core/HashAlgorithm/blake2b384> ;
        rdf:rest _:Nbf3b97710804403cb398af39776da0e8 .

    _:N54056810820d48cf8ab5b16acee5b46e sh:datatype xsd:dateTimeStamp ;
        sh:maxCount 1 ;
        sh:nodeKind sh:Literal ;
        sh:path ns1:startTime ;
        sh:pattern "^\\d\\d\\d\\d-\\d\\d-\\d\\dT\\d\\d:\\d\\d:\\d\\dZ$" .

    _:N5448c070514c428eaa4d89cbdbc61908 sh:datatype xsd:string ;
        sh:maxCount 1 ;
        sh:nodeKind sh:Literal ;
        sh:path ns1:contentType ;
        sh:pattern "^[^\\/]+\\/[^\\/]+$" .

    _:N5451d9c16af6442d9bcc23c043b3d0da sh:datatype xsd:string ;
        sh:maxCount 1 ;
        sh:minCount 1 ;
        sh:nodeKind sh:Literal ;
        sh:path <https://spdx.org/rdf/3.0.1/terms/SimpleLicensing/licenseExpression> .

    _:N54ddca5880464f17bd5206be1ecb8932 sh:datatype xsd:string ;
        sh:maxCount 1 ;
        sh:minCount 1 ;
        sh:nodeKind sh:Literal ;
        sh:path ns4:vectorString .

    _:N54e5abc4b90c409dad8d267544c234b8 rdf:first <https://spdx.org/rdf/3.0.1/terms/Core/ExternalIdentifierType/gitoid> ;
        rdf:rest _:N6ebdcc276c2045f2acfaeb5858a7baad .

    _:N552625ddd9864602a0ee19418b5be3ad sh:datatype xsd:anyURI ;
        sh:maxCount 1 ;
        sh:minCount 1 ;
        sh:nodeKind sh:Literal ;
        sh:path ns1:namespace .

    _:N5558fc14d38647a4adb03cde65e127f0 rdf:first <https://spdx.org/rdf/3.0.1/terms/AI/EnergyUnitType/kilowattHour> ;
        rdf:rest _:N15137679a21c43828dd693e3a1badc84 .

    _:N56610830d7ac4b88becc196329620d76 sh:class ns1:Element ;
        sh:nodeKind sh:IRI ;
        sh:path ns1:element .

    _:N5667607f85ea4d4891c6ad8b90baadfa rdf:first <https://spdx.org/rdf/3.0.1/terms/Software/SoftwarePurpose/firmware> ;
        rdf:rest _:N7300e3d820e94c01b833874bbbe92f6a .

    _:N57193ba6e13446fc98d8f8fbfd6100e0 rdf:first <https://spdx.org/rdf/3.0.1/terms/Core/ExternalIdentifierType/packageUrl> ;
        rdf:rest _:Nfe767162ad12488387d2c12a8e8824e6 .

    _:N571ba0ddccae4cfea03176732d3c43eb rdf:first <https://spdx.org/rdf/3.0.1/terms/Core/RelationshipType/other> ;
        rdf:rest _:N6b8daa042c1a4e3487034b8a1683d1e6 .

    _:N580b2e41639f459ca779e7f403e8a1a0 sh:class ns1:PositiveIntegerRange ;
        sh:maxCount 1 ;
        sh:nodeKind sh:BlankNodeOrIRI ;
        sh:path ns3:byteRange .

    _:N5813afc202be42548985f66dd533b449 rdf:first <https://spdx.org/rdf/3.0.1/terms/Core/ProfileIdentifierType/software> ;
        rdf:rest _:N4a711386f320400fa625658b20fcaece .

    _:N58d8aa01956a407ca1b31dc2f502c413 rdf:first <https://spdx.org/rdf/3.0.1/terms/Software/SoftwarePurpose/diskImage> ;
        rdf:rest _:N3963aaabe6d3491399d37f148c43248a .

    _:N58e74d9233994aba923e2ff87f590d6c rdf:first <https://spdx.org/rdf/3.0.1/terms/Core/HashAlgorithm/sha3_512> ;
        rdf:rest () .

    _:N591e1d014a0149b78d304cb4bee48359 rdf:first <https://spdx.org/rdf/3.0.1/terms/Core/RelationshipType/hasExample> ;
        rdf:rest _:Nefa8228af069485099168e4a1d9a6aa1 .

    _:N59b80956043b497382ab07351645a641 rdf:first <https://spdx.org/rdf/3.0.1/terms/Core/RelationshipType/dependsOn> ;
        rdf:rest _:N84decc28a52b477090d3e4e5dc1f76b5 .

    _:N5a131180d5ee42c6924c671e204fea68 rdf:first <https://spdx.org/rdf/3.0.1/terms/Core/RelationshipType/affects> ;
        rdf:rest _:Ne2946aff117f486a89194b1ed5ccc270 .

    _:N5ad39dcdd3c84f519f77a0cca2985866 rdf:first <https://spdx.org/rdf/3.0.1/terms/Core/HashAlgorithm/blake2b512> ;
        rdf:rest _:N763eeeb1374047e2ba764ef55bf982a5 .

    _:N5b03c7def40e4e7eb19a3694c1805931 rdf:first <https://spdx.org/rdf/3.0.1/terms/Core/SupportType/noSupport> ;
        rdf:rest _:Nf88fa8dffd174f1ebb2610c2cd259ac2 .

    _:N5b879168bf5441abbf3604c9325a5bdd rdf:first <https://spdx.org/rdf/3.0.1/terms/Core/ExternalIdentifierType/swid> ;
        rdf:rest _:Nc040b0823ac7474685d89da36f9b2a6f .

    _:N5bcf96480af248baace930d2e86442eb rdf:first <https://spdx.org/rdf/3.0.1/terms/Core/LifecycleScopeType/build> ;
        rdf:rest _:N015d5660aba34b1ca246001ab6fc6ef7 .

    _:N5c04428de4e14d74824de2780dc99cbb sh:hasValue <https://spdx.org/rdf/3.0.1/terms/SimpleLicensing/AnyLicenseInfo> .

    _:N5c04e2eaeb8d44b48535608e5aed9b28 sh:datatype xsd:dateTimeStamp ;
        sh:maxCount 1 ;
        sh:nodeKind sh:Literal ;
        sh:path ns1:endTime ;
        sh:pattern "^\\d\\d\\d\\d-\\d\\d-\\d\\dT\\d\\d:\\d\\d:\\d\\dZ$" .

    _:N5c84929041474695a6ed261ce7b4ad19 sh:datatype xsd:string ;
        sh:nodeKind sh:Literal ;
        sh:path ns1:locator .

    _:N5cb5df020da54023a0414a7b6630c2dc rdf:first <https://spdx.org/rdf/3.0.1/terms/Core/HashAlgorithm/sha3_384> ;
        rdf:rest _:N6e496e9d0578433abbbab2cde03d2ba1 .

    _:N5cddeb9dcb2146139887c2fd1e84cfa9 sh:datatype xsd:boolean ;
        sh:maxCount 1 ;
        sh:nodeKind sh:Literal ;
        sh:path ns5:isFsfLibre .

    _:N5d3cfef88942468f8626584333640c31 sh:message "https://spdx.org/rdf/3.0.1/terms/Extension/Extension is an abstract class and should not be instantiated directly. Instantiate a subclass instead."@en ;
        sh:not _:N13ceb50f498b427f8678e0084e8f5ace ;
        sh:path rdf:type .

    _:N5f5c21c2ca56420e9b21ac77bfae6cb9 rdf:first <https://spdx.org/rdf/3.0.1/terms/Core/RelationshipType/hasAssociatedVulnerability> ;
        rdf:rest _:N4ae21911384f4b8ba646f7789dce9351 .

    _:N6083ef6744964e4fb2296ead9376a998 rdf:first <https://spdx.org/rdf/3.0.1/terms/Dataset/DatasetType/numeric> ;
        rdf:rest _:Nd5969ece16cd4f8a88841f2da3d11133 .

    _:N6097953061744c33b80298571399ff7c sh:datatype xsd:string ;
        sh:maxCount 1 ;
        sh:minCount 1 ;
        sh:nodeKind sh:Literal ;
        sh:path ns1:identifier .

    _:N6176b4e9374646ff969084bff63ba5d8 rdf:first <https://spdx.org/rdf/3.0.1/terms/Core/HashAlgorithm/sha1> ;
        rdf:rest _:N70028c43e63c48f38714f3547a811092 .

    _:N61bbd7824de24d589f5770de480ab78c rdf:first <https://spdx.org/rdf/3.0.1/terms/Core/RelationshipType/underInvestigationFor> ;
        rdf:rest _:Nabd28212c3054e198740821f1c2ee6eb .

    _:N6254eb0c38204b3b809ee94f2ea1e3f1 rdf:first <https://spdx.org/rdf/3.0.1/terms/Dataset/DatasetAvailabilityType/scrapingScript> ;
        rdf:rest () .

    _:N642e588df72d4639b95a7dcaf108f295 sh:datatype xsd:boolean ;
        sh:maxCount 1 ;
        sh:minCount 1 ;
        sh:nodeKind sh:Literal ;
        sh:path ns4:exploited .

    _:N648f9ffbb9ba43b6aab8f8d5f154cc28 sh:datatype xsd:string ;
        sh:maxCount 1 ;
        sh:nodeKind sh:Literal ;
        sh:path ns5:obsoletedBy .

    _:N64af1f3f4fce4843a9f68808b4785623 rdf:first <https://spdx.org/rdf/3.0.1/terms/Core/ExternalRefType/bower> ;
        rdf:rest _:N6f27fdc33b5946519f24bada9b69840a .

    _:N64ed95f303d04309afba135fd30c3506 rdf:first <https://spdx.org/rdf/3.0.1/terms/Core/ProfileIdentifierType/extension> ;
        rdf:rest _:N39c989915c2d4c92b69c3a9dedcf3c7a .

    _:N64f93ff472734041b10fdc6d28dfa4fb rdf:first <https://spdx.org/rdf/3.0.1/terms/Software/SoftwarePurpose/patch> ;
        rdf:rest _:N15b8d7dbed8a4fe19ecbbc9433b7daf2 .

    _:N655a4f76a80043e59c274b12cb5b98cb sh:datatype xsd:string ;
        sh:maxCount 1 ;
        sh:minCount 1 ;
        sh:nodeKind sh:Literal ;
        sh:path ns4:vectorString .

    _:N65d68fe531bd4a79bbf148d2cb0e410e sh:class ns1:PresenceType ;
        sh:in _:N8c5ccf49055d4e2a9519cda0fb7a0fd8 ;
        sh:maxCount 1 ;
        sh:nodeKind sh:IRI ;
        sh:path ns6:hasSensitivePersonalInformation .

    _:N672fab4a7fc044949e885d5809f89577 sh:class ns1:Agent ;
        sh:nodeKind sh:IRI ;
        sh:path ns1:originatedBy .

    _:N67ba0e8f8a184940ad3e478f5b0b74a5 rdf:first <https://spdx.org/rdf/3.0.1/terms/Core/ExternalIdentifierType/cve> ;
        rdf:rest _:N143985a756e44389b9f2dd3a852b8a0b .

    _:N683ff685a95941dfbff264b5fb2feb94 sh:datatype xsd:string ;
        sh:maxCount 1 ;
        sh:nodeKind sh:Literal ;
        sh:path ns2:informationAboutApplication .

    _:N699042cb282e4591be72fdb7601f10ee rdf:first <https://spdx.org/rdf/3.0.1/terms/Core/ExternalRefType/other> ;
        rdf:rest _:Na4f82f9f480a4159be194ab0df8decf1 .

    _:N69d74818048847a386ab183dd27d4165 rdf:first <https://spdx.org/rdf/3.0.1/terms/Software/SbomType/deployed> ;
        rdf:rest _:Ndf8711be211943e9b35bdd0c473d9a29 .

    _:N69f1d00a23cc4b8e8a94de780133c16f sh:class ns1:SupportType ;
        sh:in _:Nbf2fdc103a7c411f987812e1faa847e6 ;
        sh:nodeKind sh:IRI ;
        sh:path ns1:supportLevel .

    _:N6acc1c288e61445bb0a50d0490a0c267 sh:datatype xsd:dateTimeStamp ;
        sh:maxCount 1 ;
        sh:nodeKind sh:Literal ;
        sh:path ns4:publishedTime ;
        sh:pattern "^\\d\\d\\d\\d-\\d\\d-\\d\\dT\\d\\d:\\d\\d:\\d\\dZ$" .

    _:N6b000a1e4c674af7918e4f41aabac3e5 rdf:first <https://spdx.org/rdf/3.0.1/terms/Security/SsvcDecisionType/attend> ;
        rdf:rest _:N34851da2662f43dfba6075ee0badd951 .

    _:N6b07fbd78cf44270865f58743c1d4717 sh:datatype xsd:string ;
        sh:maxCount 1 ;
        sh:nodeKind sh:Literal ;
        sh:path <https://spdx.org/rdf/3.0.1/terms/Extension/cdxPropValue> .

    _:N6b7d2f2b1e9347958af25c5247b1f2a2 rdf:first <https://spdx.org/rdf/3.0.1/terms/Core/HashAlgorithm/sha1> ;
        rdf:rest _:N94c84f442cbe44fc9495129c2c6f4d29 .

    _:N6b8daa042c1a4e3487034b8a1683d1e6 rdf:first <https://spdx.org/rdf/3.0.1/terms/Core/RelationshipType/packagedBy> ;
        rdf:rest _:Nd6211b304e2a40ffa051e5aaa5b99c5f .

    _:N6bd1a6d665974f37b6330aee72463c40 sh:datatype xsd:anyURI ;
        sh:maxCount 1 ;
        sh:minCount 1 ;
        sh:nodeKind sh:Literal ;
        sh:path ns3:contentIdentifierValue .

    _:N6bebaaa660264c1eb2284e229de83b07 rdf:first <https://spdx.org/rdf/3.0.1/terms/Core/ExternalRefType/sourceArtifact> ;
        rdf:rest _:N1d0f7a3442d1402692990d48696cca6e .

    _:N6c7a51ed84ac4676a3ba3d01dc04d315 sh:datatype xsd:anyURI ;
        sh:nodeKind sh:Literal ;
        sh:path ns5:seeAlso .

    _:N6d18b467590e4ae986b20549403ebfc4 sh:class ns1:CreationInfo ;
        sh:maxCount 1 ;
        sh:minCount 1 ;
        sh:nodeKind sh:BlankNodeOrIRI ;
        sh:path ns1:creationInfo .

    _:N6dfda762ba7a4348b0dfbb53ab48e812 rdf:first <https://spdx.org/rdf/3.0.1/terms/Core/ExternalRefType/issueTracker> ;
        rdf:rest _:N1d060b61efbb4904bb56b16b3884b365 .

    _:N6e496e9d0578433abbbab2cde03d2ba1 rdf:first <https://spdx.org/rdf/3.0.1/terms/Core/HashAlgorithm/sha3_512> ;
        rdf:rest () .

    _:N6ebdcc276c2045f2acfaeb5858a7baad rdf:first <https://spdx.org/rdf/3.0.1/terms/Core/ExternalIdentifierType/other> ;
        rdf:rest _:N57193ba6e13446fc98d8f8fbfd6100e0 .

    _:N6f27fdc33b5946519f24bada9b69840a rdf:first <https://spdx.org/rdf/3.0.1/terms/Core/ExternalRefType/buildMeta> ;
        rdf:rest _:N07f2acb5ed1f4a24bc28f6fc41863899 .

    _:N6f332b14dad848a1a73af602a8bf6c70 sh:datatype xsd:nonNegativeInteger ;
        sh:maxCount 1 ;
        sh:nodeKind sh:Literal ;
        sh:path ns6:datasetSize .

    _:N6f7c535ec5984714bdc5cd9e6f23c8a7 sh:datatype xsd:string ;
        sh:nodeKind sh:Literal ;
        sh:path ns2:standardCompliance .

    _:N6f9dc4a33ddc47779b896997a7746cb2 rdf:first <https://spdx.org/rdf/3.0.1/terms/Core/HashAlgorithm/crystalsDilithium> ;
        rdf:rest _:N264db893a85d4367bd49adef5d62f643 .

    _:N70028c43e63c48f38714f3547a811092 rdf:first <https://spdx.org/rdf/3.0.1/terms/Core/HashAlgorithm/sha224> ;
        rdf:rest _:Nf1a6104f6e414fdebc77a3062c7a18f0 .

    _:N72245f846f4c4a56aaff12fd8a595f1b sh:class <https://spdx.org/rdf/3.0.1/terms/Extension/CdxPropertyEntry> ;
        sh:minCount 1 ;
        sh:nodeKind sh:BlankNodeOrIRI ;
        sh:path <https://spdx.org/rdf/3.0.1/terms/Extension/cdxProperty> .

    _:N7300e3d820e94c01b833874bbbe92f6a rdf:first <https://spdx.org/rdf/3.0.1/terms/Software/SoftwarePurpose/framework> ;
        rdf:rest _:Nfa2d65d7f9bb43ecbd05131316536012 .

    _:N737b16f66b5e4fa4bb411e7725fd81ff rdf:first <https://spdx.org/rdf/3.0.1/terms/Dataset/DatasetType/timeseries> ;
        rdf:rest _:N87b6d8e42b184c6a981b3f359a59a275 .

    _:N7459ec882b2e4d8e802d52e7a2b74ef9 rdf:first <https://spdx.org/rdf/3.0.1/terms/Core/RelationshipType/hasVariant> ;
        rdf:rest _:Nf09d4eb43b1e447aa8077f75ea2bc29f .

    _:N7496f10ba6df409c83e99a8f72f1aa78 rdf:first <https://spdx.org/rdf/3.0.1/terms/Software/SoftwarePurpose/archive> ;
        rdf:rest _:Nd7b3f48439f7499caa72322311ab1809 .

    _:N763eeeb1374047e2ba764ef55bf982a5 rdf:first <https://spdx.org/rdf/3.0.1/terms/Core/HashAlgorithm/blake3> ;
        rdf:rest _:N434acd04bf4f4e8e98eb06fc4e5a571e .

    _:N77174bb20392458ca2d4327110d21509 rdf:first <https://spdx.org/rdf/3.0.1/terms/Core/RelationshipType/generates> ;
        rdf:rest _:N315f408bdbab45dab111243059344360 .

    _:N7731592841b44d1f9105c81c87ead7bb sh:datatype xsd:string ;
        sh:maxCount 1 ;
        sh:minCount 1 ;
        sh:nodeKind sh:Literal ;
        sh:path ns1:specVersion ;
        sh:pattern "^(0|[1-9]\\d*)\\.(0|[1-9]\\d*)\\.(0|[1-9]\\d*)(?:-((?:0|[1-9]\\d*|\\d*[a-zA-Z-][0-9a-zA-Z-]*)(?:\\.(?:0|[1-9]\\d*|\\d*[a-zA-Z-][0-9a-zA-Z-]*))*))?(?:\\+([0-9a-zA-Z-]+(?:\\.[0-9a-zA-Z-]+)*))?$" .

    _:N776f590148e0482d8549dcdc6b8ce19e rdf:first <https://spdx.org/rdf/3.0.1/terms/Software/SoftwarePurpose/framework> ;
        rdf:rest _:Ndaa8acc84da441a3ab24d219a6603cb1 .

    _:N77cfd96960c54e7da88fac7740281ef5 sh:class ns3:FileKindType ;
        sh:in _:N7fdf8931e545450f928e25e601810c58 ;
        sh:maxCount 1 ;
        sh:nodeKind sh:IRI ;
        sh:path ns3:fileKind .

    _:N785dc2563b5b478aa13fdc122753beea rdf:first <https://spdx.org/rdf/3.0.1/terms/Core/ExternalRefType/support> ;
        rdf:rest _:Nfe7be267e36a482ba417470876534cd6 .

    _:N794ce2b58929439f88bf8e494c93fd18 rdf:first <https://spdx.org/rdf/3.0.1/terms/Core/HashAlgorithm/sha3_224> ;
        rdf:rest _:Na3ae862844864d0c9e353b39d1c54e35 .

    _:N79fad1bbe88d423b8e5b00dd1b757091 rdf:first <https://spdx.org/rdf/3.0.1/terms/Dataset/DatasetType/graph> ;
        rdf:rest _:Ned45d5bd6b184230b8b0ea23abee2c89 .

    _:N7ada87a7db754bf287181abb5c49bac4 sh:datatype xsd:anyURI ;
        sh:maxCount 1 ;
        sh:minCount 1 ;
        sh:nodeKind sh:Literal ;
        sh:path ns4:locator .

    _:N7bb26512f3b246a189e3c1caf404b878 sh:datatype xsd:string ;
        sh:maxCount 1 ;
        sh:nodeKind sh:Literal ;
        sh:path ns3:packageVersion .

    _:N7bc39608ff4147fbb303dec6bc5b0c7a rdf:first <https://spdx.org/rdf/3.0.1/terms/Security/SsvcDecisionType/trackStar> ;
        rdf:rest () .

    _:N7c2570f4196247ea90dd5b3d7ca0b22e sh:class ns2:EnergyConsumption ;
        sh:maxCount 1 ;
        sh:nodeKind sh:BlankNodeOrIRI ;
        sh:path ns2:energyConsumption .

    _:N7cd9750385bc4a599bec4444bf204571 sh:message "https://spdx.org/rdf/3.0.1/terms/Core/Artifact is an abstract class and should not be instantiated directly. Instantiate a subclass instead."@en ;
        sh:not _:Nd4b49a969b8f429da92f35fcb6ed199d ;
        sh:path rdf:type .

    _:N7dc5b81f3a044db6ba8e80d052ea722f sh:datatype xsd:string ;
        sh:nodeKind sh:Literal ;
        sh:path ns2:modelExplainability .

    _:N7e68baec3a38407aafe0b39c6ae930b1 rdf:first <https://spdx.org/rdf/3.0.1/terms/Security/ExploitCatalogType/kev> ;
        rdf:rest _:Nb0a50d37ff4b4dc1921b26f6e04357c5 .

    _:N7e77bec6ff6048d28db32877de71ab9e sh:datatype xsd:string ;
        sh:nodeKind sh:Literal ;
        sh:path ns6:anonymizationMethodUsed .

    _:N7eec5caf32ba464ca7f4f154d9976028 rdf:first <https://spdx.org/rdf/3.0.1/terms/Core/RelationshipCompleteness/complete> ;
        rdf:rest _:Ne49a0d124e7942d4ae20fa3e686f4aff .

    _:N7f0fc372e3a741e5a8bb04b1ae7a2456 sh:hasValue ns5:License .

    _:N7f3e7e368ced487d87e98dc363b6b5cf sh:datatype xsd:string ;
        sh:maxCount 1 ;
        sh:minCount 1 ;
        sh:nodeKind sh:Literal ;
        sh:path ns4:actionStatement .

    _:N7f4bec2d3c5e42af9f82b5964d720ac9 sh:class ns3:SbomType ;
        sh:in _:N2941fbec200e4a24a6b288efdccf9f61 ;
        sh:nodeKind sh:IRI ;
        sh:path ns3:sbomType .

    _:N7fdf8931e545450f928e25e601810c58 rdf:first <https://spdx.org/rdf/3.0.1/terms/Software/FileKindType/file> ;
        rdf:rest _:Nf315956ca3d84b10bc26f57df5172a35 .

    _:N8091601a2b7b42bf86428834d69610d0 rdf:first <https://spdx.org/rdf/3.0.1/terms/Security/CvssSeverityType/low> ;
        rdf:rest _:Nfa3263ad0b85430faea9a679e491412f .

    _:N8114becca8804d67bed986f971629c1c sh:class ns1:ExternalRefType ;
        sh:in _:N25f14b85810e4dfcb200429bde931173 ;
        sh:maxCount 1 ;
        sh:nodeKind sh:IRI ;
        sh:path ns1:externalRefType .

    _:N81443e2b66644d6f8f751bad29789396 sh:class ns1:DictionaryEntry ;
        sh:nodeKind sh:BlankNodeOrIRI ;
        sh:path <https://spdx.org/rdf/3.0.1/terms/Build/environment> .

    _:N81d1f1b7a8ee4fb8b9c8253b4eb9aac0 sh:datatype xsd:decimal ;
        sh:maxCount 1 ;
        sh:minCount 1 ;
        sh:nodeKind sh:Literal ;
        sh:path ns4:score .

    _:N81e6654c1a534dc8b23f469162487360 rdf:first <https://spdx.org/rdf/3.0.1/terms/Software/ContentIdentifierType/gitoid> ;
        rdf:rest _:Nf34e651ec3bb45019e7d8ca70bb819d5 .

    _:N826a427a992d4c63a9b10b25d7bb37d2 sh:class ns1:Tool ;
        sh:nodeKind sh:IRI ;
        sh:path ns1:createdUsing .

    _:N827d4765f14f49ed9f7cc0b184462699 sh:datatype xsd:string ;
        sh:maxCount 1 ;
        sh:nodeKind sh:Literal ;
        sh:path ns4:statusNotes .

    _:N833037d94cbe4a28b7d115fbffced3f7 sh:hasValue ns5:LicenseAddition .

    _:N83403ff4e6134ab283336f5b2abf62bb rdf:first <https://spdx.org/rdf/3.0.1/terms/Core/RelationshipType/hasStaticLink> ;
        rdf:rest _:Nee7ca7458799465b8708ca0804ada9bf .

    _:N83875d26a4e04788b5ed28a8d0f61329 rdf:first <https://spdx.org/rdf/3.0.1/terms/Software/SbomType/analyzed> ;
        rdf:rest () .

    _:N83d1d8ce6a5f4da29db196af54f27038 sh:datatype xsd:string ;
        sh:maxCount 1 ;
        sh:nodeKind sh:Literal ;
        sh:path ns5:obsoletedBy .

    _:N83e7170013b548ba92e291f418b50a47 sh:datatype xsd:string ;
        sh:nodeKind sh:Literal ;
        sh:path ns1:standardName .

    _:N840f91254c8c467788b8d2ccb69e172c sh:class ns1:DictionaryEntry ;
        sh:nodeKind sh:BlankNodeOrIRI ;
        sh:path ns2:metric .

    _:N84436e39e61e449db908a48de410450c sh:datatype xsd:decimal ;
        sh:maxCount 1 ;
        sh:minCount 1 ;
        sh:nodeKind sh:Literal ;
        sh:path ns4:score .

    _:N84c05a3a3f2d4eb2b75ccdc291749aad rdf:first <https://spdx.org/rdf/3.0.1/terms/Core/RelationshipType/fixedBy> ;
        rdf:rest _:N1ae6ad8ea0d143daba2c967f177264a0 .

    _:N84decc28a52b477090d3e4e5dc1f76b5 rdf:first <https://spdx.org/rdf/3.0.1/terms/Core/RelationshipType/descendantOf> ;
        rdf:rest _:Nc53b869aa32c4abeb2aef472b430dfe8 .

    _:N851b534965d74670af9fa39d53f3f95a rdf:first <https://spdx.org/rdf/3.0.1/terms/Software/SoftwarePurpose/archive> ;
        rdf:rest _:N471e042c9abf46e69e190e4a59ac0d24 .

    _:N866ac4b0ae744cccbb182a6c431cf182 rdf:first <https://spdx.org/rdf/3.0.1/terms/Core/HashAlgorithm/md2> ;
        rdf:rest _:Nc084da4952184f3ca0728e80ffc7a035 .

    _:N86ea4c3d0f134ddba38a472bb6f04517 rdf:first <https://spdx.org/rdf/3.0.1/terms/Software/SoftwarePurpose/filesystemImage> ;
        rdf:rest _:N5667607f85ea4d4891c6ad8b90baadfa .

    _:N86fa428dffca47ed9477433da6de995f sh:message "https://spdx.org/rdf/3.0.1/terms/Security/VexVulnAssessmentRelationship is an abstract class and should not be instantiated directly. Instantiate a subclass instead."@en ;
        sh:not _:Nca198a180eab425bb1941c939fbcab9c ;
        sh:path rdf:type .

    _:N872def5434844a1b9ac1992760ce63c5 rdf:first <https://spdx.org/rdf/3.0.1/terms/Software/SoftwarePurpose/configuration> ;
        rdf:rest _:Nd8d8699f10904874990e571e6f77ad59 .

    _:N87ae6f2c35244fb3828abd80ac3d36af sh:hasValue ns4:VulnAssessmentRelationship .

    _:N87b6d8e42b184c6a981b3f359a59a275 rdf:first <https://spdx.org/rdf/3.0.1/terms/Dataset/DatasetType/timestamp> ;
        rdf:rest _:Nc79f6766e4d6437cac337c11f90e0eee .

    _:N8801efb6feb44626a0acd767c310b7a5 sh:class ns5:LicenseAddition ;
        sh:maxCount 1 ;
        sh:minCount 1 ;
        sh:nodeKind sh:IRI ;
        sh:path ns5:subjectAddition .

    _:N88520471170848b4821b898c22e609cf rdf:first <https://spdx.org/rdf/3.0.1/terms/Core/HashAlgorithm/adler32> ;
        rdf:rest _:N40fa50df7da84543bc78883423152ecb .

    _:N88a5ef940b0c4ebbbcdc22280bec27ce rdf:first <https://spdx.org/rdf/3.0.1/terms/AI/EnergyUnitType/other> ;
        rdf:rest () .

    _:N89a86d261e23427e9d1f83e49522a1db sh:datatype xsd:string ;
        sh:nodeKind sh:Literal ;
        sh:path ns6:dataPreprocessing .

    _:N8a001b06f8f846f58ca16289c8bb98e9 sh:datatype xsd:string ;
        sh:maxCount 1 ;
        sh:minCount 1 ;
        sh:nodeKind sh:Literal ;
        sh:path <https://spdx.org/rdf/3.0.1/terms/SimpleLicensing/licenseText> .

    _:N8aa24eb458c14bee98a6ad4e083f766f rdf:first <https://spdx.org/rdf/3.0.1/terms/Dataset/DatasetType/audio> ;
        rdf:rest _:Nbbf24ad315794321bb1d985b1f28c8a3 .

    _:N8aa30e7bba764b98a907f64507d46c15 rdf:first <https://spdx.org/rdf/3.0.1/terms/Software/SoftwarePurpose/executable> ;
        rdf:rest _:N0055f76237eb4d249deebcb85dc89088 .

    _:N8bedee90de324e0ca9f0bf438f29e49d rdf:first <https://spdx.org/rdf/3.0.1/terms/Dataset/ConfidentialityLevelType/green> ;
        rdf:rest _:Ne0dc762a420d4018aaeba934fde552fe .

    _:N8c5ccf49055d4e2a9519cda0fb7a0fd8 rdf:first <https://spdx.org/rdf/3.0.1/terms/Core/PresenceType/yes> ;
        rdf:rest _:N0ce73a98987540c29f974f5ff5da483f .

    _:N8e47b331646c4f46b0249c7d7101ed4a rdf:first <https://spdx.org/rdf/3.0.1/terms/Core/HashAlgorithm/md6> ;
        rdf:rest _:N51872cae29bf4b38b2304fa980844191 .

    _:N8ec3a357913b4e8f9be6010fede1f88b sh:class ns1:Element ;
        sh:nodeKind sh:IRI ;
        sh:path ns1:rootElement .

    _:N8f02949295a84de8b9950130e13d33e2 rdf:first <https://spdx.org/rdf/3.0.1/terms/Core/ExternalRefType/certificationReport> ;
        rdf:rest _:Ndb01c4cf1af6441ea4c8d4808886e884 .

    _:N8fba8ca1dfd046078082d95db6abfb8d rdf:first <https://spdx.org/rdf/3.0.1/terms/Core/ProfileIdentifierType/build> ;
        rdf:rest _:Nd29358933a074ca88299aa8413cbd962 .

    _:N905723b1e2d246c5b994e7adf8b2b9ba rdf:first <https://spdx.org/rdf/3.0.1/terms/Software/SoftwarePurpose/model> ;
        rdf:rest _:N29cee72ea302413db6fb90c4cf46a270 .

    _:N9067cfbcf2ce44789dab84e7b2d41316 sh:datatype xsd:anyURI ;
        sh:maxCount 1 ;
        sh:nodeKind sh:Literal ;
        sh:path ns3:downloadLocation .

    _:N90beb5cae77044a7865d4fa65f54cadb rdf:first <https://spdx.org/rdf/3.0.1/terms/Core/ExternalRefType/socialMedia> ;
        rdf:rest _:N6bebaaa660264c1eb2284e229de83b07 .

    _:N911618dbe2d54add968ac9b704f36082 rdf:first <https://spdx.org/rdf/3.0.1/terms/Core/RelationshipType/configures> ;
        rdf:rest _:Nd09e22bbdc8449edb83262056f959a72 .

    _:N91d59f3e252f4ccfacb8cf348a59dca2 rdf:first <https://spdx.org/rdf/3.0.1/terms/Core/ExternalRefType/securityPenTestReport> ;
        rdf:rest _:N286dd473156f45b1bed255af1c1ce34e .

    _:N92e29980c8364c5393f9dce3e78d390e rdf:first <https://spdx.org/rdf/3.0.1/terms/AI/SafetyRiskAssessmentType/serious> ;
        rdf:rest _:N94b85bd9ca5c4ccd949118b7de9e48d8 .

    _:N92fed260ea0a4ea4b3bb10f7c976a849 rdf:first <https://spdx.org/rdf/3.0.1/terms/Core/ProfileIdentifierType/dataset> ;
        rdf:rest _:N64ed95f303d04309afba135fd30c3506 .

    _:N93878faf06ee404eae2601c9c5364c74 rdf:first <https://spdx.org/rdf/3.0.1/terms/Core/ExternalRefType/releaseNotes> ;
        rdf:rest _:Nd1665fb26bf943038e1a3156b58a5dcf .

    _:N93d18c08169a49b08ba0231691a7a086 rdf:first <https://spdx.org/rdf/3.0.1/terms/Core/PresenceType/yes> ;
        rdf:rest _:Nf955824d93954485a31f46e30fe5a82e .

    _:N943f36b7c5ef4596ab447543bb558d7e sh:datatype xsd:string ;
        sh:maxCount 1 ;
        sh:nodeKind sh:Literal ;
        sh:path ns1:statement .

    _:N946dc0093cc7454e829aecf1150d1bd8 rdf:first <https://spdx.org/rdf/3.0.1/terms/Core/SupportType/endOfSupport> ;
        rdf:rest _:N5b03c7def40e4e7eb19a3694c1805931 .

    _:N94b85bd9ca5c4ccd949118b7de9e48d8 rdf:first <https://spdx.org/rdf/3.0.1/terms/AI/SafetyRiskAssessmentType/high> ;
        rdf:rest _:Nac447033179640a1839d6a23f8a4bac8 .

    _:N94c84f442cbe44fc9495129c2c6f4d29 rdf:first <https://spdx.org/rdf/3.0.1/terms/Core/HashAlgorithm/sha224> ;
        rdf:rest _:N37ea1088bfd243d5a54936253404904a .

    _:N96974ebfb89648cb9f4323f638c46390 rdf:first <https://spdx.org/rdf/3.0.1/terms/Core/RelationshipType/hasPrerequisite> ;
        rdf:rest _:N456a031dc13e4a0e956d1c1983fc6234 .

    _:N96e1c86992b3468f80e525e24d023a59 rdf:first <https://spdx.org/rdf/3.0.1/terms/Security/CvssSeverityType/medium> ;
        rdf:rest _:N8091601a2b7b42bf86428834d69610d0 .

    _:N9762c762152e444a9dca17520d90f823 rdf:first <https://spdx.org/rdf/3.0.1/terms/Core/RelationshipType/hasDependencyManifest> ;
        rdf:rest _:Nc9114f801a9442a7a95e253e5ea338a1 .

    _:N9923bb8ce2714e80aed0235ac5044f48 rdf:first <https://spdx.org/rdf/3.0.1/terms/Software/SbomType/source> ;
        rdf:rest _:N1be37168f2354f8aa16fac868e264502 .

    _:N9a8a5fa4b5934f22a6ae715b8269924d rdf:first <https://spdx.org/rdf/3.0.1/terms/Core/ExternalRefType/license> ;
        rdf:rest _:N699042cb282e4591be72fdb7601f10ee .

    _:N9a8e89767d65423f85dd078f4056b9a9 rdf:first <https://spdx.org/rdf/3.0.1/terms/Core/PresenceType/noAssertion> ;
        rdf:rest () .

    _:N9b60d6fcf46f4094acac3c7d16abd05f sh:datatype xsd:string ;
        sh:maxCount 1 ;
        sh:nodeKind sh:Literal ;
        sh:path ns5:standardLicenseTemplate .

    _:N9b90b2b1c947470cbbdfbb46863b1cea rdf:first <https://spdx.org/rdf/3.0.1/terms/Core/ExternalRefType/binaryArtifact> ;
        rdf:rest _:N64af1f3f4fce4843a9f68808b4785623 .

    _:N9c4632e5374e4c0e943bd16b59a9edd3 rdf:first <https://spdx.org/rdf/3.0.1/terms/Core/ExternalRefType/securityAdversaryModel> ;
        rdf:rest _:Nd2d209d9dac042c6987fdad136a13fa7 .

    _:N9cf6f08e0ba349fe9ae58b98f2ce8df6 rdf:first <https://spdx.org/rdf/3.0.1/terms/Software/SoftwarePurpose/specification> ;
        rdf:rest _:Nb72bd898c2c24a21a1368707f44fe3da .

    _:N9d2d3f5922e74c2ea3e0b15c523461bb sh:datatype xsd:string ;
        sh:maxCount 1 ;
        sh:minCount 1 ;
        sh:nodeKind sh:Literal ;
        sh:path ns1:hashValue .

    _:N9d3e8c20daa5400b957c25be113efe89 sh:class ns1:DictionaryEntry ;
        sh:nodeKind sh:BlankNodeOrIRI ;
        sh:path <https://spdx.org/rdf/3.0.1/terms/Build/parameter> .

    _:N9d62f61296a94ba9bac275dfb9f7f6b9 rdf:first <https://spdx.org/rdf/3.0.1/terms/Software/SoftwarePurpose/operatingSystem> ;
        rdf:rest _:Ndfc05559f3e446d6bd80e4983c94ec07 .

    _:N9dca46da15a4481796f46a2098859f31 sh:class ns4:CvssSeverityType ;
        sh:in _:N2f234aa991c24d8d8673af6d5de553f9 ;
        sh:maxCount 1 ;
        sh:minCount 1 ;
        sh:nodeKind sh:IRI ;
        sh:path ns4:severity .

    _:N9ef0c5442da84b0fae93ce92032c52f8 sh:class ns6:DatasetAvailabilityType ;
        sh:in _:Ne8786002b6ab44e39a20ff31b6688cc1 ;
        sh:maxCount 1 ;
        sh:nodeKind sh:IRI ;
        sh:path ns6:datasetAvailability .

    _:N9f51729e24eb42d4965a4a74fe302d3a sh:datatype xsd:string ;
        sh:maxCount 1 ;
        sh:minCount 1 ;
        sh:nodeKind sh:Literal ;
        sh:path ns1:prefix .

    _:N9fba27fae73449d2b5c74d5d14893170 sh:class ns5:License ;
        sh:maxCount 1 ;
        sh:minCount 1 ;
        sh:nodeKind sh:IRI ;
        sh:path ns5:subjectLicense .

    _:N9fbdc56679684b249b8cc7d20288fa52 sh:datatype xsd:string ;
        sh:maxCount 1 ;
        sh:nodeKind sh:Literal ;
        sh:path ns1:context .

    _:N9ff461b37d8d4675bc31d843a227b96c rdf:first <https://spdx.org/rdf/3.0.1/terms/Core/RelationshipType/hasDocumentation> ;
        rdf:rest _:N2591b91740354a0ead11f5294ea11e44 .

    _:Na103288173fb4ea0ba60d930d0c18dbb rdf:first <https://spdx.org/rdf/3.0.1/terms/Core/RelationshipType/exploitCreatedBy> ;
        rdf:rest _:N84c05a3a3f2d4eb2b75ccdc291749aad .

    _:Na28e863b0b24448aaf988665801a3d38 rdf:first <https://spdx.org/rdf/3.0.1/terms/Software/SoftwarePurpose/application> ;
        rdf:rest _:N7496f10ba6df409c83e99a8f72f1aa78 .

    _:Na360199da8ee498c93cf88f92c327427 sh:datatype xsd:anyURI ;
        sh:maxCount 1 ;
        sh:minCount 1 ;
        sh:nodeKind sh:Literal ;
        sh:path ns1:externalSpdxId .

    _:Na3ae862844864d0c9e353b39d1c54e35 rdf:first <https://spdx.org/rdf/3.0.1/terms/Core/HashAlgorithm/sha3_256> ;
        rdf:rest _:N04fbf9eb972a43e08f04e6eee07296c3 .

    _:Na3ccc8a5475e4877bc9d318834c95e4e sh:datatype xsd:string ;
        sh:maxCount 1 ;
        sh:minCount 1 ;
        sh:nodeKind sh:Literal ;
        sh:path ns1:key .

    _:Na4040cdcb4ed4696ad904d1a44fe4aec rdf:first <https://spdx.org/rdf/3.0.1/terms/Core/PresenceType/yes> ;
        rdf:rest _:Nf64cf3651c21474ebfc875ade4db0b1f .

    _:Na40a3f8ce0f7462b8ead4004753da036 rdf:first <https://spdx.org/rdf/3.0.1/terms/Core/RelationshipType/ancestorOf> ;
        rdf:rest _:Nc743a765459641c38beddfc4d7a13c70 .

    _:Na4bc0bf98fa0440298278fca181bb030 rdf:first <https://spdx.org/rdf/3.0.1/terms/Core/RelationshipType/hasOptionalComponent> ;
        rdf:rest _:N445a5c48a1f14e23b5b70e2bfbc3948b .

    _:Na4f82f9f480a4159be194ab0df8decf1 rdf:first <https://spdx.org/rdf/3.0.1/terms/Core/ExternalRefType/privacyAssessment> ;
        rdf:rest _:Nae131dd0307e4997b4885499012ddc57 .

    _:Na5d356b0fa3f4b5fbf2a1946869d2d30 rdf:first <https://spdx.org/rdf/3.0.1/terms/AI/SafetyRiskAssessmentType/low> ;
        rdf:rest () .

    _:Na6c5560266a54e1ba3c5fff179ece5c0 rdf:first <https://spdx.org/rdf/3.0.1/terms/Software/SoftwarePurpose/model> ;
        rdf:rest _:Nc996f369b91b456990206121452324c8 .

    _:Na76c1d0d30514ffb8beb4d48a0b220ff sh:datatype xsd:dateTimeStamp ;
        sh:maxCount 1 ;
        sh:nodeKind sh:Literal ;
        sh:path ns4:modifiedTime ;
        sh:pattern "^\\d\\d\\d\\d-\\d\\d-\\d\\dT\\d\\d:\\d\\d:\\d\\dZ$" .

    _:Na7ae4c31f5884568a3bf48b6f9676216 sh:class <https://spdx.org/rdf/3.0.1/terms/SimpleLicensing/AnyLicenseInfo> ;
        sh:minCount 2 ;
        sh:nodeKind sh:IRI ;
        sh:path ns5:member .

    _:Na7e4738fe27648738164082e104e7554 rdf:first <https://spdx.org/rdf/3.0.1/terms/Software/SoftwarePurpose/evidence> ;
        rdf:rest _:Nf748a63fc75449c08db90a5cf6902e7e .

    _:Na8466e22ae484f8ab197aa7b0d012695 sh:datatype xsd:dateTimeStamp ;
        sh:maxCount 1 ;
        sh:nodeKind sh:Literal ;
        sh:path <https://spdx.org/rdf/3.0.1/terms/Build/buildStartTime> ;
        sh:pattern "^\\d\\d\\d\\d-\\d\\d-\\d\\dT\\d\\d:\\d\\d:\\d\\dZ$" .

    _:Na8d7257080104ce9b07959b84ec00e76 rdf:first <https://spdx.org/rdf/3.0.1/terms/Software/SoftwarePurpose/library> ;
        rdf:rest _:N42136f4bf09e450cba628f5056116c44 .

    _:Na8df8b76bfd84e51baaca8c4cdbfaec2 sh:class ns1:DictionaryEntry ;
        sh:nodeKind sh:BlankNodeOrIRI ;
        sh:path <https://spdx.org/rdf/3.0.1/terms/SimpleLicensing/customIdToUri> .

    _:Na8e8b62a6c9243ecb48de2e3205d6272 sh:class ns4:ExploitCatalogType ;
        sh:in _:N7e68baec3a38407aafe0b39c6ae930b1 ;
        sh:maxCount 1 ;
        sh:minCount 1 ;
        sh:nodeKind sh:IRI ;
        sh:path ns4:catalogType .

    _:Na95bb880efe24674b0c277cef84cdbc1 rdf:first <https://spdx.org/rdf/3.0.1/terms/Core/RelationshipType/republishedBy> ;
        rdf:rest _:Nfdfcbc8b2a2b478c988e0af07be221d1 .

    _:Na973b83d67cf4ff5908fc21c0448ae8c rdf:first <https://spdx.org/rdf/3.0.1/terms/Software/SoftwarePurpose/data> ;
        rdf:rest _:Nd24c7e340a4a492586e8ed6c4ffe30c0 .

    _:Na9b1443df1ee423b9650e785c0822d4e rdf:first <https://spdx.org/rdf/3.0.1/terms/Software/SoftwarePurpose/specification> ;
        rdf:rest _:N0e59217e851a4ed5aa13df590bab757a .

    _:Na9e1257751b449adb626e23b2a5c824c rdf:first <https://spdx.org/rdf/3.0.1/terms/Core/ExternalRefType/vulnerabilityDisclosureReport> ;
        rdf:rest _:Nff0b442f3d624934ad38d24167047308 .

    _:Naba532c8417a4c379b511d2a06a9d2fe sh:message "https://spdx.org/rdf/3.0.1/terms/Core/Element is an abstract class and should not be instantiated directly. Instantiate a subclass instead."@en ;
        sh:not _:Nc909d96b399d4098a1f291c2e4c67299 ;
        sh:path rdf:type .

    _:Nabd28212c3054e198740821f1c2ee6eb rdf:first <https://spdx.org/rdf/3.0.1/terms/Core/RelationshipType/usesTool> ;
        rdf:rest () .

    _:Nabdb0a76ad4947e4993004af784ba9b7 sh:datatype xsd:string ;
        sh:maxCount 1 ;
        sh:nodeKind sh:Literal ;
        sh:path ns1:comment .

    _:Nac312cc87c4a4f1abaef94b1b46deaa7 rdf:first <https://spdx.org/rdf/3.0.1/terms/Software/SoftwarePurpose/source> ;
        rdf:rest _:Na9b1443df1ee423b9650e785c0822d4e .

    _:Nac447033179640a1839d6a23f8a4bac8 rdf:first <https://spdx.org/rdf/3.0.1/terms/AI/SafetyRiskAssessmentType/medium> ;
        rdf:rest _:Na5d356b0fa3f4b5fbf2a1946869d2d30 .

    _:Nae0ececb588e4377a9d54f80ce52155c sh:class ns1:NamespaceMap ;
        sh:nodeKind sh:BlankNodeOrIRI ;
        sh:path ns1:namespaceMap .

    _:Nae131dd0307e4997b4885499012ddc57 rdf:first <https://spdx.org/rdf/3.0.1/terms/Core/ExternalRefType/productMetadata> ;
        rdf:rest _:Nb15be321afc843e1b6514206c1829813 .

    _:Nae4301a313374dd297ef6012748ea2da rdf:first <https://spdx.org/rdf/3.0.1/terms/Dataset/DatasetAvailabilityType/query> ;
        rdf:rest _:N1b70e585aedf4769b01c68baae40b4f4 .

    _:Naf442b313a8c4fefa96ecbd06003ea73 rdf:first <https://spdx.org/rdf/3.0.1/terms/Core/SupportType/limitedSupport> ;
        rdf:rest _:N946dc0093cc7454e829aecf1150d1bd8 .

    _:Nb0268a8c77ec4002a3462358e1880e18 rdf:first <https://spdx.org/rdf/3.0.1/terms/Core/PresenceType/noAssertion> ;
        rdf:rest () .

    _:Nb0a50d37ff4b4dc1921b26f6e04357c5 rdf:first <https://spdx.org/rdf/3.0.1/terms/Security/ExploitCatalogType/other> ;
        rdf:rest () .

    _:Nb0b20bb7cff8408f8497d39ae505afd0 rdf:first <https://spdx.org/rdf/3.0.1/terms/Core/RelationshipType/expandsTo> ;
        rdf:rest _:Na103288173fb4ea0ba60d930d0c18dbb .

    _:Nb0cacc9c6dba43949be9de7002ca8e9d sh:datatype xsd:string ;
        sh:maxCount 1 ;
        sh:nodeKind sh:Literal ;
        sh:path ns5:standardLicenseHeader .

    _:Nb15be321afc843e1b6514206c1829813 rdf:first <https://spdx.org/rdf/3.0.1/terms/Core/ExternalRefType/purchaseOrder> ;
        rdf:rest _:Nfc78c72b45be4605a9d284181cfec39f .

    _:Nb195befe2d4c41458b75e269d6d5d20d sh:datatype xsd:string ;
        sh:maxCount 1 ;
        sh:nodeKind sh:Literal ;
        sh:path ns5:listVersionAdded .

    _:Nb20751516ec94669b1cd6f091b402af8 sh:datatype xsd:string ;
        sh:maxCount 1 ;
        sh:minCount 1 ;
        sh:nodeKind sh:Literal ;
        sh:path ns5:additionText .

    _:Nb231c2e250ea41fa9d72b8605352f378 sh:class ns1:ExternalIdentifierType ;
        sh:in _:N341b65da06ac49e990a60307d9c787ac ;
        sh:maxCount 1 ;
        sh:minCount 1 ;
        sh:nodeKind sh:IRI ;
        sh:path ns1:externalIdentifierType .

    _:Nb28b73f573b7440bbbbf82e84e8e8b21 rdf:first <https://spdx.org/rdf/3.0.1/terms/Core/RelationshipType/hasMetadata> ;
        rdf:rest _:Na4bc0bf98fa0440298278fca181bb030 .

    _:Nb32bea549ae34bab9c5aef4829b9ee83 sh:datatype xsd:decimal ;
        sh:maxCount 1 ;
        sh:minCount 1 ;
        sh:nodeKind sh:Literal ;
        sh:path ns4:percentile .

    _:Nb341386f04fc4f4fbd57a5ececcf95ae sh:class ns6:DatasetType ;
        sh:in _:N8aa24eb458c14bee98a6ad4e083f766f ;
        sh:minCount 1 ;
        sh:nodeKind sh:IRI ;
        sh:path ns6:datasetType .

    _:Nb358c8f5280a4bcb8f424632e755e642 sh:class ns1:Agent ;
        sh:minCount 1 ;
        sh:nodeKind sh:IRI ;
        sh:path ns1:createdBy .

    _:Nb3940c1a89ea40fd93067b312aa7ec47 sh:datatype xsd:dateTimeStamp ;
        sh:maxCount 1 ;
        sh:nodeKind sh:Literal ;
        sh:path ns4:publishedTime ;
        sh:pattern "^\\d\\d\\d\\d-\\d\\d-\\d\\dT\\d\\d:\\d\\d:\\d\\dZ$" .

    _:Nb3de9ed0037c4b249b07b05a9af68f5b sh:class ns1:HashAlgorithm ;
        sh:in _:N1a98fafcbfca426eb77dc5e8d4edfe45 ;
        sh:maxCount 1 ;
        sh:minCount 1 ;
        sh:nodeKind sh:IRI ;
        sh:path ns1:algorithm .

    _:Nb45b5d6cdcf54be991e8c990a24f18f1 rdf:first <https://spdx.org/rdf/3.0.1/terms/Core/RelationshipCompleteness/incomplete> ;
        rdf:rest _:N7eec5caf32ba464ca7f4f154d9976028 .

    _:Nb481d463371b4fd59dca299a88605aed rdf:first <https://spdx.org/rdf/3.0.1/terms/Core/HashAlgorithm/sha512> ;
        rdf:rest _:N794ce2b58929439f88bf8e494c93fd18 .

    _:Nb49c833ce7884b33a80694404333f830 rdf:first <https://spdx.org/rdf/3.0.1/terms/Software/SoftwarePurpose/application> ;
        rdf:rest _:N851b534965d74670af9fa39d53f3f95a .

    _:Nb6114b281470409dba07ab5b55d23066 sh:datatype xsd:string ;
        sh:nodeKind sh:Literal ;
        sh:path ns2:domain .

    _:Nb63b9b48ace04747b731a24ec5937acf sh:datatype xsd:anyURI ;
        sh:maxCount 1 ;
        sh:nodeKind sh:Literal ;
        sh:path ns3:homePage .

    _:Nb70a709fefb24fcf8edc194e9535bbe1 rdf:first <https://spdx.org/rdf/3.0.1/terms/Core/LifecycleScopeType/runtime> ;
        rdf:rest _:Nbd06212c046d4d16ac3d41b4e9d552d6 .

    _:Nb72bd898c2c24a21a1368707f44fe3da rdf:first <https://spdx.org/rdf/3.0.1/terms/Software/SoftwarePurpose/test> ;
        rdf:rest () .

    _:Nb81e695d822f480b95b13e66da588ed6 rdf:first <https://spdx.org/rdf/3.0.1/terms/Core/HashAlgorithm/other> ;
        rdf:rest _:N6b7d2f2b1e9347958af25c5247b1f2a2 .

    _:Nb873ceb870fd443ea791544deae8e0ea sh:class <https://spdx.org/rdf/3.0.1/terms/Extension/Extension> ;
        sh:nodeKind sh:BlankNodeOrIRI ;
        sh:path ns1:extension .

    _:Nb8a805ff74d04f7f859cadce5a785aa2 rdf:first <https://spdx.org/rdf/3.0.1/terms/Core/HashAlgorithm/md4> ;
        rdf:rest _:N265fe36ac5d944b0975defd743c05a30 .

    _:Nb8cfa0626ffe40b4bf076a3698bb7221 sh:hasValue ns3:SoftwareArtifact .

    _:Nb926c51e6e424f4d91bff7da1f5c5f5d sh:datatype xsd:dateTimeStamp ;
        sh:maxCount 1 ;
        sh:nodeKind sh:Literal ;
        sh:path ns4:modifiedTime ;
        sh:pattern "^\\d\\d\\d\\d-\\d\\d-\\d\\dT\\d\\d:\\d\\d:\\d\\dZ$" .

    _:Nb93310f68d2e4dd79db3e0e8f3d9faec rdf:first <https://spdx.org/rdf/3.0.1/terms/Security/VexJustificationType/inlineMitigationsAlreadyExist> ;
        rdf:rest () .

    _:Nba905dda1acc45f59ef2886c287094d8 rdf:first <https://spdx.org/rdf/3.0.1/terms/Core/RelationshipType/modifiedBy> ;
        rdf:rest _:N571ba0ddccae4cfea03176732d3c43eb .

    _:Nba9d94c6ccef43378e341caf081b2205 sh:hasValue ns5:ExtendableLicense .

    _:Nbb9bd3c264b5448dad629d6045fe3eaf rdf:first <https://spdx.org/rdf/3.0.1/terms/Core/HashAlgorithm/md6> ;
        rdf:rest _:Nb81e695d822f480b95b13e66da588ed6 .

    _:Nbba9abfd6a68448dbef334e60ce75826 sh:datatype xsd:anyURI ;
        sh:nodeKind sh:Literal ;
        sh:path ns1:identifierLocator .

    _:Nbbf24ad315794321bb1d985b1f28c8a3 rdf:first <https://spdx.org/rdf/3.0.1/terms/Dataset/DatasetType/categorical> ;
        rdf:rest _:N79fad1bbe88d423b8e5b00dd1b757091 .

    _:Nbd06212c046d4d16ac3d41b4e9d552d6 rdf:first <https://spdx.org/rdf/3.0.1/terms/Core/LifecycleScopeType/other> ;
        rdf:rest () .

    _:Nbf2fdc103a7c411f987812e1faa847e6 rdf:first <https://spdx.org/rdf/3.0.1/terms/Core/SupportType/development> ;
        rdf:rest _:N52681db5aa364b8bb16f1726e4656eb3 .

    _:Nbf306a0291d44bd6b1f42fc2c74225df rdf:first <https://spdx.org/rdf/3.0.1/terms/Core/ExternalRefType/runtimeAnalysisReport> ;
        rdf:rest _:Nffbbcc687d964159af05c5ecc0cca051 .

    _:Nbf3b97710804403cb398af39776da0e8 rdf:first <https://spdx.org/rdf/3.0.1/terms/Core/HashAlgorithm/blake2b512> ;
        rdf:rest _:Nca8243e5d66f40628b2529790c124525 .

    _:Nbf4048df97c34977adb9353a253edd11 rdf:first <https://spdx.org/rdf/3.0.1/terms/Software/SoftwarePurpose/container> ;
        rdf:rest _:Na973b83d67cf4ff5908fc21c0448ae8c .

    _:Nc0140fcc182b4ab38eff7add9d74a59f rdf:first <https://spdx.org/rdf/3.0.1/terms/Core/ExternalRefType/mavenCentral> ;
        rdf:rest _:N0db09bc77e6147aaa587b2360854742c .

    _:Nc040b0823ac7474685d89da36f9b2a6f rdf:first <https://spdx.org/rdf/3.0.1/terms/Core/ExternalIdentifierType/urlScheme> ;
        rdf:rest () .

    _:Nc045fbbe74684a038b56bd5c153fdabf sh:class ns1:Agent ;
        sh:maxCount 1 ;
        sh:nodeKind sh:IRI ;
        sh:path ns1:suppliedBy .

    _:Nc05a6979941045b19ff160e0990b67c9 sh:datatype xsd:dateTimeStamp ;
        sh:maxCount 1 ;
        sh:nodeKind sh:Literal ;
        sh:path ns1:validUntilTime ;
        sh:pattern "^\\d\\d\\d\\d-\\d\\d-\\d\\dT\\d\\d:\\d\\d:\\d\\dZ$" .

    _:Nc084da4952184f3ca0728e80ffc7a035 rdf:first <https://spdx.org/rdf/3.0.1/terms/Core/HashAlgorithm/md4> ;
        rdf:rest _:N1e9da875ffa041578e3c8769129e85f2 .

    _:Nc0c5231e0c44437eaef8bba4677a31f6 sh:class ns4:VexJustificationType ;
        sh:in _:Nf65aac0dbdfe489aa8ddacda2a16b8c9 ;
        sh:maxCount 1 ;
        sh:nodeKind sh:IRI ;
        sh:path ns4:justificationType .

    _:Nc135d7690cec4e9eacf2c4b3838d3ce0 sh:datatype xsd:string ;
        sh:nodeKind sh:Literal ;
        sh:path ns6:knownBias .

    _:Nc25bd3f108cd40cd96d0f893c3e5741d rdf:first <https://spdx.org/rdf/3.0.1/terms/Core/ExternalRefType/nuget> ;
        rdf:rest _:N9a8a5fa4b5934f22a6ae715b8269924d .

    _:Nc3165c42f0c545518d95fae69d79698c rdf:first <https://spdx.org/rdf/3.0.1/terms/Core/ExternalRefType/cwe> ;
        rdf:rest _:N00a75e275a744df5ad99e30ebba988d0 .

    _:Nc3dcd26154a042baa9b172f9b87fb480 rdf:first <https://spdx.org/rdf/3.0.1/terms/Security/VexJustificationType/vulnerableCodeNotPresent> ;
        rdf:rest _:N3ce7cee25ad3415e976ed9d7b79b0394 .

    _:Nc40a347af0ca48028766e58ea8649917 sh:datatype xsd:string ;
        sh:maxCount 1 ;
        sh:nodeKind sh:Literal ;
        sh:path ns5:standardAdditionTemplate .

    _:Nc461500b62594ca3bda4bc0a9780673b rdf:first <https://spdx.org/rdf/3.0.1/terms/Software/SoftwarePurpose/configuration> ;
        rdf:rest _:Nbf4048df97c34977adb9353a253edd11 .

    _:Nc4b1b7aa97b74620bae4bc433f2b3f89 rdf:first <https://spdx.org/rdf/3.0.1/terms/Core/ExternalRefType/exportControlAssessment> ;
        rdf:rest _:N3523f55fb2c04444a15f8bf5108e4f4d .

    _:Nc53b869aa32c4abeb2aef472b430dfe8 rdf:first <https://spdx.org/rdf/3.0.1/terms/Core/RelationshipType/describes> ;
        rdf:rest _:Nd3dedb0f3b9f4fdb9390fed6f9cd4fe0 .

    _:Nc743a765459641c38beddfc4d7a13c70 rdf:first <https://spdx.org/rdf/3.0.1/terms/Core/RelationshipType/availableFrom> ;
        rdf:rest _:N911618dbe2d54add968ac9b704f36082 .

    _:Nc7472f25ff1a48419a5476b02e425121 rdf:first <https://spdx.org/rdf/3.0.1/terms/Security/CvssSeverityType/high> ;
        rdf:rest _:N96e1c86992b3468f80e525e24d023a59 .

    _:Nc7843f2d449645178198127dcec9cd3e sh:datatype xsd:string ;
        sh:maxCount 1 ;
        sh:nodeKind sh:Literal ;
        sh:path <https://spdx.org/rdf/3.0.1/terms/SimpleLicensing/licenseListVersion> ;
        sh:pattern "^(0|[1-9]\\d*)\\.(0|[1-9]\\d*)\\.(0|[1-9]\\d*)(?:-((?:0|[1-9]\\d*|\\d*[a-zA-Z-][0-9a-zA-Z-]*)(?:\\.(?:0|[1-9]\\d*|\\d*[a-zA-Z-][0-9a-zA-Z-]*))*))?(?:\\+([0-9a-zA-Z-]+(?:\\.[0-9a-zA-Z-]+)*))?$" .

    _:Nc7934e8be9ac4597a30ceb464f3d5037 sh:class ns1:Element ;
        sh:maxCount 1 ;
        sh:minCount 1 ;
        sh:nodeKind sh:IRI ;
        sh:path ns1:from .

    _:Nc79f6766e4d6437cac337c11f90e0eee rdf:first <https://spdx.org/rdf/3.0.1/terms/Dataset/DatasetType/video> ;
        rdf:rest () .

    _:Nc83c7ff0a3a746feab4b5250822afaad rdf:first <https://spdx.org/rdf/3.0.1/terms/Core/RelationshipType/delegatedTo> ;
        rdf:rest _:N59b80956043b497382ab07351645a641 .

    _:Nc873d15abf06445dab3257eedd5eee6f rdf:first <https://spdx.org/rdf/3.0.1/terms/Software/SoftwarePurpose/library> ;
        rdf:rest _:Nd96f6c46a1bd4bbbbfb7f367962be985 .

    _:Nc8909d7de8dc47cb82651301dd403cf5 sh:class ns1:HashAlgorithm ;
        sh:in _:N88520471170848b4821b898c22e609cf ;
        sh:maxCount 1 ;
        sh:minCount 1 ;
        sh:nodeKind sh:IRI ;
        sh:path ns1:algorithm .

    _:Nc909d96b399d4098a1f291c2e4c67299 sh:hasValue ns1:Element .

    _:Nc9114f801a9442a7a95e253e5ea338a1 rdf:first <https://spdx.org/rdf/3.0.1/terms/Core/RelationshipType/hasDistributionArtifact> ;
        rdf:rest _:N9ff461b37d8d4675bc31d843a227b96c .

    _:Nc996f369b91b456990206121452324c8 rdf:first <https://spdx.org/rdf/3.0.1/terms/Software/SoftwarePurpose/module> ;
        rdf:rest _:N9d62f61296a94ba9bac275dfb9f7f6b9 .

    _:Nc9e50174e3d448448737206a174eb9e1 sh:hasValue ns1:ElementCollection .

    _:Nca198a180eab425bb1941c939fbcab9c sh:hasValue ns4:VexVulnAssessmentRelationship .

    _:Nca8243e5d66f40628b2529790c124525 rdf:first <https://spdx.org/rdf/3.0.1/terms/Core/HashAlgorithm/blake3> ;
        rdf:rest _:N6f9dc4a33ddc47779b896997a7746cb2 .

    _:Ncae5f5c7bcc644478c0d7931eff17663 sh:class ns1:ExternalRef ;
        sh:nodeKind sh:BlankNodeOrIRI ;
        sh:path ns1:externalRef .

    _:Ncaf5eb2ed5ff4a08aa3c180f3cf81900 rdf:first <https://spdx.org/rdf/3.0.1/terms/Core/ExternalRefType/dynamicAnalysisReport> ;
        rdf:rest _:Ndfff919535f0488e9db6ef64d416876b .

    _:Ncb08ebb7079c43059ae88abc8e6192ba rdf:first <https://spdx.org/rdf/3.0.1/terms/Core/ExternalRefType/altWebPage> ;
        rdf:rest _:N9b90b2b1c947470cbbdfbb46863b1cea .

    _:Ncb100fcbde1f40d78a139ebc861c1dc3 rdf:first <https://spdx.org/rdf/3.0.1/terms/Security/CvssSeverityType/medium> ;
        rdf:rest _:N07b7170e552e4a4796c656e12821a04e .

    _:Ncd1772ea8f2143b89f9aeaa4912b5ca1 rdf:first <https://spdx.org/rdf/3.0.1/terms/Software/SoftwarePurpose/filesystemImage> ;
        rdf:rest _:Nfbad6437a2194acd8b1f96b47b89d0fa .

    _:Nce85940987124e80ab8a09c3b530105f sh:datatype xsd:string ;
        sh:maxCount 1 ;
        sh:nodeKind sh:Literal ;
        sh:path ns3:copyrightText .

    _:Ncffed33ec761432298dbbe9a975cab49 rdf:first <https://spdx.org/rdf/3.0.1/terms/Core/ProfileIdentifierType/expandedLicensing> ;
        rdf:rest _:Nfb1129952e7a4d6b92b3e98ce66441c2 .

    _:Nd02644afb1dc49c1a5d3579aee9238e5 sh:class ns3:SoftwareArtifact ;
        sh:maxCount 1 ;
        sh:nodeKind sh:IRI ;
        sh:path ns4:assessedElement .

    _:Nd0757799307e48a4b05ca61c03827be6 sh:class <https://spdx.org/rdf/3.0.1/terms/SimpleLicensing/AnyLicenseInfo> ;
        sh:maxCount 1 ;
        sh:nodeKind sh:IRI ;
        sh:path ns1:dataLicense .

    _:Nd09e22bbdc8449edb83262056f959a72 rdf:first <https://spdx.org/rdf/3.0.1/terms/Core/RelationshipType/contains> ;
        rdf:rest _:N2f649d29104c43b194e0945809fea0bb .

    _:Nd15fc2a0dfc74dfebb9e5275ca4e5990 sh:datatype xsd:string ;
        sh:maxCount 1 ;
        sh:minCount 1 ;
        sh:nodeKind sh:Literal ;
        sh:path ns4:vectorString .

    _:Nd1665fb26bf943038e1a3156b58a5dcf rdf:first <https://spdx.org/rdf/3.0.1/terms/Core/ExternalRefType/releaseHistory> ;
        rdf:rest _:N4a2164f0942e45a196c2f32e1eb124aa .

    _:Nd1687fdd5f6e44d68f2b4f7da570cb9f sh:datatype xsd:dateTimeStamp ;
        sh:maxCount 1 ;
        sh:nodeKind sh:Literal ;
        sh:path ns4:actionStatementTime ;
        sh:pattern "^\\d\\d\\d\\d-\\d\\d-\\d\\dT\\d\\d:\\d\\d:\\d\\dZ$" .

    _:Nd1eb01108791459183768f6a56873247 rdf:first <https://spdx.org/rdf/3.0.1/terms/Core/RelationshipType/publishedBy> ;
        rdf:rest _:Nd215247809f54a9a8c062fe37138df77 .

    _:Nd1fe6a7527e042b3818f71d453c8fef5 rdf:first <https://spdx.org/rdf/3.0.1/terms/Core/RelationshipType/hasDeletedFile> ;
        rdf:rest _:N9762c762152e444a9dca17520d90f823 .

    _:Nd215247809f54a9a8c062fe37138df77 rdf:first <https://spdx.org/rdf/3.0.1/terms/Core/RelationshipType/reportedBy> ;
        rdf:rest _:Na95bb880efe24674b0c277cef84cdbc1 .

    _:Nd22fb99bf3914c40933f3c2889844f93 sh:datatype xsd:string ;
        sh:maxCount 1 ;
        sh:nodeKind sh:Literal ;
        sh:path ns6:datasetNoise .

    _:Nd24c7e340a4a492586e8ed6c4ffe30c0 rdf:first <https://spdx.org/rdf/3.0.1/terms/Software/SoftwarePurpose/device> ;
        rdf:rest _:N51aef2d74cdd4cacb76c17b047be429e .

    _:Nd270bd036dc54b30ae14d2e15e4efc18 rdf:first <https://spdx.org/rdf/3.0.1/terms/Core/RelationshipType/hasDataFile> ;
        rdf:rest _:Nd461b716331545f8a10527a341fbc05f .

    _:Nd29358933a074ca88299aa8413cbd962 rdf:first <https://spdx.org/rdf/3.0.1/terms/Core/ProfileIdentifierType/ai> ;
        rdf:rest _:N92fed260ea0a4ea4b3bb10f7c976a849 .

    _:Nd2d209d9dac042c6987fdad136a13fa7 rdf:first <https://spdx.org/rdf/3.0.1/terms/Core/ExternalRefType/securityFix> ;
        rdf:rest _:N27000931246a42d2886129c31ac2dcc7 .

    _:Nd2d7de6410a34b5492acba9e9b453748 rdf:first <https://spdx.org/rdf/3.0.1/terms/Software/SoftwarePurpose/file> ;
        rdf:rest _:N86ea4c3d0f134ddba38a472bb6f04517 .

    _:Nd3bbfec37f114f2ba626d3e104fe8b99 rdf:first <https://spdx.org/rdf/3.0.1/terms/Software/SoftwarePurpose/device> ;
        rdf:rest _:N58d8aa01956a407ca1b31dc2f502c413 .

    _:Nd3dedb0f3b9f4fdb9390fed6f9cd4fe0 rdf:first <https://spdx.org/rdf/3.0.1/terms/Core/RelationshipType/doesNotAffect> ;
        rdf:rest _:Nb0b20bb7cff8408f8497d39ae505afd0 .

    _:Nd461b716331545f8a10527a341fbc05f rdf:first <https://spdx.org/rdf/3.0.1/terms/Core/RelationshipType/hasDeclaredLicense> ;
        rdf:rest _:Nd1fe6a7527e042b3818f71d453c8fef5 .

    _:Nd4b49a969b8f429da92f35fcb6ed199d sh:hasValue ns1:Artifact .

    _:Nd572e06c587345cd87d1d4094ca0fadb sh:datatype xsd:anyURI ;
        sh:nodeKind sh:Literal ;
        sh:path ns5:seeAlso .

    _:Nd5969ece16cd4f8a88841f2da3d11133 rdf:first <https://spdx.org/rdf/3.0.1/terms/Dataset/DatasetType/other> ;
        rdf:rest _:N12bda6abdf98496c9a1d5833ce99465e .

    _:Nd6211b304e2a40ffa051e5aaa5b99c5f rdf:first <https://spdx.org/rdf/3.0.1/terms/Core/RelationshipType/patchedBy> ;
        rdf:rest _:Nd1eb01108791459183768f6a56873247 .

    _:Nd66d5f38bdf145a99b1715d40993517c sh:datatype xsd:dateTimeStamp ;
        sh:maxCount 1 ;
        sh:nodeKind sh:Literal ;
        sh:path ns4:withdrawnTime ;
        sh:pattern "^\\d\\d\\d\\d-\\d\\d-\\d\\dT\\d\\d:\\d\\d:\\d\\dZ$" .

    _:Nd69ae884faaa40898d49c158f8a742fb sh:class ns2:EnergyConsumptionDescription ;
        sh:nodeKind sh:BlankNodeOrIRI ;
        sh:path ns2:trainingEnergyConsumption .

    _:Nd6f96cdb35ca487ebe5f0c1ef4d318eb sh:datatype xsd:positiveInteger ;
        sh:maxCount 1 ;
        sh:minCount 1 ;
        sh:nodeKind sh:Literal ;
        sh:path ns1:endIntegerRange .

    _:Nd70830e62e09431f9f5ac0ca57ad91de sh:datatype xsd:string ;
        sh:maxCount 1 ;
        sh:nodeKind sh:Literal ;
        sh:path <https://spdx.org/rdf/3.0.1/terms/Build/buildId> .

    _:Nd79c9dbb4e544a9d890ab2c44df9dc6d rdf:first <https://spdx.org/rdf/3.0.1/terms/Core/HashAlgorithm/sha384> ;
        rdf:rest _:Nb481d463371b4fd59dca299a88605aed .

    _:Nd7add987f24d4d6680bce9a2d944db6a sh:class ns3:File ;
        sh:maxCount 1 ;
        sh:minCount 1 ;
        sh:nodeKind sh:IRI ;
        sh:path ns3:snippetFromFile .

    _:Nd7b3f48439f7499caa72322311ab1809 rdf:first <https://spdx.org/rdf/3.0.1/terms/Software/SoftwarePurpose/bom> ;
        rdf:rest _:N872def5434844a1b9ac1992760ce63c5 .

    _:Nd7fa1d4fbb0a46e39831eeb358241747 rdf:first <https://spdx.org/rdf/3.0.1/terms/Software/SoftwarePurpose/requirement> ;
        rdf:rest _:Nac312cc87c4a4f1abaef94b1b46deaa7 .

    _:Nd8d8699f10904874990e571e6f77ad59 rdf:first <https://spdx.org/rdf/3.0.1/terms/Software/SoftwarePurpose/container> ;
        rdf:rest _:N3823ee9f07c34e0ca71f9c6c5354ad8d .

    _:Nd96f6c46a1bd4bbbbfb7f367962be985 rdf:first <https://spdx.org/rdf/3.0.1/terms/Software/SoftwarePurpose/manifest> ;
        rdf:rest _:N905723b1e2d246c5b994e7adf8b2b9ba .

    _:Nd97fd6bc795a4c92b7847c716752f010 sh:class ns4:CvssSeverityType ;
        sh:in _:N4aa50d0271014a36b5d3cbddad0a30f3 ;
        sh:maxCount 1 ;
        sh:minCount 1 ;
        sh:nodeKind sh:IRI ;
        sh:path ns4:severity .

    _:Nd9e9103cee9c41ea980d92b72d415fa7 rdf:first <https://spdx.org/rdf/3.0.1/terms/Security/CvssSeverityType/none> ;
        rdf:rest () .

    _:Nda712abeccdd49c09c5c2bc685e05ee4 sh:datatype xsd:boolean ;
        sh:maxCount 1 ;
        sh:nodeKind sh:Literal ;
        sh:path ns5:isDeprecatedAdditionId .

    _:Ndaa8acc84da441a3ab24d219a6603cb1 rdf:first <https://spdx.org/rdf/3.0.1/terms/Software/SoftwarePurpose/install> ;
        rdf:rest _:Nc873d15abf06445dab3257eedd5eee6f .

    _:Ndae7379c02584fffb6506e7a8828e22a sh:datatype xsd:string ;
        sh:maxCount 1 ;
        sh:minCount 1 ;
        sh:nodeKind sh:Literal ;
        sh:path <https://spdx.org/rdf/3.0.1/terms/SimpleLicensing/licenseText> .

    _:Ndb01c4cf1af6441ea4c8d4808886e884 rdf:first <https://spdx.org/rdf/3.0.1/terms/Core/ExternalRefType/componentAnalysisReport> ;
        rdf:rest _:Nc3165c42f0c545518d95fae69d79698c .

    _:Ndb95de258758441cb6ae88d3925e8f63 rdf:first <https://spdx.org/rdf/3.0.1/terms/Core/ExternalIdentifierType/cpe23> ;
        rdf:rest _:N67ba0e8f8a184940ad3e478f5b0b74a5 .

    _:Ndce32759bb544bfa9ada6aa6fa7ea708 rdf:first <https://spdx.org/rdf/3.0.1/terms/Dataset/DatasetType/noAssertion> ;
        rdf:rest _:N6083ef6744964e4fb2296ead9376a998 .

    _:Ndd5dcc6f3a544027a8a159152e96038b rdf:first <https://spdx.org/rdf/3.0.1/terms/Core/SupportType/deployed> ;
        rdf:rest _:Naf442b313a8c4fefa96ecbd06003ea73 .

    _:Nde0b031cd5a84bd9b7232a8ab9b869b1 sh:datatype xsd:string ;
        sh:maxCount 1 ;
        sh:nodeKind sh:Literal ;
        sh:path ns6:datasetUpdateMechanism .

    _:Ndf3547c4313b46d5a449051395fdc15f sh:datatype xsd:string ;
        sh:maxCount 1 ;
        sh:nodeKind sh:Literal ;
        sh:path ns1:name .

    _:Ndf582cda94a94023a3f5a11a839021c1 sh:datatype xsd:decimal ;
        sh:maxCount 1 ;
        sh:minCount 1 ;
        sh:nodeKind sh:Literal ;
        sh:path ns4:probability .

    _:Ndf8711be211943e9b35bdd0c473d9a29 rdf:first <https://spdx.org/rdf/3.0.1/terms/Software/SbomType/runtime> ;
        rdf:rest _:N83875d26a4e04788b5ed28a8d0f61329 .

    _:Ndfc05559f3e446d6bd80e4983c94ec07 rdf:first <https://spdx.org/rdf/3.0.1/terms/Software/SoftwarePurpose/other> ;
        rdf:rest _:N11bf493c9a9d45a5a782561a62bededf .

    _:Ndfff919535f0488e9db6ef64d416876b rdf:first <https://spdx.org/rdf/3.0.1/terms/Core/ExternalRefType/eolNotice> ;
        rdf:rest _:Nc4b1b7aa97b74620bae4bc433f2b3f89 .

    _:Ne0dc762a420d4018aaeba934fde552fe rdf:first <https://spdx.org/rdf/3.0.1/terms/Dataset/ConfidentialityLevelType/clear> ;
        rdf:rest () .

    _:Ne1a811cecaeb4f3ea40377cb54d1a8ad sh:datatype xsd:string ;
        sh:maxCount 1 ;
        sh:nodeKind sh:Literal ;
        sh:path ns2:limitation .

    _:Ne2946aff117f486a89194b1ed5ccc270 rdf:first <https://spdx.org/rdf/3.0.1/terms/Core/RelationshipType/amendedBy> ;
        rdf:rest _:Na40a3f8ce0f7462b8ead4004753da036 .

    _:Ne3190c214db5431e89558087e85a5b81 rdf:first <https://spdx.org/rdf/3.0.1/terms/Dataset/DatasetType/syntactic> ;
        rdf:rest _:N17835996c18345acb753167a8e04a7e7 .

    _:Ne49a0d124e7942d4ae20fa3e686f4aff rdf:first <https://spdx.org/rdf/3.0.1/terms/Core/RelationshipCompleteness/noAssertion> ;
        rdf:rest () .

    _:Ne69badf11b7147abb2046a897c76c730 sh:datatype xsd:dateTimeStamp ;
        sh:maxCount 1 ;
        sh:nodeKind sh:Literal ;
        sh:path ns1:builtTime ;
        sh:pattern "^\\d\\d\\d\\d-\\d\\d-\\d\\dT\\d\\d:\\d\\d:\\d\\dZ$" .

    _:Ne6b4111dd98f4642bdc8313bb4485ac4 sh:datatype xsd:string ;
        sh:maxCount 1 ;
        sh:minCount 1 ;
        sh:nodeKind sh:Literal ;
        sh:path ns1:hashValue .

    _:Ne72021f629d34d889aa64dd671270777 sh:datatype xsd:positiveInteger ;
        sh:maxCount 1 ;
        sh:minCount 1 ;
        sh:nodeKind sh:Literal ;
        sh:path ns1:beginIntegerRange .

    _:Ne761637246cf43209f897d0766c1ff4b rdf:first <https://spdx.org/rdf/3.0.1/terms/Core/HashAlgorithm/blake2b256> ;
        rdf:rest _:N5351eb3f50eb48b394de1195b7ab0833 .

    _:Ne78c54b8bce04bcb9d2ca46f04e2f189 rdf:first <https://spdx.org/rdf/3.0.1/terms/Core/ExternalIdentifierType/swhid> ;
        rdf:rest _:N5b879168bf5441abbf3604c9325a5bdd .

    _:Ne7bb452ea72c40559a74147d8436b910 sh:class ns3:SoftwarePurpose ;
        sh:in _:Nb49c833ce7884b33a80694404333f830 ;
        sh:maxCount 1 ;
        sh:nodeKind sh:IRI ;
        sh:path ns3:primaryPurpose .

    _:Ne81a57a701844ae68d91471cca52a8d2 rdf:first <https://spdx.org/rdf/3.0.1/terms/Core/HashAlgorithm/sha512> ;
        rdf:rest _:N0de811ecc9ec4518b617ae1b51981680 .

    _:Ne852771926b4432ab9b7910fdcae1056 sh:class ns1:DictionaryEntry ;
        sh:nodeKind sh:BlankNodeOrIRI ;
        sh:path ns6:sensor .

    _:Ne85767bf657647678f43e419fe3d7b41 sh:datatype xsd:string ;
        sh:maxCount 1 ;
        sh:nodeKind sh:Literal ;
        sh:path ns4:vexVersion .

    _:Ne8786002b6ab44e39a20ff31b6688cc1 rdf:first <https://spdx.org/rdf/3.0.1/terms/Dataset/DatasetAvailabilityType/clickthrough> ;
        rdf:rest _:N058f54e17ad24bb188ce1059e8fb8749 .

    _:Nea626a2a6c9a4deab1b1cdd962d00ea7 sh:datatype xsd:string ;
        sh:nodeKind sh:Literal ;
        sh:path <https://spdx.org/rdf/3.0.1/terms/Build/configSourceEntrypoint> .

    _:Nea67e787267c4806a636ab1b755ac4c2 rdf:first <https://spdx.org/rdf/3.0.1/terms/Core/ExternalRefType/npm> ;
        rdf:rest _:Nc25bd3f108cd40cd96d0f893c3e5741d .

    _:Ned45d5bd6b184230b8b0ea23abee2c89 rdf:first <https://spdx.org/rdf/3.0.1/terms/Dataset/DatasetType/image> ;
        rdf:rest _:Ndce32759bb544bfa9ada6aa6fa7ea708 .

    _:Nedc283c28c9b44ccad4b01a90a31f2ca sh:class ns2:SafetyRiskAssessmentType ;
        sh:in _:N92e29980c8364c5393f9dce3e78d390e ;
        sh:maxCount 1 ;
        sh:nodeKind sh:IRI ;
        sh:path ns2:safetyRiskAssessment .

    _:Neddd67434de24b47b73290d608b6f7fe rdf:first <https://spdx.org/rdf/3.0.1/terms/Software/SoftwarePurpose/documentation> ;
        rdf:rest _:N4ff24d426d9d4742af402bb81fac3595 .

    _:Nee0116ffe8b74e748a52829e474a1d0a sh:class ns1:ExternalMap ;
        sh:nodeKind sh:BlankNodeOrIRI ;
        sh:path ns1:import .

    _:Nee7ca7458799465b8708ca0804ada9bf rdf:first <https://spdx.org/rdf/3.0.1/terms/Core/RelationshipType/hasTest> ;
        rdf:rest _:N477d8d78964845ceba553659dc2db168 .

    _:Nef0aceefa2a54c08adc29b69c2987c08 sh:class ns1:LifecycleScopeType ;
        sh:in _:Nfb08edf68286483aa0c3904920da86d8 ;
        sh:maxCount 1 ;
        sh:nodeKind sh:IRI ;
        sh:path ns1:scope .

    _:Nefa8228af069485099168e4a1d9a6aa1 rdf:first <https://spdx.org/rdf/3.0.1/terms/Core/RelationshipType/hasHost> ;
        rdf:rest _:N37db31524a794bbd8b57460903c356d7 .

    _:Nf09d4eb43b1e447aa8077f75ea2bc29f rdf:first <https://spdx.org/rdf/3.0.1/terms/Core/RelationshipType/invokedBy> ;
        rdf:rest _:Nba905dda1acc45f59ef2886c287094d8 .

    _:Nf1a6104f6e414fdebc77a3062c7a18f0 rdf:first <https://spdx.org/rdf/3.0.1/terms/Core/HashAlgorithm/sha256> ;
        rdf:rest _:N2c39a98a694448f6aa6a7b9a28962f36 .

    _:Nf25c1da35dd24967a70cec4affc61874 sh:class ns1:Artifact ;
        sh:maxCount 1 ;
        sh:nodeKind sh:IRI ;
        sh:path ns1:definingArtifact .

    _:Nf2f53884af9d4eb2a1400a9c7c189a80 rdf:first <https://spdx.org/rdf/3.0.1/terms/Core/AnnotationType/other> ;
        rdf:rest _:N3aa7cebacf8742c3893b955cd12bf58c .

    _:Nf315956ca3d84b10bc26f57df5172a35 rdf:first <https://spdx.org/rdf/3.0.1/terms/Software/FileKindType/directory> ;
        rdf:rest () .

    _:Nf34e651ec3bb45019e7d8ca70bb819d5 rdf:first <https://spdx.org/rdf/3.0.1/terms/Software/ContentIdentifierType/swhid> ;
        rdf:rest () .

    _:Nf3b79d08d7a146179b7b5d74e752f9e9 rdf:first <https://spdx.org/rdf/3.0.1/terms/Core/HashAlgorithm/md2> ;
        rdf:rest _:Nb8a805ff74d04f7f859cadce5a785aa2 .

    _:Nf456142b643f465ba3425afbe9dc23e9 sh:datatype xsd:string ;
        sh:maxCount 1 ;
        sh:nodeKind sh:Literal ;
        sh:path ns3:sourceInfo .

    _:Nf5021cf34b954bf2a06973ed99d25813 rdf:first <https://spdx.org/rdf/3.0.1/terms/Core/PresenceType/noAssertion> ;
        rdf:rest () .

    _:Nf56f6c0a984245cebdfaf7de7413c7fa sh:class ns2:EnergyUnitType ;
        sh:in _:N5558fc14d38647a4adb03cde65e127f0 ;
        sh:maxCount 1 ;
        sh:minCount 1 ;
        sh:nodeKind sh:IRI ;
        sh:path ns2:energyUnit .

    _:Nf64cf3651c21474ebfc875ade4db0b1f rdf:first <https://spdx.org/rdf/3.0.1/terms/Core/PresenceType/no> ;
        rdf:rest _:Nf5021cf34b954bf2a06973ed99d25813 .

    _:Nf65aac0dbdfe489aa8ddacda2a16b8c9 rdf:first <https://spdx.org/rdf/3.0.1/terms/Security/VexJustificationType/componentNotPresent> ;
        rdf:rest _:Nc3dcd26154a042baa9b172f9b87fb480 .

    _:Nf6895f10a25a4c93bebd86ffcf1880aa sh:datatype xsd:string ;
        sh:maxCount 1 ;
        sh:nodeKind sh:Literal ;
        sh:path ns5:licenseXml .

    _:Nf748a63fc75449c08db90a5cf6902e7e rdf:first <https://spdx.org/rdf/3.0.1/terms/Software/SoftwarePurpose/executable> ;
        rdf:rest _:Nd2d7de6410a34b5492acba9e9b453748 .

    _:Nf79a3a3329be4b8fbccf847359371718 sh:datatype xsd:anyURI ;
        sh:maxCount 1 ;
        sh:nodeKind sh:Literal ;
        sh:path ns3:packageUrl .

    _:Nf88fa8dffd174f1ebb2610c2cd259ac2 rdf:first <https://spdx.org/rdf/3.0.1/terms/Core/SupportType/noAssertion> ;
        rdf:rest () .

    _:Nf91ae204c3344f3dbfe89daa20fec99d rdf:first <https://spdx.org/rdf/3.0.1/terms/Software/SoftwarePurpose/source> ;
        rdf:rest _:N9cf6f08e0ba349fe9ae58b98f2ce8df6 .

    _:Nf955824d93954485a31f46e30fe5a82e rdf:first <https://spdx.org/rdf/3.0.1/terms/Core/PresenceType/no> ;
        rdf:rest _:N9a8e89767d65423f85dd078f4056b9a9 .

    _:Nfa2d65d7f9bb43ecbd05131316536012 rdf:first <https://spdx.org/rdf/3.0.1/terms/Software/SoftwarePurpose/install> ;
        rdf:rest _:Na8d7257080104ce9b07959b84ec00e76 .

    _:Nfa3263ad0b85430faea9a679e491412f rdf:first <https://spdx.org/rdf/3.0.1/terms/Security/CvssSeverityType/none> ;
        rdf:rest () .

    _:Nfa471bceb89b4edaa32262f73d08f93f sh:message "https://spdx.org/rdf/3.0.1/terms/ExpandedLicensing/License is an abstract class and should not be instantiated directly. Instantiate a subclass instead."@en ;
        sh:not _:N7f0fc372e3a741e5a8bb04b1ae7a2456 ;
        sh:path rdf:type .

    _:Nfa8ad30b19ec414288e9039e2e1f534e sh:class ns1:Element ;
        sh:maxCount 1 ;
        sh:minCount 1 ;
        sh:nodeKind sh:IRI ;
        sh:path ns1:subject .

    _:Nfb08edf68286483aa0c3904920da86d8 rdf:first <https://spdx.org/rdf/3.0.1/terms/Core/LifecycleScopeType/design> ;
        rdf:rest _:N08c8d3c9a7fb4e99847505287f582007 .

    _:Nfb1129952e7a4d6b92b3e98ce66441c2 rdf:first <https://spdx.org/rdf/3.0.1/terms/Core/ProfileIdentifierType/security> ;
        rdf:rest _:N8fba8ca1dfd046078082d95db6abfb8d .

    _:Nfb56dda28f4e4167ae11a43fab219b2f sh:class ns1:DictionaryEntry ;
        sh:nodeKind sh:BlankNodeOrIRI ;
        sh:path ns2:hyperparameter .

    _:Nfbad6437a2194acd8b1f96b47b89d0fa rdf:first <https://spdx.org/rdf/3.0.1/terms/Software/SoftwarePurpose/firmware> ;
        rdf:rest _:N776f590148e0482d8549dcdc6b8ce19e .

    _:Nfc78c72b45be4605a9d284181cfec39f rdf:first <https://spdx.org/rdf/3.0.1/terms/Core/ExternalRefType/qualityAssessmentReport> ;
        rdf:rest _:N93878faf06ee404eae2601c9c5364c74 .

    _:Nfc923ccf1ea740df81bd77a3cddf7027 sh:datatype xsd:string ;
        sh:maxCount 1 ;
        sh:nodeKind sh:Literal ;
        sh:path ns1:summary .

    _:Nfdfcbc8b2a2b478c988e0af07be221d1 rdf:first <https://spdx.org/rdf/3.0.1/terms/Core/RelationshipType/serializedInArtifact> ;
        rdf:rest _:N241832593c8748c0b8e5815721925b63 .

    _:Nfe767162ad12488387d2c12a8e8824e6 rdf:first <https://spdx.org/rdf/3.0.1/terms/Core/ExternalIdentifierType/securityOther> ;
        rdf:rest _:Ne78c54b8bce04bcb9d2ca46f04e2f189 .

    _:Nfe7be267e36a482ba417470876534cd6 rdf:first <https://spdx.org/rdf/3.0.1/terms/Core/ExternalRefType/vcs> ;
        rdf:rest _:Na9e1257751b449adb626e23b2a5c824c .

    _:Nff0b442f3d624934ad38d24167047308 rdf:first <https://spdx.org/rdf/3.0.1/terms/Core/ExternalRefType/vulnerabilityExploitabilityAssessment> ;
        rdf:rest () .

    _:Nff823a63d7084b458218a829ce330580 rdf:first <https://spdx.org/rdf/3.0.1/terms/Core/RelationshipType/trainedOn> ;
        rdf:rest _:N61bbd7824de24d589f5770de480ab78c .

    _:Nffbbcc687d964159af05c5ecc0cca051 rdf:first <https://spdx.org/rdf/3.0.1/terms/Core/ExternalRefType/secureSoftwareAttestation> ;
        rdf:rest _:N145fd66cc8f7451a9314fd48034adb1a .
}

